<?xml version="1.0"?>


<!DOCTYPE rdf:RDF [
    <!ENTITY terms "http://purl.org/dc/terms/" >
    <!ENTITY vann "http://purl.org/vocab/vann/" >
    <!ENTITY lemon "http://lemon-model.net/lemon#" >
    <!ENTITY ns "http://creativecommons.org/ns#" >
    <!ENTITY owl "http://www.w3.org/2002/07/owl#" >
    <!ENTITY dc "http://purl.org/dc/elements/1.1/#" >
    <!ENTITY dcr "http://www.isocat.org/ns/dcr.rdf#" >
    <!ENTITY xsd "http://www.w3.org/2001/XMLSchema#" >
    <!ENTITY owl2xml "http://www.w3.org/2006/12/owl2-xml#" >
    <!ENTITY rdfs "http://www.w3.org/2000/01/rdf-schema#" >
    <!ENTITY rdf "http://www.w3.org/1999/02/22-rdf-syntax-ns#" >
    <!ENTITY lexinfo "http://www.lexinfo.net/ontology/2.0/lexinfo#" >
]>


<rdf:RDF xmlns="http://www.lexinfo.net/ontology/2.0/lexinfo#"
     xml:base="http://www.lexinfo.net/ontology/2.0/lexinfo"
     xmlns:dc="http://purl.org/dc/elements/1.1/#"
     xmlns:ns="http://creativecommons.org/ns#"
     xmlns:lexinfo="http://www.lexinfo.net/ontology/2.0/lexinfo#"
     xmlns:terms="http://purl.org/dc/terms/"
     xmlns:vann="http://purl.org/vocab/vann/"
     xmlns:dcr="http://www.isocat.org/ns/dcr.rdf#"
     xmlns:rdfs="http://www.w3.org/2000/01/rdf-schema#"
     xmlns:owl2xml="http://www.w3.org/2006/12/owl2-xml#"
     xmlns:owl="http://www.w3.org/2002/07/owl#"
     xmlns:xsd="http://www.w3.org/2001/XMLSchema#"
     xmlns:rdf="http://www.w3.org/1999/02/22-rdf-syntax-ns#"
     xmlns:lemon="http://lemon-model.net/lemon#">
    <owl:Ontology rdf:about="http://www.lexinfo.net/ontology/2.0/lexinfo">
        <rdfs:label xml:lang="en">LexInfo</rdfs:label>
        <terms:issued rdf:datatype="&xsd;date">2010-11-22</terms:issued>
        <terms:modified rdf:datatype="&xsd;date">2014-06-14</terms:modified>
        <vann:preferredNamespaceUri rdf:datatype="&xsd;anyURI">http://www.lexinfo.net/ontology/2.0/lexinfo#</vann:preferredNamespaceUri>
        <owl:versionInfo xml:lang="en">2.0</owl:versionInfo>
        <rdfs:comment xml:lang="en">An ontology of types, values and properties to be used with the lemon model, partially derived from ISOcat.</rdfs:comment>
        <rdfs:comment xml:lang="ru">Онтология типов, значений и свойств для использования с моделью lemon, частично полученная из ISOcat.</rdfs:comment>        
        <terms:title xml:lang="en">LexInfo</terms:title>
        <vann:preferredNamespacePrefix>lexinfo</vann:preferredNamespacePrefix>
        <terms:description xml:lang="en">An ontology of types, values and properties to be used with the lemon model, partially derived from ISOcat.</terms:description>
        <terms:description xml:lang="ru">Онтология типов, значений и свойств для использования с моделью lemon, частично полученная из ISOcat.</terms:description>        
        <terms:rights xml:lang="en">Copyright 2010 Monnet Project</terms:rights>
        <terms:publisher rdf:resource="http://john.mccr.ae/"/>
        <terms:creator rdf:resource="http://john.mccr.ae/"/>
        <terms:contributor rdf:resource="http://john.mccr.ae/"/>
        <owl:imports rdf:resource="http://lemon-model.net/lemon"/>
        <terms:contributor rdf:resource="http://www.cimiano.de/philipp"/>
        <terms:contributor rdf:resource="http://www.paulbuitelaar.net/"/>
        <terms:rights rdf:resource="https://creativecommons.org/licenses/by/4.0/"/>
        <ns:license rdf:resource="https://creativecommons.org/licenses/by/4.0/"/>
    </owl:Ontology>
    


    <!-- 
    ///////////////////////////////////////////////////////////////////////////////////////
    //
    // Annotation properties
    //
    ///////////////////////////////////////////////////////////////////////////////////////
     -->

    


    <!-- http://creativecommons.org/ns#license -->

    <owl:AnnotationProperty rdf:about="&ns;license"/>
    


    <!-- http://purl.org/dc/elements/1.1/#creator -->

    <owl:AnnotationProperty rdf:about="&dc;creator"/>
    


    <!-- http://purl.org/dc/terms/contributor -->

    <owl:AnnotationProperty rdf:about="&terms;contributor"/>
    


    <!-- http://purl.org/dc/terms/creator -->

    <owl:AnnotationProperty rdf:about="&terms;creator"/>
    


    <!-- http://purl.org/dc/terms/description -->

    <owl:AnnotationProperty rdf:about="&terms;description"/>
    


    <!-- http://purl.org/dc/terms/issued -->

    <owl:AnnotationProperty rdf:about="&terms;issued"/>
    


    <!-- http://purl.org/dc/terms/modified -->

    <owl:AnnotationProperty rdf:about="&terms;modified"/>
    


    <!-- http://purl.org/dc/terms/rights -->

    <owl:AnnotationProperty rdf:about="&terms;rights"/>
    


    <!-- http://purl.org/dc/terms/title -->

    <owl:AnnotationProperty rdf:about="&terms;title"/>
    


    <!-- http://purl.org/vocab/vann/preferredNamespacePrefix -->

    <owl:AnnotationProperty rdf:about="&vann;preferredNamespacePrefix"/>
    


    <!-- http://purl.org/vocab/vann/preferredNamespaceUri -->

    <owl:AnnotationProperty rdf:about="&vann;preferredNamespaceUri"/>
    


    <!-- http://www.isocat.org/ns/dcr.rdf#datcat -->

    <owl:AnnotationProperty rdf:about="&dcr;datcat"/>
    


    <!-- http://www.lexinfo.net/ontology/2.0/lexinfo#example -->

    <owl:AnnotationProperty rdf:about="&lexinfo;example">
        <rdfs:label xml:lang="en">example</rdfs:label>
        <rdfs:label xml:lang="ru">пример</rdfs:label>        
        <rdfs:comment xml:lang="en">An example of the usage of a frame.</rdfs:comment>
        <rdfs:comment xml:lang="ru">Пример использования фрейма</rdfs:comment>
    </owl:AnnotationProperty>
    


    <!-- http://www.lexinfo.net/ontology/2.0/lexinfo#languageSpecific -->

    <owl:AnnotationProperty rdf:about="&lexinfo;languageSpecific"/>
    


    <!-- 
    ///////////////////////////////////////////////////////////////////////////////////////
    //
    // Object Properties
    //
    ///////////////////////////////////////////////////////////////////////////////////////
     -->

    


    <!-- http://lemon-model.net/lemon#broader -->

    <owl:ObjectProperty rdf:about="&lemon;broader"/>
    


    <!-- http://lemon-model.net/lemon#context -->

    <owl:ObjectProperty rdf:about="&lemon;context"/>
    


    <!-- http://lemon-model.net/lemon#definition -->

    <owl:ObjectProperty rdf:about="&lemon;definition"/>
    


    <!-- http://lemon-model.net/lemon#equivalent -->

    <owl:ObjectProperty rdf:about="&lemon;equivalent"/>
    


    <!-- http://lemon-model.net/lemon#formVariant -->

    <owl:ObjectProperty rdf:about="&lemon;formVariant"/>
    


    <!-- http://lemon-model.net/lemon#incompatible -->

    <owl:ObjectProperty rdf:about="&lemon;incompatible"/>
    


    <!-- http://lemon-model.net/lemon#lexicalVariant -->

    <owl:ObjectProperty rdf:about="&lemon;lexicalVariant"/>
    


    <!-- http://lemon-model.net/lemon#marker -->

    <owl:ObjectProperty rdf:about="&lemon;marker"/>
    


    <!-- http://lemon-model.net/lemon#narrower -->

    <owl:ObjectProperty rdf:about="&lemon;narrower"/>
    


    <!-- http://lemon-model.net/lemon#property -->

    <owl:ObjectProperty rdf:about="&lemon;property"/>
    


    <!-- http://lemon-model.net/lemon#senseRelation -->

    <owl:ObjectProperty rdf:about="&lemon;senseRelation"/>
    


    <!-- http://lemon-model.net/lemon#synArg -->

    <owl:ObjectProperty rdf:about="&lemon;synArg"/>
    


    <!-- http://lemon-model.net/lemon#synBehavior -->

    <owl:ObjectProperty rdf:about="&lemon;synBehavior"/>


    <!-- http://www.lexinfo.net/ontology/2.0/lexinfo#abbreviationFor -->

    <owl:ObjectProperty rdf:about="&lexinfo;abbreviationFor">
        <rdfs:label xml:lang="en">abbreviationFor</rdfs:label>
        <rdfs:label xml:lang="ru">сокращение для</rdfs:label>        
        <rdfs:comment xml:lang="en">A linking element used to identify a relation between an abbreviation and its full or expanded form.</rdfs:comment>
        <rdfs:comment xml:lang="ru">Связующий элемент, используемый для обозначения связи между аббревиатурой и ее полной или расширенной формой.</rdfs:comment>        
        <dc:creator>Wright, Sue Ellen</dc:creator>
        <owl:versionInfo>1:0</owl:versionInfo>
        <dcr:datcat rdf:resource="http://www.isocat.org/datcat/DC-65"/>
        <rdfs:isDefinedBy rdf:resource="http://www.lexinfo.net/ontology/2.0/lexinfo"/>
        <rdfs:subPropertyOf rdf:resource="&lexinfo;contractionFor"/>
    </owl:ObjectProperty>
    


    <!-- http://www.lexinfo.net/ontology/2.0/lexinfo#accusativeCaseForm -->

    <owl:ObjectProperty rdf:about="&lexinfo;accusativeCaseForm">
        <rdfs:isDefinedBy rdf:resource="http://www.lexinfo.net/ontology/2.0/lexinfo"/>
        <rdfs:subPropertyOf rdf:resource="&lexinfo;formCaseVariant"/>
    </owl:ObjectProperty>
    


    <!-- http://www.lexinfo.net/ontology/2.0/lexinfo#acronymFor -->

    <owl:ObjectProperty rdf:about="&lexinfo;acronymFor">
        <rdfs:label xml:lang="en">acronymFor</rdfs:label>
        <rdfs:label xml:lang="ru">акроним для</rdfs:label>        
        <owl:versionInfo>1:0</owl:versionInfo>
        <dc:creator>Wright, Sue Ellen</dc:creator>
        <rdfs:comment xml:lang="en">A linking element used to identify a relation between an acronym and its full or expanded form.</rdfs:comment>
        <rdfs:comment xml:lang="ru">Связующий элемент, используемый для идентификации связи между акронимом и его полной или расширенной формой.</rdfs:comment>
        <dcr:datcat rdf:resource="http://www.isocat.org/datcat/DC-66"/>
        <rdfs:isDefinedBy rdf:resource="http://www.lexinfo.net/ontology/2.0/lexinfo"/>
        <rdfs:subPropertyOf rdf:resource="&lexinfo;contractionFor"/>
    </owl:ObjectProperty>
    


    <!-- http://www.lexinfo.net/ontology/2.0/lexinfo#adjunct -->

    <owl:ObjectProperty rdf:about="&lexinfo;adjunct">
        <rdfs:subPropertyOf rdf:resource="&lemon;synArg"/>
        <rdfs:isDefinedBy rdf:resource="http://www.lexinfo.net/ontology/2.0/lexinfo"/>
        <rdfs:range rdf:resource="&lexinfo;Adjunct"/>
    </owl:ObjectProperty>
    


    <!-- http://www.lexinfo.net/ontology/2.0/lexinfo#adpositionalObject -->

    <owl:ObjectProperty rdf:about="&lexinfo;adpositionalObject">
        <rdfs:isDefinedBy rdf:resource="http://www.lexinfo.net/ontology/2.0/lexinfo"/>
        <rdfs:range rdf:resource="&lexinfo;AdpositionalObject"/>
        <rdfs:subPropertyOf rdf:resource="&lexinfo;object"/>
    </owl:ObjectProperty>
    


    <!-- http://www.lexinfo.net/ontology/2.0/lexinfo#adverbialComplement -->

    <owl:ObjectProperty rdf:about="&lexinfo;adverbialComplement">
        <rdfs:isDefinedBy rdf:resource="http://www.lexinfo.net/ontology/2.0/lexinfo"/>
        <rdfs:subPropertyOf rdf:resource="&lexinfo;complement"/>
    </owl:ObjectProperty>
    


    <!-- http://www.lexinfo.net/ontology/2.0/lexinfo#animacy -->

    <owl:ObjectProperty rdf:about="&lexinfo;animacy">
        <rdfs:label xml:lang="en">animacy</rdfs:label>
        <rdfs:label xml:lang="ru">одушевленность</rdfs:label>
        <owl:versionInfo>1:0</owl:versionInfo>
        <dc:creator>Francopoulo, Gil</dc:creator>
        <dc:creator>Wright, Sue Ellen</dc:creator>
        <rdfs:comment xml:lang="en">The characteristic of a word indicating that in a given discourse community, its referent is considered to be alive or to possess a quality of volition or consciousness.</rdfs:comment>
        <rdfs:comment xml:lang="ru">Характеристика слова, указывающего, что в данном дискурсе его референт считается живым или обладает качеством воли или сознания.</rdfs:comment>        
        <dcr:datcat rdf:resource="http://www.isocat.org/datcat/DC-1902"/>
        <dcr:datcat rdf:resource="http://www.isocat.org/datcat/DC-78"/>
        <rdfs:isDefinedBy rdf:resource="http://www.lexinfo.net/ontology/2.0/lexinfo"/>
        <rdfs:range rdf:resource="&lexinfo;Animacy"/>
        <rdfs:subPropertyOf rdf:resource="&lexinfo;morphosyntacticProperty"/>
    </owl:ObjectProperty>
    


    <!-- http://www.lexinfo.net/ontology/2.0/lexinfo#antonym -->

    <owl:ObjectProperty rdf:about="&lexinfo;antonym">
        <rdfs:label xml:lang="en">antonym term</rdfs:label>
        <rdfs:label xml:lang="ru">антонимичное понятие</rdfs:label>        
        <dc:creator>Wright, Sue Ellen</dc:creator>
        <owl:versionInfo>1:0</owl:versionInfo>
        <rdfs:comment xml:lang="en">A term or lexeme whose concept or sense constitutes the opposite of the concept represented by a second term or lexeme.</rdfs:comment>
        <rdfs:comment xml:lang="ru">Термин или лексема, понятие или смысл которых противоположны понятию, представленному вторым термином или лексемой.</rdfs:comment>
        <rdfs:subPropertyOf rdf:resource="&lemon;incompatible"/>
        <dcr:datcat rdf:resource="http://www.isocat.org/datcat/DC-83"/>
        <rdfs:isDefinedBy rdf:resource="http://www.lexinfo.net/ontology/2.0/lexinfo"/>
    </owl:ObjectProperty>
    


    <!-- http://www.lexinfo.net/ontology/2.0/lexinfo#approximate -->

    <owl:ObjectProperty rdf:about="&lexinfo;approximate">
        <rdfs:label xml:lang="en">approximate</rdfs:label>
        <rdfs:label xml:lang="ru">аппроксимация</rdfs:label>        
        <rdfs:comment xml:lang="en">Property used to qualify something similar but not exactly the same</rdfs:comment>
        <rdfs:comment xml:lang="ru">Свойство, используемое, чтобы квалифицировать нечто подобное, но не точно такое же.</rdfs:comment>        
        <dc:creator>Francopoulo, Gil</dc:creator>
        <owl:versionInfo>1:0</owl:versionInfo>
        <rdfs:subPropertyOf rdf:resource="&lemon;senseRelation"/>
        <dcr:datcat rdf:resource="http://www.isocat.org/datcat/DC-2206"/>
        <rdfs:isDefinedBy rdf:resource="http://www.lexinfo.net/ontology/2.0/lexinfo"/>
    </owl:ObjectProperty>
    


    <!-- http://www.lexinfo.net/ontology/2.0/lexinfo#approximateSynonym -->

    <owl:ObjectProperty rdf:about="&lexinfo;approximateSynonym">
        <rdfs:subPropertyOf rdf:resource="&lemon;senseRelation"/>
        <rdfs:isDefinedBy rdf:resource="http://www.lexinfo.net/ontology/2.0/lexinfo"/>
    </owl:ObjectProperty>
    


    <!-- http://www.lexinfo.net/ontology/2.0/lexinfo#aspect -->

    <owl:ObjectProperty rdf:about="&lexinfo;aspect">
        <rdfs:label xml:lang="en">aspect</rdfs:label>
        <rdfs:label xml:lang="ru">вид</rdfs:label>        
        <dc:creator>Francopoulo, Gil</dc:creator>
        <owl:versionInfo>1:0</owl:versionInfo>
        <rdfs:comment xml:lang="en">Category associated to verbs and referring to the way the grammar marks the duration or type of temporal activity.</rdfs:comment>
        <rdfs:comment xml:lang="ru">Категория, связанная с глаголом и указывающая на то, как грамматика ообозначает продолжительность или тип временного действия.</rdfs:comment>
        <dcr:datcat rdf:resource="http://www.isocat.org/datcat/DC-1242"/>
        <rdfs:isDefinedBy rdf:resource="http://www.lexinfo.net/ontology/2.0/lexinfo"/>
        <rdfs:range rdf:resource="&lexinfo;Aspect"/>
        <rdfs:subPropertyOf rdf:resource="&lexinfo;morphosyntacticProperty"/>
    </owl:ObjectProperty>
    


    <!-- http://www.lexinfo.net/ontology/2.0/lexinfo#associativeRelation -->

    <owl:ObjectProperty rdf:about="&lexinfo;associativeRelation">
        <rdfs:label xml:lang="en">concept relation</rdfs:label>
        <rdfs:label xml:lang="ru">отношение понятий</rdfs:label>        
        <rdfs:comment xml:lang="en">A relation between two concepts having a non-hierarchical thematic connection by virtue of experience.</rdfs:comment>
        <rdfs:comment xml:lang="ru">Отношение между двумя понятиями, имеющими неиерархическую тематическую связь на основании опыта</rdfs:comment>
        <owl:versionInfo>1:0</owl:versionInfo>
        <dc:creator>Wright, Sue Ellen</dc:creator>
        <dcr:datcat rdf:resource="http://www.isocat.org/datcat/DC-88"/>
        <rdfs:isDefinedBy rdf:resource="http://www.lexinfo.net/ontology/2.0/lexinfo"/>
        <rdfs:subPropertyOf rdf:resource="&lexinfo;relatedTerm"/>
    </owl:ObjectProperty>
    


    <!-- http://www.lexinfo.net/ontology/2.0/lexinfo#attributiveArg -->

    <owl:ObjectProperty rdf:about="&lexinfo;attributiveArg">
        <rdfs:subPropertyOf rdf:resource="&lemon;synArg"/>
        <rdfs:isDefinedBy rdf:resource="http://www.lexinfo.net/ontology/2.0/lexinfo"/>
        <rdfs:range rdf:resource="&lexinfo;AttributiveArgument"/>
    </owl:ObjectProperty>
    


    <!-- http://www.lexinfo.net/ontology/2.0/lexinfo#case -->

    <owl:ObjectProperty rdf:about="&lexinfo;case">
        <rdfs:label xml:lang="en">case</rdfs:label>
        <rdfs:label xml:lang="ru">падеж</rdfs:label>
        <dc:creator>Francopoulo, Gil</dc:creator>
        <rdfs:comment xml:lang="en">In a given sentence, the way in which the form of a word changes in order to express a relationship with one or several words of the sentence. The morphological modification may apply to nouns, pronouns noun phrase constituents, such as adjectives or numerals.</rdfs:comment>
        <rdfs:comment xml:lang="ru">Способ изменения формы слова для выражения связи с одним или несколькими членами предложения. Данная морфологическая модификация может применяться к существительным, местоимениям, составляющим именных груп таких, как прилагательные или числительные.</rdfs:comment>
        <owl:versionInfo>1:0</owl:versionInfo>
        <dcr:datcat rdf:resource="http://www.isocat.org/datcat/DC-1840"/>
        <rdfs:isDefinedBy rdf:resource="http://www.lexinfo.net/ontology/2.0/lexinfo"/>
        <rdfs:range rdf:resource="&lexinfo;Case"/>
        <rdfs:subPropertyOf rdf:resource="&lexinfo;morphosyntacticProperty"/>
    </owl:ObjectProperty>
    


    <!-- http://www.lexinfo.net/ontology/2.0/lexinfo#causallyRelatedConcept -->

    <owl:ObjectProperty rdf:about="&lexinfo;causallyRelatedConcept">
        <rdfs:label xml:lang="en">causallyRelatedConcept</rdfs:label>
        <rdfs:label xml:lang="ru">причинно-следственная связь</rdfs:label>        
        <owl:versionInfo>1:0</owl:versionInfo>
        <rdfs:comment xml:lang="en">A concept that is related to another concept by virtue of the fact that it plays a causative role with respect to that concept.</rdfs:comment>
        <rdfs:comment xml:lang="ru">Понятие, связанное с другим понятием в силу того, что последнее играет каузативную роль в отношении первого понятия.</rdfs:comment>
        <dc:creator>Wright, Sue Ellen</dc:creator>
        <rdfs:subPropertyOf rdf:resource="&lemon;senseRelation"/>
        <dcr:datcat rdf:resource="http://www.isocat.org/datcat/DC-123"/>
        <rdfs:isDefinedBy rdf:resource="http://www.lexinfo.net/ontology/2.0/lexinfo"/>
    </owl:ObjectProperty>
    


    <!-- http://www.lexinfo.net/ontology/2.0/lexinfo#clausalArg -->

    <owl:ObjectProperty rdf:about="&lexinfo;clausalArg">
        <rdfs:subPropertyOf rdf:resource="&lemon;synArg"/>
        <rdfs:isDefinedBy rdf:resource="http://www.lexinfo.net/ontology/2.0/lexinfo"/>
        <rdfs:range rdf:resource="&lexinfo;ClausalArgument"/>
    </owl:ObjectProperty>
    


    <!-- http://www.lexinfo.net/ontology/2.0/lexinfo#clippedTermFor -->

    <owl:ObjectProperty rdf:about="&lexinfo;clippedTermFor">
        <rdfs:label xml:lang="en">clippedTermFor</rdfs:label>
        <rdfs:label xml:lang="ru">усеченный термин для</rdfs:label>        
        <owl:versionInfo>1:0</owl:versionInfo>
        <rdfs:comment xml:lang="en">A linking element used to identify a relation between a clipped term and its full or expanded form.</rdfs:comment>
        <rdfs:comment xml:lang="ru">Связующий элемент, используемый для идентификации отношения между сокращённым термином и его полной или расширенной формой.</rdfs:comment>
        <dc:creator>Wright, Sue Ellen</dc:creator>
        <dcr:datcat rdf:resource="http://www.isocat.org/datcat/DC-130"/>
        <rdfs:isDefinedBy rdf:resource="http://www.lexinfo.net/ontology/2.0/lexinfo"/>
        <rdfs:subPropertyOf rdf:resource="&lexinfo;derivedForm"/>
    </owl:ObjectProperty>
    


    <!-- http://www.lexinfo.net/ontology/2.0/lexinfo#cliticness -->

    <owl:ObjectProperty rdf:about="&lexinfo;cliticness">
        <rdfs:label xml:lang="en">cliticness</rdfs:label>
        <rdfs:label xml:lang="ru">клитичность</rdfs:label>        
        <dc:creator>Francopoulo, Gil</dc:creator>
        <rdfs:comment xml:lang="en">Categorization of the different types of clitics</rdfs:comment>
        <rdfs:comment xml:lang="ru">Классификация различных типов клитик</rdfs:comment>
        <owl:versionInfo>1:0</owl:versionInfo>
        <dcr:datcat rdf:resource="http://www.isocat.org/datcat/DC-1903"/>
        <rdfs:isDefinedBy rdf:resource="http://www.lexinfo.net/ontology/2.0/lexinfo"/>
        <rdfs:range rdf:resource="&lexinfo;Cliticness"/>
        <rdfs:subPropertyOf rdf:resource="&lexinfo;morphosyntacticProperty"/>
    </owl:ObjectProperty>
    


    <!-- http://www.lexinfo.net/ontology/2.0/lexinfo#collocation -->

    <owl:ObjectProperty rdf:about="&lexinfo;collocation">
        <rdfs:subPropertyOf rdf:resource="&lemon;senseRelation"/>
        <rdfs:isDefinedBy rdf:resource="http://www.lexinfo.net/ontology/2.0/lexinfo"/>
    </owl:ObjectProperty>
    


    <!-- http://www.lexinfo.net/ontology/2.0/lexinfo#comparativeAdjunct -->

    <owl:ObjectProperty rdf:about="&lexinfo;comparativeAdjunct">
        <rdfs:isDefinedBy rdf:resource="http://www.lexinfo.net/ontology/2.0/lexinfo"/>
        <rdfs:range rdf:resource="&lexinfo;ComparativeAdjunct"/>
        <rdfs:subPropertyOf rdf:resource="&lexinfo;predicativeAdjunct"/>
    </owl:ObjectProperty>
    


    <!-- http://www.lexinfo.net/ontology/2.0/lexinfo#comparativeDegreeForm -->

    <owl:ObjectProperty rdf:about="&lexinfo;comparativeDegreeForm">
        <rdfs:isDefinedBy rdf:resource="http://www.lexinfo.net/ontology/2.0/lexinfo"/>
        <rdfs:subPropertyOf rdf:resource="&lexinfo;formDegreeVariant"/>
    </owl:ObjectProperty>
    


    <!-- http://www.lexinfo.net/ontology/2.0/lexinfo#complement -->

    <owl:ObjectProperty rdf:about="&lexinfo;complement">
        <rdfs:label xml:lang="en">complement</rdfs:label>
        <rdfs:label xml:lang="ru">дополнение</rdfs:label>        
        <rdfs:comment xml:lang="en">A noun phrase that follows a copula or similar verb, as for example an idiot in the sentence He is an idiot. - A clause that serves as the subject or direct object of a verb or the direct object of a preposition, as for example that he would be early in the sentence I hoped that he would be early</rdfs:comment>
        <rdfs:comment xml:lang="ru">Именная группа, которая следует за связкой или подобным глаголом, например, как "an idiot/идиот" в предложении "He is an idiot/Он (есть) идиот". - Предложение, которое служит субъектом или прямым дополнением глагола или прямым дополнением предлога, как, например, "that he would be early/ что он будет рано" в предложении "I hoped that he would be early/Я надеялся, что он будет рано".</rdfs:comment>
        <rdfs:subPropertyOf rdf:resource="&lemon;synArg"/>
        <dcr:datcat rdf:resource="http://www.isocat.org/datcat/DC-1257"/>
        <rdfs:isDefinedBy rdf:resource="http://www.lexinfo.net/ontology/2.0/lexinfo"/>
        <rdfs:range rdf:resource="&lexinfo;Complement"/>
    </owl:ObjectProperty>
    


    <!-- http://www.lexinfo.net/ontology/2.0/lexinfo#contractionFor -->

    <owl:ObjectProperty rdf:about="&lexinfo;contractionFor">
        <rdfs:label xml:lang="en">contractionFor</rdfs:label>
        <rdfs:label xml:lang="ru">сокращение для</rdfs:label>        
        <rdfs:comment xml:lang="en">The full form that corresponds to a contracted form.</rdfs:comment>
        <rdfs:comment xml:lang="ru">Полная форма, соответствующая сокращённой форме.</rdfs:comment>
        <owl:versionInfo>1:0</owl:versionInfo>
        <dc:creator>Wright, Sue Ellen</dc:creator>
        <dcr:datcat rdf:resource="http://www.isocat.org/datcat/DC-157"/>
        <rdfs:isDefinedBy rdf:resource="http://www.lexinfo.net/ontology/2.0/lexinfo"/>
        <rdfs:subPropertyOf rdf:resource="&lexinfo;derivedForm"/>
    </owl:ObjectProperty>
    


    <!-- http://www.lexinfo.net/ontology/2.0/lexinfo#coordinateConcept -->

    <owl:ObjectProperty rdf:about="&lexinfo;coordinateConcept">
        <rdfs:label xml:lang="en">coordinateConcept</rdfs:label>
        <rdfs:label xml:lang="ru">соподчиненное понятие</rdfs:label>        
        <owl:versionInfo>1:0</owl:versionInfo>
        <dc:creator>Wright, Sue Ellen</dc:creator>
        <rdfs:comment xml:lang="en">A subordinate concept having the same nearest superordinate concept and same criterion of subdivision as some other concept in a given concept system.</rdfs:comment>
        <rdfs:comment xml:lang="ru">Подчиненное понятие, имеющее одно видовое понятие и один критерий подразделения, как и другое понятие в данной системе.</rdfs:comment>
        <dcr:datcat rdf:resource="http://www.isocat.org/datcat/DC-158"/>
        <rdfs:isDefinedBy rdf:resource="http://www.lexinfo.net/ontology/2.0/lexinfo"/>
        <rdfs:subPropertyOf rdf:resource="&lexinfo;relatedTerm"/>
    </owl:ObjectProperty>
    


    <!-- http://www.lexinfo.net/ontology/2.0/lexinfo#copulativeArg -->

    <owl:ObjectProperty rdf:about="&lexinfo;copulativeArg">
        <rdfs:comment xml:lang="en">Used with copula constructions. This represents the subject/object in a copula construction. As such constructions are reversible this property is used instead of the usual verb subject/object. E,g., Barack Obama is the president/The president is Barack Obama</rdfs:comment>
        <rdfs:comment xml:lang="ru">Используется с конструкциями глагола-связки и представляет собой субъект/объект данной конструкции. Поскольку такие конструкции являются двусторонними, то используются вместо обычного субъекта/объекта полнозначного глагола. Например, Barack Obama is the president. - Барак Обама - президент./ The president is Barack Obama. - Президент - Барак Обама.</rdfs:comment>
        <rdfs:subPropertyOf rdf:resource="&lemon;synArg"/>
        <rdfs:isDefinedBy rdf:resource="http://www.lexinfo.net/ontology/2.0/lexinfo"/>
    </owl:ObjectProperty>
    


    <!-- http://www.lexinfo.net/ontology/2.0/lexinfo#copulativeSubject -->

    <owl:ObjectProperty rdf:about="&lexinfo;copulativeSubject">
        <rdfs:comment xml:lang="en">Indicates the subject of a copula construction. It is assumed that by using this the copula construction is not reversible e.g., He is happy/*happy is him</rdfs:comment>
        <rdfs:comment xml:lang="ru">Указывает на субъект конструкции с глаголом-связкой. Предполагается, что использование этой конструкции не является двусторонним. Например, He is happy. - Он счастлив. /*happy is him - *Счастлив - это он.</rdfs:comment>
        <rdfs:isDefinedBy rdf:resource="http://www.lexinfo.net/ontology/2.0/lexinfo"/>
        <rdfs:subPropertyOf rdf:resource="&lexinfo;copulativeArg"/>
        <rdfs:subPropertyOf rdf:resource="&lexinfo;subject"/>
    </owl:ObjectProperty>
    


    <!-- http://www.lexinfo.net/ontology/2.0/lexinfo#dating -->

    <owl:ObjectProperty rdf:about="&lexinfo;dating">
        <rdfs:label xml:lang="en">dating</rdfs:label>
        <rdfs:label xml:lang="ru">датирование</rdfs:label>        
        <owl:versionInfo>1:0</owl:versionInfo>
        <rdfs:comment xml:lang="en">Indication specifying whether the usage is old or modern.</rdfs:comment>
        <rdfs:comment xml:lang="ru">Показатель, указывающий на то, является ли употребление устаревшим или современным.</rdfs:comment>
        <dc:creator>Francopoulo, Gil</dc:creator>
        <rdfs:subPropertyOf rdf:resource="&lemon;property"/>
        <dcr:datcat rdf:resource="http://www.isocat.org/datcat/DC-1959"/>
        <rdfs:isDefinedBy rdf:resource="http://www.lexinfo.net/ontology/2.0/lexinfo"/>
        <rdfs:range rdf:resource="&lexinfo;Dating"/>
    </owl:ObjectProperty>
    


    <!-- http://www.lexinfo.net/ontology/2.0/lexinfo#dativeCaseForm -->

    <owl:ObjectProperty rdf:about="&lexinfo;dativeCaseForm">
        <rdfs:isDefinedBy rdf:resource="http://www.lexinfo.net/ontology/2.0/lexinfo"/>
        <rdfs:subPropertyOf rdf:resource="&lexinfo;formCaseVariant"/>
    </owl:ObjectProperty>
    


    <!-- http://www.lexinfo.net/ontology/2.0/lexinfo#declarativeClause -->

    <owl:ObjectProperty rdf:about="&lexinfo;declarativeClause">
        <rdfs:isDefinedBy rdf:resource="http://www.lexinfo.net/ontology/2.0/lexinfo"/>
        <rdfs:subPropertyOf rdf:resource="&lexinfo;clausalArg"/>
    </owl:ObjectProperty>
    


    <!-- http://www.lexinfo.net/ontology/2.0/lexinfo#definiteness -->

    <owl:ObjectProperty rdf:about="&lexinfo;definiteness">
        <rdfs:label xml:lang="en">definiteness</rdfs:label>
        <rdfs:label xml:lang="ru">определенность</rdfs:label>        
        <dc:creator>Francopoulo, Gil</dc:creator>
        <owl:versionInfo>1:0</owl:versionInfo>
        <rdfs:comment xml:lang="en">Property about the possiblity to identify an entity.</rdfs:comment>
        <rdfs:comment xml:lang="ru">Свойство, показывающее возможность идентификации сущности.</rdfs:comment>
        <dcr:datcat rdf:resource="http://www.isocat.org/datcat/DC-1926"/>
        <rdfs:isDefinedBy rdf:resource="http://www.lexinfo.net/ontology/2.0/lexinfo"/>
        <rdfs:range rdf:resource="&lexinfo;Definiteness"/>
        <rdfs:subPropertyOf rdf:resource="&lexinfo;morphosyntacticProperty"/>
    </owl:ObjectProperty>
    


    <!-- http://www.lexinfo.net/ontology/2.0/lexinfo#degree -->

    <owl:ObjectProperty rdf:about="&lexinfo;degree">
        <rdfs:label xml:lang="en">degree</rdfs:label>
        <rdfs:label xml:lang="ru">степень</rdfs:label>        
        <dc:creator>Francopoulo, Gil</dc:creator>
        <owl:versionInfo>1:0</owl:versionInfo>
        <rdfs:comment xml:lang="en">Property concerning comparison.</rdfs:comment>
        <rdfs:comment xml:lang="ru">Свойство сравнения.</rdfs:comment>
        <dcr:datcat rdf:resource="http://www.isocat.org/datcat/DC-1419"/>
        <rdfs:isDefinedBy rdf:resource="http://www.lexinfo.net/ontology/2.0/lexinfo"/>
        <rdfs:range rdf:resource="&lexinfo;Degree"/>
        <rdfs:subPropertyOf rdf:resource="&lexinfo;morphosyntacticProperty"/>
    </owl:ObjectProperty>
    


    <!-- http://www.lexinfo.net/ontology/2.0/lexinfo#derivedForm -->

    <owl:ObjectProperty rdf:about="&lexinfo;derivedForm">
        <rdfs:subPropertyOf rdf:resource="&lemon;lexicalVariant"/>
        <rdfs:isDefinedBy rdf:resource="http://www.lexinfo.net/ontology/2.0/lexinfo"/>
    </owl:ObjectProperty>
    


    <!-- http://www.lexinfo.net/ontology/2.0/lexinfo#description -->

    <owl:ObjectProperty rdf:about="&lexinfo;description">
        <rdfs:label xml:lang="en">description</rdfs:label>
        <rdfs:label xml:lang="ru">описание</rdfs:label>        
        <owl:versionInfo>1:0</owl:versionInfo>
        <rdfs:comment xml:lang="en">A description in general prose text of the issues that are indicated by the context. The description field can occur at many different places in a component and profile.</rdfs:comment>
        <rdfs:comment xml:lang="ru">Описание в прозаическом тексте проблем, обозначенных контекстом. Поле описания может встречаться во многих разных местах в любом компоненте структуры текста или в кратком очерке.</rdfs:comment>
        <dc:creator>Wittenburg, Peter</dc:creator>
        <rdfs:subPropertyOf rdf:resource="&lemon;definition"/>
        <dcr:datcat rdf:resource="http://www.isocat.org/datcat/DC-2520"/>
        <rdfs:isDefinedBy rdf:resource="http://www.lexinfo.net/ontology/2.0/lexinfo"/>
    </owl:ObjectProperty>
    


    <!-- http://www.lexinfo.net/ontology/2.0/lexinfo#directObject -->

    <owl:ObjectProperty rdf:about="&lexinfo;directObject">
        <rdfs:label xml:lang="en">direct object</rdfs:label>
        <rdfs:label xml:lang="ru">прямое дополнение</rdfs:label>        
        <rdfs:comment xml:lang="en">relation between a phrase and a verb, in which the relation is central to the verb</rdfs:comment>
        <rdfs:comment xml:lang="ru">Отношение между составляющей и глаголом, в котором связь является главной для глагола</rdfs:comment>
        <dcr:datcat rdf:resource="http://www.isocat.org/datacat/DC-2263"/>
        <rdfs:isDefinedBy rdf:resource="http://www.lexinfo.net/ontology/2.0/lexinfo"/>
        <rdfs:range rdf:resource="&lexinfo;DirectObject"/>
        <rdfs:subPropertyOf rdf:resource="&lexinfo;object"/>
    </owl:ObjectProperty>
    


    <!-- http://www.lexinfo.net/ontology/2.0/lexinfo#dualNumberForm -->

    <owl:ObjectProperty rdf:about="&lexinfo;dualNumberForm">
        <rdfs:isDefinedBy rdf:resource="http://www.lexinfo.net/ontology/2.0/lexinfo"/>
        <rdfs:subPropertyOf rdf:resource="&lexinfo;formNumberVariant"/>
    </owl:ObjectProperty>
    


    <!-- http://www.lexinfo.net/ontology/2.0/lexinfo#etymologicalRoot -->

    <owl:ObjectProperty rdf:about="&lexinfo;etymologicalRoot">
        <rdfs:label xml:lang="en">etymological root</rdfs:label>
        <rdfs:label xml:lang="ru">этимологический корень</rdfs:label>        
        <rdfs:comment xml:lang="en">Morpheme that has a particular status with regards to the word&apos;s etymology.</rdfs:comment>
        <rdfs:comment xml:lang="ru">Морфема, имеющая особый статус в связи с этимологией слова.</rdfs:comment>
        <dc:creator>Francopoulo, Gil</dc:creator>
        <owl:versionInfo>1:0</owl:versionInfo>
        <rdfs:subPropertyOf rdf:resource="&lemon;lexicalVariant"/>
        <dcr:datcat rdf:resource="http://www.isocat.org/datcat/DC-1987"/>
        <rdfs:isDefinedBy rdf:resource="http://www.lexinfo.net/ontology/2.0/lexinfo"/>
    </owl:ObjectProperty>
    


    <!-- http://www.lexinfo.net/ontology/2.0/lexinfo#etymology -->

    <owl:ObjectProperty rdf:about="&lexinfo;etymology">
        <rdfs:label xml:lang="en">etymology</rdfs:label>
        <rdfs:label xml:lang="ru">этимология</rdfs:label>
        <owl:versionInfo>1:0</owl:versionInfo>
        <rdfs:comment xml:lang="en">Information on the origin of a word and the development of its meaning.</rdfs:comment>
        <rdfs:comment xml:lang="ru">Информация о происхождении слова и развитии его значения.</rdfs:comment>
        <dc:creator>Wright, Sue Ellen</dc:creator>
        <rdfs:subPropertyOf rdf:resource="&lemon;definition"/>
        <dcr:datcat rdf:resource="http://www.isocat.org/datcat/DC-221"/>
        <rdfs:isDefinedBy rdf:resource="http://www.lexinfo.net/ontology/2.0/lexinfo"/>
    </owl:ObjectProperty>
    


    <!-- http://www.lexinfo.net/ontology/2.0/lexinfo#exact -->

    <owl:ObjectProperty rdf:about="&lexinfo;exact">
        <rdfs:label xml:lang="en">exact</rdfs:label>
        <rdfs:label xml:lang="ru">точный</rdfs:label>        
        <owl:versionInfo>1:0</owl:versionInfo>
        <dc:creator>Francopoulo, Gil</dc:creator>
        <rdfs:comment xml:lang="en">Completely correct in every detail</rdfs:comment>
        <rdfs:comment xml:lang="ru">Полностью правильный в каждой детали.</rdfs:comment>
        <rdfs:subPropertyOf rdf:resource="&lemon;equivalent"/>
        <dcr:datcat rdf:resource="http://www.isocat.org/datcat/DC-2205"/>
        <rdfs:isDefinedBy rdf:resource="http://www.lexinfo.net/ontology/2.0/lexinfo"/>
    </owl:ObjectProperty>
    


    <!-- http://www.lexinfo.net/ontology/2.0/lexinfo#explanation -->

    <owl:ObjectProperty rdf:about="&lexinfo;explanation">
        <rdfs:label xml:lang="en">explanation</rdfs:label>
        <rdfs:label xml:lang="ru">пояснение</rdfs:label>        
        <rdfs:comment xml:lang="en">A statement that describes and clarifies a concept and makes it understandable, but does not necessarily differentiate it from other concepts.</rdfs:comment>
        <rdfs:comment xml:lang="ru">Утверждение, которое описывает и разъясняет концепт и делает его понятным, но не обязательно отличает его от других концептов.</rdfs:comment>
        <dc:creator>Wright, Sue Ellen</dc:creator>
        <owl:versionInfo>1:0</owl:versionInfo>
        <rdfs:subPropertyOf rdf:resource="&lemon;definition"/>
        <dcr:datcat rdf:resource="http://www.isocat.org/datcat/DC-223"/>
        <rdfs:isDefinedBy rdf:resource="http://www.lexinfo.net/ontology/2.0/lexinfo"/>
    </owl:ObjectProperty>
    


    <!-- http://www.lexinfo.net/ontology/2.0/lexinfo#finiteness -->

    <owl:ObjectProperty rdf:about="&lexinfo;finiteness">
        <rdfs:label xml:lang="en">finitness</rdfs:label>
        <rdfs:label xml:lang="ru">спрягаемость</rdfs:label>        
        <dc:creator>Francopoulo, Gil</dc:creator>
        <owl:versionInfo>1:0</owl:versionInfo>
        <rdfs:comment xml:lang="en">Property referring to finite and non-finite status of a verbal form.</rdfs:comment>
        <rdfs:comment xml:lang="ru">Свойство, показывающее что глагольная форма может быть личной и неличной.</rdfs:comment>
        <dcr:datcat rdf:resource="http://www.isocat.org/datcat/DC-1893"/>
        <rdfs:isDefinedBy rdf:resource="http://www.lexinfo.net/ontology/2.0/lexinfo"/>
        <rdfs:range rdf:resource="&lexinfo;Finiteness"/>
        <rdfs:subPropertyOf rdf:resource="&lexinfo;morphosyntacticProperty"/>
    </owl:ObjectProperty>
    


    <!-- http://www.lexinfo.net/ontology/2.0/lexinfo#firstPersonForm -->

    <owl:ObjectProperty rdf:about="&lexinfo;firstPersonForm">
        <rdfs:isDefinedBy rdf:resource="http://www.lexinfo.net/ontology/2.0/lexinfo"/>
        <rdfs:subPropertyOf rdf:resource="&lexinfo;formPersonVariant"/>
    </owl:ObjectProperty>
    


    <!-- http://www.lexinfo.net/ontology/2.0/lexinfo#formCaseVariant -->

    <owl:ObjectProperty rdf:about="&lexinfo;formCaseVariant">
        <rdfs:subPropertyOf rdf:resource="&lemon;formVariant"/>
        <rdfs:isDefinedBy rdf:resource="http://www.lexinfo.net/ontology/2.0/lexinfo"/>
    </owl:ObjectProperty>
    


    <!-- http://www.lexinfo.net/ontology/2.0/lexinfo#formDegreeVariant -->

    <owl:ObjectProperty rdf:about="&lexinfo;formDegreeVariant">
        <rdfs:subPropertyOf rdf:resource="&lemon;formVariant"/>
        <rdfs:isDefinedBy rdf:resource="http://www.lexinfo.net/ontology/2.0/lexinfo"/>
    </owl:ObjectProperty>
    


    <!-- http://www.lexinfo.net/ontology/2.0/lexinfo#formMoodVariant -->

    <owl:ObjectProperty rdf:about="&lexinfo;formMoodVariant">
        <rdfs:subPropertyOf rdf:resource="&lemon;formVariant"/>
        <rdfs:isDefinedBy rdf:resource="http://www.lexinfo.net/ontology/2.0/lexinfo"/>
    </owl:ObjectProperty>
    


    <!-- http://www.lexinfo.net/ontology/2.0/lexinfo#formNumberVariant -->

    <owl:ObjectProperty rdf:about="&lexinfo;formNumberVariant">
        <rdfs:subPropertyOf rdf:resource="&lemon;formVariant"/>
        <rdfs:isDefinedBy rdf:resource="http://www.lexinfo.net/ontology/2.0/lexinfo"/>
    </owl:ObjectProperty>
    


    <!-- http://www.lexinfo.net/ontology/2.0/lexinfo#formPersonVariant -->

    <owl:ObjectProperty rdf:about="&lexinfo;formPersonVariant">
        <rdfs:subPropertyOf rdf:resource="&lemon;formVariant"/>
        <rdfs:isDefinedBy rdf:resource="http://www.lexinfo.net/ontology/2.0/lexinfo"/>
    </owl:ObjectProperty>
    


    <!-- http://www.lexinfo.net/ontology/2.0/lexinfo#formPositivityVariant -->

    <owl:ObjectProperty rdf:about="&lexinfo;formPositivityVariant">
        <rdfs:subPropertyOf rdf:resource="&lemon;formVariant"/>
        <rdfs:isDefinedBy rdf:resource="http://www.lexinfo.net/ontology/2.0/lexinfo"/>
    </owl:ObjectProperty>
    


    <!-- http://www.lexinfo.net/ontology/2.0/lexinfo#formTenseVariant -->

    <owl:ObjectProperty rdf:about="&lexinfo;formTenseVariant">
        <rdfs:subPropertyOf rdf:resource="&lemon;formVariant"/>
        <rdfs:isDefinedBy rdf:resource="http://www.lexinfo.net/ontology/2.0/lexinfo"/>
    </owl:ObjectProperty>
    


    <!-- http://www.lexinfo.net/ontology/2.0/lexinfo#frequency -->

    <owl:ObjectProperty rdf:about="&lexinfo;frequency">
        <rdfs:label xml:lang="en">frequency</rdfs:label>
        <rdfs:label xml:lang="ru">частота</rdfs:label>        
        <rdfs:comment xml:lang="en">The relative commonness with which a term occurs.</rdfs:comment>
        <rdfs:comment xml:lang="ru">Относительная распространенность термина.</rdfs:comment>
        <dc:creator>Francopoulo, Gil</dc:creator>
        <owl:versionInfo>1:0</owl:versionInfo>
        <dc:creator>Wright, Sue Ellen</dc:creator>
        <rdfs:subPropertyOf rdf:resource="&lemon;property"/>
        <dcr:datcat rdf:resource="http://www.isocat.org/datcat/DC-1965"/>
        <dcr:datcat rdf:resource="http://www.isocat.org/datcat/DC-233"/>
        <rdfs:isDefinedBy rdf:resource="http://www.lexinfo.net/ontology/2.0/lexinfo"/>
        <rdfs:range rdf:resource="&lexinfo;Frequency"/>
    </owl:ObjectProperty>
    


    <!-- http://www.lexinfo.net/ontology/2.0/lexinfo#fullFormFor -->

    <owl:ObjectProperty rdf:about="&lexinfo;fullFormFor">
        <rdfs:label xml:lang="en">fullFormFor</rdfs:label>
        <rdfs:label xml:lang="ru">полная форма для</rdfs:label>
        <dc:creator>Wright, Sue Ellen</dc:creator>
        <rdfs:comment xml:lang="en">A linking element used to identify a relation between any full form of a term or lexical unit and its abbreviated form.</rdfs:comment>
        <rdfs:comment xml:lang="ru">Связующий элемент, используемый для идентификации связи между любой полной формой термина или лексической единицы и их сокращенной формой.</rdfs:comment>
        <owl:versionInfo>1:0</owl:versionInfo>
        <rdfs:subPropertyOf rdf:resource="&lemon;lexicalVariant"/>
        <dcr:datcat rdf:resource="http://www.isocat.org/datcat/DC-241"/>
        <rdfs:isDefinedBy rdf:resource="http://www.lexinfo.net/ontology/2.0/lexinfo"/>
    </owl:ObjectProperty>
    


    <!-- http://www.lexinfo.net/ontology/2.0/lexinfo#futureTenseForm -->

    <owl:ObjectProperty rdf:about="&lexinfo;futureTenseForm">
        <rdfs:isDefinedBy rdf:resource="http://www.lexinfo.net/ontology/2.0/lexinfo"/>
        <rdfs:subPropertyOf rdf:resource="&lexinfo;formTenseVariant"/>
    </owl:ObjectProperty>
    


    <!-- http://www.lexinfo.net/ontology/2.0/lexinfo#gender -->

    <owl:ObjectProperty rdf:about="&lexinfo;gender">
        <rdfs:label xml:lang="en">grammatical gender</rdfs:label>
        <rdfs:label xml:lang="ru">грамматический род</rdfs:label>
        <rdfs:comment xml:lang="en">A grammatical category that indicates grammatical relationships between words in sentences.</rdfs:comment>
        <rdfs:comment xml:lang="ru">Грамматическая категория, которая обозначает грамматические отношения между словами в предложениях.</rdfs:comment>
        <dcr:datcat rdf:resource="http://www.isocat.org/datcat/DC-1297"/>
        <dcr:datcat rdf:resource="http://www.isocat.org/datcat/DC-245"/>
        <rdfs:isDefinedBy rdf:resource="http://www.lexinfo.net/ontology/2.0/lexinfo"/>
        <rdfs:range rdf:resource="&lexinfo;Gender"/>
        <rdfs:subPropertyOf rdf:resource="&lexinfo;morphosyntacticProperty"/>
    </owl:ObjectProperty>
    


    <!-- http://www.lexinfo.net/ontology/2.0/lexinfo#genitiveCaseForm -->

    <owl:ObjectProperty rdf:about="&lexinfo;genitiveCaseForm">
        <rdfs:isDefinedBy rdf:resource="http://www.lexinfo.net/ontology/2.0/lexinfo"/>
        <rdfs:subPropertyOf rdf:resource="&lexinfo;formCaseVariant"/>
    </owl:ObjectProperty>
    


    <!-- http://www.lexinfo.net/ontology/2.0/lexinfo#genitiveObject -->

    <owl:ObjectProperty rdf:about="&lexinfo;genitiveObject">
        <rdfs:isDefinedBy rdf:resource="http://www.lexinfo.net/ontology/2.0/lexinfo"/>
        <rdfs:range rdf:resource="&lexinfo;GenitiveObject"/>
        <rdfs:subPropertyOf rdf:resource="&lexinfo;object"/>
    </owl:ObjectProperty>
    


    <!-- http://www.lexinfo.net/ontology/2.0/lexinfo#geographicalVariant -->

    <owl:ObjectProperty rdf:about="&lexinfo;geographicalVariant">
        <rdfs:label xml:lang="en">geographical variant</rdfs:label>
        <rdfs:label xml:lang="ru">географический вариант</rdfs:label>
        <dc:creator>Francopoulo, Gil</dc:creator>
        <owl:versionInfo>1:0</owl:versionInfo>
        <rdfs:comment xml:lang="en">Description of a specific form used in a certain region as opposed to another form used in another region</rdfs:comment>
        <rdfs:comment xml:lang="ru">Описание особой формы, используемой в определенном регионе, в отличие от другой формы, используемой в другом регионе.</rdfs:comment>
        <rdfs:subPropertyOf rdf:resource="&lemon;lexicalVariant"/>
        <dcr:datcat rdf:resource="http://www.isocat.org/datcat/DC-1851"/>
        <rdfs:isDefinedBy rdf:resource="http://www.lexinfo.net/ontology/2.0/lexinfo"/>
    </owl:ObjectProperty>
    


    <!-- http://www.lexinfo.net/ontology/2.0/lexinfo#gerundClause -->

    <owl:ObjectProperty rdf:about="&lexinfo;gerundClause">
        <rdfs:isDefinedBy rdf:resource="http://www.lexinfo.net/ontology/2.0/lexinfo"/>
        <rdfs:subPropertyOf rdf:resource="&lexinfo;clausalArg"/>
    </owl:ObjectProperty>
    


    <!-- http://www.lexinfo.net/ontology/2.0/lexinfo#gloss -->

    <owl:ObjectProperty rdf:about="&lexinfo;gloss">
        <rdfs:label xml:lang="en">gloss</rdfs:label>
        <rdfs:label xml:lang="ru">глосса</rdfs:label>        
        <owl:versionInfo>1:0</owl:versionInfo>
        <rdfs:comment xml:lang="en">In TEI: A phrase or word used to provide a gloss or definition for some other word or phrase.
In 1951: Any editorial comment.</rdfs:comment>
        <rdfs:comment xml:lang="ru">В ИКТ (TEI): фраза или слово, используемое для пояснения или определения какого-либо другого слова или фразы.
В 1951 году: любой редакторский комментарий.</rdfs:comment>
        <dc:creator>Wright, Sue Ellen</dc:creator>
        <rdfs:subPropertyOf rdf:resource="&lemon;definition"/>
        <dcr:datcat rdf:resource="http://www.isocat.org/datcat/DC-244"/>
        <rdfs:isDefinedBy rdf:resource="http://www.lexinfo.net/ontology/2.0/lexinfo"/>
    </owl:ObjectProperty>
    


    <!-- http://www.lexinfo.net/ontology/2.0/lexinfo#head -->

    <owl:ObjectProperty rdf:about="&lexinfo;head">
        <rdfs:subPropertyOf rdf:resource="&lemon;lexicalVariant"/>
        <rdfs:isDefinedBy rdf:resource="http://www.lexinfo.net/ontology/2.0/lexinfo"/>
    </owl:ObjectProperty>
    


    <!-- http://www.lexinfo.net/ontology/2.0/lexinfo#holonymTerm -->

    <owl:ObjectProperty rdf:about="&lexinfo;holonymTerm">
        <rdfs:label xml:lang="en">holonym</rdfs:label>
        <rdfs:label xml:lang="ru">холоним</rdfs:label>        
        <rdfs:comment xml:lang="en">Indicates that the referenced element is a part of this object</rdfs:comment>
        <rdfs:comment xml:lang="ru">Обозначает, что упоминаемый элемент является частью данного объекта.</rdfs:comment>
        <rdfs:isDefinedBy rdf:resource="http://www.lexinfo.net/ontology/2.0/lexinfo"/>
        <owl:inverseOf rdf:resource="&lexinfo;meronymTerm"/>
        <rdfs:subPropertyOf rdf:resource="&lexinfo;partitiveRelation"/>
    </owl:ObjectProperty>
    


    <!-- http://www.lexinfo.net/ontology/2.0/lexinfo#homograph -->

    <owl:ObjectProperty rdf:about="&lexinfo;homograph">
        <rdfs:label xml:lang="en">homograph</rdfs:label>
        <rdfs:label xml:lang="ru">омограф</rdfs:label>        
        <dc:creator>Wright, Sue Ellen</dc:creator>
        <dc:creator>Francopoulo, Gil</dc:creator>
        <rdfs:comment xml:lang="en">Word that is written like another, but that has a different pronunciation, meaning, and/or origin.</rdfs:comment>
        <rdfs:comment xml:lang="ru">Слово, имеющее сходное написание с другим словом, но при этом имеющее другое произношение, значение и /или происхождение.</rdfs:comment>
        <owl:versionInfo>1:0</owl:versionInfo>
        <rdfs:comment xml:lang="en">A word that is spelled like another, but that has a different pronunciation, meaning, and/or origin.</rdfs:comment>
        <rdfs:comment xml:lang="ru">Слово, имеющее сходное написание с другим словом, но при этом имеющее другое произношение, значение и /или происхождение.</rdfs:comment>        
        <rdfs:subPropertyOf rdf:resource="&lemon;lexicalVariant"/>
        <dcr:datcat rdf:resource="http://www.isocat.org/datcat/DC-1300"/>
        <dcr:datcat rdf:resource="http://www.isocat.org/datcat/DC-260"/>
        <rdfs:isDefinedBy rdf:resource="http://www.lexinfo.net/ontology/2.0/lexinfo"/>
    </owl:ObjectProperty>
    


    <!-- http://www.lexinfo.net/ontology/2.0/lexinfo#homonym -->

    <owl:ObjectProperty rdf:about="&lexinfo;homonym">
        <rdfs:label xml:lang="en">homonym</rdfs:label>
        <rdfs:label xml:lang="ru">омоним</rdfs:label>        
        <owl:versionInfo>1:0</owl:versionInfo>
        <dc:creator>Francopoulo, Gil</dc:creator>
        <rdfs:comment xml:lang="en">A word that is pronounced like another word and that can be spelled the same way (homograph) or can merely sound the same (homophone).</rdfs:comment>
        <rdfs:comment xml:lang="ru">Слово, имеющее сходное произношение с другим словом, которое может иметь и сходное с ним написание (омограф), или может иметь только сходное с ним звучание (омофон).</rdfs:comment>
        <rdfs:comment xml:lang="en">Word that sounds the same and is written the same as another word but is different in meaning.</rdfs:comment>
        <rdfs:comment xml:lang="ru">Слово, которое имеет сходное звучание и написание с другим словом, но отличается по смыслу.</rdfs:comment>
        <dc:creator>Wright, Sue Ellen</dc:creator>
        <rdfs:subPropertyOf rdf:resource="&lemon;lexicalVariant"/>
        <dcr:datcat rdf:resource="http://www.isocat.org/datcat/DC-1301"/>
        <dcr:datcat rdf:resource="http://www.isocat.org/datcat/DC-262"/>
        <rdfs:isDefinedBy rdf:resource="http://www.lexinfo.net/ontology/2.0/lexinfo"/>
    </owl:ObjectProperty>
    


    <!-- http://www.lexinfo.net/ontology/2.0/lexinfo#homophone -->

    <owl:ObjectProperty rdf:about="&lexinfo;homophone">
        <rdfs:label xml:lang="en">homophone</rdfs:label>
        <rdfs:label xml:lang="ru">омофон</rdfs:label>        
        <dc:creator>Francopoulo, Gil</dc:creator>
        <rdfs:comment xml:lang="en">Word that sounds like another word, but is different in writiing or meaning.</rdfs:comment>
        <rdfs:comment xml:lang="ru">Слово, звучащее так же, как другое слово, но отличающееся написанием или значением.</rdfs:comment>
        <owl:versionInfo>1:0</owl:versionInfo>
        <rdfs:comment xml:lang="en">A word that is pronounced in the same way as another word but that is spelled differently.</rdfs:comment>
        <rdfs:comment xml:lang="ru">Слово, произносимое так же, как и другое слово, но имеющее другое написание.</rdfs:comment>
        <dc:creator>Wright, Sue Ellen</dc:creator>
        <rdfs:subPropertyOf rdf:resource="&lemon;lexicalVariant"/>
        <dcr:datcat rdf:resource="http://www.isocat.org/datcat/DC-1302"/>
        <dcr:datcat rdf:resource="http://www.isocat.org/datcat/DC-263"/>
        <rdfs:isDefinedBy rdf:resource="http://www.lexinfo.net/ontology/2.0/lexinfo"/>
    </owl:ObjectProperty>
    


    <!-- http://www.lexinfo.net/ontology/2.0/lexinfo#hypernym -->

    <owl:ObjectProperty rdf:about="&lexinfo;hypernym">
        <rdfs:subPropertyOf rdf:resource="&lemon;broader"/>
        <rdfs:isDefinedBy rdf:resource="http://www.lexinfo.net/ontology/2.0/lexinfo"/>
    </owl:ObjectProperty>
    


    <!-- http://www.lexinfo.net/ontology/2.0/lexinfo#hyponym -->

    <owl:ObjectProperty rdf:about="&lexinfo;hyponym">
        <rdfs:subPropertyOf rdf:resource="&lemon;narrower"/>
        <rdfs:isDefinedBy rdf:resource="http://www.lexinfo.net/ontology/2.0/lexinfo"/>
    </owl:ObjectProperty>
    


    <!-- http://www.lexinfo.net/ontology/2.0/lexinfo#imperativeMoodForm -->

    <owl:ObjectProperty rdf:about="&lexinfo;imperativeMoodForm">
        <rdfs:isDefinedBy rdf:resource="http://www.lexinfo.net/ontology/2.0/lexinfo"/>
        <rdfs:subPropertyOf rdf:resource="&lexinfo;formMoodVariant"/>
    </owl:ObjectProperty>
    


    <!-- http://www.lexinfo.net/ontology/2.0/lexinfo#imperfectTenseForm -->

    <owl:ObjectProperty rdf:about="&lexinfo;imperfectTenseForm">
        <rdfs:isDefinedBy rdf:resource="http://www.lexinfo.net/ontology/2.0/lexinfo"/>
        <rdfs:subPropertyOf rdf:resource="&lexinfo;formTenseVariant"/>
    </owl:ObjectProperty>
    


    <!-- http://www.lexinfo.net/ontology/2.0/lexinfo#indicativeMoodForm -->

    <owl:ObjectProperty rdf:about="&lexinfo;indicativeMoodForm">
        <rdfs:isDefinedBy rdf:resource="http://www.lexinfo.net/ontology/2.0/lexinfo"/>
        <rdfs:subPropertyOf rdf:resource="&lexinfo;formMoodVariant"/>
    </owl:ObjectProperty>
    


    <!-- http://www.lexinfo.net/ontology/2.0/lexinfo#indirectObject -->

    <owl:ObjectProperty rdf:about="&lexinfo;indirectObject">
        <rdfs:label xml:lang="en">indirect object</rdfs:label>
        <rdfs:label xml:lang="ru">косвенное дополнение</rdfs:label>        
        <rdfs:comment xml:lang="en">An indirect object is a grammatical relation that is one means of expressing the semantic role of goal and other similar roles. It is proposed for languages in which the role is distinct from the direct object and the oblique object on the basis of multiple independent syntactic or morphological criteria, such as the following: - Having a particular case marking, commonly dative - Governing an agreement affix on the verb, such as person or number - Being distinct from oblique relations in that it may be relativized</rdfs:comment>
        <rdfs:comment xml:lang="ru">Косвенное дополнение - грамматическое отношение, которое является одним из средств выражения семантической роли цели и других подобных ролей. Оно встречается в языках, в которых значение отличается от прямого дополнения и косвенного дополнения на основе множественных независимых синтаксических или морфологических критериев таких, как:- наличие падежа, обычно дательного; - добавление к глаголу аффикса, выражающего лицо или число,- отличие от косвенных отношений в том, что он может быть релятивизирован</rdfs:comment>
        <dcr:datcat rdf:resource="http://www.isocat.org/datcat/DC-1310"/>
        <rdfs:isDefinedBy rdf:resource="http://www.lexinfo.net/ontology/2.0/lexinfo"/>
        <rdfs:range rdf:resource="&lexinfo;IndirectObject"/>
        <rdfs:subPropertyOf rdf:resource="&lexinfo;object"/>
    </owl:ObjectProperty>
    


    <!-- http://www.lexinfo.net/ontology/2.0/lexinfo#infinitiveClause -->

    <owl:ObjectProperty rdf:about="&lexinfo;infinitiveClause">
        <rdfs:isDefinedBy rdf:resource="http://www.lexinfo.net/ontology/2.0/lexinfo"/>
        <rdfs:subPropertyOf rdf:resource="&lexinfo;clausalArg"/>
    </owl:ObjectProperty>
    


    <!-- http://www.lexinfo.net/ontology/2.0/lexinfo#initialismFor -->

    <owl:ObjectProperty rdf:about="&lexinfo;initialismFor">
        <rdfs:label xml:lang="en">initialismFor</rdfs:label>
        <rdfs:label xml:lang="ru">аббревиатура для</rdfs:label>
        <owl:versionInfo>1:0</owl:versionInfo>
        <dc:creator>Wright, Sue Ellen</dc:creator>
        <rdfs:comment xml:lang="en">A linking element used to identify a relation between an initialism and its full or expanded form.</rdfs:comment>
        <rdfs:comment xml:lang="ru">Связующий элемент, используемый для идентификации отношения между аббревиатурой и её полной или расширенной формой.</rdfs:comment>
        <dcr:datcat rdf:resource="http://www.isocat.org/datcat/DC-272"/>
        <rdfs:isDefinedBy rdf:resource="http://www.lexinfo.net/ontology/2.0/lexinfo"/>
        <rdfs:subPropertyOf rdf:resource="&lexinfo;contractionFor"/>
    </owl:ObjectProperty>
    


    <!-- http://www.lexinfo.net/ontology/2.0/lexinfo#interrogativeClause -->

    <owl:ObjectProperty rdf:about="&lexinfo;interrogativeClause">
        <rdfs:isDefinedBy rdf:resource="http://www.lexinfo.net/ontology/2.0/lexinfo"/>
        <rdfs:subPropertyOf rdf:resource="&lexinfo;clausalArg"/>
    </owl:ObjectProperty>
    


    <!-- http://www.lexinfo.net/ontology/2.0/lexinfo#interrogativeInfinitiveClause -->

    <owl:ObjectProperty rdf:about="&lexinfo;interrogativeInfinitiveClause">
        <rdfs:isDefinedBy rdf:resource="http://www.lexinfo.net/ontology/2.0/lexinfo"/>
        <rdfs:subPropertyOf rdf:resource="&lexinfo;clausalArg"/>
    </owl:ObjectProperty>
    


    <!-- http://www.lexinfo.net/ontology/2.0/lexinfo#memberHolonym -->

    <owl:ObjectProperty rdf:about="&lexinfo;memberHolonym">
        <rdfs:label xml:lang="en">member holonym</rdfs:label>
        <rdfs:label xml:lang="ru">член холоним</rdfs:label>
        <rdfs:comment xml:lang="en">Indicates the object is a member of this</rdfs:comment>
        <rdfs:comment xml:lang="ru">Указывает, что объект является его членом</rdfs:comment>
        <rdfs:isDefinedBy rdf:resource="http://www.lexinfo.net/ontology/2.0/lexinfo"/>
        <rdfs:subPropertyOf rdf:resource="&lexinfo;holonymTerm"/>
    </owl:ObjectProperty>
    


    <!-- http://www.lexinfo.net/ontology/2.0/lexinfo#memberMeronym -->

    <owl:ObjectProperty rdf:about="&lexinfo;memberMeronym">
        <rdfs:label xml:lang="en">member meronym</rdfs:label>
        <rdfs:label xml:lang="ru">член мероним</rdfs:label>        
        <rdfs:comment xml:lang="en">Indicates this is an element of the other</rdfs:comment>
        <rdfs:comment xml:lang="ru">Указывает, что данный элемент является элементом другого.</rdfs:comment>
        <rdfs:isDefinedBy rdf:resource="http://www.lexinfo.net/ontology/2.0/lexinfo"/>
        <rdfs:subPropertyOf rdf:resource="&lexinfo;meronymTerm"/>
    </owl:ObjectProperty>
    


    <!-- http://www.lexinfo.net/ontology/2.0/lexinfo#meronymTerm -->

    <owl:ObjectProperty rdf:about="&lexinfo;meronymTerm">
        <rdfs:label xml:lang="en">meronym</rdfs:label>
        <rdfs:label xml:lang="ru">мероним</rdfs:label>        
        <rdfs:comment xml:lang="en">Indicates this is a part of another concept</rdfs:comment>
        <rdfs:comment xml:lang="ru">Указывает, что данный элемент является частью другого понятия.</rdfs:comment>
        <rdfs:isDefinedBy rdf:resource="http://www.lexinfo.net/ontology/2.0/lexinfo"/>
        <rdfs:subPropertyOf rdf:resource="&lexinfo;partitiveRelation"/>
    </owl:ObjectProperty>
    


    <!-- http://www.lexinfo.net/ontology/2.0/lexinfo#modificationType -->

    <owl:ObjectProperty rdf:about="&lexinfo;modificationType">
        <rdfs:label xml:lang="en">modification type</rdfs:label>
        <rdfs:label xml:lang="ru">тип модификации</rdfs:label>        
        <owl:versionInfo>1:0</owl:versionInfo>
        <rdfs:comment xml:lang="en">Refers to the prenominal or postnominal positions of determiners which distinguish different forms.</rdfs:comment>
        <rdfs:comment xml:lang="ru">Относится к преноминальным и постноминальным определителям, т.е. стоящим перед или после существительного, которые служат для дифференциации форм.</rdfs:comment>
        <dc:creator>Francopoulo, Gil</dc:creator>
        <dcr:datcat rdf:resource="http://www.isocat.org/datcat/DC-1931"/>
        <rdfs:isDefinedBy rdf:resource="http://www.lexinfo.net/ontology/2.0/lexinfo"/>
        <rdfs:range rdf:resource="&lexinfo;ModificationType"/>
        <rdfs:subPropertyOf rdf:resource="&lexinfo;morphosyntacticProperty"/>
    </owl:ObjectProperty>
    


    <!-- http://www.lexinfo.net/ontology/2.0/lexinfo#mood -->

    <owl:ObjectProperty rdf:about="&lexinfo;mood">
        <rdfs:label xml:lang="en">mood</rdfs:label>
        <rdfs:label xml:lang="ru">наклонение</rdfs:label>        
        <rdfs:comment xml:lang="en">In TEI: contains information about the grammatical mood of verbs (e.g. indicative, subjunctive, imperative).</rdfs:comment>
        <rdfs:comment xml:lang="ru">В ИКТ (TEI): содержит информацию о грамматическом наклонении глагола (например, изъявительное, сослагательное, повелительное).</rdfs:comment>
        <owl:versionInfo>1:0</owl:versionInfo>
        <dc:creator>Wright, Sue Ellen</dc:creator>
        <dcr:datcat rdf:resource="http://www.isocat.org/datcat/DC-366"/>
        <rdfs:isDefinedBy rdf:resource="http://www.lexinfo.net/ontology/2.0/lexinfo"/>
        <rdfs:range rdf:resource="&lexinfo;Mood"/>
        <rdfs:subPropertyOf rdf:resource="&lexinfo;morphosyntacticProperty"/>
    </owl:ObjectProperty>
    


    <!-- http://www.lexinfo.net/ontology/2.0/lexinfo#morphosyntacticProperty -->

    <owl:ObjectProperty rdf:about="&lexinfo;morphosyntacticProperty">
        <rdfs:subPropertyOf rdf:resource="&lemon;property"/>
        <rdfs:isDefinedBy rdf:resource="http://www.lexinfo.net/ontology/2.0/lexinfo"/>
        <rdfs:range rdf:resource="&lexinfo;MorphosyntacticProperty"/>
    </owl:ObjectProperty>
    


    <!-- http://www.lexinfo.net/ontology/2.0/lexinfo#negative -->

    <owl:ObjectProperty rdf:about="&lexinfo;negative">
        <rdfs:label xml:lang="en">negative</rdfs:label>
        <rdfs:label xml:lang="ru">отрицание</rdfs:label>        
        <dc:creator>Francopoulo, Gil</dc:creator>
        <rdfs:comment xml:lang="en">denotes the negation or the absence</rdfs:comment>
        <rdfs:comment xml:lang="ru">обозначает отрицание или отсутствие</rdfs:comment>
        <owl:versionInfo>1:0</owl:versionInfo>
        <dcr:datcat rdf:resource="http://www.isocat.org/datcat/DC-1839"/>
        <rdfs:isDefinedBy rdf:resource="http://www.lexinfo.net/ontology/2.0/lexinfo"/>
        <rdfs:range rdf:resource="&lexinfo;Negative"/>
        <rdfs:subPropertyOf rdf:resource="&lexinfo;morphosyntacticProperty"/>
    </owl:ObjectProperty>
    


    <!-- http://www.lexinfo.net/ontology/2.0/lexinfo#negativeForm -->

    <owl:ObjectProperty rdf:about="&lexinfo;negativeForm">
        <rdfs:isDefinedBy rdf:resource="http://www.lexinfo.net/ontology/2.0/lexinfo"/>
        <rdfs:subPropertyOf rdf:resource="&lexinfo;formPositivityVariant"/>
    </owl:ObjectProperty>
    


    <!-- http://www.lexinfo.net/ontology/2.0/lexinfo#nominativeCaseForm -->

    <owl:ObjectProperty rdf:about="&lexinfo;nominativeCaseForm">
        <rdfs:isDefinedBy rdf:resource="http://www.lexinfo.net/ontology/2.0/lexinfo"/>
        <rdfs:subPropertyOf rdf:resource="&lexinfo;formCaseVariant"/>
    </owl:ObjectProperty>
    


    <!-- http://www.lexinfo.net/ontology/2.0/lexinfo#normativeAuthorization -->

    <owl:ObjectProperty rdf:about="&lexinfo;normativeAuthorization">
        <rdfs:label xml:lang="en">normative authorization</rdfs:label>
        <rdfs:label xml:lang="ru">нормативное</rdfs:label>        
        <dc:creator>Wright, Sue Ellen</dc:creator>
        <owl:versionInfo>1:0</owl:versionInfo>
        <rdfs:comment xml:lang="en">A term status qualifier assigned by an authoritative body, such as a standards body or a governmental entity with a regulatory function.</rdfs:comment>
        <rdfs:comment xml:lang="ru">Определитель статуса термина, предписанный официальный органом таким, как учреждение стандартизации или государственная организация, выполняющая нормативно-регулятивную функцию.</rdfs:comment>
        <rdfs:subPropertyOf rdf:resource="&lemon;context"/>
        <dcr:datcat rdf:resource="http://www.isocat.org/datcat/DC-374"/>
        <rdfs:isDefinedBy rdf:resource="http://www.lexinfo.net/ontology/2.0/lexinfo"/>
        <rdfs:range rdf:resource="&lexinfo;NormativeAuthorization"/>
    </owl:ObjectProperty>
    


    <!-- http://www.lexinfo.net/ontology/2.0/lexinfo#note -->

    <owl:ObjectProperty rdf:about="&lexinfo;note">
        <rdfs:label xml:lang="en">note</rdfs:label>
        <rdfs:label xml:lang="ru">примечание</rdfs:label>        
        <rdfs:comment xml:lang="en">A statement that provides further information on any part of a language resource entry.</rdfs:comment>
        <rdfs:comment xml:lang="ru">Утверждение, дающее дополнительную информацию о любом разделе словарной статьи, описывающей ресурсы языка.</rdfs:comment>        
        <dc:creator>Wright, Sue Ellen</dc:creator>
        <owl:versionInfo>1:0</owl:versionInfo>
        <rdfs:subPropertyOf rdf:resource="&lemon;definition"/>
        <dcr:datcat rdf:resource="http://www.isocat.org/datcat/DC-382"/>
        <rdfs:isDefinedBy rdf:resource="http://www.lexinfo.net/ontology/2.0/lexinfo"/>
    </owl:ObjectProperty>
    


    <!-- http://www.lexinfo.net/ontology/2.0/lexinfo#number -->

    <owl:ObjectProperty rdf:about="&lexinfo;number">
        <rdfs:label xml:lang="en">grammatical number</rdfs:label>
        <rdfs:label xml:lang="ru">грамматическое число</rdfs:label>
        <dc:creator>Wright, Sue Ellen</dc:creator>
        <rdfs:comment xml:lang="en">Grammatical category for the variation in form of nouns, pronouns, and any words agreeing with them, depending on how many persons or things are referred to.</rdfs:comment>
        <rdfs:comment xml:lang="ru">Грамматическая категория для изменения формы существительных, местоимений и любых других слов, согласующихся с ними, в зависимости от того, сколько человек или вещей обозначаются.</rdfs:comment>
        <rdfs:comment xml:lang="en">In many languages, the grammatical distinction that indicates the number of objects referred to by the term or word.</rdfs:comment>
        <rdfs:comment xml:lang="ru">Во многих языках грамматическая дифференциация, указывающая на количество объектов, обозначаемых термином или словом.</rdfs:comment>
        <owl:versionInfo>1:0</owl:versionInfo>
        <dc:creator>Francopoulo, Gil</dc:creator>
        <dcr:datcat rdf:resource="http://www.isocat.org/datcat/DC-1298"/>
        <dcr:datcat rdf:resource="http://www.isocat.org/datcat/DC-251"/>
        <rdfs:isDefinedBy rdf:resource="http://www.lexinfo.net/ontology/2.0/lexinfo"/>
        <rdfs:range rdf:resource="&lexinfo;Number"/>
        <rdfs:subPropertyOf rdf:resource="&lexinfo;morphosyntacticProperty"/>
    </owl:ObjectProperty>
    


    <!-- http://www.lexinfo.net/ontology/2.0/lexinfo#object -->

    <owl:ObjectProperty rdf:about="&lexinfo;object">
        <rdfs:subPropertyOf rdf:resource="&lemon;synArg"/>
        <rdfs:isDefinedBy rdf:resource="http://www.lexinfo.net/ontology/2.0/lexinfo"/>
        <rdfs:range rdf:resource="&lexinfo;Object"/>
    </owl:ObjectProperty>
    


    <!-- http://www.lexinfo.net/ontology/2.0/lexinfo#objectComplement -->

    <owl:ObjectProperty rdf:about="&lexinfo;objectComplement">
        <rdfs:isDefinedBy rdf:resource="http://www.lexinfo.net/ontology/2.0/lexinfo"/>
        <rdfs:range rdf:resource="&lexinfo;ObjectComplement"/>
        <rdfs:subPropertyOf rdf:resource="&lexinfo;complement"/>
    </owl:ObjectProperty>
    


    <!-- http://www.lexinfo.net/ontology/2.0/lexinfo#partHolonym -->

    <owl:ObjectProperty rdf:about="&lexinfo;partHolonym">
        <rdfs:label xml:lang="en">part holonym</rdfs:label>
        <rdfs:label xml:lang="ru">часть холоним</rdfs:label>        
        <rdfs:comment xml:lang="en">Indicates a part of this object</rdfs:comment>
        <rdfs:comment xml:lang="ru">Обозначает часть данного объекта</rdfs:comment>        
        <rdfs:isDefinedBy rdf:resource="http://www.lexinfo.net/ontology/2.0/lexinfo"/>
        <rdfs:subPropertyOf rdf:resource="&lexinfo;holonymTerm"/>
    </owl:ObjectProperty>
    


    <!-- http://www.lexinfo.net/ontology/2.0/lexinfo#partMeronym -->

    <owl:ObjectProperty rdf:about="&lexinfo;partMeronym">
        <rdfs:label xml:lang="en">part meronym</rdfs:label>
        <rdfs:label xml:lang="ru">часть мероним</rdfs:label>        
        <rdfs:comment xml:lang="en">Indicates this a component of the other concept</rdfs:comment>
        <rdfs:comment xml:lang="ru">Обозначает, что это является компонентом другого понятия.</rdfs:comment>
        <rdfs:isDefinedBy rdf:resource="http://www.lexinfo.net/ontology/2.0/lexinfo"/>
        <rdfs:subPropertyOf rdf:resource="&lexinfo;meronymTerm"/>
    </owl:ObjectProperty>
    


    <!-- http://www.lexinfo.net/ontology/2.0/lexinfo#partOfSpeech -->

    <owl:ObjectProperty rdf:about="&lexinfo;partOfSpeech">
        <rdfs:label xml:lang="en">part of speech</rdfs:label>
        <rdfs:label xml:lang="ru">часть речи</rdfs:label>        
        <rdfs:comment xml:lang="en">Term used to describe how a particular word is used in a sentence.</rdfs:comment>
        <rdfs:comment xml:lang="ru">Термин, используемый для описания того, как отдельное слово используется в предложении.</rdfs:comment>        
        <rdfs:comment xml:lang="en">A category assigned to a word based on its grammatical and semantic properties.</rdfs:comment>
        <rdfs:comment xml:lang="ru">Категория, приписанная слову, на основе его грамматических и семантических свойств.</rdfs:comment>        
        <dc:creator>Wright, Sue Ellen</dc:creator>
        <owl:versionInfo>1:0</owl:versionInfo>
        <dc:creator>Francopoulo, Gil</dc:creator>
        <dcr:datcat rdf:resource="http://www.isocat.org/datcat/DC-1345"/>
        <dcr:datcat rdf:resource="http://www.isocat.org/datcat/DC-396"/>
        <rdfs:isDefinedBy rdf:resource="http://www.lexinfo.net/ontology/2.0/lexinfo"/>
        <rdfs:range rdf:resource="&lexinfo;PartOfSpeech"/>
        <rdfs:subPropertyOf rdf:resource="&lexinfo;morphosyntacticProperty"/>
    </owl:ObjectProperty>
    


    <!-- http://www.lexinfo.net/ontology/2.0/lexinfo#participleFormOf -->

    <owl:ObjectProperty rdf:about="&lexinfo;participleFormOf">
        <rdfs:comment xml:lang="en">Indicates that one lexical entry is the participle form of another, e.g., the adjective &apos;reassuring&apos; is the participle of &apos;to reassure&apos;</rdfs:comment>
        <rdfs:comment xml:lang="ru">Указывает, что одна лексическая сущность является причастной формой другой сущности, например, reassuring/обнадёживающий - это причастная форма reassure/обнадёживать</rdfs:comment>        
        <rdfs:isDefinedBy rdf:resource="http://www.lexinfo.net/ontology/2.0/lexinfo"/>
        <rdfs:subPropertyOf rdf:resource="&lexinfo;derivedForm"/>
    </owl:ObjectProperty>
    


    <!-- http://www.lexinfo.net/ontology/2.0/lexinfo#partitiveRelation -->

    <owl:ObjectProperty rdf:about="&lexinfo;partitiveRelation">
        <rdfs:label xml:lang="en">partitive relation</rdfs:label>
        <rdfs:label xml:lang="ru">партитивное отношение</rdfs:label>        
        <rdfs:comment xml:lang="en">A relation between two concepts where one of the concepts constitutes the whole and the other concept a part of that whole.</rdfs:comment>
        <rdfs:comment xml:lang="ru">Отношение между двумя понятиями, в котором одно понятие составляет целое, а второе – часть того целого.</rdfs:comment>
        <owl:versionInfo>1:0</owl:versionInfo>
        <dc:creator>Wright, Sue Ellen</dc:creator>
        <rdfs:subPropertyOf rdf:resource="&lemon;senseRelation"/>
        <dcr:datcat rdf:resource="http://www.isocat.org/datcat/DC-397"/>
        <rdfs:isDefinedBy rdf:resource="http://www.lexinfo.net/ontology/2.0/lexinfo"/>
    </owl:ObjectProperty>
    


    <!-- http://www.lexinfo.net/ontology/2.0/lexinfo#pastTenseForm -->

    <owl:ObjectProperty rdf:about="&lexinfo;pastTenseForm">
        <rdfs:isDefinedBy rdf:resource="http://www.lexinfo.net/ontology/2.0/lexinfo"/>
        <rdfs:subPropertyOf rdf:resource="&lexinfo;formTenseVariant"/>
    </owl:ObjectProperty>
    


    <!-- http://www.lexinfo.net/ontology/2.0/lexinfo#person -->

    <owl:ObjectProperty rdf:about="&lexinfo;person">
        <rdfs:label xml:lang="en">person</rdfs:label>
        <rdfs:label xml:lang="ru">лицо</rdfs:label>        
        <owl:versionInfo>1:0</owl:versionInfo>
        <rdfs:comment xml:lang="en">Indication of grammatical person (1st, 2nd, 3rd, etc.) associated with a given inflected form.</rdfs:comment>
        <rdfs:comment xml:lang="ru">Обозначение грамматического лица (1 л., 2л., 3 л. и т.д.), связанное с данной флективной формой.</rdfs:comment>
        <dc:creator>Francopoulo, Gil</dc:creator>
        <dcr:datcat rdf:resource="http://www.isocat.org/datcat/DC-1328"/>
        <rdfs:isDefinedBy rdf:resource="http://www.lexinfo.net/ontology/2.0/lexinfo"/>
        <rdfs:range rdf:resource="&lexinfo;Person"/>
        <rdfs:subPropertyOf rdf:resource="&lexinfo;morphosyntacticProperty"/>
    </owl:ObjectProperty>
    


    <!-- http://www.lexinfo.net/ontology/2.0/lexinfo#pertainsTo -->

    <owl:ObjectProperty rdf:about="&lexinfo;pertainsTo">
        <rdfs:subPropertyOf rdf:resource="&lemon;senseRelation"/>
        <rdfs:isDefinedBy rdf:resource="http://www.lexinfo.net/ontology/2.0/lexinfo"/>
    </owl:ObjectProperty>
    


    <!-- http://www.lexinfo.net/ontology/2.0/lexinfo#pluralNumberForm -->

    <owl:ObjectProperty rdf:about="&lexinfo;pluralNumberForm">
        <rdfs:isDefinedBy rdf:resource="http://www.lexinfo.net/ontology/2.0/lexinfo"/>
        <rdfs:subPropertyOf rdf:resource="&lexinfo;formNumberVariant"/>
    </owl:ObjectProperty>
    


    <!-- http://www.lexinfo.net/ontology/2.0/lexinfo#positiveDegreeForm -->

    <owl:ObjectProperty rdf:about="&lexinfo;positiveDegreeForm">
        <rdfs:isDefinedBy rdf:resource="http://www.lexinfo.net/ontology/2.0/lexinfo"/>
        <rdfs:subPropertyOf rdf:resource="&lexinfo;formDegreeVariant"/>
    </owl:ObjectProperty>
    


    <!-- http://www.lexinfo.net/ontology/2.0/lexinfo#positiveForm -->

    <owl:ObjectProperty rdf:about="&lexinfo;positiveForm">
        <rdfs:isDefinedBy rdf:resource="http://www.lexinfo.net/ontology/2.0/lexinfo"/>
        <rdfs:subPropertyOf rdf:resource="&lexinfo;formPositivityVariant"/>
    </owl:ObjectProperty>
    


    <!-- http://www.lexinfo.net/ontology/2.0/lexinfo#possessiveAdjunct -->

    <owl:ObjectProperty rdf:about="&lexinfo;possessiveAdjunct">
        <rdfs:isDefinedBy rdf:resource="http://www.lexinfo.net/ontology/2.0/lexinfo"/>
        <rdfs:range rdf:resource="&lexinfo;PossessiveAdjunct"/>
        <rdfs:subPropertyOf rdf:resource="&lexinfo;adjunct"/>
    </owl:ObjectProperty>
    


    <!-- http://www.lexinfo.net/ontology/2.0/lexinfo#possessiveInfinitiveClause -->

    <owl:ObjectProperty rdf:about="&lexinfo;possessiveInfinitiveClause">
        <rdfs:isDefinedBy rdf:resource="http://www.lexinfo.net/ontology/2.0/lexinfo"/>
        <rdfs:subPropertyOf rdf:resource="&lexinfo;clausalArg"/>
    </owl:ObjectProperty>
    


    <!-- http://www.lexinfo.net/ontology/2.0/lexinfo#postPositiveArg -->

    <owl:ObjectProperty rdf:about="&lexinfo;postPositiveArg">
        <rdfs:comment xml:lang="en">Indicates an argument of an adjective indicated by post-positive modification. An example in english would be that &quot;that is something interesting&quot;, where the adjective interesting post-postively modifies something</rdfs:comment>
        <rdfs:comment xml:lang="ru">Указывает на прилагательное в постпозитивной форме (т.е. находится в позиции после определяемого слова). Пример для русского языка - "это что-то интересное", где прилагательное "интересное" постпозитивно определяет "что-то".</rdfs:comment>
        <rdfs:subPropertyOf rdf:resource="&lemon;synArg"/>
        <rdfs:isDefinedBy rdf:resource="http://www.lexinfo.net/ontology/2.0/lexinfo"/>
        <rdfs:range rdf:resource="&lexinfo;PostPositiveArgument"/>
    </owl:ObjectProperty>
    


    <!-- http://www.lexinfo.net/ontology/2.0/lexinfo#predicativeAdjective -->

    <owl:ObjectProperty rdf:about="&lexinfo;predicativeAdjective">
        <rdfs:isDefinedBy rdf:resource="http://www.lexinfo.net/ontology/2.0/lexinfo"/>
        <rdfs:range rdf:resource="&lexinfo;PredicativeAdjective"/>
        <rdfs:subPropertyOf rdf:resource="&lexinfo;complement"/>
    </owl:ObjectProperty>
    


    <!-- http://www.lexinfo.net/ontology/2.0/lexinfo#predicativeAdjunct -->

    <owl:ObjectProperty rdf:about="&lexinfo;predicativeAdjunct">
        <rdfs:isDefinedBy rdf:resource="http://www.lexinfo.net/ontology/2.0/lexinfo"/>
        <rdfs:range rdf:resource="&lexinfo;Adjunct"/>
        <rdfs:subPropertyOf rdf:resource="&lexinfo;adjunct"/>
    </owl:ObjectProperty>
    


    <!-- http://www.lexinfo.net/ontology/2.0/lexinfo#predicativeAdverb -->

    <owl:ObjectProperty rdf:about="&lexinfo;predicativeAdverb">
        <rdfs:isDefinedBy rdf:resource="http://www.lexinfo.net/ontology/2.0/lexinfo"/>
        <rdfs:range rdf:resource="&lexinfo;PredicativeAdverb"/>
        <rdfs:subPropertyOf rdf:resource="&lexinfo;complement"/>
    </owl:ObjectProperty>
    


    <!-- http://www.lexinfo.net/ontology/2.0/lexinfo#predicativeNominative -->

    <owl:ObjectProperty rdf:about="&lexinfo;predicativeNominative">
        <rdfs:isDefinedBy rdf:resource="http://www.lexinfo.net/ontology/2.0/lexinfo"/>
        <rdfs:range rdf:resource="&lexinfo;PredicativeNominative"/>
        <rdfs:subPropertyOf rdf:resource="&lexinfo;complement"/>
    </owl:ObjectProperty>
    


    <!-- http://www.lexinfo.net/ontology/2.0/lexinfo#prepositionalAdjunct -->

    <owl:ObjectProperty rdf:about="&lexinfo;prepositionalAdjunct">
        <rdfs:isDefinedBy rdf:resource="http://www.lexinfo.net/ontology/2.0/lexinfo"/>
        <rdfs:range rdf:resource="&lexinfo;PrepositionalAdjunct"/>
        <rdfs:subPropertyOf rdf:resource="&lexinfo;adjunct"/>
    </owl:ObjectProperty>
    


    <!-- http://www.lexinfo.net/ontology/2.0/lexinfo#prepositionalGerundClause -->

    <owl:ObjectProperty rdf:about="&lexinfo;prepositionalGerundClause">
        <rdfs:isDefinedBy rdf:resource="http://www.lexinfo.net/ontology/2.0/lexinfo"/>
        <rdfs:subPropertyOf rdf:resource="&lexinfo;clausalArg"/>
    </owl:ObjectProperty>
    


    <!-- http://www.lexinfo.net/ontology/2.0/lexinfo#prepositionalInterrogativeClause -->

    <owl:ObjectProperty rdf:about="&lexinfo;prepositionalInterrogativeClause">
        <rdfs:isDefinedBy rdf:resource="http://www.lexinfo.net/ontology/2.0/lexinfo"/>
        <rdfs:subPropertyOf rdf:resource="&lexinfo;clausalArg"/>
    </owl:ObjectProperty>
    


    <!-- http://www.lexinfo.net/ontology/2.0/lexinfo#prepositionalObject -->

    <owl:ObjectProperty rdf:about="&lexinfo;prepositionalObject">
        <rdfs:isDefinedBy rdf:resource="http://www.lexinfo.net/ontology/2.0/lexinfo"/>
        <rdfs:range rdf:resource="&lexinfo;PrepositionalObject"/>
        <rdfs:subPropertyOf rdf:resource="&lexinfo;adpositionalObject"/>
    </owl:ObjectProperty>
    


    <!-- http://www.lexinfo.net/ontology/2.0/lexinfo#presentTenseForm -->

    <owl:ObjectProperty rdf:about="&lexinfo;presentTenseForm">
        <rdfs:isDefinedBy rdf:resource="http://www.lexinfo.net/ontology/2.0/lexinfo"/>
        <rdfs:subPropertyOf rdf:resource="&lexinfo;formTenseVariant"/>
    </owl:ObjectProperty>
    


    <!-- http://www.lexinfo.net/ontology/2.0/lexinfo#quasiEquivalent -->

    <owl:ObjectProperty rdf:about="&lexinfo;quasiEquivalent">
        <rdfs:subPropertyOf rdf:resource="&lemon;senseRelation"/>
        <dcr:datcat rdf:resource="http://www.isocat.org/datcat/DC-177"/>
        <rdfs:isDefinedBy rdf:resource="http://www.lexinfo.net/ontology/2.0/lexinfo"/>
    </owl:ObjectProperty>
    


    <!-- http://www.lexinfo.net/ontology/2.0/lexinfo#referentType -->

    <owl:ObjectProperty rdf:about="&lexinfo;referentType">
        <rdfs:label xml:lang="en">referent type</rdfs:label>
        <rdfs:label xml:lang="ru">Тип референта</rdfs:label>        
        <dc:creator>Francopoulo, Gil</dc:creator>
        <rdfs:comment xml:lang="en">Type of concrete object or concept (the referent) that an expression represents (the reference).</rdfs:comment>
        <rdfs:comment xml:lang="ru">Тип конкретного объекта или понятия (референт), который представлен выражением (референция).</rdfs:comment>
        <owl:versionInfo>1:0</owl:versionInfo>
        <dcr:datcat rdf:resource="http://www.isocat.org/datcat/DC-1376"/>
        <rdfs:isDefinedBy rdf:resource="http://www.lexinfo.net/ontology/2.0/lexinfo"/>
        <rdfs:range rdf:resource="&lexinfo;ReferentType"/>
        <rdfs:subPropertyOf rdf:resource="&lexinfo;morphosyntacticProperty"/>
    </owl:ObjectProperty>
    


    <!-- http://www.lexinfo.net/ontology/2.0/lexinfo#register -->

    <owl:ObjectProperty rdf:about="&lexinfo;register">
        <rdfs:label xml:lang="en">register</rdfs:label>
        <rdfs:label xml:lang="ru">реестр</rdfs:label>        
        <rdfs:comment xml:lang="en">Classification indicating the relative level of language individually assigned to a lexeme or term or to a text type.</rdfs:comment>
        <rdfs:comment xml:lang="ru">Классификация, указывающая на относительный уровень языка, индивидуально приписанный лексеме, или термину, или типу текста.</rdfs:comment>
        <dc:creator>Wright, Sue Ellen</dc:creator>
        <owl:versionInfo>1:0</owl:versionInfo>
        <dc:creator>Francopoulo, Gil</dc:creator>
        <rdfs:subPropertyOf rdf:resource="&lemon;context"/>
        <dcr:datcat rdf:resource="http://www.isocat.org/datcat/DC-1988"/>
        <dcr:datcat rdf:resource="http://www.isocat.org/datcat/DC-423"/>
        <rdfs:isDefinedBy rdf:resource="http://www.lexinfo.net/ontology/2.0/lexinfo"/>
        <rdfs:range rdf:resource="&lexinfo;Register"/>
    </owl:ObjectProperty>
    


    <!-- http://www.lexinfo.net/ontology/2.0/lexinfo#relatedTerm -->

    <owl:ObjectProperty rdf:about="&lexinfo;relatedTerm">
        <rdfs:label xml:lang="en">relatedTerm</rdfs:label>
        <rdfs:label xml:lang="ru">родственный термин</rdfs:label>        
        <rdfs:comment xml:lang="en">A term connected to another term by a coordinate or associative relation.</rdfs:comment>
        <rdfs:comment xml:lang="ru">Термин, связанный с другим термином сочинительным или ассоциативным отношением.</rdfs:comment>
        <owl:versionInfo>1:0</owl:versionInfo>
        <dc:creator>Wright, Sue Ellen</dc:creator>
        <rdfs:subPropertyOf rdf:resource="&lemon;senseRelation"/>
        <dcr:datcat rdf:resource="http://www.isocat.org/datcat/DC-438"/>
        <rdfs:isDefinedBy rdf:resource="http://www.lexinfo.net/ontology/2.0/lexinfo"/>
    </owl:ObjectProperty>
    


    <!-- http://www.lexinfo.net/ontology/2.0/lexinfo#root -->

    <owl:ObjectProperty rdf:about="&lexinfo;root">
        <rdfs:label xml:lang="en">root</rdfs:label>
        <rdfs:label xml:lang="ru">основа</rdfs:label>        
        <rdfs:comment xml:lang="en">base of a word</rdfs:comment>
        <rdfs:comment xml:lang="ru">основа слова</rdfs:comment>
        <owl:versionInfo>1:0</owl:versionInfo>
        <dc:creator>Francopoulo, Gil</dc:creator>
        <rdfs:subPropertyOf rdf:resource="&lemon;lexicalVariant"/>
        <dcr:datcat rdf:resource="http://www.isocat.org/datcat/DC-2231"/>
        <rdfs:isDefinedBy rdf:resource="http://www.lexinfo.net/ontology/2.0/lexinfo"/>
    </owl:ObjectProperty>
    


    <!-- http://www.lexinfo.net/ontology/2.0/lexinfo#secondPersonForm -->

    <owl:ObjectProperty rdf:about="&lexinfo;secondPersonForm">
        <rdfs:isDefinedBy rdf:resource="http://www.lexinfo.net/ontology/2.0/lexinfo"/>
        <rdfs:subPropertyOf rdf:resource="&lexinfo;formPersonVariant"/>
    </owl:ObjectProperty>
    


    <!-- http://www.lexinfo.net/ontology/2.0/lexinfo#senseExample -->

    <owl:ObjectProperty rdf:about="&lexinfo;senseExample">
        <rdfs:label xml:lang="en">sense example</rdfs:label>
        <rdfs:label xml:lang="ru">Смысловой пример</rdfs:label>        
        <dc:creator>Wright, Sue Ellen</dc:creator>
        <rdfs:comment xml:lang="en">Descriptive material that provides a sample of an object or entity defined in the entry.</rdfs:comment>
        <rdfs:comment xml:lang="ru">Описательный материал, который предоставляет образец объекта или сущности, определенных в записи.</rdfs:comment>        
        <owl:versionInfo>1:0</owl:versionInfo>
        <dc:creator>Francopoulo, Gil</dc:creator>
        <rdfs:subPropertyOf rdf:resource="&lemon;definition"/>
        <dcr:datcat rdf:resource="http://www.isocat.org/datcat/DC-1958"/>
        <dcr:datcat rdf:resource="http://www.isocat.org/datcat/DC-222"/>
        <rdfs:isDefinedBy rdf:resource="http://www.lexinfo.net/ontology/2.0/lexinfo"/>
    </owl:ObjectProperty>
    


    <!-- http://www.lexinfo.net/ontology/2.0/lexinfo#sententialClause -->

    <owl:ObjectProperty rdf:about="&lexinfo;sententialClause">
        <rdfs:isDefinedBy rdf:resource="http://www.lexinfo.net/ontology/2.0/lexinfo"/>
        <rdfs:subPropertyOf rdf:resource="&lexinfo;clausalArg"/>
    </owl:ObjectProperty>
    


    <!-- http://www.lexinfo.net/ontology/2.0/lexinfo#shortFormFor -->

    <owl:ObjectProperty rdf:about="&lexinfo;shortFormFor">
        <rdfs:label xml:lang="en">short form for</rdfs:label>
        <rdfs:label xml:lang="ru">краткая форма для</rdfs:label>        
        <dc:creator>Wright, Sue Ellen</dc:creator>
        <owl:versionInfo>1:0</owl:versionInfo>
        <rdfs:comment xml:lang="en">A linking element used to identify a relation between a short form and its full or expanded form.</rdfs:comment>
        <rdfs:comment xml:lang="ru">Связующий элемент, используемый для идентификации отношения между краткой формой и ее полной или расширенной формой.</rdfs:comment>
        <dcr:datcat rdf:resource="http://www.isocat.org/datcat/DC-468"/>
        <rdfs:isDefinedBy rdf:resource="http://www.lexinfo.net/ontology/2.0/lexinfo"/>
        <rdfs:subPropertyOf rdf:resource="&lexinfo;contractionFor"/>
    </owl:ObjectProperty>
    


    <!-- http://www.lexinfo.net/ontology/2.0/lexinfo#singularNumberForm -->

    <owl:ObjectProperty rdf:about="&lexinfo;singularNumberForm">
        <rdfs:isDefinedBy rdf:resource="http://www.lexinfo.net/ontology/2.0/lexinfo"/>
        <rdfs:subPropertyOf rdf:resource="&lexinfo;formNumberVariant"/>
    </owl:ObjectProperty>
    


    <!-- http://www.lexinfo.net/ontology/2.0/lexinfo#subject -->

    <owl:ObjectProperty rdf:about="&lexinfo;subject">
        <rdfs:label xml:lang="en">subject</rdfs:label>
        <rdfs:label xml:lang="ru">субъект</rdfs:label>        
        <rdfs:comment xml:lang="en">relation between a phrase and a verb, that represents the person or thing that performs the action or about which something is stated</rdfs:comment>
        <rdfs:comment xml:lang="ru">Отношение между фразой и глаголом, которое представляет человека или вещь, выполняющую действие или о которой что-либо говорится (тема).</rdfs:comment>
        <rdfs:subPropertyOf rdf:resource="&lemon;synArg"/>
        <dcr:datcat rdf:resource="http://www.isocat.org/datcat/DC-2261"/>
        <rdfs:isDefinedBy rdf:resource="http://www.lexinfo.net/ontology/2.0/lexinfo"/>
        <rdfs:range rdf:resource="&lexinfo;Subject"/>
    </owl:ObjectProperty>
    


    <!-- http://www.lexinfo.net/ontology/2.0/lexinfo#subjunctiveClause -->

    <owl:ObjectProperty rdf:about="&lexinfo;subjunctiveClause">
        <rdfs:isDefinedBy rdf:resource="http://www.lexinfo.net/ontology/2.0/lexinfo"/>
        <rdfs:subPropertyOf rdf:resource="&lexinfo;clausalArg"/>
    </owl:ObjectProperty>
    


    <!-- http://www.lexinfo.net/ontology/2.0/lexinfo#subjunctiveMoodForm -->

    <owl:ObjectProperty rdf:about="&lexinfo;subjunctiveMoodForm">
        <rdfs:isDefinedBy rdf:resource="http://www.lexinfo.net/ontology/2.0/lexinfo"/>
        <rdfs:subPropertyOf rdf:resource="&lexinfo;formMoodVariant"/>
    </owl:ObjectProperty>
    


    <!-- http://www.lexinfo.net/ontology/2.0/lexinfo#substanceHolonym -->

    <owl:ObjectProperty rdf:about="&lexinfo;substanceHolonym">
        <rdfs:label xml:lang="en">substance holonym</rdfs:label>
        <rdfs:label xml:lang="ru">субстанция холоним</rdfs:label>        
        <rdfs:comment xml:lang="en">Indicates what this is composed of</rdfs:comment>
        <rdfs:comment xml:lang="ru">Указывает, из чего это состоит.</rdfs:comment>
        <rdfs:isDefinedBy rdf:resource="http://www.lexinfo.net/ontology/2.0/lexinfo"/>
        <rdfs:subPropertyOf rdf:resource="&lexinfo;holonymTerm"/>
    </owl:ObjectProperty>
    


    <!-- http://www.lexinfo.net/ontology/2.0/lexinfo#substanceMeronym -->

    <owl:ObjectProperty rdf:about="&lexinfo;substanceMeronym">
        <rdfs:label xml:lang="en">substance meronym</rdfs:label>
        <rdfs:label xml:lang="ru">субстанция мероним</rdfs:label>        
        <rdfs:comment xml:lang="en">Indicates this is a substance that composes the other</rdfs:comment>
        <rdfs:comment xml:lang="ru">Указывает, что это субстанция, включенная в другую.</rdfs:comment>
        <rdfs:isDefinedBy rdf:resource="http://www.lexinfo.net/ontology/2.0/lexinfo"/>
        <rdfs:subPropertyOf rdf:resource="&lexinfo;meronymTerm"/>
    </owl:ObjectProperty>
    


    <!-- http://www.lexinfo.net/ontology/2.0/lexinfo#superlativeAdjunct -->

    <owl:ObjectProperty rdf:about="&lexinfo;superlativeAdjunct">
        <rdfs:isDefinedBy rdf:resource="http://www.lexinfo.net/ontology/2.0/lexinfo"/>
        <rdfs:range rdf:resource="&lexinfo;SuperlativeAdjunct"/>
        <rdfs:subPropertyOf rdf:resource="&lexinfo;predicativeAdjunct"/>
    </owl:ObjectProperty>
    


    <!-- http://www.lexinfo.net/ontology/2.0/lexinfo#superlativeDegreeForm -->

    <owl:ObjectProperty rdf:about="&lexinfo;superlativeDegreeForm">
        <rdfs:isDefinedBy rdf:resource="http://www.lexinfo.net/ontology/2.0/lexinfo"/>
        <rdfs:subPropertyOf rdf:resource="&lexinfo;formDegreeVariant"/>
    </owl:ObjectProperty>
    


    <!-- http://www.lexinfo.net/ontology/2.0/lexinfo#synonym -->

    <owl:ObjectProperty rdf:about="&lexinfo;synonym">
        <rdfs:subPropertyOf rdf:resource="&lemon;equivalent"/>
        <rdfs:isDefinedBy rdf:resource="http://www.lexinfo.net/ontology/2.0/lexinfo"/>
    </owl:ObjectProperty>
    


    <!-- http://www.lexinfo.net/ontology/2.0/lexinfo#temporalQualifier -->

    <owl:ObjectProperty rdf:about="&lexinfo;temporalQualifier">
        <rdfs:label xml:lang="en">temporal qualifier</rdfs:label>
        <rdfs:label xml:lang="ru">определитель времени</rdfs:label>        
        <rdfs:comment xml:lang="en">An attribution of a term or lexeme with respect to its use over time.</rdfs:comment>
        <rdfs:comment xml:lang="ru">Определение термина или лексемы в отношении его использования с течением времени.</rdfs:comment>
        <dc:creator>Wright, Sue Ellen</dc:creator>
        <owl:versionInfo>1:0</owl:versionInfo>
        <rdfs:subPropertyOf rdf:resource="&lemon;context"/>
        <dcr:datcat rdf:resource="http://www.isocat.org/datcat/DC-503"/>
        <rdfs:isDefinedBy rdf:resource="http://www.lexinfo.net/ontology/2.0/lexinfo"/>
        <rdfs:range rdf:resource="&lexinfo;TemporalQualifier"/>
    </owl:ObjectProperty>
    


    <!-- http://www.lexinfo.net/ontology/2.0/lexinfo#tense -->

    <owl:ObjectProperty rdf:about="&lexinfo;tense">
        <rdfs:label xml:lang="en">tense</rdfs:label>
        <rdfs:label xml:lang="ru">время</rdfs:label>
        <dc:creator>Francopoulo, Gil</dc:creator>
        <owl:versionInfo>1:0</owl:versionInfo>
        <rdfs:comment xml:lang="en">Property referring to the way the grammar marks the time at which the action denoted by the verb took place.</rdfs:comment>
        <rdfs:comment xml:lang="ru">Свойство, относящееся к тому, как грамматика указывает время для действия, обозначенного глаголом.</rdfs:comment>
        <dcr:datcat rdf:resource="http://www.isocat.org/datcat/DC-1286"/>
        <rdfs:isDefinedBy rdf:resource="http://www.lexinfo.net/ontology/2.0/lexinfo"/>
        <rdfs:range rdf:resource="&lexinfo;Tense"/>
        <rdfs:subPropertyOf rdf:resource="&lexinfo;morphosyntacticProperty"/>
    </owl:ObjectProperty>
    


    <!-- http://www.lexinfo.net/ontology/2.0/lexinfo#termElement -->

    <owl:ObjectProperty rdf:about="&lexinfo;termElement">
        <rdfs:label xml:lang="en">lexTermElement</rdfs:label>
        <rdfs:label xml:lang="ru">Элемент термина/лексемы</rdfs:label>        
        <rdfs:comment xml:lang="en">Any logically significant portion of a larger term or lexeme.</rdfs:comment>
        <rdfs:comment xml:lang="ru">Любая логически значимая часть более крупного термина или лексемы.</rdfs:comment>
        <dc:creator>Wright, Sue Ellen</dc:creator>
        <owl:versionInfo>1:0</owl:versionInfo>
        <rdfs:subPropertyOf rdf:resource="&lemon;property"/>
        <dcr:datcat rdf:resource="http://www.isocat.org/datcat/DC-289"/>
        <rdfs:isDefinedBy rdf:resource="http://www.lexinfo.net/ontology/2.0/lexinfo"/>
        <rdfs:range rdf:resource="&lexinfo;TermElement"/>
    </owl:ObjectProperty>
    


    <!-- http://www.lexinfo.net/ontology/2.0/lexinfo#termType -->

    <owl:ObjectProperty rdf:about="&lexinfo;termType">
        <rdfs:label xml:lang="en">lexTermType</rdfs:label>
        <rdfs:label xml:lang="ru">Тип термина/лексемы</rdfs:label>        
        <dc:creator>Wright, Sue Ellen</dc:creator>
        <owl:versionInfo>1:0</owl:versionInfo>
        <rdfs:comment xml:lang="en">An attribute assigned to a lexeme or a term.</rdfs:comment>
        <rdfs:comment xml:lang="ru">Определение, приписанное лексеме или термину.</rdfs:comment>
        <rdfs:subPropertyOf rdf:resource="&lemon;property"/>
        <dcr:datcat rdf:resource="http://www.isocat.org/datcat/DC-315"/>
        <rdfs:isDefinedBy rdf:resource="http://www.lexinfo.net/ontology/2.0/lexinfo"/>
        <rdfs:range rdf:resource="&lexinfo;TermType"/>
    </owl:ObjectProperty>
    


    <!-- http://www.lexinfo.net/ontology/2.0/lexinfo#thirdPersonForm -->

    <owl:ObjectProperty rdf:about="&lexinfo;thirdPersonForm">
        <rdfs:isDefinedBy rdf:resource="http://www.lexinfo.net/ontology/2.0/lexinfo"/>
        <rdfs:subPropertyOf rdf:resource="&lexinfo;formPersonVariant"/>
    </owl:ObjectProperty>
    


    <!-- http://www.lexinfo.net/ontology/2.0/lexinfo#translation -->

    <owl:ObjectProperty rdf:about="&lexinfo;translation">
        <rdfs:subPropertyOf rdf:resource="&lemon;senseRelation"/>
        <rdfs:isDefinedBy rdf:resource="http://www.lexinfo.net/ontology/2.0/lexinfo"/>
    </owl:ObjectProperty>
    


    <!-- http://www.lexinfo.net/ontology/2.0/lexinfo#usageNote -->

    <owl:ObjectProperty rdf:about="&lexinfo;usageNote">
        <rdfs:label xml:lang="en">usage note</rdfs:label>
        <rdfs:label xml:lang="ru">комментарий об использовании</rdfs:label>        
        <owl:versionInfo>1:0</owl:versionInfo>
        <rdfs:comment xml:lang="en">A note containing information on the usage of the associated word or term.</rdfs:comment>
        <rdfs:comment xml:lang="ru">Комментарий, содержащий информацию об использовании слова или термина.</rdfs:comment>
        <dc:creator>Wright, Sue Ellen</dc:creator>
        <rdfs:subPropertyOf rdf:resource="&lemon;definition"/>
        <dcr:datcat rdf:resource="http://www.isocat.org/datcat/DC-526"/>
        <rdfs:isDefinedBy rdf:resource="http://www.lexinfo.net/ontology/2.0/lexinfo"/>
    </owl:ObjectProperty>
    


    <!-- http://www.lexinfo.net/ontology/2.0/lexinfo#verbFormMood -->

    <owl:ObjectProperty rdf:about="&lexinfo;verbFormMood">
        <rdfs:label xml:lang="en">verb form mood</rdfs:label>
        <rdfs:label xml:lang="ru">наклонение глагольной формы</rdfs:label>        
        <dc:creator>Francopoulo, Gil</dc:creator>
        <rdfs:comment xml:lang="en">One of a set of distinctive forms that are used to signal modality. Modality is a facet of illocutionary point or general intent of a speaker, or a speaker&apos;s degree of commitment to the expressed proposition&apos;s believability, obligatoriness, desirability or reality.</rdfs:comment>
        <rdfs:comment xml:lang="ru">Одна из набора отличительных форм, которые используются для указания модальности. Модальность - это аспект иллокутивной точки или общего намерения говорящего или степень достоверности, обязательности, желательности или реальности высказанного говорящим предложения.</rdfs:comment>
        <owl:versionInfo>1:0</owl:versionInfo>
        <dcr:datcat rdf:resource="http://www.isocat.org/datcat/DC-1427"/>
        <rdfs:isDefinedBy rdf:resource="http://www.lexinfo.net/ontology/2.0/lexinfo"/>
        <rdfs:range rdf:resource="&lexinfo;VerbFormMood"/>
        <rdfs:subPropertyOf rdf:resource="&lexinfo;morphosyntacticProperty"/>
    </owl:ObjectProperty>
    


    <!-- http://www.lexinfo.net/ontology/2.0/lexinfo#voice -->

    <owl:ObjectProperty rdf:about="&lexinfo;voice">
        <rdfs:label xml:lang="en">voice</rdfs:label>
        <rdfs:label xml:lang="ru">залог</rdfs:label>        
        <dc:creator>Francopoulo, Gil</dc:creator>
        <owl:versionInfo>1:0</owl:versionInfo>
        <rdfs:comment xml:lang="en">Way sentences may alter the relationship between the subject and object of a verb, without changing the meaning of the sentence.</rdfs:comment>
        <rdfs:comment xml:lang="ru">Способ, которым предложения могут изменить отношения между субъектом и объектом глагола, не изменяя значения предложения.</rdfs:comment>
        <dcr:datcat rdf:resource="http://www.isocat.org/datcat/DC-1413"/>
        <rdfs:isDefinedBy rdf:resource="http://www.lexinfo.net/ontology/2.0/lexinfo"/>
        <rdfs:range rdf:resource="&lexinfo;Voice"/>
        <rdfs:subPropertyOf rdf:resource="&lexinfo;morphosyntacticProperty"/>
    </owl:ObjectProperty>
    


    <!-- 
    ///////////////////////////////////////////////////////////////////////////////////////
    //
    // Data properties
    //
    ///////////////////////////////////////////////////////////////////////////////////////
     -->


    <owl:DatatypeProperty rdf:about="&lexinfo;confidence">
        <rdfs:label xml:lang="en">Confidence</rdfs:label>
        <rdfs:label xml:lang="ru">Уверенность</rdfs:label>        
        <rdfs:comment xml:lang="en">The confidence in a given relationship.</rdfs:comment>
        <rdfs:comment xml:lang="ru">Уверенность в данной связи.</rdfs:comment>
        <dc:creator rdf:resource="http://john.mccr.ae"/>
    </owl:DatatypeProperty>

    <owl:DatatypeProperty rdf:about="&lexinfo;translationConfidence">
        <rdfs:subPropertyOf rdf:resource="&lexinfo;confidence"/>
        <rdfs:label xml:lang="en">Translation confidence</rdfs:label>
        <rdfs:label xml:lang="ru">Уверенность в переводе</rdfs:label>        
        <rdfs:comment xml:lang="en">The confidence in a given translation.</rdfs:comment>
        <rdfs:comment xml:lang="ru">Уверенность в определенном переводе</rdfs:comment>
    </owl:DatatypeProperty>



    <!-- http://lemon-model.net/lemon#optional -->

    <owl:DatatypeProperty rdf:about="&lemon;optional"/>
    


    <!-- http://lemon-model.net/lemon#representation -->

    <owl:DatatypeProperty rdf:about="&lemon;representation"/>
    


    <!-- http://lemon-model.net/lemon#separator -->

    <owl:DatatypeProperty rdf:about="&lemon;separator">
        <dcr:datcat rdf:resource="http://www.isocat.org/datcat/DC-1863"/>
        <rdfs:isDefinedBy rdf:resource="http://www.lexinfo.net/ontology/2.0/lexinfo"/>
    </owl:DatatypeProperty>
    

    <!-- http://www.lexinfo.net/ontology/2.0/lexinfo#pronunciation -->

    <owl:DatatypeProperty rdf:about="&lexinfo;pronunciation">
        <rdfs:label xml:lang="en">pronunciation</rdfs:label>
        <rdfs:label xml:lang="ru">произношение</rdfs:label>        
        <rdfs:comment xml:lang="en">The representation of the manner by which a term or word is articulated.</rdfs:comment>
        <rdfs:comment xml:lang="ru">Представление способа, которым слово или термин артикулируется.</rdfs:comment>        
        <dc:creator>Wright, Sue Ellen</dc:creator>
        <owl:versionInfo>1:0</owl:versionInfo>
        <rdfs:subPropertyOf rdf:resource="&lemon;representation"/>
        <dcr:datcat rdf:resource="http://www.isocat.org/datcat/DC-407"/>
        <rdfs:isDefinedBy rdf:resource="http://www.lexinfo.net/ontology/2.0/lexinfo"/>
        <rdfs:range rdf:resource="&xsd;string"/>
    </owl:DatatypeProperty>
    


    <!-- http://www.lexinfo.net/ontology/2.0/lexinfo#romanization -->

    <owl:DatatypeProperty rdf:about="&lexinfo;romanization">
        <rdfs:label xml:lang="en">romanization</rdfs:label>
        <rdfs:label xml:lang="ru">латинизация</rdfs:label>        
        <dc:creator>Francopoulo, Gil</dc:creator>
        <rdfs:comment xml:lang="en">Transcription or transliteration from non-Latin script into Latin script.</rdfs:comment>
        <rdfs:comment xml:lang="ru">Транскрипция или транслитерация из нелатинского шрифта в латинский.</rdfs:comment>
        <owl:versionInfo>1:0</owl:versionInfo>
        <rdfs:subPropertyOf rdf:resource="&lemon;representation"/>
        <dcr:datcat rdf:resource="http://www.isocat.org/datcat/DC-1873"/>
        <rdfs:isDefinedBy rdf:resource="http://www.lexinfo.net/ontology/2.0/lexinfo"/>
        <rdfs:range rdf:resource="&xsd;string"/>
    </owl:DatatypeProperty>
    


    <!-- http://www.lexinfo.net/ontology/2.0/lexinfo#segmentation -->

    <owl:DatatypeProperty rdf:about="&lexinfo;segmentation">
        <rdfs:label xml:lang="en">segmentation</rdfs:label>
        <rdfs:label xml:lang="ru">членение</rdfs:label>        
        <owl:versionInfo>1:0</owl:versionInfo>
        <rdfs:comment xml:lang="en">Specification of the pointers in time or sequence that indicates the segmentation process.</rdfs:comment>
        <rdfs:comment xml:lang="ru">Спецификация указателей во времени или последовательности, которая указывает на процесс членения.</rdfs:comment>
        <dc:creator>Wittenburg, Peter</dc:creator>
        <rdfs:subPropertyOf rdf:resource="&lemon;representation"/>
        <dcr:datcat rdf:resource="http://www.isocat.org/datcat/DC-2578"/>
        <rdfs:isDefinedBy rdf:resource="http://www.lexinfo.net/ontology/2.0/lexinfo"/>
        <rdfs:range rdf:resource="&xsd;string"/>
    </owl:DatatypeProperty>
    


    <!-- http://www.lexinfo.net/ontology/2.0/lexinfo#transliteration -->

    <owl:DatatypeProperty rdf:about="&lexinfo;transliteration">
        <rdfs:label xml:lang="en">transliteration</rdfs:label>
        <rdfs:label xml:lang="ru">транслитерация</rdfs:label>        
        <dc:creator>Francopoulo, Gil</dc:creator>
        <owl:versionInfo>1:0</owl:versionInfo>
        <rdfs:comment xml:lang="en">Form resulting from the conversion of one writing system into another</rdfs:comment>
        <rdfs:comment xml:lang="ru">Форма, полученная в результате преобразования одной письменной системы в другую.</rdfs:comment>
        <rdfs:subPropertyOf rdf:resource="&lemon;representation"/>
        <dcr:datcat rdf:resource="http://www.isocat.org/datcat/DC-1848"/>
        <rdfs:isDefinedBy rdf:resource="http://www.lexinfo.net/ontology/2.0/lexinfo"/>
        <rdfs:range rdf:resource="&xsd;string"/>
    </owl:DatatypeProperty>
    


    <!-- 
    ///////////////////////////////////////////////////////////////////////////////////////
    //
    // Classes
    //
    ///////////////////////////////////////////////////////////////////////////////////////
     -->

    


    <!-- http://lemon-model.net/lemon#Argument -->

    <owl:Class rdf:about="&lemon;Argument"/>
    


    <!-- http://lemon-model.net/lemon#Frame -->

    <owl:Class rdf:about="&lemon;Frame"/>
    


    <!-- http://lemon-model.net/lemon#Part -->

    <owl:Class rdf:about="&lemon;Part"/>
    


    <!-- http://lemon-model.net/lemon#Phrase -->

    <owl:Class rdf:about="&lemon;Phrase"/>
    


    <!-- http://lemon-model.net/lemon#PropertyValue -->

    <owl:Class rdf:about="&lemon;PropertyValue"/>
    


    <!-- http://lemon-model.net/lemon#RaisableArgument -->

    <owl:Class rdf:about="&lemon;RaisableArgument">
        <rdfs:subClassOf rdf:resource="&lemon;Argument"/>
    </owl:Class>
    


    <!-- http://lemon-model.net/lemon#SenseContext -->

    <owl:Class rdf:about="&lemon;SenseContext"/>
    


    <!-- http://lemon-model.net/lemon#Word -->

    <owl:Class rdf:about="&lemon;Word"/>
    


    <!-- http://purl.org/vocommons/voaf#Vocabulary -->

    <owl:Class rdf:about="http://purl.org/vocommons/voaf#Vocabulary"/>
    


    <!-- http://www.lexinfo.net/ontology/2.0/lexinfo#AbbreviatedForm -->

    <owl:Class rdf:about="&lexinfo;AbbreviatedForm">
        <rdfs:subClassOf rdf:resource="&lexinfo;TermType"/>
        <rdfs:isDefinedBy rdf:resource="http://www.lexinfo.net/ontology/2.0/lexinfo"/>
    </owl:Class>
    


    <!-- http://www.lexinfo.net/ontology/2.0/lexinfo#AccusativePostPositiveArgument -->

    <owl:Class rdf:about="&lexinfo;AccusativePostPositiveArgument">
        <owl:equivalentClass>
            <owl:Class>
                <owl:intersectionOf rdf:parseType="Collection">
                    <rdf:Description rdf:about="&lexinfo;PostPositiveArgument"/>
                    <owl:Restriction>
                        <owl:onProperty rdf:resource="&lemon;marker"/>
                        <owl:hasValue rdf:resource="&lexinfo;accusativeCase"/>
                    </owl:Restriction>
                </owl:intersectionOf>
            </owl:Class>
        </owl:equivalentClass>
        <rdfs:subClassOf rdf:resource="&lexinfo;PostPositiveArgument"/>
        <rdfs:isDefinedBy rdf:resource="http://www.lexinfo.net/ontology/2.0/lexinfo"/>
    </owl:Class>
    


    <!-- http://www.lexinfo.net/ontology/2.0/lexinfo#AdjectivalComplementFrame -->

    <owl:Class rdf:about="&lexinfo;AdjectivalComplementFrame">
        <owl:equivalentClass>
            <owl:Class>
                <owl:intersectionOf rdf:parseType="Collection">
                    <rdf:Description rdf:about="&lexinfo;VerbFrame"/>
                    <owl:Restriction>
                        <owl:onProperty rdf:resource="&lexinfo;predicativeAdjective"/>
                        <owl:minCardinality rdf:datatype="&xsd;nonNegativeInteger">1</owl:minCardinality>
                    </owl:Restriction>
                </owl:intersectionOf>
            </owl:Class>
        </owl:equivalentClass>
        <rdfs:subClassOf rdf:resource="&lexinfo;VerbFrame"/>
        <rdfs:isDefinedBy rdf:resource="http://www.lexinfo.net/ontology/2.0/lexinfo"/>
    </owl:Class>
    


    <!-- http://www.lexinfo.net/ontology/2.0/lexinfo#Adjective -->

    <owl:Class rdf:about="&lexinfo;Adjective">
        <owl:equivalentClass>
            <owl:Restriction>
                <owl:onProperty rdf:resource="&lexinfo;partOfSpeech"/>
                <owl:someValuesFrom rdf:resource="&lexinfo;AdjectivePOS"/>
            </owl:Restriction>
        </owl:equivalentClass>
        <rdfs:subClassOf rdf:resource="&lemon;Word"/>
        <rdfs:subClassOf>
            <owl:Restriction>
                <owl:onProperty rdf:resource="&lemon;synBehavior"/>
                <owl:allValuesFrom rdf:resource="&lexinfo;AdjectiveFrame"/>
            </owl:Restriction>
        </rdfs:subClassOf>
        <rdfs:isDefinedBy rdf:resource="http://www.lexinfo.net/ontology/2.0/lexinfo"/>
    </owl:Class>
    


    <!-- http://www.lexinfo.net/ontology/2.0/lexinfo#AdjectiveAccusativePostPositiveFrame -->

    <owl:Class rdf:about="&lexinfo;AdjectiveAccusativePostPositiveFrame">
        <owl:equivalentClass>
            <owl:Class>
                <owl:intersectionOf rdf:parseType="Collection">
                    <rdf:Description rdf:about="&lexinfo;AdjectivePostPositiveFrame"/>
                    <owl:Restriction>
                        <owl:onProperty rdf:resource="&lexinfo;postPositiveArg"/>
                        <owl:someValuesFrom rdf:resource="&lexinfo;AccusativePostPositiveArgument"/>
                    </owl:Restriction>
                </owl:intersectionOf>
            </owl:Class>
        </owl:equivalentClass>
        <rdfs:subClassOf rdf:resource="&lexinfo;AdjectivePostPositiveFrame"/>
        <example xml:lang="de">wird wurden unseren irrtum GEWAHR</example>
        <rdfs:isDefinedBy rdf:resource="http://www.lexinfo.net/ontology/2.0/lexinfo"/>
    </owl:Class>
    


    <!-- http://www.lexinfo.net/ontology/2.0/lexinfo#AdjectiveAttributiveFrame -->

    <owl:Class rdf:about="&lexinfo;AdjectiveAttributiveFrame">
        <owl:equivalentClass>
            <owl:Class>
                <owl:intersectionOf rdf:parseType="Collection">
                    <rdf:Description rdf:about="&lexinfo;AdjectiveFrame"/>
                    <owl:Restriction>
                        <owl:onProperty rdf:resource="&lexinfo;attributiveArg"/>
                        <owl:minCardinality rdf:datatype="&xsd;nonNegativeInteger">1</owl:minCardinality>
                    </owl:Restriction>
                </owl:intersectionOf>
            </owl:Class>
        </owl:equivalentClass>
        <rdfs:subClassOf rdf:resource="&lexinfo;AdjectiveFrame"/>
        <example xml:lang="en">the RED ball</example>
        <rdfs:isDefinedBy rdf:resource="http://www.lexinfo.net/ontology/2.0/lexinfo"/>
    </owl:Class>
    


    <!-- http://www.lexinfo.net/ontology/2.0/lexinfo#AdjectiveComparativeFrame -->

    <owl:Class rdf:about="&lexinfo;AdjectiveComparativeFrame">
        <owl:equivalentClass>
            <owl:Class>
                <owl:intersectionOf rdf:parseType="Collection">
                    <rdf:Description rdf:about="&lexinfo;AdjectiveFrame"/>
                    <owl:Restriction>
                        <owl:onProperty rdf:resource="&lexinfo;comparativeAdjunct"/>
                        <owl:cardinality rdf:datatype="&xsd;nonNegativeInteger">1</owl:cardinality>
                    </owl:Restriction>
                    <owl:Restriction>
                        <owl:onProperty rdf:resource="&lexinfo;copulativeSubject"/>
                        <owl:cardinality rdf:datatype="&xsd;nonNegativeInteger">1</owl:cardinality>
                    </owl:Restriction>
                </owl:intersectionOf>
            </owl:Class>
        </owl:equivalentClass>
        <rdfs:subClassOf rdf:resource="&lexinfo;AdjectiveFrame"/>
        <example xml:lang="en">new york is BIGGER THAN berlin</example>
        <rdfs:isDefinedBy rdf:resource="http://www.lexinfo.net/ontology/2.0/lexinfo"/>
    </owl:Class>
    


    <!-- http://www.lexinfo.net/ontology/2.0/lexinfo#AdjectiveDativePostPositiveFrame -->

    <owl:Class rdf:about="&lexinfo;AdjectiveDativePostPositiveFrame">
        <owl:equivalentClass>
            <owl:Class>
                <owl:intersectionOf rdf:parseType="Collection">
                    <rdf:Description rdf:about="&lexinfo;AdjectivePostPositiveFrame"/>
                    <owl:Restriction>
                        <owl:onProperty rdf:resource="&lexinfo;postPositiveArg"/>
                        <owl:someValuesFrom rdf:resource="&lexinfo;DativePostPositiveArgument"/>
                    </owl:Restriction>
                </owl:intersectionOf>
            </owl:Class>
        </owl:equivalentClass>
        <rdfs:subClassOf rdf:resource="&lexinfo;AdjectivePostPositiveFrame"/>
        <example xml:lang="de">er ist seinem bruder ÄHNLICH</example>
        <rdfs:isDefinedBy rdf:resource="http://www.lexinfo.net/ontology/2.0/lexinfo"/>
    </owl:Class>
    


    <!-- http://www.lexinfo.net/ontology/2.0/lexinfo#AdjectiveFrame -->

    <owl:Class rdf:about="&lexinfo;AdjectiveFrame">
        <rdfs:subClassOf rdf:resource="&lemon;Frame"/>
    </owl:Class>
    


    <!-- http://www.lexinfo.net/ontology/2.0/lexinfo#AdjectiveGenitivePostPositiveFrame -->

    <owl:Class rdf:about="&lexinfo;AdjectiveGenitivePostPositiveFrame">
        <owl:equivalentClass>
            <owl:Class>
                <owl:intersectionOf rdf:parseType="Collection">
                    <rdf:Description rdf:about="&lexinfo;AdjectivePostPositiveFrame"/>
                    <owl:Restriction>
                        <owl:onProperty rdf:resource="&lexinfo;postPositiveArg"/>
                        <owl:someValuesFrom rdf:resource="&lexinfo;GenitivePostPositiveArgument"/>
                    </owl:Restriction>
                </owl:intersectionOf>
            </owl:Class>
        </owl:equivalentClass>
        <rdfs:subClassOf rdf:resource="&lexinfo;AdjectivePostPositiveFrame"/>
        <example xml:lang="de">er ist des hochverrats SCHULDIG</example>
        <rdfs:isDefinedBy rdf:resource="http://www.lexinfo.net/ontology/2.0/lexinfo"/>
    </owl:Class>
    


    <!-- http://www.lexinfo.net/ontology/2.0/lexinfo#AdjectiveImpersonalFrame -->

    <owl:Class rdf:about="&lexinfo;AdjectiveImpersonalFrame">
        <owl:equivalentClass>
            <owl:Class>
                <owl:intersectionOf rdf:parseType="Collection">
                    <rdf:Description rdf:about="&lexinfo;AdjectiveFrame"/>
                    <owl:Restriction>
                        <owl:onProperty rdf:resource="&lexinfo;object"/>
                        <owl:minCardinality rdf:datatype="&xsd;nonNegativeInteger">1</owl:minCardinality>
                    </owl:Restriction>
                    <owl:Restriction>
                        <owl:onProperty rdf:resource="&lexinfo;copulativeSubject"/>
                        <owl:cardinality rdf:datatype="&xsd;nonNegativeInteger">0</owl:cardinality>
                    </owl:Restriction>
                </owl:intersectionOf>
            </owl:Class>
        </owl:equivalentClass>
        <rdfs:subClassOf rdf:resource="&lexinfo;AdjectiveFrame"/>
        <example xml:lang="de">es ist mir HEISS</example>
        <rdfs:isDefinedBy rdf:resource="http://www.lexinfo.net/ontology/2.0/lexinfo"/>
    </owl:Class>
    


    <!-- http://www.lexinfo.net/ontology/2.0/lexinfo#AdjectivePOS -->

    <owl:Class rdf:about="&lexinfo;AdjectivePOS">
        <rdfs:subClassOf rdf:resource="&lexinfo;PartOfSpeech"/>
        <rdfs:isDefinedBy rdf:resource="http://www.lexinfo.net/ontology/2.0/lexinfo"/>
    </owl:Class>
    


    <!-- http://www.lexinfo.net/ontology/2.0/lexinfo#AdjectivePPFrame -->

    <owl:Class rdf:about="&lexinfo;AdjectivePPFrame">
        <owl:equivalentClass>
            <owl:Class>
                <owl:intersectionOf rdf:parseType="Collection">
                    <rdf:Description rdf:about="&lexinfo;AdjectivePredicativeFrame"/>
                    <rdf:Description rdf:about="&lexinfo;PrepositionalFrame"/>
                </owl:intersectionOf>
            </owl:Class>
        </owl:equivalentClass>
        <rdfs:subClassOf rdf:resource="&lexinfo;AdjectiveFrame"/>
        <example xml:lang="en">he is RELATED TO her</example>
        <rdfs:isDefinedBy rdf:resource="http://www.lexinfo.net/ontology/2.0/lexinfo"/>
    </owl:Class>
    


    <!-- http://www.lexinfo.net/ontology/2.0/lexinfo#AdjectivePhrase -->

    <owl:Class rdf:about="&lexinfo;AdjectivePhrase">
        <owl:equivalentClass>
            <owl:Class>
                <owl:intersectionOf rdf:parseType="Collection">
                    <rdf:Description rdf:about="&lemon;Phrase"/>
                    <owl:Restriction>
                        <owl:onProperty rdf:resource="&lexinfo;head"/>
                        <owl:someValuesFrom rdf:resource="&lexinfo;Adjective"/>
                    </owl:Restriction>
                </owl:intersectionOf>
            </owl:Class>
        </owl:equivalentClass>
        <rdfs:subClassOf rdf:resource="&lemon;Phrase"/>
        <rdfs:isDefinedBy rdf:resource="http://www.lexinfo.net/ontology/2.0/lexinfo"/>
    </owl:Class>
    


    <!-- http://www.lexinfo.net/ontology/2.0/lexinfo#AdjectivePostPositiveFrame -->

    <owl:Class rdf:about="&lexinfo;AdjectivePostPositiveFrame">
        <owl:equivalentClass>
            <owl:Class>
                <owl:intersectionOf rdf:parseType="Collection">
                    <rdf:Description rdf:about="&lexinfo;AdjectiveFrame"/>
                    <owl:Restriction>
                        <owl:onProperty rdf:resource="&lexinfo;copulativeArg"/>
                        <owl:cardinality rdf:datatype="&xsd;nonNegativeInteger">1</owl:cardinality>
                    </owl:Restriction>
                    <owl:Restriction>
                        <owl:onProperty rdf:resource="&lexinfo;postPositiveArg"/>
                        <owl:cardinality rdf:datatype="&xsd;nonNegativeInteger">1</owl:cardinality>
                    </owl:Restriction>
                </owl:intersectionOf>
            </owl:Class>
        </owl:equivalentClass>
        <rdfs:subClassOf rdf:resource="&lexinfo;AdjectiveFrame"/>
        <example xml:lang="en">that is something INTERESTING</example>
        <rdfs:isDefinedBy rdf:resource="http://www.lexinfo.net/ontology/2.0/lexinfo"/>
    </owl:Class>
    


    <!-- http://www.lexinfo.net/ontology/2.0/lexinfo#AdjectivePredicateFrame -->

    <owl:Class rdf:about="&lexinfo;AdjectivePredicateFrame">
        <owl:equivalentClass>
            <owl:Class>
                <owl:intersectionOf rdf:parseType="Collection">
                    <rdf:Description rdf:about="&lexinfo;AdjectiveAttributiveFrame"/>
                    <rdf:Description rdf:about="&lexinfo;AdjectivePredicativeFrame"/>
                </owl:intersectionOf>
            </owl:Class>
        </owl:equivalentClass>
        <rdfs:subClassOf rdf:resource="&lexinfo;AdjectiveFrame"/>
        <rdfs:comment xml:lang="en">Note this frame should be used when both attributive and predicative use of the adjective is allowed</rdfs:comment>
        <rdfs:comment xml:lang="ru">Используется в случае, когда возможны определительное и предикативное значение прилагательного</rdfs:comment>
        <rdfs:isDefinedBy rdf:resource="http://www.lexinfo.net/ontology/2.0/lexinfo"/>
    </owl:Class>
    


    <!-- http://www.lexinfo.net/ontology/2.0/lexinfo#AdjectivePredicativeFrame -->

    <owl:Class rdf:about="&lexinfo;AdjectivePredicativeFrame">
        <owl:equivalentClass>
            <owl:Class>
                <owl:intersectionOf rdf:parseType="Collection">
                    <rdf:Description rdf:about="&lexinfo;AdjectiveFrame"/>
                    <owl:Restriction>
                        <owl:onProperty rdf:resource="&lexinfo;copulativeSubject"/>
                        <owl:cardinality rdf:datatype="&xsd;nonNegativeInteger">1</owl:cardinality>
                    </owl:Restriction>
                </owl:intersectionOf>
            </owl:Class>
        </owl:equivalentClass>
        <rdfs:subClassOf rdf:resource="&lexinfo;AdjectiveFrame"/>
        <example xml:lang="en">he is HAPPY</example>
        <rdfs:isDefinedBy rdf:resource="http://www.lexinfo.net/ontology/2.0/lexinfo"/>
    </owl:Class>
    


    <!-- http://www.lexinfo.net/ontology/2.0/lexinfo#AdjectiveScaleFrame -->

    <owl:Class rdf:about="&lexinfo;AdjectiveScaleFrame">
        <owl:equivalentClass>
            <owl:Class>
                <owl:intersectionOf rdf:parseType="Collection">
                    <owl:Restriction>
                        <owl:onProperty rdf:resource="&lexinfo;adverbialComplement"/>
                        <owl:cardinality rdf:datatype="&xsd;nonNegativeInteger">1</owl:cardinality>
                    </owl:Restriction>
                    <owl:Restriction>
                        <owl:onProperty rdf:resource="&lexinfo;copulativeSubject"/>
                        <owl:cardinality rdf:datatype="&xsd;nonNegativeInteger">1</owl:cardinality>
                    </owl:Restriction>
                </owl:intersectionOf>
            </owl:Class>
        </owl:equivalentClass>
        <rdfs:subClassOf rdf:resource="&lexinfo;AdjectiveFrame"/>
        <example xml:lang="en">Everest is 8,848m HIGH</example>
        <rdfs:isDefinedBy rdf:resource="http://www.lexinfo.net/ontology/2.0/lexinfo"/>
    </owl:Class>
    


    <!-- http://www.lexinfo.net/ontology/2.0/lexinfo#AdjectiveSuperlativeFrame -->

    <owl:Class rdf:about="&lexinfo;AdjectiveSuperlativeFrame">
        <owl:equivalentClass>
            <owl:Class>
                <owl:intersectionOf rdf:parseType="Collection">
                    <rdf:Description rdf:about="&lexinfo;AdjectiveFrame"/>
                    <owl:Restriction>
                        <owl:onProperty rdf:resource="&lexinfo;superlativeAdjunct"/>
                        <owl:minCardinality rdf:datatype="&xsd;nonNegativeInteger">1</owl:minCardinality>
                    </owl:Restriction>
                    <owl:Restriction>
                        <owl:onProperty rdf:resource="&lexinfo;copulativeSubject"/>
                        <owl:cardinality rdf:datatype="&xsd;nonNegativeInteger">1</owl:cardinality>
                    </owl:Restriction>
                </owl:intersectionOf>
            </owl:Class>
        </owl:equivalentClass>
        <rdfs:subClassOf rdf:resource="&lexinfo;AdjectiveFrame"/>
        <example xml:lang="en">tokyo is the BIGGEST of all metropoles</example>
        <rdfs:isDefinedBy rdf:resource="http://www.lexinfo.net/ontology/2.0/lexinfo"/>
    </owl:Class>
    


    <!-- http://www.lexinfo.net/ontology/2.0/lexinfo#Adjunct -->

    <owl:Class rdf:about="&lexinfo;Adjunct">
        <rdfs:subClassOf rdf:resource="&lemon;Argument"/>
        <rdfs:subClassOf>
            <owl:Restriction>
                <owl:onProperty rdf:resource="&lemon;optional"/>
                <owl:hasValue rdf:datatype="&xsd;boolean">true</owl:hasValue>
            </owl:Restriction>
        </rdfs:subClassOf>
        <rdfs:isDefinedBy rdf:resource="http://www.lexinfo.net/ontology/2.0/lexinfo"/>
    </owl:Class>
    


    <!-- http://www.lexinfo.net/ontology/2.0/lexinfo#Adposition -->

    <owl:Class rdf:about="&lexinfo;Adposition">
        <owl:equivalentClass>
            <owl:Restriction>
                <owl:onProperty rdf:resource="&lexinfo;partOfSpeech"/>
                <owl:someValuesFrom rdf:resource="&lexinfo;AdpositionPOS"/>
            </owl:Restriction>
        </owl:equivalentClass>
        <rdfs:subClassOf rdf:resource="&lemon;Word"/>
        <rdfs:isDefinedBy rdf:resource="http://www.lexinfo.net/ontology/2.0/lexinfo"/>
    </owl:Class>
    


    <!-- http://www.lexinfo.net/ontology/2.0/lexinfo#AdpositionPOS -->

    <owl:Class rdf:about="&lexinfo;AdpositionPOS">
        <rdfs:subClassOf rdf:resource="&lexinfo;PartOfSpeech"/>
        <rdfs:isDefinedBy rdf:resource="http://www.lexinfo.net/ontology/2.0/lexinfo"/>
    </owl:Class>
    


    <!-- http://www.lexinfo.net/ontology/2.0/lexinfo#AdpositionalObject -->

    <owl:Class rdf:about="&lexinfo;AdpositionalObject">
        <owl:equivalentClass>
            <owl:Class>
                <owl:intersectionOf rdf:parseType="Collection">
                    <rdf:Description rdf:about="&lexinfo;Object"/>
                    <owl:Restriction>
                        <owl:onProperty rdf:resource="&lemon;marker"/>
                        <owl:someValuesFrom rdf:resource="&lexinfo;Adposition"/>
                    </owl:Restriction>
                </owl:intersectionOf>
            </owl:Class>
        </owl:equivalentClass>
        <rdfs:subClassOf rdf:resource="&lexinfo;Object"/>
        <rdfs:subClassOf>
            <owl:Restriction>
                <owl:onProperty rdf:resource="&lemon;marker"/>
                <owl:someValuesFrom rdf:resource="&lexinfo;Adposition"/>
            </owl:Restriction>
        </rdfs:subClassOf>
        <rdfs:isDefinedBy rdf:resource="http://www.lexinfo.net/ontology/2.0/lexinfo"/>
    </owl:Class>
    


    <!-- http://www.lexinfo.net/ontology/2.0/lexinfo#Adverb -->

    <owl:Class rdf:about="&lexinfo;Adverb">
        <owl:equivalentClass>
            <owl:Restriction>
                <owl:onProperty rdf:resource="&lexinfo;partOfSpeech"/>
                <owl:someValuesFrom rdf:resource="&lexinfo;AdverbPOS"/>
            </owl:Restriction>
        </owl:equivalentClass>
        <rdfs:subClassOf rdf:resource="&lemon;Word"/>
        <rdfs:isDefinedBy rdf:resource="http://www.lexinfo.net/ontology/2.0/lexinfo"/>
    </owl:Class>
    


    <!-- http://www.lexinfo.net/ontology/2.0/lexinfo#AdverbPOS -->

    <owl:Class rdf:about="&lexinfo;AdverbPOS">
        <rdfs:subClassOf rdf:resource="&lexinfo;PartOfSpeech"/>
        <rdfs:isDefinedBy rdf:resource="http://www.lexinfo.net/ontology/2.0/lexinfo"/>
    </owl:Class>
    


    <!-- http://www.lexinfo.net/ontology/2.0/lexinfo#AdverbialComplementFrame -->

    <owl:Class rdf:about="&lexinfo;AdverbialComplementFrame">
        <owl:equivalentClass>
            <owl:Class>
                <owl:intersectionOf rdf:parseType="Collection">
                    <rdf:Description rdf:about="&lexinfo;VerbFrame"/>
                    <owl:Restriction>
                        <owl:onProperty rdf:resource="&lexinfo;predicativeAdverb"/>
                        <owl:minCardinality rdf:datatype="&xsd;nonNegativeInteger">1</owl:minCardinality>
                    </owl:Restriction>
                </owl:intersectionOf>
            </owl:Class>
        </owl:equivalentClass>
        <rdfs:subClassOf rdf:resource="&lexinfo;VerbFrame"/>
        <rdfs:isDefinedBy rdf:resource="http://www.lexinfo.net/ontology/2.0/lexinfo"/>
    </owl:Class>
    


    <!-- http://www.lexinfo.net/ontology/2.0/lexinfo#Affix -->

    <owl:Class rdf:about="&lexinfo;Affix">
        <owl:equivalentClass>
            <owl:Restriction>
                <owl:onProperty rdf:resource="&lexinfo;termElement"/>
                <owl:hasValue rdf:resource="&lexinfo;affix"/>
            </owl:Restriction>
        </owl:equivalentClass>
        <rdfs:subClassOf rdf:resource="&lemon;Part"/>
        <rdfs:isDefinedBy rdf:resource="http://www.lexinfo.net/ontology/2.0/lexinfo"/>
    </owl:Class>
    


    <!-- http://www.lexinfo.net/ontology/2.0/lexinfo#Animacy -->

    <owl:Class rdf:about="&lexinfo;Animacy">
        <rdfs:subClassOf rdf:resource="&lexinfo;MorphosyntacticProperty"/>
        <rdfs:isDefinedBy rdf:resource="http://www.lexinfo.net/ontology/2.0/lexinfo"/>
    </owl:Class>
    


    <!-- http://www.lexinfo.net/ontology/2.0/lexinfo#ArbitraryControl -->

    <owl:Class rdf:about="&lexinfo;ArbitraryControl">
        <rdfs:subClassOf rdf:resource="&lexinfo;Control"/>
        <rdfs:comment xml:lang="en">Indicates either the subject or object of the main clause may be the omitted argument of the subclause</rdfs:comment>
        <rdfs:comment xml:lang="ru">Указывает на субъект или объект главного предложения, которые могут быть опущенным аргументом подчинительного предложения</rdfs:comment>
        <rdfs:isDefinedBy rdf:resource="http://www.lexinfo.net/ontology/2.0/lexinfo"/>
    </owl:Class>
    


    <!-- http://www.lexinfo.net/ontology/2.0/lexinfo#Article -->

    <owl:Class rdf:about="&lexinfo;Article">
        <owl:equivalentClass>
            <owl:Restriction>
                <owl:onProperty rdf:resource="&lexinfo;partOfSpeech"/>
                <owl:someValuesFrom rdf:resource="&lexinfo;ArticlePOS"/>
            </owl:Restriction>
        </owl:equivalentClass>
        <rdfs:subClassOf rdf:resource="&lexinfo;Determiner"/>
        <rdfs:isDefinedBy rdf:resource="http://www.lexinfo.net/ontology/2.0/lexinfo"/>
    </owl:Class>
    


    <!-- http://www.lexinfo.net/ontology/2.0/lexinfo#ArticlePOS -->

    <owl:Class rdf:about="&lexinfo;ArticlePOS">
        <rdfs:subClassOf rdf:resource="&lexinfo;DeterminerPOS"/>
        <rdfs:isDefinedBy rdf:resource="http://www.lexinfo.net/ontology/2.0/lexinfo"/>
    </owl:Class>
    


    <!-- http://www.lexinfo.net/ontology/2.0/lexinfo#Aspect -->

    <owl:Class rdf:about="&lexinfo;Aspect">
        <rdfs:subClassOf rdf:resource="&lexinfo;MorphosyntacticProperty"/>
        <rdfs:isDefinedBy rdf:resource="http://www.lexinfo.net/ontology/2.0/lexinfo"/>
    </owl:Class>
    


    <!-- http://www.lexinfo.net/ontology/2.0/lexinfo#AttributiveArgument -->

    <owl:Class rdf:about="&lexinfo;AttributiveArgument">
        <rdfs:subClassOf rdf:resource="&lemon;Argument"/>
        <rdfs:isDefinedBy rdf:resource="http://www.lexinfo.net/ontology/2.0/lexinfo"/>
    </owl:Class>
    


    <!-- http://www.lexinfo.net/ontology/2.0/lexinfo#Case -->

    <owl:Class rdf:about="&lexinfo;Case">
        <rdfs:subClassOf rdf:resource="&lexinfo;MorphosyntacticProperty"/>
        <rdfs:isDefinedBy rdf:resource="http://www.lexinfo.net/ontology/2.0/lexinfo"/>
    </owl:Class>
    


    <!-- http://www.lexinfo.net/ontology/2.0/lexinfo#ClausalArgument -->

    <owl:Class rdf:about="&lexinfo;ClausalArgument">
        <rdfs:subClassOf rdf:resource="&lemon;Argument"/>
        <rdfs:isDefinedBy rdf:resource="http://www.lexinfo.net/ontology/2.0/lexinfo"/>
    </owl:Class>
    


    <!-- http://www.lexinfo.net/ontology/2.0/lexinfo#Cliticness -->

    <owl:Class rdf:about="&lexinfo;Cliticness">
        <rdfs:subClassOf rdf:resource="&lexinfo;MorphosyntacticProperty"/>
        <rdfs:isDefinedBy rdf:resource="http://www.lexinfo.net/ontology/2.0/lexinfo"/>
    </owl:Class>
    


    <!-- http://www.lexinfo.net/ontology/2.0/lexinfo#CommonNoun -->

    <owl:Class rdf:about="&lexinfo;CommonNoun">
        <owl:equivalentClass>
            <owl:Restriction>
                <owl:onProperty rdf:resource="&lexinfo;partOfSpeech"/>
                <owl:hasValue rdf:resource="&lexinfo;commonNoun"/>
            </owl:Restriction>
        </owl:equivalentClass>
        <rdfs:subClassOf rdf:resource="&lexinfo;Noun"/>
        <rdfs:isDefinedBy rdf:resource="http://www.lexinfo.net/ontology/2.0/lexinfo"/>
    </owl:Class>
    


    <!-- http://www.lexinfo.net/ontology/2.0/lexinfo#ComparativeAdjunct -->

    <owl:Class rdf:about="&lexinfo;ComparativeAdjunct">
        <rdfs:subClassOf rdf:resource="&lexinfo;Adjunct"/>
        <rdfs:isDefinedBy rdf:resource="http://www.lexinfo.net/ontology/2.0/lexinfo"/>
    </owl:Class>
    


    <!-- http://www.lexinfo.net/ontology/2.0/lexinfo#Complement -->

    <owl:Class rdf:about="&lexinfo;Complement">
        <rdfs:subClassOf rdf:resource="&lemon;Argument"/>
        <rdfs:isDefinedBy rdf:resource="http://www.lexinfo.net/ontology/2.0/lexinfo"/>
    </owl:Class>
    


    <!-- http://www.lexinfo.net/ontology/2.0/lexinfo#Conjunction -->

    <owl:Class rdf:about="&lexinfo;Conjunction">
        <owl:equivalentClass>
            <owl:Restriction>
                <owl:onProperty rdf:resource="&lexinfo;partOfSpeech"/>
                <owl:someValuesFrom rdf:resource="&lexinfo;ConjunctionPOS"/>
            </owl:Restriction>
        </owl:equivalentClass>
        <rdfs:subClassOf rdf:resource="&lemon;Word"/>
        <rdfs:isDefinedBy rdf:resource="http://www.lexinfo.net/ontology/2.0/lexinfo"/>
    </owl:Class>
    


    <!-- http://www.lexinfo.net/ontology/2.0/lexinfo#ConjunctionPOS -->

    <owl:Class rdf:about="&lexinfo;ConjunctionPOS">
        <rdfs:subClassOf rdf:resource="&lexinfo;PartOfSpeech"/>
        <rdfs:isDefinedBy rdf:resource="http://www.lexinfo.net/ontology/2.0/lexinfo"/>
    </owl:Class>
    


    <!-- http://www.lexinfo.net/ontology/2.0/lexinfo#Control -->

    <owl:Class rdf:about="&lexinfo;Control">
        <rdfs:subClassOf rdf:resource="&lemon;Frame"/>
        <rdfs:comment xml:lang="en">Control indicates how a an argument from a main clause will be utilized in a subclause. This class includes both control structures and raising structures</rdfs:comment>
        <rdfs:comment xml:lang="en">Указывает, как аргумент главного предложения будет использован в подчинительном предложении. В этот класс включены классы control structures и raising structures</rdfs:comment>
        <rdfs:isDefinedBy rdf:resource="http://www.lexinfo.net/ontology/2.0/lexinfo"/>
    </owl:Class>
    


    <!-- http://www.lexinfo.net/ontology/2.0/lexinfo#Dating -->

    <owl:Class rdf:about="&lexinfo;Dating">
        <rdfs:subClassOf rdf:resource="&lemon;PropertyValue"/>
        <rdfs:isDefinedBy rdf:resource="http://www.lexinfo.net/ontology/2.0/lexinfo"/>
    </owl:Class>
    


    <!-- http://www.lexinfo.net/ontology/2.0/lexinfo#DativePostPositiveArgument -->

    <owl:Class rdf:about="&lexinfo;DativePostPositiveArgument">
        <owl:equivalentClass>
            <owl:Class>
                <owl:intersectionOf rdf:parseType="Collection">
                    <rdf:Description rdf:about="&lexinfo;PostPositiveArgument"/>
                    <owl:Restriction>
                        <owl:onProperty rdf:resource="&lemon;marker"/>
                        <owl:hasValue rdf:resource="&lexinfo;dativeCase"/>
                    </owl:Restriction>
                </owl:intersectionOf>
            </owl:Class>
        </owl:equivalentClass>
        <rdfs:subClassOf rdf:resource="&lexinfo;PostPositiveArgument"/>
        <rdfs:isDefinedBy rdf:resource="http://www.lexinfo.net/ontology/2.0/lexinfo"/>
    </owl:Class>
    


    <!-- http://www.lexinfo.net/ontology/2.0/lexinfo#DativeTransitiveFrame -->

    <owl:Class rdf:about="&lexinfo;DativeTransitiveFrame">
        <owl:equivalentClass>
            <owl:Class>
                <owl:intersectionOf rdf:parseType="Collection">
                    <rdf:Description rdf:about="&lexinfo;VerbFrame"/>
                    <owl:Restriction>
                        <owl:onProperty rdf:resource="&lexinfo;directObject"/>
                        <owl:cardinality rdf:datatype="&xsd;nonNegativeInteger">0</owl:cardinality>
                    </owl:Restriction>
                    <owl:Restriction>
                        <owl:onProperty rdf:resource="&lexinfo;indirectObject"/>
                        <owl:cardinality rdf:datatype="&xsd;nonNegativeInteger">1</owl:cardinality>
                    </owl:Restriction>
                    <owl:Restriction>
                        <owl:onProperty rdf:resource="&lexinfo;subject"/>
                        <owl:cardinality rdf:datatype="&xsd;nonNegativeInteger">1</owl:cardinality>
                    </owl:Restriction>
                </owl:intersectionOf>
            </owl:Class>
        </owl:equivalentClass>
        <rdfs:subClassOf rdf:resource="&lexinfo;VerbFrame"/>
        <example xml:lang="de">ich DANKE dir</example>
        <rdfs:isDefinedBy rdf:resource="http://www.lexinfo.net/ontology/2.0/lexinfo"/>
    </owl:Class>
    


    <!-- http://www.lexinfo.net/ontology/2.0/lexinfo#DeclarativeClause -->

    <owl:Class rdf:about="&lexinfo;DeclarativeClause">
        <rdfs:subClassOf rdf:resource="&lexinfo;ClausalArgument"/>
        <rdfs:comment xml:lang="en">A clause beginning with the declarative conjunction (&quot;that&quot; in English)</rdfs:comment>
        <rdfs:isDefinedBy rdf:resource="http://www.lexinfo.net/ontology/2.0/lexinfo"/>
    </owl:Class>
    


    <!-- http://www.lexinfo.net/ontology/2.0/lexinfo#DeclarativeFrame -->

    <owl:Class rdf:about="&lexinfo;DeclarativeFrame">
        <owl:equivalentClass>
            <owl:Class>
                <owl:intersectionOf rdf:parseType="Collection">
                    <rdf:Description rdf:about="&lexinfo;VerbFrame"/>
                    <owl:Restriction>
                        <owl:onProperty rdf:resource="&lexinfo;declarativeClause"/>
                        <owl:minCardinality rdf:datatype="&xsd;nonNegativeInteger">1</owl:minCardinality>
                    </owl:Restriction>
                </owl:intersectionOf>
            </owl:Class>
        </owl:equivalentClass>
        <rdfs:subClassOf rdf:resource="&lexinfo;VerbFrame"/>
        <rdfs:comment xml:lang="en">Declarative frames take a clause as an argument, this argument is marker with the declarative conjunction (&quot;that&quot; in English)</rdfs:comment>
        <rdfs:comment xml:lang="ru">Берёт предложение как аргумент, при том что данный аргумент - это маркер (описательный союз) (&quot;that&quot; в анлийском языке) (&quot;который&quot;, &quot;что&quot; в русском языке)</rdfs:comment>
        <rdfs:isDefinedBy rdf:resource="http://www.lexinfo.net/ontology/2.0/lexinfo"/>
    </owl:Class>
    


    <!-- http://www.lexinfo.net/ontology/2.0/lexinfo#Definiteness -->

    <owl:Class rdf:about="&lexinfo;Definiteness">
        <rdfs:subClassOf rdf:resource="&lexinfo;MorphosyntacticProperty"/>
        <rdfs:isDefinedBy rdf:resource="http://www.lexinfo.net/ontology/2.0/lexinfo"/>
    </owl:Class>
    


    <!-- http://www.lexinfo.net/ontology/2.0/lexinfo#Degree -->

    <owl:Class rdf:about="&lexinfo;Degree">
        <rdfs:subClassOf rdf:resource="&lexinfo;MorphosyntacticProperty"/>
        <rdfs:isDefinedBy rdf:resource="http://www.lexinfo.net/ontology/2.0/lexinfo"/>
    </owl:Class>
    


    <!-- http://www.lexinfo.net/ontology/2.0/lexinfo#Determiner -->

    <owl:Class rdf:about="&lexinfo;Determiner">
        <owl:equivalentClass>
            <owl:Restriction>
                <owl:onProperty rdf:resource="&lexinfo;partOfSpeech"/>
                <owl:someValuesFrom rdf:resource="&lexinfo;DeterminerPOS"/>
            </owl:Restriction>
        </owl:equivalentClass>
        <rdfs:subClassOf rdf:resource="&lemon;Word"/>
        <rdfs:isDefinedBy rdf:resource="http://www.lexinfo.net/ontology/2.0/lexinfo"/>
    </owl:Class>
    


    <!-- http://www.lexinfo.net/ontology/2.0/lexinfo#DeterminerPOS -->

    <owl:Class rdf:about="&lexinfo;DeterminerPOS">
        <rdfs:subClassOf rdf:resource="&lexinfo;PartOfSpeech"/>
        <rdfs:isDefinedBy rdf:resource="http://www.lexinfo.net/ontology/2.0/lexinfo"/>
    </owl:Class>
    


    <!-- http://www.lexinfo.net/ontology/2.0/lexinfo#DirectObject -->

    <owl:Class rdf:about="&lexinfo;DirectObject">
        <rdfs:subClassOf rdf:resource="&lexinfo;Object"/>
        <rdfs:isDefinedBy rdf:resource="http://www.lexinfo.net/ontology/2.0/lexinfo"/>
    </owl:Class>
    


    <!-- http://www.lexinfo.net/ontology/2.0/lexinfo#DitransitiveDoubleAccusativeFrame -->

    <owl:Class rdf:about="&lexinfo;DitransitiveDoubleAccusativeFrame">
        <owl:equivalentClass>
            <owl:Class>
                <owl:intersectionOf rdf:parseType="Collection">
                    <rdf:Description rdf:about="&lexinfo;VerbFrame"/>
                    <owl:Restriction>
                        <owl:onProperty rdf:resource="&lexinfo;directObject"/>
                        <owl:cardinality rdf:datatype="&xsd;nonNegativeInteger">2</owl:cardinality>
                    </owl:Restriction>
                    <owl:Restriction>
                        <owl:onProperty rdf:resource="&lexinfo;subject"/>
                        <owl:cardinality rdf:datatype="&xsd;nonNegativeInteger">1</owl:cardinality>
                    </owl:Restriction>
                </owl:intersectionOf>
            </owl:Class>
        </owl:equivalentClass>
        <rdfs:subClassOf rdf:resource="&lexinfo;VerbFrame"/>
        <example xml:lang="de">das KOSTET ihn sein leben</example>
        <rdfs:isDefinedBy rdf:resource="http://www.lexinfo.net/ontology/2.0/lexinfo"/>
    </owl:Class>
    


    <!-- http://www.lexinfo.net/ontology/2.0/lexinfo#DitransitiveFrame -->

    <owl:Class rdf:about="&lexinfo;DitransitiveFrame">
        <owl:equivalentClass>
            <owl:Class>
                <owl:intersectionOf rdf:parseType="Collection">
                    <rdf:Description rdf:about="&lexinfo;VerbFrame"/>
                    <owl:Restriction>
                        <owl:onProperty rdf:resource="&lexinfo;directObject"/>
                        <owl:cardinality rdf:datatype="&xsd;nonNegativeInteger">1</owl:cardinality>
                    </owl:Restriction>
                    <owl:Restriction>
                        <owl:onProperty rdf:resource="&lexinfo;indirectObject"/>
                        <owl:cardinality rdf:datatype="&xsd;nonNegativeInteger">1</owl:cardinality>
                    </owl:Restriction>
                    <owl:Restriction>
                        <owl:onProperty rdf:resource="&lexinfo;subject"/>
                        <owl:cardinality rdf:datatype="&xsd;nonNegativeInteger">1</owl:cardinality>
                    </owl:Restriction>
                </owl:intersectionOf>
            </owl:Class>
        </owl:equivalentClass>
        <rdfs:subClassOf rdf:resource="&lexinfo;VerbFrame"/>
        <example xml:lang="de">mein vater SCHREIBT ihr einen brief</example>
        <example xml:lang="en">i GAVE him it</example>
        <rdfs:isDefinedBy rdf:resource="http://www.lexinfo.net/ontology/2.0/lexinfo"/>
    </owl:Class>
    


    <!-- http://www.lexinfo.net/ontology/2.0/lexinfo#DitransitiveFrame_For -->

    <owl:Class rdf:about="&lexinfo;DitransitiveFrame_For">
        <rdfs:subClassOf rdf:resource="&lexinfo;DitransitiveFrame"/>
        <languageSpecific>en</languageSpecific>
        <example xml:lang="en">she BOUGHT him it
she BOUGHT it FOR him</example>
        <rdfs:isDefinedBy rdf:resource="http://www.lexinfo.net/ontology/2.0/lexinfo"/>
    </owl:Class>
    


    <!-- http://www.lexinfo.net/ontology/2.0/lexinfo#DitransitiveFrame_To -->

    <owl:Class rdf:about="&lexinfo;DitransitiveFrame_To">
        <rdfs:subClassOf rdf:resource="&lexinfo;DitransitiveFrame"/>
        <languageSpecific>en</languageSpecific>
        <example xml:lang="en">he GAVE his mother a present
he GAVE a present TO his mother</example>
        <rdfs:isDefinedBy rdf:resource="http://www.lexinfo.net/ontology/2.0/lexinfo"/>
    </owl:Class>
    


    <!-- http://www.lexinfo.net/ontology/2.0/lexinfo#Finiteness -->

    <owl:Class rdf:about="&lexinfo;Finiteness">
        <rdfs:subClassOf rdf:resource="&lexinfo;MorphosyntacticProperty"/>
        <rdfs:isDefinedBy rdf:resource="http://www.lexinfo.net/ontology/2.0/lexinfo"/>
    </owl:Class>
    


    <!-- http://www.lexinfo.net/ontology/2.0/lexinfo#Frequency -->

    <owl:Class rdf:about="&lexinfo;Frequency">
        <rdfs:subClassOf rdf:resource="&lemon;SenseContext"/>
        <rdfs:isDefinedBy rdf:resource="http://www.lexinfo.net/ontology/2.0/lexinfo"/>
    </owl:Class>
    


    <!-- http://www.lexinfo.net/ontology/2.0/lexinfo#FusedPreposition -->

    <owl:Class rdf:about="&lexinfo;FusedPreposition">
        <owl:equivalentClass>
            <owl:Restriction>
                <owl:onProperty rdf:resource="&lexinfo;partOfSpeech"/>
                <owl:someValuesFrom rdf:resource="&lexinfo;FusedPrepositionPOS"/>
            </owl:Restriction>
        </owl:equivalentClass>
        <rdfs:subClassOf rdf:resource="&lemon;Word"/>
        <rdfs:comment xml:lang="en">A word that is a fusion of a preposition and some other word... examples include the German words &quot;zum&quot; and &quot;daran&quot;</rdfs:comment>
        <rdfs:comment xml:lang="ru">Слияние предлога и любого другого слова. Примеры включают немецкие слова &quot;zum&quot; и &quot;daran&quot;</rdfs:comment>
        <rdfs:isDefinedBy rdf:resource="http://www.lexinfo.net/ontology/2.0/lexinfo"/>
    </owl:Class>
    


    <!-- http://www.lexinfo.net/ontology/2.0/lexinfo#FusedPrepositionPOS -->

    <owl:Class rdf:about="&lexinfo;FusedPrepositionPOS">
        <rdfs:subClassOf rdf:resource="&lexinfo;PartOfSpeech"/>
        <rdfs:isDefinedBy rdf:resource="http://www.lexinfo.net/ontology/2.0/lexinfo"/>
    </owl:Class>
    


    <!-- http://www.lexinfo.net/ontology/2.0/lexinfo#Gender -->

    <owl:Class rdf:about="&lexinfo;Gender">
        <rdfs:subClassOf rdf:resource="&lexinfo;MorphosyntacticProperty"/>
        <rdfs:isDefinedBy rdf:resource="http://www.lexinfo.net/ontology/2.0/lexinfo"/>
    </owl:Class>
    


    <!-- http://www.lexinfo.net/ontology/2.0/lexinfo#GenitiveDitransitiveFrame -->

    <owl:Class rdf:about="&lexinfo;GenitiveDitransitiveFrame">
        <owl:equivalentClass>
            <owl:Class>
                <owl:intersectionOf rdf:parseType="Collection">
                    <rdf:Description rdf:about="&lexinfo;VerbFrame"/>
                    <owl:Restriction>
                        <owl:onProperty rdf:resource="&lexinfo;directObject"/>
                        <owl:cardinality rdf:datatype="&xsd;nonNegativeInteger">1</owl:cardinality>
                    </owl:Restriction>
                    <owl:Restriction>
                        <owl:onProperty rdf:resource="&lexinfo;genitiveObject"/>
                        <owl:cardinality rdf:datatype="&xsd;nonNegativeInteger">1</owl:cardinality>
                    </owl:Restriction>
                    <owl:Restriction>
                        <owl:onProperty rdf:resource="&lexinfo;subject"/>
                        <owl:cardinality rdf:datatype="&xsd;nonNegativeInteger">1</owl:cardinality>
                    </owl:Restriction>
                </owl:intersectionOf>
            </owl:Class>
        </owl:equivalentClass>
        <rdfs:subClassOf rdf:resource="&lexinfo;VerbFrame"/>
        <example xml:lang="de">man KLAGTE ihn des diebstahls AN</example>
        <rdfs:isDefinedBy rdf:resource="http://www.lexinfo.net/ontology/2.0/lexinfo"/>
    </owl:Class>
    


    <!-- http://www.lexinfo.net/ontology/2.0/lexinfo#GenitiveObject -->

    <owl:Class rdf:about="&lexinfo;GenitiveObject">
        <owl:equivalentClass>
            <owl:Restriction>
                <owl:onProperty rdf:resource="&lemon;marker"/>
                <owl:hasValue rdf:resource="&lexinfo;genitiveCase"/>
            </owl:Restriction>
        </owl:equivalentClass>
        <rdfs:subClassOf rdf:resource="&lexinfo;Object"/>
        <rdfs:isDefinedBy rdf:resource="http://www.lexinfo.net/ontology/2.0/lexinfo"/>
    </owl:Class>
    


    <!-- http://www.lexinfo.net/ontology/2.0/lexinfo#GenitivePostPositiveArgument -->

    <owl:Class rdf:about="&lexinfo;GenitivePostPositiveArgument">
        <owl:equivalentClass>
            <owl:Class>
                <owl:intersectionOf rdf:parseType="Collection">
                    <rdf:Description rdf:about="&lexinfo;PostPositiveArgument"/>
                    <owl:Restriction>
                        <owl:onProperty rdf:resource="&lemon;marker"/>
                        <owl:hasValue rdf:resource="&lexinfo;genitiveCase"/>
                    </owl:Restriction>
                </owl:intersectionOf>
            </owl:Class>
        </owl:equivalentClass>
        <rdfs:subClassOf rdf:resource="&lexinfo;PostPositiveArgument"/>
        <rdfs:isDefinedBy rdf:resource="http://www.lexinfo.net/ontology/2.0/lexinfo"/>
    </owl:Class>
    


    <!-- http://www.lexinfo.net/ontology/2.0/lexinfo#GenitiveTransitiveFrame -->

    <owl:Class rdf:about="&lexinfo;GenitiveTransitiveFrame">
        <owl:equivalentClass>
            <owl:Class>
                <owl:intersectionOf rdf:parseType="Collection">
                    <rdf:Description rdf:about="&lexinfo;VerbFrame"/>
                    <owl:Restriction>
                        <owl:onProperty rdf:resource="&lexinfo;genitiveObject"/>
                        <owl:cardinality rdf:datatype="&xsd;nonNegativeInteger">1</owl:cardinality>
                    </owl:Restriction>
                    <owl:Restriction>
                        <owl:onProperty rdf:resource="&lexinfo;subject"/>
                        <owl:cardinality rdf:datatype="&xsd;nonNegativeInteger">1</owl:cardinality>
                    </owl:Restriction>
                </owl:intersectionOf>
            </owl:Class>
        </owl:equivalentClass>
        <rdfs:subClassOf rdf:resource="&lexinfo;VerbFrame"/>
        <example xml:lang="de">wir BEDENKEN jenes mannes</example>
        <rdfs:isDefinedBy rdf:resource="http://www.lexinfo.net/ontology/2.0/lexinfo"/>
    </owl:Class>
    


    <!-- http://www.lexinfo.net/ontology/2.0/lexinfo#Gerund -->

    <owl:Class rdf:about="&lexinfo;Gerund">
        <rdfs:subClassOf rdf:resource="&lexinfo;ClausalArgument"/>
        <rdfs:comment xml:lang="en">A clause, whose head is a non-finite verb form, which is used in place of an argument. In English these use the &quot;-ing&quot; suffix</rdfs:comment>
        <rdfs:comment xml:lang="ru">Предлложение, в котором главным словом (аргументом) является нефинитный глагол. Примеры из английского языка: &quot;-ing&quot;</rdfs:comment>
        <rdfs:isDefinedBy rdf:resource="http://www.lexinfo.net/ontology/2.0/lexinfo"/>
    </owl:Class>
    


    <!-- http://www.lexinfo.net/ontology/2.0/lexinfo#GerundACFrame -->

    <owl:Class rdf:about="&lexinfo;GerundACFrame">
        <owl:equivalentClass>
            <owl:Class>
                <owl:intersectionOf rdf:parseType="Collection">
                    <rdf:Description rdf:about="&lexinfo;ArbitraryControl"/>
                    <rdf:Description rdf:about="&lexinfo;GerundFrame"/>
                </owl:intersectionOf>
            </owl:Class>
        </owl:equivalentClass>
        <rdfs:subClassOf rdf:resource="&lexinfo;GerundFrame"/>
        <rdfs:isDefinedBy rdf:resource="http://www.lexinfo.net/ontology/2.0/lexinfo"/>
    </owl:Class>
    


    <!-- http://www.lexinfo.net/ontology/2.0/lexinfo#GerundFrame -->

    <owl:Class rdf:about="&lexinfo;GerundFrame">
        <owl:equivalentClass>
            <owl:Class>
                <owl:intersectionOf rdf:parseType="Collection">
                    <rdf:Description rdf:about="&lexinfo;VerbFrame"/>
                    <owl:Restriction>
                        <owl:onProperty rdf:resource="&lemon;synArg"/>
                        <owl:someValuesFrom rdf:resource="&lexinfo;Gerund"/>
                    </owl:Restriction>
                </owl:intersectionOf>
            </owl:Class>
        </owl:equivalentClass>
        <rdfs:subClassOf rdf:resource="&lexinfo;VerbFrame"/>
        <rdfs:comment xml:lang="en">Indicates one of the arguments is a gerund clause</rdfs:comment>
        <rdfs:comment xml:lang="ru">Указывает на аргумент предложения, выраженный герундием</rdfs:comment>
        <rdfs:isDefinedBy rdf:resource="http://www.lexinfo.net/ontology/2.0/lexinfo"/>
    </owl:Class>
    


    <!-- http://www.lexinfo.net/ontology/2.0/lexinfo#GerundOCFrame -->

    <owl:Class rdf:about="&lexinfo;GerundOCFrame">
        <owl:equivalentClass>
            <owl:Class>
                <owl:intersectionOf rdf:parseType="Collection">
                    <rdf:Description rdf:about="&lexinfo;GerundFrame"/>
                    <rdf:Description rdf:about="&lexinfo;ObjectControl"/>
                </owl:intersectionOf>
            </owl:Class>
        </owl:equivalentClass>
        <rdfs:subClassOf rdf:resource="&lexinfo;GerundFrame"/>
        <rdfs:isDefinedBy rdf:resource="http://www.lexinfo.net/ontology/2.0/lexinfo"/>
    </owl:Class>
    


    <!-- http://www.lexinfo.net/ontology/2.0/lexinfo#GerundSCFrame -->

    <owl:Class rdf:about="&lexinfo;GerundSCFrame">
        <owl:equivalentClass>
            <owl:Class>
                <owl:intersectionOf rdf:parseType="Collection">
                    <rdf:Description rdf:about="&lexinfo;GerundFrame"/>
                    <rdf:Description rdf:about="&lexinfo;SubjectControl"/>
                </owl:intersectionOf>
            </owl:Class>
        </owl:equivalentClass>
        <rdfs:subClassOf rdf:resource="&lexinfo;GerundFrame"/>
        <rdfs:isDefinedBy rdf:resource="http://www.lexinfo.net/ontology/2.0/lexinfo"/>
    </owl:Class>
    


    <!-- http://www.lexinfo.net/ontology/2.0/lexinfo#ImpersonalFrame -->

    <owl:Class rdf:about="&lexinfo;ImpersonalFrame">
        <owl:equivalentClass>
            <owl:Class>
                <owl:intersectionOf rdf:parseType="Collection">
                    <rdf:Description rdf:about="&lexinfo;VerbFrame"/>
                    <owl:Restriction>
                        <owl:onProperty rdf:resource="&lexinfo;subject"/>
                        <owl:cardinality rdf:datatype="&xsd;nonNegativeInteger">0</owl:cardinality>
                    </owl:Restriction>
                </owl:intersectionOf>
            </owl:Class>
        </owl:equivalentClass>
        <rdfs:subClassOf rdf:resource="&lexinfo;VerbFrame"/>
        <rdfs:isDefinedBy rdf:resource="http://www.lexinfo.net/ontology/2.0/lexinfo"/>
    </owl:Class>
    


    <!-- http://www.lexinfo.net/ontology/2.0/lexinfo#ImpersonalIntransitiveFrame -->

    <owl:Class rdf:about="&lexinfo;ImpersonalIntransitiveFrame">
        <owl:equivalentClass>
            <owl:Class>
                <owl:intersectionOf rdf:parseType="Collection">
                    <rdf:Description rdf:about="&lexinfo;ImpersonalFrame"/>
                    <owl:Restriction>
                        <owl:onProperty rdf:resource="&lexinfo;object"/>
                        <owl:cardinality rdf:datatype="&xsd;nonNegativeInteger">0</owl:cardinality>
                    </owl:Restriction>
                </owl:intersectionOf>
            </owl:Class>
        </owl:equivalentClass>
        <rdfs:subClassOf rdf:resource="&lexinfo;ImpersonalFrame"/>
        <rdfs:isDefinedBy rdf:resource="http://www.lexinfo.net/ontology/2.0/lexinfo"/>
    </owl:Class>
    


    <!-- http://www.lexinfo.net/ontology/2.0/lexinfo#ImpersonalIntransitivePPFrame -->

    <owl:Class rdf:about="&lexinfo;ImpersonalIntransitivePPFrame">
        <owl:equivalentClass>
            <owl:Class>
                <owl:intersectionOf rdf:parseType="Collection">
                    <rdf:Description rdf:about="&lexinfo;ImpersonalIntransitiveFrame"/>
                    <rdf:Description rdf:about="&lexinfo;PrepositionalFrame"/>
                </owl:intersectionOf>
            </owl:Class>
        </owl:equivalentClass>
        <rdfs:subClassOf rdf:resource="&lexinfo;ImpersonalTransitiveFrame"/>
        <rdfs:subClassOf rdf:resource="&lexinfo;PrepositionalFrame"/>
        <example xml:lang="en">it REEKS OF tar</example>
        <rdfs:isDefinedBy rdf:resource="http://www.lexinfo.net/ontology/2.0/lexinfo"/>
    </owl:Class>
    


    <!-- http://www.lexinfo.net/ontology/2.0/lexinfo#ImpersonalTransitiveFrame -->

    <owl:Class rdf:about="&lexinfo;ImpersonalTransitiveFrame">
        <owl:equivalentClass>
            <owl:Class>
                <owl:intersectionOf rdf:parseType="Collection">
                    <rdf:Description rdf:about="&lexinfo;ImpersonalFrame"/>
                    <owl:Restriction>
                        <owl:onProperty rdf:resource="&lexinfo;directObject"/>
                        <owl:minCardinality rdf:datatype="&xsd;nonNegativeInteger">1</owl:minCardinality>
                    </owl:Restriction>
                </owl:intersectionOf>
            </owl:Class>
        </owl:equivalentClass>
        <rdfs:subClassOf rdf:resource="&lexinfo;ImpersonalFrame"/>
        <example xml:lang="de">es JUCKT mich</example>
        <rdfs:isDefinedBy rdf:resource="http://www.lexinfo.net/ontology/2.0/lexinfo"/>
    </owl:Class>
    


    <!-- http://www.lexinfo.net/ontology/2.0/lexinfo#IndirectObject -->

    <owl:Class rdf:about="&lexinfo;IndirectObject">
        <rdfs:subClassOf rdf:resource="&lexinfo;Object"/>
        <rdfs:isDefinedBy rdf:resource="http://www.lexinfo.net/ontology/2.0/lexinfo"/>
    </owl:Class>
    


    <!-- http://www.lexinfo.net/ontology/2.0/lexinfo#InfinitiveClause -->

    <owl:Class rdf:about="&lexinfo;InfinitiveClause">
        <rdfs:subClassOf rdf:resource="&lexinfo;ClausalArgument"/>
        <rdfs:comment xml:lang="en">A clause whose main verb is infinitive</rdfs:comment>
        <rdfs:comment xml:lang="ru">Предложение, в котором основной глагол - инфйинитив</rdfs:comment>
        <rdfs:isDefinedBy rdf:resource="http://www.lexinfo.net/ontology/2.0/lexinfo"/>
    </owl:Class>
    


    <!-- http://www.lexinfo.net/ontology/2.0/lexinfo#InfinitiveFrame -->

    <owl:Class rdf:about="&lexinfo;InfinitiveFrame">
        <owl:equivalentClass>
            <owl:Class>
                <owl:intersectionOf rdf:parseType="Collection">
                    <rdf:Description rdf:about="&lexinfo;VerbFrame"/>
                    <owl:Restriction>
                        <owl:onProperty rdf:resource="&lexinfo;infinitiveClause"/>
                        <owl:minCardinality rdf:datatype="&xsd;nonNegativeInteger">1</owl:minCardinality>
                    </owl:Restriction>
                </owl:intersectionOf>
            </owl:Class>
        </owl:equivalentClass>
        <rdfs:subClassOf rdf:resource="&lexinfo;VerbFrame"/>
        <rdfs:comment xml:lang="en">Infinitive frames take an infinitive clause as an argument</rdfs:comment>
        <rdfs:comment xml:lang="ru">Указывает на инфинитив как аргумент предложения</rdfs:comment>
        <rdfs:isDefinedBy rdf:resource="http://www.lexinfo.net/ontology/2.0/lexinfo"/>
    </owl:Class>
    


    <!-- http://www.lexinfo.net/ontology/2.0/lexinfo#Infix -->

    <owl:Class rdf:about="&lexinfo;Infix">
        <owl:equivalentClass>
            <owl:Restriction>
                <owl:onProperty rdf:resource="&lexinfo;termElement"/>
                <owl:someValuesFrom rdf:resource="&lexinfo;Infix"/>
            </owl:Restriction>
        </owl:equivalentClass>
        <rdfs:subClassOf rdf:resource="&lexinfo;Affix"/>
        <rdfs:isDefinedBy rdf:resource="http://www.lexinfo.net/ontology/2.0/lexinfo"/>
    </owl:Class>
    


    <!-- http://www.lexinfo.net/ontology/2.0/lexinfo#Interjection -->

    <owl:Class rdf:about="&lexinfo;Interjection">
        <owl:equivalentClass>
            <owl:Restriction>
                <owl:onProperty rdf:resource="&lexinfo;partOfSpeech"/>
                <owl:hasValue rdf:resource="&lexinfo;interjection"/>
            </owl:Restriction>
        </owl:equivalentClass>
        <rdfs:subClassOf rdf:resource="&lemon;Word"/>
        <rdfs:isDefinedBy rdf:resource="http://www.lexinfo.net/ontology/2.0/lexinfo"/>
    </owl:Class>
    


    <!-- http://www.lexinfo.net/ontology/2.0/lexinfo#InterrogativeClause -->

    <owl:Class rdf:about="&lexinfo;InterrogativeClause">
        <rdfs:subClassOf rdf:resource="&lexinfo;ClausalArgument"/>
        <rdfs:comment xml:lang="en">A subclause that begins interrogative construction (&quot;wh&quot;-word in English)</rdfs:comment>
        <rdfs:comment xml:lang="ru">Подчинительное предложение, которое начинается вопросительными конструкциями (&quot;wh&quot;-слова в английском языке, вопросительные слова (что, какой, который и т.д.) в русском языке)</rdfs:comment>
        <rdfs:isDefinedBy rdf:resource="http://www.lexinfo.net/ontology/2.0/lexinfo"/>
    </owl:Class>
    


    <!-- http://www.lexinfo.net/ontology/2.0/lexinfo#InterrogativeFrame -->

    <owl:Class rdf:about="&lexinfo;InterrogativeFrame">
        <owl:equivalentClass>
            <owl:Class>
                <owl:intersectionOf rdf:parseType="Collection">
                    <rdf:Description rdf:about="&lexinfo;VerbFrame"/>
                    <owl:Restriction>
                        <owl:onProperty rdf:resource="&lexinfo;interrogativeClause"/>
                        <owl:minCardinality rdf:datatype="&xsd;nonNegativeInteger">1</owl:minCardinality>
                    </owl:Restriction>
                </owl:intersectionOf>
            </owl:Class>
        </owl:equivalentClass>
        <rdfs:subClassOf rdf:resource="&lexinfo;VerbFrame"/>
        <rdfs:comment xml:lang="en">Indicates the frame has a subframe indicated with the appropriate interrogative (e.g., &quot;who&quot;, &quot;where&quot;, &quot;how&quot;)</rdfs:comment>
        <rdfs:comment xml:lang="ru">Указывает на вопросительные слова в подчинительном предложении (например, &quot;кто&quot;, &quot;где&quot;, &quot;как&quot;)</rdfs:comment>
        <rdfs:isDefinedBy rdf:resource="http://www.lexinfo.net/ontology/2.0/lexinfo"/>
    </owl:Class>
    


    <!-- http://www.lexinfo.net/ontology/2.0/lexinfo#InterrogativeInfinitiveFrame -->

    <owl:Class rdf:about="&lexinfo;InterrogativeInfinitiveFrame">
        <owl:equivalentClass>
            <owl:Class>
                <owl:intersectionOf rdf:parseType="Collection">
                    <rdf:Description rdf:about="&lexinfo;VerbFrame"/>
                    <owl:Restriction>
                        <owl:onProperty rdf:resource="&lexinfo;interrogativeInfinitiveClause"/>
                        <owl:minCardinality rdf:datatype="&xsd;nonNegativeInteger">1</owl:minCardinality>
                    </owl:Restriction>
                </owl:intersectionOf>
            </owl:Class>
        </owl:equivalentClass>
        <rdfs:subClassOf rdf:resource="&lexinfo;VerbFrame"/>
        <rdfs:comment xml:lang="en">Indicates the frame has an argument that is a clause with both an interrogative and the clause is in the infinitive form</rdfs:comment>
        <rdfs:comment xml:lang="ru">Указывает на предложение, в котором есть вопросительное слово и инфинитив</rdfs:comment>
        <rdfs:isDefinedBy rdf:resource="http://www.lexinfo.net/ontology/2.0/lexinfo"/>
    </owl:Class>
    


    <!-- http://www.lexinfo.net/ontology/2.0/lexinfo#IntransitiveAdjectivalComplementFrame -->

    <owl:Class rdf:about="&lexinfo;IntransitiveAdjectivalComplementFrame">
        <owl:equivalentClass>
            <owl:Class>
                <owl:intersectionOf rdf:parseType="Collection">
                    <rdf:Description rdf:about="&lexinfo;IntransitiveFrame"/>
                    <owl:Restriction>
                        <owl:onProperty rdf:resource="&lexinfo;predicativeAdjective"/>
                        <owl:minCardinality rdf:datatype="&xsd;nonNegativeInteger">1</owl:minCardinality>
                    </owl:Restriction>
                </owl:intersectionOf>
            </owl:Class>
        </owl:equivalentClass>
        <rdfs:subClassOf rdf:resource="&lexinfo;IntransitiveFrame"/>
        <example xml:lang="en">his reputation SANK low</example>
        <rdfs:isDefinedBy rdf:resource="http://www.lexinfo.net/ontology/2.0/lexinfo"/>
    </owl:Class>
    


    <!-- http://www.lexinfo.net/ontology/2.0/lexinfo#IntransitiveAdverbialComplementFrame -->

    <owl:Class rdf:about="&lexinfo;IntransitiveAdverbialComplementFrame">
        <owl:equivalentClass>
            <owl:Class>
                <owl:intersectionOf rdf:parseType="Collection">
                    <rdf:Description rdf:about="&lexinfo;IntransitiveFrame"/>
                    <owl:Restriction>
                        <owl:onProperty rdf:resource="&lexinfo;predicativeAdverb"/>
                        <owl:minCardinality rdf:datatype="&xsd;nonNegativeInteger">1</owl:minCardinality>
                    </owl:Restriction>
                </owl:intersectionOf>
            </owl:Class>
        </owl:equivalentClass>
        <rdfs:subClassOf rdf:resource="&lexinfo;IntransitiveFrame"/>
        <example xml:lang="en">he SEEMED well</example>
        <rdfs:isDefinedBy rdf:resource="http://www.lexinfo.net/ontology/2.0/lexinfo"/>
    </owl:Class>
    


    <!-- http://www.lexinfo.net/ontology/2.0/lexinfo#IntransitiveDeclarativeFrame -->

    <owl:Class rdf:about="&lexinfo;IntransitiveDeclarativeFrame">
        <owl:equivalentClass>
            <owl:Class>
                <owl:intersectionOf rdf:parseType="Collection">
                    <rdf:Description rdf:about="&lexinfo;DeclarativeFrame"/>
                    <rdf:Description rdf:about="&lexinfo;IntransitiveFrame"/>
                </owl:intersectionOf>
            </owl:Class>
        </owl:equivalentClass>
        <rdfs:subClassOf rdf:resource="&lexinfo;DeclarativeFrame"/>
        <example xml:lang="en">i KNOW [that is a bad idea]</example>
        <rdfs:isDefinedBy rdf:resource="http://www.lexinfo.net/ontology/2.0/lexinfo"/>
    </owl:Class>
    


    <!-- http://www.lexinfo.net/ontology/2.0/lexinfo#IntransitiveFrame -->

    <owl:Class rdf:about="&lexinfo;IntransitiveFrame">
        <owl:equivalentClass>
            <owl:Class>
                <owl:intersectionOf rdf:parseType="Collection">
                    <rdf:Description rdf:about="&lexinfo;VerbFrame"/>
                    <owl:Restriction>
                        <owl:onProperty rdf:resource="&lexinfo;directObject"/>
                        <owl:cardinality rdf:datatype="&xsd;nonNegativeInteger">0</owl:cardinality>
                    </owl:Restriction>
                    <owl:Restriction>
                        <owl:onProperty rdf:resource="&lexinfo;subject"/>
                        <owl:cardinality rdf:datatype="&xsd;nonNegativeInteger">1</owl:cardinality>
                    </owl:Restriction>
                </owl:intersectionOf>
            </owl:Class>
        </owl:equivalentClass>
        <rdfs:subClassOf rdf:resource="&lexinfo;VerbFrame"/>
        <example xml:lang="en">he LEFT</example>
        <rdfs:isDefinedBy rdf:resource="http://www.lexinfo.net/ontology/2.0/lexinfo"/>
    </owl:Class>
    


    <!-- http://www.lexinfo.net/ontology/2.0/lexinfo#IntransitiveInfinitiveACFrame -->

    <owl:Class rdf:about="&lexinfo;IntransitiveInfinitiveACFrame">
        <owl:equivalentClass>
            <owl:Class>
                <owl:intersectionOf rdf:parseType="Collection">
                    <rdf:Description rdf:about="&lexinfo;ArbitraryControl"/>
                    <rdf:Description rdf:about="&lexinfo;InfinitiveFrame"/>
                    <rdf:Description rdf:about="&lexinfo;IntransitiveFrame"/>
                </owl:intersectionOf>
            </owl:Class>
        </owl:equivalentClass>
        <rdfs:subClassOf rdf:resource="&lexinfo;InfinitiveFrame"/>
        <example xml:lang="en">I HELPED [to save the child]</example>
        <rdfs:isDefinedBy rdf:resource="http://www.lexinfo.net/ontology/2.0/lexinfo"/>
    </owl:Class>
    


    <!-- http://www.lexinfo.net/ontology/2.0/lexinfo#IntransitiveInfinitiveRSFrame -->

    <owl:Class rdf:about="&lexinfo;IntransitiveInfinitiveRSFrame">
        <owl:equivalentClass>
            <owl:Class>
                <owl:intersectionOf rdf:parseType="Collection">
                    <rdf:Description rdf:about="&lexinfo;InfinitiveFrame"/>
                    <rdf:Description rdf:about="&lexinfo;IntransitiveFrame"/>
                    <rdf:Description rdf:about="&lexinfo;RaisingSubject"/>
                </owl:intersectionOf>
            </owl:Class>
        </owl:equivalentClass>
        <rdfs:subClassOf rdf:resource="&lexinfo;InfinitiveFrame"/>
        <example xml:lang="en">he SEEMED [to be happy]</example>
        <rdfs:isDefinedBy rdf:resource="http://www.lexinfo.net/ontology/2.0/lexinfo"/>
    </owl:Class>
    


    <!-- http://www.lexinfo.net/ontology/2.0/lexinfo#IntransitiveInfinitiveSCFrame -->

    <owl:Class rdf:about="&lexinfo;IntransitiveInfinitiveSCFrame">
        <owl:equivalentClass>
            <owl:Class>
                <owl:intersectionOf rdf:parseType="Collection">
                    <rdf:Description rdf:about="&lexinfo;InfinitiveFrame"/>
                    <rdf:Description rdf:about="&lexinfo;IntransitiveFrame"/>
                    <rdf:Description rdf:about="&lexinfo;SubjectControl"/>
                </owl:intersectionOf>
            </owl:Class>
        </owl:equivalentClass>
        <rdfs:subClassOf rdf:resource="&lexinfo;InfinitiveFrame"/>
        <example xml:lang="en">I WANTED [to come]</example>
        <rdfs:isDefinedBy rdf:resource="http://www.lexinfo.net/ontology/2.0/lexinfo"/>
    </owl:Class>
    


    <!-- http://www.lexinfo.net/ontology/2.0/lexinfo#IntransitiveInterrogativeFrame -->

    <owl:Class rdf:about="&lexinfo;IntransitiveInterrogativeFrame">
        <owl:equivalentClass>
            <owl:Class>
                <owl:intersectionOf rdf:parseType="Collection">
                    <rdf:Description rdf:about="&lexinfo;InterrogativeFrame"/>
                    <rdf:Description rdf:about="&lexinfo;IntransitiveFrame"/>
                </owl:intersectionOf>
            </owl:Class>
        </owl:equivalentClass>
        <rdfs:subClassOf rdf:resource="&lexinfo;InterrogativeFrame"/>
        <rdfs:comment xml:lang="en">he ASKED [what he should do]</rdfs:comment>
        <rdfs:isDefinedBy rdf:resource="http://www.lexinfo.net/ontology/2.0/lexinfo"/>
    </owl:Class>
    


    <!-- http://www.lexinfo.net/ontology/2.0/lexinfo#IntransitiveInterrogativeInfinitiveFrame -->

    <owl:Class rdf:about="&lexinfo;IntransitiveInterrogativeInfinitiveFrame">
        <owl:equivalentClass>
            <owl:Class>
                <owl:intersectionOf rdf:parseType="Collection">
                    <rdf:Description rdf:about="&lexinfo;InterrogativeInfinitiveFrame"/>
                    <rdf:Description rdf:about="&lexinfo;IntransitiveFrame"/>
                </owl:intersectionOf>
            </owl:Class>
        </owl:equivalentClass>
        <rdfs:subClassOf rdf:resource="&lexinfo;InterrogativeInfinitiveFrame"/>
        <example xml:lang="en">he ASKED [what to do]</example>
        <rdfs:isDefinedBy rdf:resource="http://www.lexinfo.net/ontology/2.0/lexinfo"/>
    </owl:Class>
    


    <!-- http://www.lexinfo.net/ontology/2.0/lexinfo#IntransitiveNominalComplementFrame -->

    <owl:Class rdf:about="&lexinfo;IntransitiveNominalComplementFrame">
        <owl:equivalentClass>
            <owl:Class>
                <owl:intersectionOf rdf:parseType="Collection">
                    <rdf:Description rdf:about="&lexinfo;IntransitiveFrame"/>
                    <owl:Restriction>
                        <owl:onProperty rdf:resource="&lexinfo;predicativeNominative"/>
                        <owl:minCardinality rdf:datatype="&xsd;nonNegativeInteger">1</owl:minCardinality>
                    </owl:Restriction>
                </owl:intersectionOf>
            </owl:Class>
        </owl:equivalentClass>
        <rdfs:subClassOf rdf:resource="&lexinfo;IntransitiveFrame"/>
        <example xml:lang="en">he SEEMED a fool</example>
        <rdfs:isDefinedBy rdf:resource="http://www.lexinfo.net/ontology/2.0/lexinfo"/>
    </owl:Class>
    


    <!-- http://www.lexinfo.net/ontology/2.0/lexinfo#IntransitivePPDeclarativeFrame -->

    <owl:Class rdf:about="&lexinfo;IntransitivePPDeclarativeFrame">
        <owl:equivalentClass>
            <owl:Class>
                <owl:intersectionOf rdf:parseType="Collection">
                    <rdf:Description rdf:about="&lexinfo;DeclarativeFrame"/>
                    <rdf:Description rdf:about="&lexinfo;IntransitivePPFrame"/>
                </owl:intersectionOf>
            </owl:Class>
        </owl:equivalentClass>
        <rdfs:subClassOf rdf:resource="&lexinfo;DeclarativeFrame"/>
        <example xml:lang="en">the SUGGESTED to him [that he should go]</example>
        <rdfs:isDefinedBy rdf:resource="http://www.lexinfo.net/ontology/2.0/lexinfo"/>
    </owl:Class>
    


    <!-- http://www.lexinfo.net/ontology/2.0/lexinfo#IntransitivePPFrame -->

    <owl:Class rdf:about="&lexinfo;IntransitivePPFrame">
        <owl:equivalentClass>
            <owl:Class>
                <owl:intersectionOf rdf:parseType="Collection">
                    <rdf:Description rdf:about="&lexinfo;IntransitiveFrame"/>
                    <rdf:Description rdf:about="&lexinfo;PPFrame"/>
                </owl:intersectionOf>
            </owl:Class>
        </owl:equivalentClass>
        <rdfs:subClassOf rdf:resource="&lexinfo;IntransitiveFrame"/>
        <example xml:lang="en">he TOOK CARE OF her</example>
        <rdfs:isDefinedBy rdf:resource="http://www.lexinfo.net/ontology/2.0/lexinfo"/>
    </owl:Class>
    


    <!-- http://www.lexinfo.net/ontology/2.0/lexinfo#IntransitiveSententialFrame -->

    <owl:Class rdf:about="&lexinfo;IntransitiveSententialFrame">
        <owl:equivalentClass>
            <owl:Class>
                <owl:intersectionOf rdf:parseType="Collection">
                    <rdf:Description rdf:about="&lexinfo;IntransitiveFrame"/>
                    <rdf:Description rdf:about="&lexinfo;SententialFrame"/>
                </owl:intersectionOf>
            </owl:Class>
        </owl:equivalentClass>
        <rdfs:subClassOf rdf:resource="&lexinfo;SententialFrame"/>
        <example xml:lang="en">they THOUGHT he was always late</example>
        <rdfs:isDefinedBy rdf:resource="http://www.lexinfo.net/ontology/2.0/lexinfo"/>
    </owl:Class>
    


    <!-- http://www.lexinfo.net/ontology/2.0/lexinfo#ModificationType -->

    <owl:Class rdf:about="&lexinfo;ModificationType">
        <rdfs:subClassOf rdf:resource="&lexinfo;MorphosyntacticProperty"/>
        <rdfs:isDefinedBy rdf:resource="http://www.lexinfo.net/ontology/2.0/lexinfo"/>
    </owl:Class>
    


    <!-- http://www.lexinfo.net/ontology/2.0/lexinfo#Mood -->

    <owl:Class rdf:about="&lexinfo;Mood">
        <rdfs:subClassOf rdf:resource="&lexinfo;MorphosyntacticProperty"/>
        <rdfs:isDefinedBy rdf:resource="http://www.lexinfo.net/ontology/2.0/lexinfo"/>
    </owl:Class>
    


    <!-- http://www.lexinfo.net/ontology/2.0/lexinfo#MorphosyntacticProperty -->

    <owl:Class rdf:about="&lexinfo;MorphosyntacticProperty">
        <rdfs:subClassOf rdf:resource="&lemon;PropertyValue"/>
        <rdfs:isDefinedBy rdf:resource="http://www.lexinfo.net/ontology/2.0/lexinfo"/>
    </owl:Class>
    


    <!-- http://www.lexinfo.net/ontology/2.0/lexinfo#Negative -->

    <owl:Class rdf:about="&lexinfo;Negative">
        <rdfs:subClassOf rdf:resource="&lexinfo;MorphosyntacticProperty"/>
        <rdfs:isDefinedBy rdf:resource="http://www.lexinfo.net/ontology/2.0/lexinfo"/>
    </owl:Class>
    


    <!-- http://www.lexinfo.net/ontology/2.0/lexinfo#NominalComplementFrame -->

    <owl:Class rdf:about="&lexinfo;NominalComplementFrame">
        <owl:equivalentClass>
            <owl:Class>
                <owl:intersectionOf rdf:parseType="Collection">
                    <rdf:Description rdf:about="&lexinfo;VerbFrame"/>
                    <owl:Restriction>
                        <owl:onProperty rdf:resource="&lexinfo;predicativeNominative"/>
                        <owl:minCardinality rdf:datatype="&xsd;nonNegativeInteger">1</owl:minCardinality>
                    </owl:Restriction>
                </owl:intersectionOf>
            </owl:Class>
        </owl:equivalentClass>
        <rdfs:subClassOf rdf:resource="&lexinfo;VerbFrame"/>
        <rdfs:isDefinedBy rdf:resource="http://www.lexinfo.net/ontology/2.0/lexinfo"/>
    </owl:Class>
    


    <!-- http://www.lexinfo.net/ontology/2.0/lexinfo#NormativeAuthorization -->

    <owl:Class rdf:about="&lexinfo;NormativeAuthorization">
        <rdfs:subClassOf rdf:resource="&lemon;SenseContext"/>
        <rdfs:isDefinedBy rdf:resource="http://www.lexinfo.net/ontology/2.0/lexinfo"/>
    </owl:Class>
    


    <!-- http://www.lexinfo.net/ontology/2.0/lexinfo#Noun -->

    <owl:Class rdf:about="&lexinfo;Noun">
        <owl:equivalentClass>
            <owl:Restriction>
                <owl:onProperty rdf:resource="&lexinfo;partOfSpeech"/>
                <owl:someValuesFrom rdf:resource="&lexinfo;NounPOS"/>
            </owl:Restriction>
        </owl:equivalentClass>
        <rdfs:subClassOf rdf:resource="&lemon;Word"/>
        <rdfs:subClassOf>
            <owl:Restriction>
                <owl:onProperty rdf:resource="&lemon;synBehavior"/>
                <owl:allValuesFrom rdf:resource="&lexinfo;NounFrame"/>
            </owl:Restriction>
        </rdfs:subClassOf>
        <rdfs:isDefinedBy rdf:resource="http://www.lexinfo.net/ontology/2.0/lexinfo"/>
    </owl:Class>
    


    <!-- http://www.lexinfo.net/ontology/2.0/lexinfo#NounFrame -->

    <owl:Class rdf:about="&lexinfo;NounFrame">
        <rdfs:subClassOf rdf:resource="&lemon;Frame"/>
        <rdfs:isDefinedBy rdf:resource="http://www.lexinfo.net/ontology/2.0/lexinfo"/>
    </owl:Class>
    


    <!-- http://www.lexinfo.net/ontology/2.0/lexinfo#NounPOS -->

    <owl:Class rdf:about="&lexinfo;NounPOS">
        <rdfs:subClassOf rdf:resource="&lexinfo;PartOfSpeech"/>
        <rdfs:isDefinedBy rdf:resource="http://www.lexinfo.net/ontology/2.0/lexinfo"/>
    </owl:Class>
    


    <!-- http://www.lexinfo.net/ontology/2.0/lexinfo#NounPPFrame -->

    <owl:Class rdf:about="&lexinfo;NounPPFrame">
        <owl:equivalentClass>
            <owl:Class>
                <owl:intersectionOf rdf:parseType="Collection">
                    <rdf:Description rdf:about="&lexinfo;NounPredicateFrame"/>
                    <rdf:Description rdf:about="&lexinfo;PrepositionalFrame"/>
                </owl:intersectionOf>
            </owl:Class>
        </owl:equivalentClass>
        <rdfs:subClassOf rdf:resource="&lexinfo;NounFrame"/>
        <rdfs:isDefinedBy rdf:resource="http://www.lexinfo.net/ontology/2.0/lexinfo"/>
    </owl:Class>
    


    <!-- http://www.lexinfo.net/ontology/2.0/lexinfo#NounPhrase -->

    <owl:Class rdf:about="&lexinfo;NounPhrase">
        <owl:equivalentClass>
            <owl:Class>
                <owl:intersectionOf rdf:parseType="Collection">
                    <rdf:Description rdf:about="&lemon;Phrase"/>
                    <owl:Restriction>
                        <owl:onProperty rdf:resource="&lexinfo;head"/>
                        <owl:someValuesFrom rdf:resource="&lexinfo;Noun"/>
                    </owl:Restriction>
                </owl:intersectionOf>
            </owl:Class>
        </owl:equivalentClass>
        <rdfs:subClassOf rdf:resource="&lemon;Phrase"/>
        <rdfs:isDefinedBy rdf:resource="http://www.lexinfo.net/ontology/2.0/lexinfo"/>
    </owl:Class>
    
    <!-- http://www.lexinfo.net/ontology/2.0/lexinfo#PrepositionPhrase -->

    <owl:Class rdf:about="&lexinfo;PrepositionPhrase">
        <owl:equivalentClass>
            <owl:Class>
                <owl:intersectionOf rdf:parseType="Collection">
                    <rdf:Description rdf:about="&lemon;Phrase"/>
                    <owl:Restriction>
                        <owl:onProperty rdf:resource="&lexinfo;head"/>
                        <owl:someValuesFrom rdf:resource="&lexinfo;Preposition"/>
                    </owl:Restriction>
                </owl:intersectionOf>
            </owl:Class>
        </owl:equivalentClass>
        <rdfs:subClassOf rdf:resource="&lemon;Phrase"/>
        <rdfs:isDefinedBy rdf:resource="http://www.lexinfo.net/ontology/2.0/lexinfo"/>
    </owl:Class>
    



    <!-- http://www.lexinfo.net/ontology/2.0/lexinfo#NounPossessiveFrame -->

    <owl:Class rdf:about="&lexinfo;NounPossessiveFrame">
        <owl:equivalentClass>
            <owl:Class>
                <owl:intersectionOf rdf:parseType="Collection">
                    <rdf:Description rdf:about="&lexinfo;NounFrame"/>
                    <owl:Restriction>
                        <owl:onProperty rdf:resource="&lexinfo;copulativeArg"/>
                        <owl:minCardinality rdf:datatype="&xsd;nonNegativeInteger">1</owl:minCardinality>
                    </owl:Restriction>
                    <owl:Restriction>
                        <owl:onProperty rdf:resource="&lexinfo;possessiveAdjunct"/>
                        <owl:onClass rdf:resource="&lexinfo;PossessiveAdjunct"/>
                        <owl:minQualifiedCardinality rdf:datatype="&xsd;nonNegativeInteger">1</owl:minQualifiedCardinality>
                    </owl:Restriction>
                </owl:intersectionOf>
            </owl:Class>
        </owl:equivalentClass>
        <rdfs:subClassOf rdf:resource="&lexinfo;NounFrame"/>
        <example xml:lang="en">the CAPITAL OF france is paris</example>
        <rdfs:isDefinedBy rdf:resource="http://www.lexinfo.net/ontology/2.0/lexinfo"/>
    </owl:Class>
    


    <!-- http://www.lexinfo.net/ontology/2.0/lexinfo#NounPredicateFrame -->

    <owl:Class rdf:about="&lexinfo;NounPredicateFrame">
        <owl:equivalentClass>
            <owl:Class>
                <owl:intersectionOf rdf:parseType="Collection">
                    <rdf:Description rdf:about="&lexinfo;NounFrame"/>
                    <owl:Restriction>
                        <owl:onProperty rdf:resource="&lexinfo;copulativeArg"/>
                        <owl:minCardinality rdf:datatype="&xsd;nonNegativeInteger">1</owl:minCardinality>
                    </owl:Restriction>
                </owl:intersectionOf>
            </owl:Class>
        </owl:equivalentClass>
        <rdfs:subClassOf rdf:resource="&lexinfo;NounFrame"/>
        <example xml:lang="en">he is a MAN</example>
        <rdfs:isDefinedBy rdf:resource="http://www.lexinfo.net/ontology/2.0/lexinfo"/>
    </owl:Class>
    


    <!-- http://www.lexinfo.net/ontology/2.0/lexinfo#Number -->

    <owl:Class rdf:about="&lexinfo;Number">
        <rdfs:subClassOf rdf:resource="&lexinfo;MorphosyntacticProperty"/>
        <rdfs:isDefinedBy rdf:resource="http://www.lexinfo.net/ontology/2.0/lexinfo"/>
    </owl:Class>
    


    <!-- http://www.lexinfo.net/ontology/2.0/lexinfo#Numeral -->

    <owl:Class rdf:about="&lexinfo;Numeral">
        <owl:equivalentClass>
            <owl:Restriction>
                <owl:onProperty rdf:resource="&lexinfo;partOfSpeech"/>
                <owl:someValuesFrom rdf:resource="&lexinfo;NumeralPOS"/>
            </owl:Restriction>
        </owl:equivalentClass>
        <rdfs:subClassOf rdf:resource="&lemon;Word"/>
        <rdfs:isDefinedBy rdf:resource="http://www.lexinfo.net/ontology/2.0/lexinfo"/>
    </owl:Class>
    


    <!-- http://www.lexinfo.net/ontology/2.0/lexinfo#NumeralPOS -->

    <owl:Class rdf:about="&lexinfo;NumeralPOS">
        <rdfs:subClassOf rdf:resource="&lexinfo;PartOfSpeech"/>
        <rdfs:isDefinedBy rdf:resource="http://www.lexinfo.net/ontology/2.0/lexinfo"/>
    </owl:Class>
    


    <!-- http://www.lexinfo.net/ontology/2.0/lexinfo#Object -->

    <owl:Class rdf:about="&lexinfo;Object">
        <rdfs:subClassOf rdf:resource="&lemon;Argument"/>
        <rdfs:subClassOf>
            <owl:Restriction>
                <owl:onProperty rdf:resource="&lemon;optional"/>
                <owl:hasValue rdf:datatype="&xsd;boolean">false</owl:hasValue>
            </owl:Restriction>
        </rdfs:subClassOf>
        <rdfs:isDefinedBy rdf:resource="http://www.lexinfo.net/ontology/2.0/lexinfo"/>
    </owl:Class>
    


    <!-- http://www.lexinfo.net/ontology/2.0/lexinfo#ObjectComplement -->

    <owl:Class rdf:about="&lexinfo;ObjectComplement">
        <rdfs:subClassOf rdf:resource="&lexinfo;Complement"/>
        <rdfs:isDefinedBy rdf:resource="http://www.lexinfo.net/ontology/2.0/lexinfo"/>
    </owl:Class>
    


    <!-- http://www.lexinfo.net/ontology/2.0/lexinfo#ObjectControl -->

    <owl:Class rdf:about="&lexinfo;ObjectControl">
        <rdfs:subClassOf rdf:resource="&lexinfo;Control"/>
        <rdfs:comment xml:lang="en">Indicates the object of the main clause is also the (omitted) object of the subclause</rdfs:comment>
        <rdfs:comment xml:lang="ru">Указывает, что объект главного предложения - это тот же (опущенный) объект подчинительного предложения</rdfs:comment>
        <rdfs:isDefinedBy rdf:resource="http://www.lexinfo.net/ontology/2.0/lexinfo"/>
    </owl:Class>
    


    <!-- http://www.lexinfo.net/ontology/2.0/lexinfo#PPFrame -->

    <owl:Class rdf:about="&lexinfo;PPFrame">
        <owl:equivalentClass>
            <owl:Class>
                <owl:intersectionOf rdf:parseType="Collection">
                    <rdf:Description rdf:about="&lexinfo;PrepositionalFrame"/>
                    <rdf:Description rdf:about="&lexinfo;VerbFrame"/>
                </owl:intersectionOf>
            </owl:Class>
        </owl:equivalentClass>
        <rdfs:subClassOf rdf:resource="&lexinfo;VerbFrame"/>
        <rdfs:isDefinedBy rdf:resource="http://www.lexinfo.net/ontology/2.0/lexinfo"/>
    </owl:Class>
    


    <!-- http://www.lexinfo.net/ontology/2.0/lexinfo#PartOfSpeech -->

    <owl:Class rdf:about="&lexinfo;PartOfSpeech">
        <rdfs:subClassOf rdf:resource="&lexinfo;MorphosyntacticProperty"/>
        <rdfs:isDefinedBy rdf:resource="http://www.lexinfo.net/ontology/2.0/lexinfo"/>
    </owl:Class>
    


    <!-- http://www.lexinfo.net/ontology/2.0/lexinfo#Particle -->

    <owl:Class rdf:about="&lexinfo;Particle">
        <owl:equivalentClass>
            <owl:Restriction>
                <owl:onProperty rdf:resource="&lexinfo;partOfSpeech"/>
                <owl:someValuesFrom rdf:resource="&lexinfo;ParticlePOS"/>
            </owl:Restriction>
        </owl:equivalentClass>
        <rdfs:subClassOf rdf:resource="&lemon;Word"/>
        <rdfs:isDefinedBy rdf:resource="http://www.lexinfo.net/ontology/2.0/lexinfo"/>
    </owl:Class>
    


    <!-- http://www.lexinfo.net/ontology/2.0/lexinfo#ParticlePOS -->

    <owl:Class rdf:about="&lexinfo;ParticlePOS">
        <rdfs:subClassOf rdf:resource="&lexinfo;PartOfSpeech"/>
        <rdfs:isDefinedBy rdf:resource="http://www.lexinfo.net/ontology/2.0/lexinfo"/>
    </owl:Class>
    


    <!-- http://www.lexinfo.net/ontology/2.0/lexinfo#Person -->

    <owl:Class rdf:about="&lexinfo;Person">
        <rdfs:subClassOf rdf:resource="&lexinfo;MorphosyntacticProperty"/>
        <rdfs:isDefinedBy rdf:resource="http://www.lexinfo.net/ontology/2.0/lexinfo"/>
    </owl:Class>
    


    <!-- http://www.lexinfo.net/ontology/2.0/lexinfo#PossessiveAdjunct -->

    <owl:Class rdf:about="&lexinfo;PossessiveAdjunct">
        <rdfs:subClassOf rdf:resource="&lexinfo;Adjunct"/>
        <rdfs:isDefinedBy rdf:resource="http://www.lexinfo.net/ontology/2.0/lexinfo"/>
    </owl:Class>
    


    <!-- http://www.lexinfo.net/ontology/2.0/lexinfo#PostPositiveArgument -->

    <owl:Class rdf:about="&lexinfo;PostPositiveArgument">
        <rdfs:subClassOf rdf:resource="&lemon;Argument"/>
        <rdfs:isDefinedBy rdf:resource="http://www.lexinfo.net/ontology/2.0/lexinfo"/>
    </owl:Class>
    


    <!-- http://www.lexinfo.net/ontology/2.0/lexinfo#Postposition -->

    <owl:Class rdf:about="&lexinfo;Postposition">
        <owl:equivalentClass>
            <owl:Restriction>
                <owl:onProperty rdf:resource="&lexinfo;partOfSpeech"/>
                <owl:hasValue rdf:resource="&lexinfo;postposition"/>
            </owl:Restriction>
        </owl:equivalentClass>
        <rdfs:subClassOf rdf:resource="&lexinfo;Adposition"/>
        <rdfs:isDefinedBy rdf:resource="http://www.lexinfo.net/ontology/2.0/lexinfo"/>
    </owl:Class>
    


    <!-- http://www.lexinfo.net/ontology/2.0/lexinfo#PredicativeAdjective -->

    <owl:Class rdf:about="&lexinfo;PredicativeAdjective">
        <rdfs:subClassOf rdf:resource="&lexinfo;Complement"/>
        <rdfs:isDefinedBy rdf:resource="http://www.lexinfo.net/ontology/2.0/lexinfo"/>
    </owl:Class>
    


    <!-- http://www.lexinfo.net/ontology/2.0/lexinfo#PredicativeAdverb -->

    <owl:Class rdf:about="&lexinfo;PredicativeAdverb">
        <rdfs:subClassOf rdf:resource="&lexinfo;Complement"/>
        <rdfs:isDefinedBy rdf:resource="http://www.lexinfo.net/ontology/2.0/lexinfo"/>
    </owl:Class>
    


    <!-- http://www.lexinfo.net/ontology/2.0/lexinfo#PredicativeNominative -->

    <owl:Class rdf:about="&lexinfo;PredicativeNominative">
        <rdfs:subClassOf rdf:resource="&lexinfo;Complement"/>
        <rdfs:isDefinedBy rdf:resource="http://www.lexinfo.net/ontology/2.0/lexinfo"/>
    </owl:Class>
    


    <!-- http://www.lexinfo.net/ontology/2.0/lexinfo#Prefix -->

    <owl:Class rdf:about="&lexinfo;Prefix">
        <owl:equivalentClass>
            <owl:Restriction>
                <owl:onProperty rdf:resource="&lexinfo;termElement"/>
                <owl:hasValue rdf:resource="&lexinfo;prefix"/>
            </owl:Restriction>
        </owl:equivalentClass>
        <rdfs:subClassOf rdf:resource="&lexinfo;Affix"/>
        <rdfs:isDefinedBy rdf:resource="http://www.lexinfo.net/ontology/2.0/lexinfo"/>
    </owl:Class>
    


    <!-- http://www.lexinfo.net/ontology/2.0/lexinfo#Preposition -->

    <owl:Class rdf:about="&lexinfo;Preposition">
        <owl:equivalentClass>
            <owl:Restriction>
                <owl:onProperty rdf:resource="&lexinfo;partOfSpeech"/>
                <owl:hasValue rdf:resource="&lexinfo;preposition"/>
            </owl:Restriction>
        </owl:equivalentClass>
        <rdfs:subClassOf rdf:resource="&lexinfo;Adposition"/>
        <rdfs:isDefinedBy rdf:resource="http://www.lexinfo.net/ontology/2.0/lexinfo"/>
    </owl:Class>
    


    <!-- http://www.lexinfo.net/ontology/2.0/lexinfo#PrepositionFrame -->

    <owl:Class rdf:about="&lexinfo;PrepositionFrame">
        <rdfs:subClassOf rdf:resource="&lemon;Frame"/>
        <rdfs:isDefinedBy rdf:resource="http://www.lexinfo.net/ontology/2.0/lexinfo"/>
    </owl:Class>
    


    <!-- http://www.lexinfo.net/ontology/2.0/lexinfo#PrepositionalAdjunct -->

    <owl:Class rdf:about="&lexinfo;PrepositionalAdjunct">
        <rdfs:subClassOf rdf:resource="&lexinfo;Adjunct"/>
        <rdfs:subClassOf>
            <owl:Restriction>
                <owl:onProperty rdf:resource="&lemon;marker"/>
                <owl:someValuesFrom rdf:resource="&lexinfo;Preposition"/>
            </owl:Restriction>
        </rdfs:subClassOf>
        <rdfs:isDefinedBy rdf:resource="http://www.lexinfo.net/ontology/2.0/lexinfo"/>
    </owl:Class>
    


    <!-- http://www.lexinfo.net/ontology/2.0/lexinfo#PrepositionalFrame -->

    <owl:Class rdf:about="&lexinfo;PrepositionalFrame">
        <owl:equivalentClass>
            <owl:Restriction>
                <owl:onProperty rdf:resource="&lexinfo;prepositionalAdjunct"/>
                <owl:minCardinality rdf:datatype="&xsd;nonNegativeInteger">1</owl:minCardinality>
            </owl:Restriction>
        </owl:equivalentClass>
        <rdfs:subClassOf rdf:resource="&lemon;Frame"/>
        <rdfs:comment xml:lang="en">Abstract frame for words that take a prepositional phrase as an argument</rdfs:comment>
        <rdfs:comment xml:lang="ru">Слова, которые используют предложные группы как аргументы</rdfs:comment>
        <rdfs:isDefinedBy rdf:resource="http://www.lexinfo.net/ontology/2.0/lexinfo"/>
    </owl:Class>
    


    <!-- http://www.lexinfo.net/ontology/2.0/lexinfo#PrepositionalInterrogativeFrame -->

    <owl:Class rdf:about="&lexinfo;PrepositionalInterrogativeFrame">
        <owl:equivalentClass>
            <owl:Class>
                <owl:intersectionOf rdf:parseType="Collection">
                    <rdf:Description rdf:about="&lexinfo;VerbFrame"/>
                    <owl:Restriction>
                        <owl:onProperty rdf:resource="&lexinfo;prepositionalInterrogativeClause"/>
                        <owl:minCardinality rdf:datatype="&xsd;nonNegativeInteger">1</owl:minCardinality>
                    </owl:Restriction>
                </owl:intersectionOf>
            </owl:Class>
        </owl:equivalentClass>
        <rdfs:subClassOf rdf:resource="&lexinfo;VerbFrame"/>
        <rdfs:isDefinedBy rdf:resource="http://www.lexinfo.net/ontology/2.0/lexinfo"/>
    </owl:Class>
    


    <!-- http://www.lexinfo.net/ontology/2.0/lexinfo#PrepositionalObject -->

    <owl:Class rdf:about="&lexinfo;PrepositionalObject">
        <owl:equivalentClass>
            <owl:Class>
                <owl:intersectionOf rdf:parseType="Collection">
                    <rdf:Description rdf:about="&lexinfo;AdpositionalObject"/>
                    <owl:Restriction>
                        <owl:onProperty rdf:resource="&lemon;marker"/>
                        <owl:someValuesFrom rdf:resource="&lexinfo;Preposition"/>
                    </owl:Restriction>
                </owl:intersectionOf>
            </owl:Class>
        </owl:equivalentClass>
        <rdfs:subClassOf rdf:resource="&lexinfo;AdpositionalObject"/>
        <rdfs:isDefinedBy rdf:resource="http://www.lexinfo.net/ontology/2.0/lexinfo"/>
    </owl:Class>
    


    <!-- http://www.lexinfo.net/ontology/2.0/lexinfo#PrepositionalPhraseFrame -->

    <owl:Class rdf:about="&lexinfo;PrepositionalPhraseFrame">
        <owl:equivalentClass>
            <owl:Class>
                <owl:intersectionOf rdf:parseType="Collection">
                    <rdf:Description rdf:about="&lexinfo;PrepositionFrame"/>
                    <owl:Restriction>
                        <owl:onProperty rdf:resource="&lexinfo;complement"/>
                        <owl:onClass rdf:resource="&lexinfo;PrepositionalAdjunct"/>
                        <owl:minQualifiedCardinality rdf:datatype="&xsd;nonNegativeInteger">1</owl:minQualifiedCardinality>
                    </owl:Restriction>
                    <owl:Restriction>
                        <owl:onProperty rdf:resource="&lexinfo;copulativeSubject"/>
                        <owl:minCardinality rdf:datatype="&xsd;nonNegativeInteger">1</owl:minCardinality>
                    </owl:Restriction>
                </owl:intersectionOf>
            </owl:Class>
        </owl:equivalentClass>
        <rdfs:subClassOf rdf:resource="&lexinfo;PrepositionFrame"/>
        <example xml:lang="en">he is IN london</example>
        <rdfs:isDefinedBy rdf:resource="http://www.lexinfo.net/ontology/2.0/lexinfo"/>
    </owl:Class>
    


    <!-- http://www.lexinfo.net/ontology/2.0/lexinfo#Pronoun -->

    <owl:Class rdf:about="&lexinfo;Pronoun">
        <owl:equivalentClass>
            <owl:Restriction>
                <owl:onProperty rdf:resource="&lexinfo;partOfSpeech"/>
                <owl:someValuesFrom rdf:resource="&lexinfo;PronounPOS"/>
            </owl:Restriction>
        </owl:equivalentClass>
        <rdfs:subClassOf rdf:resource="&lemon;Word"/>
        <rdfs:isDefinedBy rdf:resource="http://www.lexinfo.net/ontology/2.0/lexinfo"/>
    </owl:Class>
    


    <!-- http://www.lexinfo.net/ontology/2.0/lexinfo#PronounPOS -->

    <owl:Class rdf:about="&lexinfo;PronounPOS">
        <rdfs:subClassOf rdf:resource="&lexinfo;PartOfSpeech"/>
        <rdfs:isDefinedBy rdf:resource="http://www.lexinfo.net/ontology/2.0/lexinfo"/>
    </owl:Class>
    


    <!-- http://www.lexinfo.net/ontology/2.0/lexinfo#ProperNoun -->

    <owl:Class rdf:about="&lexinfo;ProperNoun">
        <owl:equivalentClass>
            <owl:Restriction>
                <owl:onProperty rdf:resource="&lexinfo;partOfSpeech"/>
                <owl:hasValue rdf:resource="&lexinfo;properNoun"/>
            </owl:Restriction>
        </owl:equivalentClass>
        <rdfs:subClassOf rdf:resource="&lexinfo;Noun"/>
        <rdfs:isDefinedBy rdf:resource="http://www.lexinfo.net/ontology/2.0/lexinfo"/>
    </owl:Class>
    


    <!-- http://www.lexinfo.net/ontology/2.0/lexinfo#RaisableSubject -->

    <owl:Class rdf:about="&lexinfo;RaisableSubject">
        <owl:equivalentClass>
            <owl:Class>
                <owl:intersectionOf rdf:parseType="Collection">
                    <rdf:Description rdf:about="&lemon;RaisableArgument"/>
                    <rdf:Description rdf:about="&lexinfo;Subject"/>
                </owl:intersectionOf>
            </owl:Class>
        </owl:equivalentClass>
        <rdfs:subClassOf rdf:resource="&lexinfo;Subject"/>
        <rdfs:isDefinedBy rdf:resource="http://www.lexinfo.net/ontology/2.0/lexinfo"/>
    </owl:Class>
    


    <!-- http://www.lexinfo.net/ontology/2.0/lexinfo#RaisingSubject -->

    <owl:Class rdf:about="&lexinfo;RaisingSubject">
        <owl:equivalentClass>
            <owl:Restriction>
                <owl:onProperty rdf:resource="&lexinfo;subject"/>
                <owl:someValuesFrom rdf:resource="&lexinfo;RaisableSubject"/>
            </owl:Restriction>
        </owl:equivalentClass>
        <rdfs:subClassOf rdf:resource="&lexinfo;Control"/>
        <rdfs:comment xml:lang="en">Indicates the syntactic subject of the main clause is in fact the subject of the subclause. The main clause should then be interpreted as being impersonal.</rdfs:comment>
        <rdfs:comment xml:lang="ru">Синтаксический субъект предложения является также и субъектом подчинительного предложения. Главное предложение при этом должно интерпретироваться как безличное.</rdfs:comment>
        <rdfs:isDefinedBy rdf:resource="http://www.lexinfo.net/ontology/2.0/lexinfo"/>
    </owl:Class>
    


    <!-- http://www.lexinfo.net/ontology/2.0/lexinfo#ReciprocalFrame -->

    <owl:Class rdf:about="&lexinfo;ReciprocalFrame">
        <owl:equivalentClass>
            <owl:Class>
                <owl:intersectionOf rdf:parseType="Collection">
                    <rdf:Description rdf:about="&lexinfo;VerbFrame"/>
                    <owl:Restriction>
                        <owl:onProperty rdf:resource="&lexinfo;subject"/>
                        <owl:minCardinality rdf:datatype="&xsd;nonNegativeInteger">2</owl:minCardinality>
                    </owl:Restriction>
                </owl:intersectionOf>
            </owl:Class>
        </owl:equivalentClass>
        <rdfs:subClassOf rdf:resource="&lexinfo;VerbFrame"/>
        <example xml:lang="en">mary and john MET</example>
        <rdfs:isDefinedBy rdf:resource="http://www.lexinfo.net/ontology/2.0/lexinfo"/>
    </owl:Class>
    


    <!-- http://www.lexinfo.net/ontology/2.0/lexinfo#ReferentType -->

    <owl:Class rdf:about="&lexinfo;ReferentType">
        <rdfs:subClassOf rdf:resource="&lexinfo;MorphosyntacticProperty"/>
        <rdfs:isDefinedBy rdf:resource="http://www.lexinfo.net/ontology/2.0/lexinfo"/>
    </owl:Class>
    


    <!-- http://www.lexinfo.net/ontology/2.0/lexinfo#ReflexiveDativeTransitiveFrame -->

    <owl:Class rdf:about="&lexinfo;ReflexiveDativeTransitiveFrame">
        <owl:equivalentClass>
            <owl:Class>
                <owl:intersectionOf rdf:parseType="Collection">
                    <rdf:Description rdf:about="&lexinfo;DativeTransitiveFrame"/>
                    <rdf:Description rdf:about="&lexinfo;ReflexiveFrame"/>
                </owl:intersectionOf>
            </owl:Class>
        </owl:equivalentClass>
        <rdfs:subClassOf rdf:resource="&lexinfo;ReflexiveFrame"/>
        <example xml:lang="de">ich TUE mir WEH</example>
        <rdfs:comment xml:lang="de">ist diese frame echt?</rdfs:comment>
        <rdfs:isDefinedBy rdf:resource="http://www.lexinfo.net/ontology/2.0/lexinfo"/>
    </owl:Class>
    


    <!-- http://www.lexinfo.net/ontology/2.0/lexinfo#ReflexiveDitransitiveFrame -->

    <owl:Class rdf:about="&lexinfo;ReflexiveDitransitiveFrame">
        <owl:equivalentClass>
            <owl:Class>
                <owl:intersectionOf rdf:parseType="Collection">
                    <rdf:Description rdf:about="&lexinfo;DitransitiveFrame"/>
                    <rdf:Description rdf:about="&lexinfo;ReflexiveFrame"/>
                    <owl:Restriction>
                        <owl:onProperty rdf:resource="&lexinfo;directObject"/>
                        <owl:someValuesFrom rdf:resource="&lexinfo;ReflexiveObject"/>
                    </owl:Restriction>
                </owl:intersectionOf>
            </owl:Class>
        </owl:equivalentClass>
        <rdfs:subClassOf rdf:resource="&lexinfo;ReflexiveFrame"/>
        <example xml:lang="de">das habe ich mir EINGEBILDET</example>
        <rdfs:isDefinedBy rdf:resource="http://www.lexinfo.net/ontology/2.0/lexinfo"/>
    </owl:Class>
    


    <!-- http://www.lexinfo.net/ontology/2.0/lexinfo#ReflexiveFrame -->

    <owl:Class rdf:about="&lexinfo;ReflexiveFrame">
        <owl:equivalentClass>
            <owl:Class>
                <owl:intersectionOf rdf:parseType="Collection">
                    <rdf:Description rdf:about="&lexinfo;VerbFrame"/>
                    <owl:Restriction>
                        <owl:onProperty rdf:resource="&lexinfo;object"/>
                        <owl:someValuesFrom rdf:resource="&lexinfo;ReflexiveObject"/>
                    </owl:Restriction>
                </owl:intersectionOf>
            </owl:Class>
        </owl:equivalentClass>
        <rdfs:subClassOf rdf:resource="&lexinfo;VerbFrame"/>
        <rdfs:isDefinedBy rdf:resource="http://www.lexinfo.net/ontology/2.0/lexinfo"/>
    </owl:Class>
    


    <!-- http://www.lexinfo.net/ontology/2.0/lexinfo#ReflexiveObject -->

    <owl:Class rdf:about="&lexinfo;ReflexiveObject">
        <rdfs:subClassOf rdf:resource="&lexinfo;Object"/>
        <rdfs:isDefinedBy rdf:resource="http://www.lexinfo.net/ontology/2.0/lexinfo"/>
    </owl:Class>
    


    <!-- http://www.lexinfo.net/ontology/2.0/lexinfo#ReflexiveReciprocalFrame -->

    <owl:Class rdf:about="&lexinfo;ReflexiveReciprocalFrame">
        <owl:equivalentClass>
            <owl:Class>
                <owl:intersectionOf rdf:parseType="Collection">
                    <rdf:Description rdf:about="&lexinfo;ReciprocalFrame"/>
                    <rdf:Description rdf:about="&lexinfo;ReflexiveFrame"/>
                </owl:intersectionOf>
            </owl:Class>
        </owl:equivalentClass>
        <rdfs:subClassOf rdf:resource="&lexinfo;ReflexiveFrame"/>
        <example xml:lang="de">hans und marie TREFFEN sich</example>
        <rdfs:isDefinedBy rdf:resource="http://www.lexinfo.net/ontology/2.0/lexinfo"/>
    </owl:Class>
    


    <!-- http://www.lexinfo.net/ontology/2.0/lexinfo#ReflexiveTransitiveFrame -->

    <owl:Class rdf:about="&lexinfo;ReflexiveTransitiveFrame">
        <owl:equivalentClass>
            <owl:Class>
                <owl:intersectionOf rdf:parseType="Collection">
                    <rdf:Description rdf:about="&lexinfo;ReflexiveFrame"/>
                    <rdf:Description rdf:about="&lexinfo;TransitiveFrame"/>
                </owl:intersectionOf>
            </owl:Class>
        </owl:equivalentClass>
        <rdfs:subClassOf rdf:resource="&lexinfo;ReflexiveFrame"/>
        <example xml:lang="de">er ERHOLT sich</example>
        <example xml:lang="fr">elle se COUCHE</example>
        <rdfs:isDefinedBy rdf:resource="http://www.lexinfo.net/ontology/2.0/lexinfo"/>
    </owl:Class>
    


    <!-- http://www.lexinfo.net/ontology/2.0/lexinfo#ReflexiveTransitivePPFrame -->

    <owl:Class rdf:about="&lexinfo;ReflexiveTransitivePPFrame">
        <owl:equivalentClass>
            <owl:Class>
                <owl:intersectionOf rdf:parseType="Collection">
                    <rdf:Description rdf:about="&lexinfo;ReflexiveFrame"/>
                    <rdf:Description rdf:about="&lexinfo;TransitivePPFrame"/>
                </owl:intersectionOf>
            </owl:Class>
        </owl:equivalentClass>
        <rdfs:subClassOf rdf:resource="&lexinfo;ReflexiveFrame"/>
        <example xml:lang="de">ich ERRINERE mich AN seinen vater</example>
        <example xml:lang="fr">elle se APPROCHE DE la gare</example>
        <rdfs:isDefinedBy rdf:resource="http://www.lexinfo.net/ontology/2.0/lexinfo"/>
    </owl:Class>
    


    <!-- http://www.lexinfo.net/ontology/2.0/lexinfo#Register -->

    <owl:Class rdf:about="&lexinfo;Register">
        <rdfs:subClassOf rdf:resource="&lemon;SenseContext"/>
        <rdfs:isDefinedBy rdf:resource="http://www.lexinfo.net/ontology/2.0/lexinfo"/>
    </owl:Class>
    


    <!-- http://www.lexinfo.net/ontology/2.0/lexinfo#SententialFrame -->

    <owl:Class rdf:about="&lexinfo;SententialFrame">
        <owl:equivalentClass>
            <owl:Class>
                <owl:intersectionOf rdf:parseType="Collection">
                    <rdf:Description rdf:about="&lexinfo;VerbFrame"/>
                    <owl:Restriction>
                        <owl:onProperty rdf:resource="&lexinfo;sententialClause"/>
                        <owl:minCardinality rdf:datatype="&xsd;nonNegativeInteger">1</owl:minCardinality>
                    </owl:Restriction>
                </owl:intersectionOf>
            </owl:Class>
        </owl:equivalentClass>
        <rdfs:subClassOf rdf:resource="&lexinfo;VerbFrame"/>
        <rdfs:comment xml:lang="en">Sentential frames take a clause as argument, no conjunction is used and the syntax of the clause is the same as a main clause</rdfs:comment>
        <rdfs:comment xml:lang="ru">Между главным и второстепенным предложениями отсутствует союз, синтаксис второстепенного предложения точно такой же, как и синтаксис главного предложения</rdfs:comment>
        <rdfs:isDefinedBy rdf:resource="http://www.lexinfo.net/ontology/2.0/lexinfo"/>
    </owl:Class>
    


    <!-- http://www.lexinfo.net/ontology/2.0/lexinfo#Subject -->

    <owl:Class rdf:about="&lexinfo;Subject">
        <rdfs:subClassOf rdf:resource="&lemon;Argument"/>
        <rdfs:subClassOf>
            <owl:Restriction>
                <owl:onProperty rdf:resource="&lemon;optional"/>
                <owl:hasValue rdf:datatype="&xsd;boolean">false</owl:hasValue>
            </owl:Restriction>
        </rdfs:subClassOf>
        <rdfs:isDefinedBy rdf:resource="http://www.lexinfo.net/ontology/2.0/lexinfo"/>
    </owl:Class>
    


    <!-- http://www.lexinfo.net/ontology/2.0/lexinfo#SubjectControl -->

    <owl:Class rdf:about="&lexinfo;SubjectControl">
        <rdfs:subClassOf rdf:resource="&lexinfo;Control"/>
        <rdfs:comment xml:lang="en">Indicates the subject of the main clause is the (omitted) subject of the subclause</rdfs:comment>
        <rdfs:comment xml:lang="ru">Субъект галвного предложения является опущенным субъектом подчинительного предложения</rdfs:comment>
        <rdfs:isDefinedBy rdf:resource="http://www.lexinfo.net/ontology/2.0/lexinfo"/>
    </owl:Class>
    


    <!-- http://www.lexinfo.net/ontology/2.0/lexinfo#SubjectlessFrame -->

    <owl:Class rdf:about="&lexinfo;SubjectlessFrame">
        <owl:equivalentClass>
            <owl:Class>
                <owl:intersectionOf rdf:parseType="Collection">
                    <rdf:Description rdf:about="&lexinfo;VerbFrame"/>
                    <owl:Restriction>
                        <owl:onProperty rdf:resource="&lexinfo;subject"/>
                        <owl:cardinality rdf:datatype="&xsd;nonNegativeInteger">0</owl:cardinality>
                    </owl:Restriction>
                </owl:intersectionOf>
            </owl:Class>
        </owl:equivalentClass>
        <rdfs:subClassOf rdf:resource="&lexinfo;VerbFrame"/>
        <rdfs:isDefinedBy rdf:resource="http://www.lexinfo.net/ontology/2.0/lexinfo"/>
    </owl:Class>
    


    <!-- http://www.lexinfo.net/ontology/2.0/lexinfo#SubjectlessIntransitiveFrame -->

    <owl:Class rdf:about="&lexinfo;SubjectlessIntransitiveFrame">
        <owl:equivalentClass>
            <owl:Class>
                <owl:intersectionOf rdf:parseType="Collection">
                    <rdf:Description rdf:about="&lexinfo;SubjectlessFrame"/>
                    <owl:Restriction>
                        <owl:onProperty rdf:resource="&lexinfo;indirectObject"/>
                        <owl:cardinality rdf:datatype="&xsd;nonNegativeInteger">1</owl:cardinality>
                    </owl:Restriction>
                </owl:intersectionOf>
            </owl:Class>
        </owl:equivalentClass>
        <rdfs:subClassOf rdf:resource="&lexinfo;SubjectlessFrame"/>
        <example xml:lang="de">mir SCHWINDELT</example>
        <rdfs:isDefinedBy rdf:resource="http://www.lexinfo.net/ontology/2.0/lexinfo"/>
    </owl:Class>
    


    <!-- http://www.lexinfo.net/ontology/2.0/lexinfo#SubjectlessIntransitivePPFrame -->

    <owl:Class rdf:about="&lexinfo;SubjectlessIntransitivePPFrame">
        <owl:equivalentClass>
            <owl:Class>
                <owl:intersectionOf rdf:parseType="Collection">
                    <rdf:Description rdf:about="&lexinfo;PPFrame"/>
                    <rdf:Description rdf:about="&lexinfo;SubjectlessIntransitiveFrame"/>
                </owl:intersectionOf>
            </owl:Class>
        </owl:equivalentClass>
        <rdfs:subClassOf rdf:resource="&lexinfo;SubjectlessIntransitiveFrame"/>
        <example xml:lang="de">mir TRÄUMT VON jener zeit</example>
        <rdfs:isDefinedBy rdf:resource="http://www.lexinfo.net/ontology/2.0/lexinfo"/>
    </owl:Class>
    


    <!-- http://www.lexinfo.net/ontology/2.0/lexinfo#SubjectlessTransitiveFrame -->

    <owl:Class rdf:about="&lexinfo;SubjectlessTransitiveFrame">
        <owl:equivalentClass>
            <owl:Class>
                <owl:intersectionOf rdf:parseType="Collection">
                    <rdf:Description rdf:about="&lexinfo;SubjectlessFrame"/>
                    <owl:Restriction>
                        <owl:onProperty rdf:resource="&lexinfo;directObject"/>
                        <owl:cardinality rdf:datatype="&xsd;nonNegativeInteger">1</owl:cardinality>
                    </owl:Restriction>
                </owl:intersectionOf>
            </owl:Class>
        </owl:equivalentClass>
        <rdfs:subClassOf rdf:resource="&lexinfo;SubjectlessFrame"/>
        <example xml:lang="de">mich FRIERT</example>
        <rdfs:isDefinedBy rdf:resource="http://www.lexinfo.net/ontology/2.0/lexinfo"/>
    </owl:Class>
    


    <!-- http://www.lexinfo.net/ontology/2.0/lexinfo#SubjectlessTransitivePPFrame -->

    <owl:Class rdf:about="&lexinfo;SubjectlessTransitivePPFrame">
        <owl:equivalentClass>
            <owl:Class>
                <owl:intersectionOf rdf:parseType="Collection">
                    <rdf:Description rdf:about="&lexinfo;PPFrame"/>
                    <rdf:Description rdf:about="&lexinfo;SubjectlessTransitiveFrame"/>
                </owl:intersectionOf>
            </owl:Class>
        </owl:equivalentClass>
        <rdfs:subClassOf rdf:resource="&lexinfo;PPFrame"/>
        <rdfs:subClassOf rdf:resource="&lexinfo;SubjectlessTransitiveFrame"/>
        <example xml:lang="de">mich EKELT VOR fleisch</example>
        <rdfs:isDefinedBy rdf:resource="http://www.lexinfo.net/ontology/2.0/lexinfo"/>
    </owl:Class>
    


    <!-- http://www.lexinfo.net/ontology/2.0/lexinfo#SubjunctiveClause -->

    <owl:Class rdf:about="&lexinfo;SubjunctiveClause">
        <rdfs:subClassOf rdf:resource="&lexinfo;ClausalArgument"/>
        <rdfs:comment xml:lang="en">A subclause that is in the subjunctive mood</rdfs:comment>
        <rdfs:comment xml:lang="ru">Подчинительное предложение в сослагательном наклонении</rdfs:comment>
        <rdfs:isDefinedBy rdf:resource="http://www.lexinfo.net/ontology/2.0/lexinfo"/>
    </owl:Class>
    


    <!-- http://www.lexinfo.net/ontology/2.0/lexinfo#Suffix -->

    <owl:Class rdf:about="&lexinfo;Suffix">
        <owl:equivalentClass>
            <owl:Restriction>
                <owl:onProperty rdf:resource="&lexinfo;termElement"/>
                <owl:hasValue rdf:resource="&lexinfo;suffix"/>
            </owl:Restriction>
        </owl:equivalentClass>
        <rdfs:subClassOf rdf:resource="&lexinfo;Affix"/>
        <rdfs:isDefinedBy rdf:resource="http://www.lexinfo.net/ontology/2.0/lexinfo"/>
    </owl:Class>
    


    <!-- http://www.lexinfo.net/ontology/2.0/lexinfo#SuperlativeAdjunct -->

    <owl:Class rdf:about="&lexinfo;SuperlativeAdjunct">
        <rdfs:subClassOf rdf:resource="&lexinfo;Adjunct"/>
        <rdfs:isDefinedBy rdf:resource="http://www.lexinfo.net/ontology/2.0/lexinfo"/>
    </owl:Class>
    


    <!-- http://www.lexinfo.net/ontology/2.0/lexinfo#Symbol -->

    <owl:Class rdf:about="&lexinfo;Symbol">
        <owl:equivalentClass>
            <owl:Restriction>
                <owl:onProperty rdf:resource="&lexinfo;partOfSpeech"/>
                <owl:someValuesFrom rdf:resource="&lexinfo;SymbolPOS"/>
            </owl:Restriction>
        </owl:equivalentClass>
        <rdfs:subClassOf rdf:resource="&lemon;Word"/>
        <rdfs:isDefinedBy rdf:resource="http://www.lexinfo.net/ontology/2.0/lexinfo"/>
    </owl:Class>
    


    <!-- http://www.lexinfo.net/ontology/2.0/lexinfo#SymbolPOS -->

    <owl:Class rdf:about="&lexinfo;SymbolPOS">
        <rdfs:subClassOf rdf:resource="&lexinfo;PartOfSpeech"/>
        <rdfs:isDefinedBy rdf:resource="http://www.lexinfo.net/ontology/2.0/lexinfo"/>
    </owl:Class>
    


    <!-- http://www.lexinfo.net/ontology/2.0/lexinfo#TemporalQualifier -->

    <owl:Class rdf:about="&lexinfo;TemporalQualifier">
        <rdfs:subClassOf rdf:resource="&lemon;SenseContext"/>
        <rdfs:isDefinedBy rdf:resource="http://www.lexinfo.net/ontology/2.0/lexinfo"/>
    </owl:Class>
    


    <!-- http://www.lexinfo.net/ontology/2.0/lexinfo#Tense -->

    <owl:Class rdf:about="&lexinfo;Tense">
        <rdfs:subClassOf rdf:resource="&lexinfo;MorphosyntacticProperty"/>
        <rdfs:isDefinedBy rdf:resource="http://www.lexinfo.net/ontology/2.0/lexinfo"/>
    </owl:Class>
    


    <!-- http://www.lexinfo.net/ontology/2.0/lexinfo#TermElement -->

    <owl:Class rdf:about="&lexinfo;TermElement">
        <rdfs:subClassOf rdf:resource="&lemon;PropertyValue"/>
        <rdfs:isDefinedBy rdf:resource="http://www.lexinfo.net/ontology/2.0/lexinfo"/>
    </owl:Class>
    


    <!-- http://www.lexinfo.net/ontology/2.0/lexinfo#TermType -->

    <owl:Class rdf:about="&lexinfo;TermType">
        <rdfs:subClassOf rdf:resource="&lemon;PropertyValue"/>
        <rdfs:isDefinedBy rdf:resource="http://www.lexinfo.net/ontology/2.0/lexinfo"/>
    </owl:Class>
    


    <!-- http://www.lexinfo.net/ontology/2.0/lexinfo#TransitiveAdjectivalComplementFrame -->

    <owl:Class rdf:about="&lexinfo;TransitiveAdjectivalComplementFrame">
        <owl:equivalentClass>
            <owl:Class>
                <owl:intersectionOf rdf:parseType="Collection">
                    <rdf:Description rdf:about="&lexinfo;AdjectivalComplementFrame"/>
                    <rdf:Description rdf:about="&lexinfo;TransitiveFrame"/>
                </owl:intersectionOf>
            </owl:Class>
        </owl:equivalentClass>
        <rdfs:subClassOf rdf:resource="&lexinfo;TransitiveFrame"/>
        <example xml:lang="en">they PAINTED it red</example>
        <rdfs:isDefinedBy rdf:resource="http://www.lexinfo.net/ontology/2.0/lexinfo"/>
    </owl:Class>
    


    <!-- http://www.lexinfo.net/ontology/2.0/lexinfo#TransitiveAdverbialComplementFrame -->

    <owl:Class rdf:about="&lexinfo;TransitiveAdverbialComplementFrame">
        <owl:equivalentClass>
            <owl:Class>
                <owl:intersectionOf rdf:parseType="Collection">
                    <rdf:Description rdf:about="&lexinfo;AdverbialComplementFrame"/>
                    <rdf:Description rdf:about="&lexinfo;TransitiveFrame"/>
                </owl:intersectionOf>
            </owl:Class>
        </owl:equivalentClass>
        <rdfs:subClassOf rdf:resource="&lexinfo;TransitiveFrame"/>
        <example xml:lang="en">she PUT the cheese back</example>
        <rdfs:isDefinedBy rdf:resource="http://www.lexinfo.net/ontology/2.0/lexinfo"/>
    </owl:Class>
    


    <!-- http://www.lexinfo.net/ontology/2.0/lexinfo#TransitiveDeclarativeFrame -->

    <owl:Class rdf:about="&lexinfo;TransitiveDeclarativeFrame">
        <owl:equivalentClass>
            <owl:Class>
                <owl:intersectionOf rdf:parseType="Collection">
                    <rdf:Description rdf:about="&lexinfo;DeclarativeFrame"/>
                    <rdf:Description rdf:about="&lexinfo;TransitiveFrame"/>
                </owl:intersectionOf>
            </owl:Class>
        </owl:equivalentClass>
        <rdfs:subClassOf rdf:resource="&lexinfo;DeclarativeFrame"/>
        <example xml:lang="en">he CONVINCED her [that she should go]</example>
        <rdfs:isDefinedBy rdf:resource="http://www.lexinfo.net/ontology/2.0/lexinfo"/>
    </owl:Class>
    


    <!-- http://www.lexinfo.net/ontology/2.0/lexinfo#TransitiveFrame -->

    <owl:Class rdf:about="&lexinfo;TransitiveFrame">
        <owl:equivalentClass>
            <owl:Class>
                <owl:intersectionOf rdf:parseType="Collection">
                    <rdf:Description rdf:about="&lexinfo;VerbFrame"/>
                    <owl:Restriction>
                        <owl:onProperty rdf:resource="&lexinfo;directObject"/>
                        <owl:cardinality rdf:datatype="&xsd;nonNegativeInteger">1</owl:cardinality>
                    </owl:Restriction>
                    <owl:Restriction>
                        <owl:onProperty rdf:resource="&lexinfo;subject"/>
                        <owl:cardinality rdf:datatype="&xsd;nonNegativeInteger">1</owl:cardinality>
                    </owl:Restriction>
                </owl:intersectionOf>
            </owl:Class>
        </owl:equivalentClass>
        <rdfs:subClassOf rdf:resource="&lexinfo;VerbFrame"/>
        <example xml:lang="en">the dog BIT the man</example>
        <rdfs:isDefinedBy rdf:resource="http://www.lexinfo.net/ontology/2.0/lexinfo"/>
    </owl:Class>
    


    <!-- http://www.lexinfo.net/ontology/2.0/lexinfo#TransitiveInfinitiveACFrame -->

    <owl:Class rdf:about="&lexinfo;TransitiveInfinitiveACFrame">
        <owl:equivalentClass>
            <owl:Class>
                <owl:intersectionOf rdf:parseType="Collection">
                    <rdf:Description rdf:about="&lexinfo;ArbitraryControl"/>
                    <rdf:Description rdf:about="&lexinfo;InfinitiveFrame"/>
                    <rdf:Description rdf:about="&lexinfo;TransitiveFrame"/>
                </owl:intersectionOf>
            </owl:Class>
        </owl:equivalentClass>
        <rdfs:subClassOf rdf:resource="&lexinfo;InfinitiveFrame"/>
        <example xml:lang="en">they CONVINCED him [to go]</example>
        <rdfs:isDefinedBy rdf:resource="http://www.lexinfo.net/ontology/2.0/lexinfo"/>
    </owl:Class>
    


    <!-- http://www.lexinfo.net/ontology/2.0/lexinfo#TransitiveInfinitiveOCFrame -->

    <owl:Class rdf:about="&lexinfo;TransitiveInfinitiveOCFrame">
        <owl:equivalentClass>
            <owl:Class>
                <owl:intersectionOf rdf:parseType="Collection">
                    <rdf:Description rdf:about="&lexinfo;InfinitiveFrame"/>
                    <rdf:Description rdf:about="&lexinfo;ObjectControl"/>
                    <rdf:Description rdf:about="&lexinfo;TransitiveFrame"/>
                </owl:intersectionOf>
            </owl:Class>
        </owl:equivalentClass>
        <rdfs:subClassOf rdf:resource="&lexinfo;InfinitiveFrame"/>
        <example xml:lang="en">i WANT john [to go]</example>
        <rdfs:isDefinedBy rdf:resource="http://www.lexinfo.net/ontology/2.0/lexinfo"/>
    </owl:Class>
    


    <!-- http://www.lexinfo.net/ontology/2.0/lexinfo#TransitiveInfinitiveSCFrame -->

    <owl:Class rdf:about="&lexinfo;TransitiveInfinitiveSCFrame">
        <owl:equivalentClass>
            <owl:Class>
                <owl:intersectionOf rdf:parseType="Collection">
                    <rdf:Description rdf:about="&lexinfo;InfinitiveFrame"/>
                    <rdf:Description rdf:about="&lexinfo;SubjectControl"/>
                    <rdf:Description rdf:about="&lexinfo;TransitiveFrame"/>
                </owl:intersectionOf>
            </owl:Class>
        </owl:equivalentClass>
        <rdfs:subClassOf rdf:resource="&lexinfo;InfinitiveFrame"/>
        <example xml:lang="en">john PROMISED mary [to resign]</example>
        <rdfs:isDefinedBy rdf:resource="http://www.lexinfo.net/ontology/2.0/lexinfo"/>
    </owl:Class>
    


    <!-- http://www.lexinfo.net/ontology/2.0/lexinfo#TransitiveInterrogativeFrame -->

    <owl:Class rdf:about="&lexinfo;TransitiveInterrogativeFrame">
        <owl:equivalentClass>
            <owl:Class>
                <owl:intersectionOf rdf:parseType="Collection">
                    <rdf:Description rdf:about="&lexinfo;InterrogativeFrame"/>
                    <rdf:Description rdf:about="&lexinfo;TransitiveFrame"/>
                </owl:intersectionOf>
            </owl:Class>
        </owl:equivalentClass>
        <rdfs:subClassOf rdf:resource="&lexinfo;InterrogativeFrame"/>
        <example xml:lang="en">he ASKED her [what he should do]</example>
        <rdfs:isDefinedBy rdf:resource="http://www.lexinfo.net/ontology/2.0/lexinfo"/>
    </owl:Class>
    


    <!-- http://www.lexinfo.net/ontology/2.0/lexinfo#TransitiveInterrogativeInfinitiveFrame -->

    <owl:Class rdf:about="&lexinfo;TransitiveInterrogativeInfinitiveFrame">
        <rdfs:subClassOf rdf:resource="&lexinfo;InterrogativeInfinitiveFrame"/>
        <example xml:lang="en">he ASKED her [what to do]</example>
        <rdfs:isDefinedBy rdf:resource="http://www.lexinfo.net/ontology/2.0/lexinfo"/>
    </owl:Class>
    


    <!-- http://www.lexinfo.net/ontology/2.0/lexinfo#TransitiveNominalComplementFrame -->

    <owl:Class rdf:about="&lexinfo;TransitiveNominalComplementFrame">
        <owl:equivalentClass>
            <owl:Class>
                <owl:intersectionOf rdf:parseType="Collection">
                    <rdf:Description rdf:about="&lexinfo;NominalComplementFrame"/>
                    <rdf:Description rdf:about="&lexinfo;TransitiveFrame"/>
                </owl:intersectionOf>
            </owl:Class>
        </owl:equivalentClass>
        <rdfs:subClassOf rdf:resource="&lexinfo;TransitiveFrame"/>
        <example xml:lang="en">they ELECTED him president</example>
        <rdfs:isDefinedBy rdf:resource="http://www.lexinfo.net/ontology/2.0/lexinfo"/>
    </owl:Class>
    


    <!-- http://www.lexinfo.net/ontology/2.0/lexinfo#TransitivePPFrame -->

    <owl:Class rdf:about="&lexinfo;TransitivePPFrame">
        <owl:equivalentClass>
            <owl:Class>
                <owl:intersectionOf rdf:parseType="Collection">
                    <rdf:Description rdf:about="&lexinfo;PPFrame"/>
                    <rdf:Description rdf:about="&lexinfo;TransitiveFrame"/>
                </owl:intersectionOf>
            </owl:Class>
        </owl:equivalentClass>
        <rdfs:subClassOf rdf:resource="&lexinfo;TransitiveFrame"/>
        <example xml:lang="en">she ADDED salt TO the stew</example>
        <rdfs:isDefinedBy rdf:resource="http://www.lexinfo.net/ontology/2.0/lexinfo"/>
    </owl:Class>
    


    <!-- http://www.lexinfo.net/ontology/2.0/lexinfo#TransitiveSententialFrame -->

    <owl:Class rdf:about="&lexinfo;TransitiveSententialFrame">
        <owl:equivalentClass>
            <owl:Class>
                <owl:intersectionOf rdf:parseType="Collection">
                    <rdf:Description rdf:about="&lexinfo;SententialFrame"/>
                    <rdf:Description rdf:about="&lexinfo;TransitiveFrame"/>
                </owl:intersectionOf>
            </owl:Class>
        </owl:equivalentClass>
        <rdfs:subClassOf rdf:resource="&lexinfo;SententialFrame"/>
        <example xml:lang="en">he TOLD the audience he was leaving</example>
        <rdfs:isDefinedBy rdf:resource="http://www.lexinfo.net/ontology/2.0/lexinfo"/>
    </owl:Class>
    


    <!-- http://www.lexinfo.net/ontology/2.0/lexinfo#Verb -->

    <owl:Class rdf:about="&lexinfo;Verb">
        <owl:equivalentClass>
            <owl:Restriction>
                <owl:onProperty rdf:resource="&lexinfo;partOfSpeech"/>
                <owl:someValuesFrom rdf:resource="&lexinfo;VerbPOS"/>
            </owl:Restriction>
        </owl:equivalentClass>
        <rdfs:subClassOf rdf:resource="&lemon;Word"/>
        <rdfs:subClassOf>
            <owl:Restriction>
                <owl:onProperty rdf:resource="&lemon;synBehavior"/>
                <owl:allValuesFrom rdf:resource="&lexinfo;VerbFrame"/>
            </owl:Restriction>
        </rdfs:subClassOf>
        <rdfs:isDefinedBy rdf:resource="http://www.lexinfo.net/ontology/2.0/lexinfo"/>
    </owl:Class>
    


    <!-- http://www.lexinfo.net/ontology/2.0/lexinfo#VerbFormMood -->

    <owl:Class rdf:about="&lexinfo;VerbFormMood">
        <rdfs:subClassOf rdf:resource="&lexinfo;MorphosyntacticProperty"/>
        <rdfs:isDefinedBy rdf:resource="http://www.lexinfo.net/ontology/2.0/lexinfo"/>
    </owl:Class>
    


    <!-- http://www.lexinfo.net/ontology/2.0/lexinfo#VerbFrame -->

    <owl:Class rdf:about="&lexinfo;VerbFrame">
        <rdfs:subClassOf rdf:resource="&lemon;Frame"/>
        <rdfs:isDefinedBy rdf:resource="http://www.lexinfo.net/ontology/2.0/lexinfo"/>
    </owl:Class>
    


    <!-- http://www.lexinfo.net/ontology/2.0/lexinfo#VerbPOS -->

    <owl:Class rdf:about="&lexinfo;VerbPOS">
        <rdfs:subClassOf rdf:resource="&lexinfo;PartOfSpeech"/>
        <rdfs:isDefinedBy rdf:resource="http://www.lexinfo.net/ontology/2.0/lexinfo"/>
    </owl:Class>
    


    <!-- http://www.lexinfo.net/ontology/2.0/lexinfo#VerbPhrase -->

    <owl:Class rdf:about="&lexinfo;VerbPhrase">
        <owl:equivalentClass>
            <owl:Class>
                <owl:intersectionOf rdf:parseType="Collection">
                    <rdf:Description rdf:about="&lemon;Phrase"/>
                    <owl:Restriction>
                        <owl:onProperty rdf:resource="&lexinfo;head"/>
                        <owl:someValuesFrom rdf:resource="&lexinfo;Verb"/>
                    </owl:Restriction>
                </owl:intersectionOf>
            </owl:Class>
        </owl:equivalentClass>
        <rdfs:subClassOf rdf:resource="&lemon;Phrase"/>
        <rdfs:isDefinedBy rdf:resource="http://www.lexinfo.net/ontology/2.0/lexinfo"/>
    </owl:Class>
    


    <!-- http://www.lexinfo.net/ontology/2.0/lexinfo#Voice -->

    <owl:Class rdf:about="&lexinfo;Voice">
        <rdfs:subClassOf rdf:resource="&lexinfo;MorphosyntacticProperty"/>
        <rdfs:isDefinedBy rdf:resource="http://www.lexinfo.net/ontology/2.0/lexinfo"/>
    </owl:Class>
    


    <!-- http://www.w3.org/2002/07/owl#Thing -->

    <owl:Class rdf:about="&owl;Thing"/>
    


    <!-- 
    ///////////////////////////////////////////////////////////////////////////////////////
    //
    // Individuals
    //
    ///////////////////////////////////////////////////////////////////////////////////////
     -->

    


    <!-- http://www.lexinfo.net/ontology/2.0/lexinfo -->

    <owl:NamedIndividual rdf:about="http://www.lexinfo.net/ontology/2.0/lexinfo">
        <rdf:type rdf:resource="http://purl.org/vocommons/voaf#Vocabulary"/>
    </owl:NamedIndividual>
    


    <!-- http://www.lexinfo.net/ontology/2.0/lexinfo#CJK_compound -->

    <owl:Thing rdf:about="&lexinfo;CJK_compound">
        <rdf:type rdf:resource="&lexinfo;TermType"/>
        <rdf:type rdf:resource="&owl;NamedIndividual"/>
        <rdfs:label xml:lang="en">compound(cjkv)</rdfs:label>
        <rdfs:label xml:lang="ru">композит в иероглифике</rdfs:label>
        <rdfs:comment xml:lang="en">A lexical unit in a CJKV language that is represented by at least two CJKV characters.</rdfs:comment>
        <rdfs:comment xml:lang="ru">Лексическая единица в иероглифике (китайской, японской, корейской и вьетнамской), которая состоит по меньшей мере из двух иероглифических символов.</rdfs:comment>
        <owl:versionInfo>1:0</owl:versionInfo>
        <dc:creator>Wright, Sue Ellen</dc:creator>
        <dcr:datcat rdf:resource="http://www.isocat.org/datcat/DC-356"/>
        <rdfs:isDefinedBy rdf:resource="http://www.lexinfo.net/ontology/2.0/lexinfo"/>
    </owl:Thing>
    


    <!-- http://www.lexinfo.net/ontology/2.0/lexinfo#abbreviatedForm -->

    <owl:Thing rdf:about="&lexinfo;abbreviatedForm">
        <rdf:type rdf:resource="&lexinfo;AbbreviatedForm"/>
        <rdf:type rdf:resource="&lexinfo;TermType"/>
        <rdf:type rdf:resource="&owl;NamedIndividual"/>
        <rdfs:label xml:lang="en">abbreviated form</rdfs:label>
        <rdfs:label xml:lang="ru">сокращённая форма</rdfs:label>
        <rdfs:comment xml:lang="en">A term or lexeme resulting from the omission of any part of the full term or lexeme while designating the same concept.</rdfs:comment>
        <rdfs:comment xml:lang="ru">Термин или лексема, возникающая в результате опущения какой-либо части полного термина или лексемы при обозначении того же понятия</rdfs:comment>        
        <dc:creator>Wright, Sue Ellen</dc:creator>
        <owl:versionInfo>1:0</owl:versionInfo>
        <dcr:datcat rdf:resource="http://www.isocat.org/datcat/DC-329"/>
        <rdfs:isDefinedBy rdf:resource="http://www.lexinfo.net/ontology/2.0/lexinfo"/>
    </owl:Thing>
    


    <!-- http://www.lexinfo.net/ontology/2.0/lexinfo#abbreviation -->

    <owl:Thing rdf:about="&lexinfo;abbreviation">
        <rdf:type rdf:resource="&lexinfo;AbbreviatedForm"/>
        <rdf:type rdf:resource="&lexinfo;TermType"/>
        <rdf:type rdf:resource="&owl;NamedIndividual"/>
        <rdfs:isDefinedBy rdf:resource="http://www.lexinfo.net/ontology/2.0/lexinfo"/>
    </owl:Thing>
    


    <!-- http://www.lexinfo.net/ontology/2.0/lexinfo#abessiveCase -->

    <owl:Thing rdf:about="&lexinfo;abessiveCase">
        <rdf:type rdf:resource="&lexinfo;Case"/>
        <rdf:type rdf:resource="&owl;NamedIndividual"/>
        <rdfs:label xml:lang="en">abessive case</rdfs:label>
        <rdfs:label xml:lang="ru">лишительный падеж</rdfs:label>        
        <dc:creator>Francopoulo, Gil</dc:creator>
        <rdfs:comment xml:lang="en">Case that expresses the lack or absence of the referent of the noun it marks.</rdfs:comment>
        <rdfs:comment xml:lang="ru">Падеж, который выражает нехватку или отсутствие определяемого объекта существительного, которое он обозначает.</rdfs:comment>        
        <owl:versionInfo>1:0</owl:versionInfo>
        <dcr:datcat rdf:resource="http://www.isocat.org/datcat/DC-1223"/>
        <rdfs:isDefinedBy rdf:resource="http://www.lexinfo.net/ontology/2.0/lexinfo"/>
    </owl:Thing>
    


    <!-- http://www.lexinfo.net/ontology/2.0/lexinfo#ablativeCase -->

    <owl:Thing rdf:about="&lexinfo;ablativeCase">
        <rdf:type rdf:resource="&lexinfo;Case"/>
        <rdf:type rdf:resource="&owl;NamedIndividual"/>
        <rdfs:label xml:lang="en">ablative case</rdfs:label>
        <rdfs:label xml:lang="ru">исходный падеж</rdfs:label>        
        <owl:versionInfo>1:0</owl:versionInfo>
        <dc:creator>Francopoulo, Gil</dc:creator>
        <rdfs:comment xml:lang="en">Case used to typically indicate locative or instrumental function.</rdfs:comment>
        <rdfs:comment xml:lang="ru">Падеж, который обычно указывает на локативную или инструментальную функцию.</rdfs:comment>        
        <dcr:datcat rdf:resource="http://www.isocat.org/datcat/DC-1224"/>
        <rdfs:isDefinedBy rdf:resource="http://www.lexinfo.net/ontology/2.0/lexinfo"/>
    </owl:Thing>
    


    <!-- http://www.lexinfo.net/ontology/2.0/lexinfo#absolutiveCase -->

    <owl:Thing rdf:about="&lexinfo;absolutiveCase">
        <rdf:type rdf:resource="&lexinfo;Case"/>
        <rdf:type rdf:resource="&owl;NamedIndividual"/>
        <rdfs:label xml:lang="en">absolutive case</rdfs:label>
        <rdfs:label xml:lang="ru">абсолютный падеж</rdfs:label>        
        <dc:creator>Francopoulo, Gil</dc:creator>
        <owl:versionInfo>1:0</owl:versionInfo>
        <rdfs:comment xml:lang="en">Case for nouns in ergative-absolute languages that would generally be the subjects of intransitive verbs or the objects of transitive verbs in the translational equivalents of nominative-accusative languages such as English.</rdfs:comment>
        <rdfs:comment xml:lang="ru">Падеж, встречающийся в эргативных языках. Падеж существительных, которые обычно были бы подлежащими при непереходных глаголах или дополнениями при переходных глаголах в переводных эквивалентах языков номинативного строя таких, как английский.</rdfs:comment>        
        <dcr:datcat rdf:resource="http://www.isocat.org/datcat/DC-1225"/>
        <rdfs:isDefinedBy rdf:resource="http://www.lexinfo.net/ontology/2.0/lexinfo"/>
    </owl:Thing>
    


    <!-- http://www.lexinfo.net/ontology/2.0/lexinfo#accusativeCase -->

    <owl:Thing rdf:about="&lexinfo;accusativeCase">
        <rdf:type rdf:resource="&lexinfo;Case"/>
        <rdf:type rdf:resource="&owl;NamedIndividual"/>
        <rdfs:label xml:lang="en">accusative case</rdfs:label>
        <rdfs:label xml:lang="ru">винительный падеж</rdfs:label>        
        <dc:creator>Francopoulo, Gil</dc:creator>
        <owl:versionInfo>1:0</owl:versionInfo>
        <rdfs:comment xml:lang="en">Case used to indicate direct object.</rdfs:comment>
        <rdfs:comment xml:lang="ru">Падеж, используемый для указания прямого объекта.</rdfs:comment>
        <dcr:datcat rdf:resource="http://www.isocat.org/datcat/DC-1226"/>
        <rdfs:isDefinedBy rdf:resource="http://www.lexinfo.net/ontology/2.0/lexinfo"/>
    </owl:Thing>
    


    <!-- http://www.lexinfo.net/ontology/2.0/lexinfo#acronym -->

    <owl:Thing rdf:about="&lexinfo;acronym">
        <rdf:type rdf:resource="&lexinfo;AbbreviatedForm"/>
        <rdf:type rdf:resource="&lexinfo;TermType"/>
        <rdf:type rdf:resource="&owl;NamedIndividual"/>
        <rdfs:label xml:lang="en">acronym</rdfs:label>
        <rdfs:label xml:lang="ru">акроним</rdfs:label>        
        <owl:versionInfo>1:0</owl:versionInfo>
        <dc:creator>Wright, Sue Ellen</dc:creator>
        <rdfs:comment xml:lang="en">An abbreviation made up of the initial letters of the components of the full form of the designation or from syllables of the full form and pronounced syllabically.</rdfs:comment>
        <rdfs:comment xml:lang="ru">Аббревиатура, состоящая из начальных букв компонентов полной формы обозначения или из слогов полной формы. Произносится  по слогам.</rdfs:comment>        
        <dcr:datcat rdf:resource="http://www.isocat.org/datcat/DC-334"/>
        <rdfs:isDefinedBy rdf:resource="http://www.lexinfo.net/ontology/2.0/lexinfo"/>
    </owl:Thing>
    


    <!-- http://www.lexinfo.net/ontology/2.0/lexinfo#activeVoice -->

    <owl:Thing rdf:about="&lexinfo;activeVoice">
        <rdf:type rdf:resource="&lexinfo;Voice"/>
        <rdf:type rdf:resource="&owl;NamedIndividual"/>
        <rdfs:label xml:lang="en">active voice</rdfs:label>
        <rdfs:label xml:lang="ru">действительный залог </rdfs:label>
        <dc:creator>Francopoulo, Gil</dc:creator>
        <rdfs:comment xml:lang="en">Value that expresses the situation where the grammatical subject is also the semantic actor of the verb.</rdfs:comment>
        <rdfs:comment xml:lang="ru">Значение, которое выражает ситуацию, когда грамматический субъект также является смысловым субъектом глагола.</rdfs:comment>        
        <owl:versionInfo>1:0</owl:versionInfo>
        <dcr:datcat rdf:resource="http://www.isocat.org/datcat/DC-1227"/>
        <rdfs:isDefinedBy rdf:resource="http://www.lexinfo.net/ontology/2.0/lexinfo"/>
    </owl:Thing>
    


    <!-- http://www.lexinfo.net/ontology/2.0/lexinfo#adessiveCase -->

    <owl:Thing rdf:about="&lexinfo;adessiveCase">
        <rdf:type rdf:resource="&lexinfo;Case"/>
        <rdf:type rdf:resource="&owl;NamedIndividual"/>
        <rdfs:label xml:lang="en">adessive case</rdfs:label>
        <rdfs:label xml:lang="ru">адессивный падеж</rdfs:label>        
        <owl:versionInfo>1:0</owl:versionInfo>
        <dc:creator>Francopoulo, Gil</dc:creator>
        <rdfs:comment xml:lang="en">Case which expresses the meaning of presence &apos;at&apos; or &apos;near&apos; a place.</rdfs:comment>
        <rdfs:comment xml:lang="ru">Падеж, который обозначает присутствие &apos;в&apos; или &apos;рядом&apos; с местом.</rdfs:comment>
        <dcr:datcat rdf:resource="http://www.isocat.org/datcat/DC-1228"/>
        <rdfs:isDefinedBy rdf:resource="http://www.lexinfo.net/ontology/2.0/lexinfo"/>
    </owl:Thing>
    


    <!-- http://www.lexinfo.net/ontology/2.0/lexinfo#aditiveCase -->

    <owl:Thing rdf:about="&lexinfo;aditiveCase">
        <rdf:type rdf:resource="&lexinfo;Case"/>
        <rdf:type rdf:resource="&owl;NamedIndividual"/>
        <rdfs:label xml:lang="en">aditive case</rdfs:label>
        <rdfs:label xml:lang="ru">адитивный падеж</rdfs:label>        
        <owl:versionInfo>1:0</owl:versionInfo>
        <dc:creator>Francopoulo, Gil</dc:creator>
        <rdfs:comment xml:lang="en">Case expressing &amp;quot;to&amp;quot; in Basque studies.</rdfs:comment>
        <rdfs:comment xml:lang="ru">Падеж, обозначающий направление в баскском языке.</rdfs:comment>        
        <dcr:datcat rdf:resource="http://www.isocat.org/datcat/DC-1229"/>
        <rdfs:isDefinedBy rdf:resource="http://www.lexinfo.net/ontology/2.0/lexinfo"/>
    </owl:Thing>
    


    <!-- http://www.lexinfo.net/ontology/2.0/lexinfo#adjective -->

    <owl:Thing rdf:about="&lexinfo;adjective">
        <rdf:type rdf:resource="&lexinfo;AdjectivePOS"/>
        <rdf:type rdf:resource="&lexinfo;PartOfSpeech"/>
        <rdf:type rdf:resource="&owl;NamedIndividual"/>
        <rdfs:label xml:lang="en">adjective</rdfs:label>
        <rdfs:label xml:lang="ru">имя прилагательное</rdfs:label>        
        <rdfs:comment xml:lang="en">Part of speech related to attributes of noun.</rdfs:comment>
        <rdfs:comment xml:lang="ru">Часть речи, обозначающая признак существительного.</rdfs:comment>
        <dc:creator>Francopoulo, Gil</dc:creator>
        <owl:versionInfo>1:0</owl:versionInfo>
        <dcr:datcat rdf:resource="http://www.isocat.org/datcat/DC-1230"/>
        <rdfs:isDefinedBy rdf:resource="http://www.lexinfo.net/ontology/2.0/lexinfo"/>
    </owl:Thing>
    


    <!-- http://www.lexinfo.net/ontology/2.0/lexinfo#adjective-i -->

    <owl:NamedIndividual rdf:about="&lexinfo;adjective-i">
        <rdf:type rdf:resource="&lexinfo;AdjectivePOS"/>
        <rdfs:comment xml:lang="en">Deverbal adjective in Japanese ending with the &apos;-i&apos; suffix in dictionary form</rdfs:comment>
        <languageSpecific>ja</languageSpecific>
    </owl:NamedIndividual>
    


    <!-- http://www.lexinfo.net/ontology/2.0/lexinfo#adjective-na -->

    <owl:NamedIndividual rdf:about="&lexinfo;adjective-na">
        <rdf:type rdf:resource="&lexinfo;AdjectivePOS"/>
        <rdfs:comment xml:lang="en">Denominal adjectives in Japanese formed from a noun plus the particle &apos;na&apos;</rdfs:comment>
        <languageSpecific>ja</languageSpecific>
    </owl:NamedIndividual>
    


    <!-- http://www.lexinfo.net/ontology/2.0/lexinfo#admittedTerm -->

    <owl:Thing rdf:about="&lexinfo;admittedTerm">
        <rdf:type rdf:resource="&lexinfo;NormativeAuthorization"/>
        <rdf:type rdf:resource="&owl;NamedIndividual"/>
        <rdfs:label xml:lang="en">admitted term</rdfs:label>
        <rdfs:label xml:lang="ru">допустимый термин</rdfs:label>        
        <dc:creator>Wright, Sue Ellen</dc:creator>
        <rdfs:comment xml:lang="en">A term rated according to the scale of a term acceptability rating as a synonym for a preferred term.</rdfs:comment>
        <rdfs:comment xml:lang="ru">Термин, рассматривающийся в соответствии со шкалой оценки приемлемости термина, как синоним предпочтительного термина.</rdfs:comment>        
        <owl:versionInfo>1:0</owl:versionInfo>
        <dcr:datcat rdf:resource="http://www.isocat.org/datcat/DC-377"/>
        <rdfs:isDefinedBy rdf:resource="http://www.lexinfo.net/ontology/2.0/lexinfo"/>
    </owl:Thing>
    


    <!-- http://www.lexinfo.net/ontology/2.0/lexinfo#adposition -->

    <owl:Thing rdf:about="&lexinfo;adposition">
        <rdf:type rdf:resource="&lexinfo;AdpositionPOS"/>
        <rdf:type rdf:resource="&lexinfo;PartOfSpeech"/>
        <rdf:type rdf:resource="&owl;NamedIndividual"/>
        <rdfs:label xml:lang="en">adposition</rdfs:label>
        <rdfs:label xml:lang="ru">прилог</rdfs:label>        
        <dc:creator>Francopoulo, Gil</dc:creator>
        <owl:versionInfo>1:0</owl:versionInfo>
        <rdfs:comment xml:lang="en">Part of speech that occurs before/inside/after a complement composed of a noun phrase, noun, pronoun or clause that functions as a noun phrase and form a single structure with the complement to express its grammatical and semantic relation to another unit.</rdfs:comment>
        <rdfs:comment xml:lang="ru">Часть речи, которая используется перед/в составе/после дополнения, состоящего из именной группы, существительного, местоимения или придаточного предложения, которое функционирует как словосочетание и формирует единую структуру с дополнением, чтобы выразить ее грамматическое и семантическое отношение к другой единице.</rdfs:comment>        
        <dcr:datcat rdf:resource="http://www.isocat.org/datcat/DC-1231"/>
        <rdfs:isDefinedBy rdf:resource="http://www.lexinfo.net/ontology/2.0/lexinfo"/>
    </owl:Thing>
    


    <!-- http://www.lexinfo.net/ontology/2.0/lexinfo#adverb -->

    <owl:Thing rdf:about="&lexinfo;adverb">
        <rdf:type rdf:resource="&lexinfo;AdverbPOS"/>
        <rdf:type rdf:resource="&lexinfo;PartOfSpeech"/>
        <rdf:type rdf:resource="&owl;NamedIndividual"/>
        <rdfs:label xml:lang="en">adverb</rdfs:label>
        <rdfs:label xml:lang="ru">наречие</rdfs:label>        
        <rdfs:comment xml:lang="en">Part of speech to refer to an heterogeneous group of words whose most frequent function is to specify the mode of action of the verb.</rdfs:comment>
        <rdfs:comment xml:lang="ru">Часть речи, которая относится к разнородной группе слов, наиболее частая функция которой заключается в том, чтобы указать способ действия глагола.</rdfs:comment>        
        <dc:creator>Francopoulo, Gil</dc:creator>
        <owl:versionInfo>1:0</owl:versionInfo>
        <dcr:datcat rdf:resource="http://www.isocat.org/datcat/DC-1232"/>
        <rdfs:isDefinedBy rdf:resource="http://www.lexinfo.net/ontology/2.0/lexinfo"/>
    </owl:Thing>
    


    <!-- http://www.lexinfo.net/ontology/2.0/lexinfo#adverbialPronoun -->

    <owl:Thing rdf:about="&lexinfo;adverbialPronoun">
        <rdf:type rdf:resource="&lexinfo;PartOfSpeech"/>
        <rdf:type rdf:resource="&lexinfo;PronounPOS"/>
        <rdf:type rdf:resource="&owl;NamedIndividual"/>
        <rdfs:label xml:lang="en">adverbial pronoun</rdfs:label>
        <rdfs:label xml:lang="ru">наречное местоимение</rdfs:label>        
        <owl:versionInfo>1:0</owl:versionInfo>
        <dc:creator>Francopoulo, Gil</dc:creator>
        <rdfs:comment>()</rdfs:comment>
        <dcr:datcat rdf:resource="http://www.isocat.org/datcat/DC-3011"/>
        <rdfs:isDefinedBy rdf:resource="http://www.lexinfo.net/ontology/2.0/lexinfo"/>
    </owl:Thing>
    


    <!-- http://www.lexinfo.net/ontology/2.0/lexinfo#affirmativeParticle -->

    <owl:Thing rdf:about="&lexinfo;affirmativeParticle">
        <rdf:type rdf:resource="&lexinfo;PartOfSpeech"/>
        <rdf:type rdf:resource="&lexinfo;ParticlePOS"/>
        <rdf:type rdf:resource="&owl;NamedIndividual"/>
        <rdfs:label xml:lang="en">affirmative particule</rdfs:label>
        <rdfs:label xml:lang="ru">утвердительная частица</rdfs:label>        
        <owl:versionInfo>1:0</owl:versionInfo>
        <dc:creator>Francopoulo, Gil</dc:creator>
        <rdfs:comment xml:lang="en">Particle used to express affirmation.</rdfs:comment>
        <rdfs:comment xml:lang="ru">Частица, используемая для выражения утверждения.</rdfs:comment>
        <dcr:datcat rdf:resource="http://www.isocat.org/datcat/DC-1918"/>
        <rdfs:isDefinedBy rdf:resource="http://www.lexinfo.net/ontology/2.0/lexinfo"/>
    </owl:Thing>
    


    <!-- http://www.lexinfo.net/ontology/2.0/lexinfo#affix -->

    <owl:Thing rdf:about="&lexinfo;affix">
        <rdf:type rdf:resource="&lexinfo;TermElement"/>
        <rdf:type rdf:resource="&owl;NamedIndividual"/>
        <rdfs:isDefinedBy rdf:resource="http://www.lexinfo.net/ontology/2.0/lexinfo"/>
    </owl:Thing>
    


    <!-- http://www.lexinfo.net/ontology/2.0/lexinfo#affixedPersonalPronoun -->

    <owl:Thing rdf:about="&lexinfo;affixedPersonalPronoun">
        <rdf:type rdf:resource="&lexinfo;PartOfSpeech"/>
        <rdf:type rdf:resource="&lexinfo;PronounPOS"/>
        <rdf:type rdf:resource="&owl;NamedIndividual"/>
        <rdfs:label xml:lang="en">affixed personal pronoun</rdfs:label>
        <rdfs:label xml:lang="ru">личный аффикс</rdfs:label>
        <rdfs:comment xml:lang="en">Personnal pronoun that is affixed, i.e. added as an affix to another word.</rdfs:comment>
        <rdfs:comment xml:lang="ru">Личное местоимение, являющееся аффиксом, добавляется в качестве аффикса к другому слову.</rdfs:comment>
        <owl:versionInfo>1:0</owl:versionInfo>
        <dc:creator>Francopoulo, Gil</dc:creator>
        <dcr:datcat rdf:resource="http://www.isocat.org/datcat/DC-2221"/>
        <rdfs:isDefinedBy rdf:resource="http://www.lexinfo.net/ontology/2.0/lexinfo"/>
    </owl:Thing>
    


    <!-- http://www.lexinfo.net/ontology/2.0/lexinfo#allativeCase -->

    <owl:Thing rdf:about="&lexinfo;allativeCase">
        <rdf:type rdf:resource="&lexinfo;Case"/>
        <rdf:type rdf:resource="&owl;NamedIndividual"/>
        <rdfs:label xml:lang="en">allative case</rdfs:label>
        <rdfs:label xml:lang="ru">аллатив, падеж приближения</rdfs:label>        
        <dc:creator>Francopoulo, Gil</dc:creator>
        <rdfs:comment xml:lang="en">Case which expresses the meaning of motion &apos;to&apos; or &apos;towards&apos; the referent it marks.</rdfs:comment>
        <rdfs:comment xml:lang="ru">Падеж, который обозначает движение  &apos;к&apos; или &apos;по направлению к&apos; референту, который он отмечает.</rdfs:comment>
        <owl:versionInfo>1:0</owl:versionInfo>
        <dcr:datcat rdf:resource="http://www.isocat.org/datcat/DC-1236"/>
        <rdfs:isDefinedBy rdf:resource="http://www.lexinfo.net/ontology/2.0/lexinfo"/>
    </owl:Thing>
    


    <!-- http://www.lexinfo.net/ontology/2.0/lexinfo#allusivePronoun -->

    <owl:Thing rdf:about="&lexinfo;allusivePronoun">
        <rdf:type rdf:resource="&lexinfo;PartOfSpeech"/>
        <rdf:type rdf:resource="&lexinfo;PronounPOS"/>
        <rdf:type rdf:resource="&owl;NamedIndividual"/>
        <rdfs:label xml:lang="en">allusive pronoun</rdfs:label>
        <rdfs:label xml:lang="ru">иносказательное местоимение</rdfs:label>        
        <rdfs:comment xml:lang="en">Pronoun that refers to something characterized by allusions.</rdfs:comment>
        <rdfs:comment xml:lang="ru">Местоимение, которое относится к чему-то, характеризуемому с помощью аллюзий.</rdfs:comment>        
        <owl:versionInfo>1:0</owl:versionInfo>
        <dc:creator>Francopoulo, Gil</dc:creator>
        <dcr:datcat rdf:resource="http://www.isocat.org/datcat/DC-2223"/>
        <rdfs:isDefinedBy rdf:resource="http://www.lexinfo.net/ontology/2.0/lexinfo"/>
    </owl:Thing>
    


    <!-- http://www.lexinfo.net/ontology/2.0/lexinfo#animate -->

    <owl:Thing rdf:about="&lexinfo;animate">
        <rdf:type rdf:resource="&lexinfo;Animacy"/>
        <rdf:type rdf:resource="&owl;NamedIndividual"/>
        <rdfs:label xml:lang="en">animate</rdfs:label>
        <rdfs:label xml:lang="ru">одушевленный</rdfs:label>
        <owl:versionInfo>1:0</owl:versionInfo>
        <rdfs:comment xml:lang="en">Perceived as alive.</rdfs:comment>
        <rdfs:comment xml:lang="ru">Воспринимается как живое</rdfs:comment>
        <dc:creator>Wright, Sue Ellen</dc:creator>
        <dc:creator>Francopoulo, Gil</dc:creator>
        <dcr:datcat rdf:resource="http://www.isocat.org/datcat/DC-1911"/>
        <dcr:datcat rdf:resource="http://www.isocat.org/datcat/DC-79"/>
        <rdfs:isDefinedBy rdf:resource="http://www.lexinfo.net/ontology/2.0/lexinfo"/>
    </owl:Thing>
    


    <!-- http://www.lexinfo.net/ontology/2.0/lexinfo#appellation -->

    <owl:Thing rdf:about="&lexinfo;appellation">
        <rdf:type rdf:resource="&lexinfo;TermType"/>
        <rdf:type rdf:resource="&owl;NamedIndividual"/>
        <rdfs:label xml:lang="en">appellation</rdfs:label>
        <rdfs:label xml:lang="ru">название</rdfs:label>        
        <owl:versionInfo>1:0</owl:versionInfo>
        <dc:creator>Wright, Sue Ellen</dc:creator>
        <rdfs:comment xml:lang="en">A designation that represents an individual concept.</rdfs:comment>
        <rdfs:comment xml:lang="ru">Обозначение, представляющее индивидуальное понятие.</rdfs:comment>
        <dcr:datcat rdf:resource="http://www.isocat.org/datcat/DC-347"/>
        <rdfs:isDefinedBy rdf:resource="http://www.lexinfo.net/ontology/2.0/lexinfo"/>
    </owl:Thing>
    


    <!-- http://www.lexinfo.net/ontology/2.0/lexinfo#archaicForm -->

    <owl:Thing rdf:about="&lexinfo;archaicForm">
        <rdf:type rdf:resource="&lexinfo;TemporalQualifier"/>
        <rdf:type rdf:resource="&owl;NamedIndividual"/>
        <rdfs:label xml:lang="en">archaic form</rdfs:label>
        <rdfs:label xml:lang="ru">устаревшая форма</rdfs:label>        
        <dc:creator>Wright, Sue Ellen</dc:creator>
        <owl:versionInfo>1:0</owl:versionInfo>
        <rdfs:comment xml:lang="en">A term or lexeme no longer in ordinary use, though retained for special purposes.</rdfs:comment>
        <rdfs:comment xml:lang="ru">Термин или лексема больше не используются, хотя сохраняется для особых целей.</rdfs:comment>        
        <dcr:datcat rdf:resource="http://www.isocat.org/datcat/DC-504"/>
        <rdfs:isDefinedBy rdf:resource="http://www.lexinfo.net/ontology/2.0/lexinfo"/>
    </owl:Thing>
    


    <!-- http://www.lexinfo.net/ontology/2.0/lexinfo#article -->

    <owl:Thing rdf:about="&lexinfo;article">
        <rdf:type rdf:resource="&lexinfo;ArticlePOS"/>
        <rdf:type rdf:resource="&lexinfo;DeterminerPOS"/>
        <rdf:type rdf:resource="&lexinfo;PartOfSpeech"/>
        <rdf:type rdf:resource="&owl;NamedIndividual"/>
        <rdfs:label xml:lang="en">article</rdfs:label>
        <rdfs:label xml:lang="ru">артикль</rdfs:label>        
        <dc:creator>Wright, Sue Ellen</dc:creator>
        <dc:creator>Francopoulo, Gil</dc:creator>
        <rdfs:comment xml:lang="en">Term used in the grammatical classification of words referring to a subclass of determiners which displays a primary role in differentiating the uses of nouns.</rdfs:comment>
        <rdfs:comment xml:lang="ru">Термин, используемый в грамматической классификации слов, относящихся к подклассу детерминантов, который отображает основную роль в дифференциации использования существительных.</rdfs:comment>        
        <rdfs:comment>...</rdfs:comment>
        <owl:versionInfo>1:0</owl:versionInfo>
        <dcr:datcat rdf:resource="http://www.isocat.org/datcat/DC-101"/>
        <dcr:datcat rdf:resource="http://www.isocat.org/datcat/DC-1892"/>
        <rdfs:isDefinedBy rdf:resource="http://www.lexinfo.net/ontology/2.0/lexinfo"/>
    </owl:Thing>
    


    <!-- http://www.lexinfo.net/ontology/2.0/lexinfo#baseElement -->

    <owl:Thing rdf:about="&lexinfo;baseElement">
        <rdf:type rdf:resource="&lexinfo;TermElement"/>
        <rdf:type rdf:resource="&owl;NamedIndividual"/>
        <rdfs:label xml:lang="en">baseElement</rdfs:label>
        <rdfs:label xml:lang="ru">начальная форма</rdfs:label>
        <dc:creator>Wright, Sue Ellen</dc:creator>
        <rdfs:comment xml:lang="en">The root form of a word or term that is used as the formal dictionary entry for the term.</rdfs:comment>
        <rdfs:comment xml:lang="ru">Корневая форма слова или термина, которая используется как словарная запись для этого термина.</rdfs:comment>
        <owl:versionInfo>1:0</owl:versionInfo>
        <dcr:datcat rdf:resource="http://www.isocat.org/datcat/DC-290"/>
        <rdfs:isDefinedBy rdf:resource="http://www.lexinfo.net/ontology/2.0/lexinfo"/>
    </owl:Thing>
    


    <!-- http://www.lexinfo.net/ontology/2.0/lexinfo#benchLevelRegister -->

    <owl:Thing rdf:about="&lexinfo;benchLevelRegister">
        <rdf:type rdf:resource="&lexinfo;Register"/>
        <rdf:type rdf:resource="&owl;NamedIndividual"/>
        <rdfs:label xml:lang="en">bench-level register</rdfs:label>
        <rdfs:label xml:lang="ru">контрольный реестр</rdfs:label>        
        <dc:creator>Francopoulo, Gil</dc:creator>
        <rdfs:comment xml:lang="en">The register of terms used in applications-oriented as opposed to theoretical or academic levels of language.</rdfs:comment>
        <rdfs:comment xml:lang="ru">Реестр терминов, используемых в приложениях, в отличие от теоретических или академических уровней языка.</rdfs:comment>        
        <owl:versionInfo>1:0</owl:versionInfo>
        <rdfs:comment xml:lang="en">Register of terms used in applications-oriented as opposed to theoretical or academic levels of language.</rdfs:comment>
        <rdfs:comment xml:lang="ru">Реестр терминов, используемых в приложениях, в отличие от теоретических или академических уровней языка.</rdfs:comment>        
        <dc:creator>Wright, Sue Ellen</dc:creator>
        <dcr:datcat rdf:resource="http://www.isocat.org/datcat/DC-1989"/>
        <dcr:datcat rdf:resource="http://www.isocat.org/datcat/DC-427"/>
        <rdfs:isDefinedBy rdf:resource="http://www.lexinfo.net/ontology/2.0/lexinfo"/>
    </owl:Thing>
    


    <!-- http://www.lexinfo.net/ontology/2.0/lexinfo#benefactiveCase -->

    <owl:Thing rdf:about="&lexinfo;benefactiveCase">
        <rdf:type rdf:resource="&lexinfo;Case"/>
        <rdf:type rdf:resource="&owl;NamedIndividual"/>
        <rdfs:label xml:lang="en">benefactive case</rdfs:label>
        <rdfs:label xml:lang="ru">бенефактив</rdfs:label>        
        <dc:creator>Francopoulo, Gil</dc:creator>
        <owl:versionInfo>1:0</owl:versionInfo>
        <rdfs:comment xml:lang="en">Case that expresses that the referent of the noun it marks receives the benefit of the situation expressed by the clause.</rdfs:comment>
        <rdfs:comment xml:lang="ru">Падеж, который выражает, что референт обозначаемого им существительного получает выгоду от ситуации, выраженной в предложении.</rdfs:comment>
        <dcr:datcat rdf:resource="http://www.isocat.org/datcat/DC-1247"/>
        <rdfs:isDefinedBy rdf:resource="http://www.lexinfo.net/ontology/2.0/lexinfo"/>
    </owl:Thing>
    


    <!-- http://www.lexinfo.net/ontology/2.0/lexinfo#bound -->

    <owl:Thing rdf:about="&lexinfo;bound">
        <rdf:type rdf:resource="&lexinfo;Cliticness"/>
        <rdf:type rdf:resource="&owl;NamedIndividual"/>
        <rdfs:label xml:lang="en">bound</rdfs:label>
        <rdfs:label xml:lang="ru">связь</rdfs:label>        
        <rdfs:comment xml:lang="en">Linked to a particular element.</rdfs:comment>
        <rdfs:comment xml:lang="ru">Связь с определенным элементом.</rdfs:comment>
        <owl:versionInfo>1:0</owl:versionInfo>
        <dc:creator>Francopoulo, Gil</dc:creator>
        <dcr:datcat rdf:resource="http://www.isocat.org/datcat/DC-1933"/>
        <rdfs:isDefinedBy rdf:resource="http://www.lexinfo.net/ontology/2.0/lexinfo"/>
    </owl:Thing>
    


    <!-- http://www.lexinfo.net/ontology/2.0/lexinfo#bullet -->

    <owl:Thing rdf:about="&lexinfo;bullet">
        <rdf:type rdf:resource="&lexinfo;PartOfSpeech"/>
        <rdf:type rdf:resource="&lexinfo;SymbolPOS"/>
        <rdf:type rdf:resource="&owl;NamedIndividual"/>
        <rdfs:label xml:lang="en">bullet</rdfs:label>
        <rdfs:label xml:lang="ru">жирная точка</rdfs:label>        
        <dc:creator>Francopoulo, Gil</dc:creator>
        <owl:versionInfo>1:0</owl:versionInfo>
        <rdfs:comment xml:lang="en">Sign used to mark an item in a list.</rdfs:comment>
        <rdfs:comment xml:lang="ru">Знак, используемый для отметки элемента в списке.</rdfs:comment>
        <dcr:datcat rdf:resource="http://www.isocat.org/datcat/DC-1438"/>
        <rdfs:isDefinedBy rdf:resource="http://www.lexinfo.net/ontology/2.0/lexinfo"/>
    </owl:Thing>
    


    <!-- http://www.lexinfo.net/ontology/2.0/lexinfo#cardinalNumeral -->

    <owl:Thing rdf:about="&lexinfo;cardinalNumeral">
        <rdf:type rdf:resource="&lexinfo;NumeralPOS"/>
        <rdf:type rdf:resource="&lexinfo;PartOfSpeech"/>
        <rdf:type rdf:resource="&owl;NamedIndividual"/>
        <rdfs:label xml:lang="en">cardinal numeral</rdfs:label>
        <rdfs:label xml:lang="ru">количественное числительное</rdfs:label>        
        <rdfs:comment xml:lang="en">A word denoting a number.</rdfs:comment>
        <rdfs:comment xml:lang="ru">Слово, обозначающее число.</rdfs:comment>
        <owl:versionInfo>1:0</owl:versionInfo>
        <dc:creator>Zeman, Dan</dc:creator>
        <dcr:datcat rdf:resource="http://www.isocat.org/datcat/DC-3027"/>
        <rdfs:isDefinedBy rdf:resource="http://www.lexinfo.net/ontology/2.0/lexinfo"/>
    </owl:Thing>
    


    <!-- http://www.lexinfo.net/ontology/2.0/lexinfo#causativeCase -->

    <owl:Thing rdf:about="&lexinfo;causativeCase">
        <rdf:type rdf:resource="&lexinfo;Case"/>
        <rdf:type rdf:resource="&owl;NamedIndividual"/>
        <rdfs:label xml:lang="en">causative case</rdfs:label>
        <rdfs:label xml:lang="ru">каузатив; побудительный залог</rdfs:label>
        <owl:versionInfo>1:0</owl:versionInfo>
        <rdfs:comment xml:lang="en">Case which expresses that the referent of the noun it marks is the cause of the situation expressed by the clause.</rdfs:comment>
        <rdfs:comment xml:lang="ru">Падеж, который выражает, что референт обозначаемого им существительного является причиной ситуации, выраженной в предложении.</rdfs:comment>
        <dc:creator>Francopoulo, Gil</dc:creator>
        <dcr:datcat rdf:resource="http://www.isocat.org/datcat/DC-1253"/>
        <rdfs:isDefinedBy rdf:resource="http://www.lexinfo.net/ontology/2.0/lexinfo"/>
    </owl:Thing>
    


    <!-- http://www.lexinfo.net/ontology/2.0/lexinfo#cessative -->

    <owl:Thing rdf:about="&lexinfo;cessative">
        <rdf:type rdf:resource="&lexinfo;Aspect"/>
        <rdf:type rdf:resource="&owl;NamedIndividual"/>
        <rdfs:label xml:lang="en">cessative</rdfs:label>
        <rdfs:label xml:lang="ru">завершённый</rdfs:label>        
        <dc:creator>Francopoulo, Gil</dc:creator>
        <owl:versionInfo>1:0</owl:versionInfo>
        <rdfs:comment xml:lang="en">Aspect that expresses the cessation of an event or state.</rdfs:comment>
        <rdfs:comment xml:lang="ru">Вид, выражающий прекращение события или состояния.</rdfs:comment>
        <dcr:datcat rdf:resource="http://www.isocat.org/datcat/DC-2001"/>
        <rdfs:isDefinedBy rdf:resource="http://www.lexinfo.net/ontology/2.0/lexinfo"/>
    </owl:Thing>
    


    <!-- http://www.lexinfo.net/ontology/2.0/lexinfo#circumposition -->

    <owl:Thing rdf:about="&lexinfo;circumposition">
        <rdf:type rdf:resource="&lexinfo;AdpositionPOS"/>
        <rdf:type rdf:resource="&lexinfo;PartOfSpeech"/>
        <rdf:type rdf:resource="&owl;NamedIndividual"/>
        <rdfs:label xml:lang="en">circumposition</rdfs:label>
        <rdfs:label xml:lang="ru">Пара прилогов</rdfs:label>
        <dc:creator>Francopoulo, Gil</dc:creator>
        <owl:versionInfo>1:0</owl:versionInfo>
        <rdfs:comment xml:lang="en">Adposition which consists of two parts which are positioned ahead and after the adpositional foci.</rdfs:comment>
        <rdfs:comment xml:lang="ru">Прилог, состоящий из двух частей, расположенных соответственно до и после слова, к которому относится.</rdfs:comment>
        <dcr:datcat rdf:resource="http://www.isocat.org/datcat/DC-1906"/>
        <rdfs:isDefinedBy rdf:resource="http://www.lexinfo.net/ontology/2.0/lexinfo"/>
    </owl:Thing>
    


    <!-- http://www.lexinfo.net/ontology/2.0/lexinfo#clippedTerm -->

    <owl:Thing rdf:about="&lexinfo;clippedTerm">
        <rdf:type rdf:resource="&lexinfo;AbbreviatedForm"/>
        <rdf:type rdf:resource="&lexinfo;TermType"/>
        <rdf:type rdf:resource="&owl;NamedIndividual"/>
        <rdfs:label xml:lang="en">clipped term</rdfs:label>
        <rdfs:label xml:lang="ru">усеченный термин</rdfs:label>        
        <dc:creator>Wright, Sue Ellen</dc:creator>
        <rdfs:comment xml:lang="en">An abbreviation formed by truncating a part of a simple term.</rdfs:comment>
        <rdfs:comment xml:lang="ru">Аббревиатура, образованная путем усечения части простого термина.</rdfs:comment>
        <owl:versionInfo>1:0</owl:versionInfo>
        <dcr:datcat rdf:resource="http://www.isocat.org/datcat/DC-335"/>
        <rdfs:isDefinedBy rdf:resource="http://www.lexinfo.net/ontology/2.0/lexinfo"/>
    </owl:Thing>
    


    <!-- http://www.lexinfo.net/ontology/2.0/lexinfo#closeParenthesis -->

    <owl:Thing rdf:about="&lexinfo;closeParenthesis">
        <rdf:type rdf:resource="&lexinfo;PartOfSpeech"/>
        <rdf:type rdf:resource="&lexinfo;SymbolPOS"/>
        <rdf:type rdf:resource="&owl;NamedIndividual"/>
        <rdfs:label xml:lang="en">close parenthesis</rdfs:label>
        <rdfs:label xml:lang="ru">закрывающая круглая скобка</rdfs:label>        
        <owl:versionInfo>1:0</owl:versionInfo>
        <dc:creator>Francopoulo, Gil</dc:creator>
        <rdfs:comment xml:lang="en">End of a parenthesis pair.</rdfs:comment>
        <rdfs:comment xml:lang="ru">Вторая скобка в паре круглых скобок.</rdfs:comment>        
        <dcr:datcat rdf:resource="http://www.isocat.org/datcat/DC-1440"/>
        <rdfs:isDefinedBy rdf:resource="http://www.lexinfo.net/ontology/2.0/lexinfo"/>
    </owl:Thing>
    


    <!-- http://www.lexinfo.net/ontology/2.0/lexinfo#collective -->

    <owl:Thing rdf:about="&lexinfo;collective">
        <rdf:type rdf:resource="&lexinfo;Number"/>
        <rdf:type rdf:resource="&owl;NamedIndividual"/>
        <rdfs:label xml:lang="en">collective</rdfs:label>
        <rdfs:label xml:lang="ru">собирательное</rdfs:label>        
        <dc:creator>Francopoulo, Gil</dc:creator>
        <owl:versionInfo>1:0</owl:versionInfo>
        <rdfs:comment xml:lang="en">A collective number is a number referring to &apos;a set of things&apos;. Languages that have this feature can use it to get a phrase like &apos;flock of sheeps&apos; by using &apos;sheep&apos; in collective number.</rdfs:comment>
        <rdfs:comment xml:lang="ru">Собирательное число - это число, обозначающее &apos;набор предметов&apos;. Языки, которые имеют это свойство, могут использовать его, чтобы получить фразу типа &apos;стадо овец&apos;, используя &apos;овца&apos; в собирательном числе.</rdfs:comment>
        <dcr:datcat rdf:resource="http://www.isocat.org/datcat/DC-1254"/>
        <rdfs:isDefinedBy rdf:resource="http://www.lexinfo.net/ontology/2.0/lexinfo"/>
    </owl:Thing>
    


    <!-- http://www.lexinfo.net/ontology/2.0/lexinfo#collectivePronoun -->

    <owl:Thing rdf:about="&lexinfo;collectivePronoun">
        <rdf:type rdf:resource="&lexinfo;PartOfSpeech"/>
        <rdf:type rdf:resource="&lexinfo;PronounPOS"/>
        <rdf:type rdf:resource="&owl;NamedIndividual"/>
        <rdfs:label xml:lang="en">collective pronoun</rdfs:label>
        <rdfs:label xml:lang="ru">собирательное местоимение</rdfs:label>        
        <rdfs:comment xml:lang="en">A pronoun that refers to all elements of a set.</rdfs:comment>
        <rdfs:comment xml:lang="ru">Местоимение, которое относится ко всем элементам набора.</rdfs:comment>
        <dc:creator>Zeman, Dan</dc:creator>
        <owl:versionInfo>1:0</owl:versionInfo>
        <dcr:datcat rdf:resource="http://www.isocat.org/datcat/DC-3006"/>
        <rdfs:isDefinedBy rdf:resource="http://www.lexinfo.net/ontology/2.0/lexinfo"/>
    </owl:Thing>
    


    <!-- http://www.lexinfo.net/ontology/2.0/lexinfo#colon -->

    <owl:Thing rdf:about="&lexinfo;colon">
        <rdf:type rdf:resource="&lexinfo;PartOfSpeech"/>
        <rdf:type rdf:resource="&lexinfo;SymbolPOS"/>
        <rdf:type rdf:resource="&owl;NamedIndividual"/>
        <rdfs:label xml:lang="en">colon</rdfs:label>
        <rdfs:label xml:lang="ru">двоеточие</rdfs:label>
        <owl:versionInfo>1:0</owl:versionInfo>
        <dc:creator>Francopoulo, Gil</dc:creator>
        <rdfs:comment xml:lang="en">Sign with two vertical points that is used in writing and printing to introduce an explanation, example or quotation.</rdfs:comment>
        <rdfs:comment xml:lang="ru">Знак с двумя вертикальными точками, используемый в письме и печати, чтобы ввести объяснение, пример или цитату.</rdfs:comment>
        <dcr:datcat rdf:resource="http://www.isocat.org/datcat/DC-1439"/>
        <rdfs:isDefinedBy rdf:resource="http://www.lexinfo.net/ontology/2.0/lexinfo"/>
    </owl:Thing>
    


    <!-- http://www.lexinfo.net/ontology/2.0/lexinfo#comitativeCase -->

    <owl:Thing rdf:about="&lexinfo;comitativeCase">
        <rdf:type rdf:resource="&lexinfo;Case"/>
        <rdf:type rdf:resource="&owl;NamedIndividual"/>
        <rdfs:label xml:lang="en">comitative case</rdfs:label>
        <rdfs:label xml:lang="ru">комитативный</rdfs:label>        
        <dc:creator>Francopoulo, Gil</dc:creator>
        <owl:versionInfo>1:0</owl:versionInfo>
        <rdfs:comment xml:lang="en">Case which expresses a meaning similar to &apos;along with&apos; or &apos;accompagnied by&apos;.</rdfs:comment>
        <rdfs:comment xml:lang="ru">Падеж, который выражает значение, подобное &apos;вместе с&apos; или &apos;в сопровождении&apos;.</rdfs:comment>
        <dcr:datcat rdf:resource="http://www.isocat.org/datcat/DC-1255"/>
        <rdfs:isDefinedBy rdf:resource="http://www.lexinfo.net/ontology/2.0/lexinfo"/>
    </owl:Thing>
    


    <!-- http://www.lexinfo.net/ontology/2.0/lexinfo#comma -->

    <owl:Thing rdf:about="&lexinfo;comma">
        <rdf:type rdf:resource="&lexinfo;PartOfSpeech"/>
        <rdf:type rdf:resource="&lexinfo;SymbolPOS"/>
        <rdf:type rdf:resource="&owl;NamedIndividual"/>
        <rdfs:label xml:lang="en">comma</rdfs:label>
        <rdfs:label xml:lang="ru">запятая</rdfs:label>        
        <owl:versionInfo>1:0</owl:versionInfo>
        <dc:creator>Francopoulo, Gil</dc:creator>
        <rdfs:comment xml:lang="en">Mark (,) used in writing to show a short pause or to separate items in a list.</rdfs:comment>
        <rdfs:comment xml:lang="ru">Знак (,) используется в письменной форме, чтобы показать короткую паузу или отдельные элементы в списке.</rdfs:comment>
        <dcr:datcat rdf:resource="http://www.isocat.org/datcat/DC-1448"/>
        <rdfs:isDefinedBy rdf:resource="http://www.lexinfo.net/ontology/2.0/lexinfo"/>
    </owl:Thing>
    


    <!-- http://www.lexinfo.net/ontology/2.0/lexinfo#commonGender -->

    <owl:Thing rdf:about="&lexinfo;commonGender">
        <rdf:type rdf:resource="&lexinfo;Gender"/>
        <rdf:type rdf:resource="&owl;NamedIndividual"/>
        <rdfs:label xml:lang="en">common gender</rdfs:label>
        <rdfs:label xml:lang="ru">общий род</rdfs:label>        
        <dc:creator>Francopoulo, Gil</dc:creator>
        <rdfs:comment xml:lang="en">Indistinguished gender for epicenes.</rdfs:comment>
        <rdfs:comment xml:lang="ru">Неразличаемый род видового слова, объединяющего в себе понятия обоих полов.</rdfs:comment>
        <owl:versionInfo>1:0</owl:versionInfo>
        <dcr:datcat rdf:resource="http://www.isocat.org/datcat/DC-1558"/>
        <rdfs:isDefinedBy rdf:resource="http://www.lexinfo.net/ontology/2.0/lexinfo"/>
    </owl:Thing>
    


    <!-- http://www.lexinfo.net/ontology/2.0/lexinfo#commonName -->

    <owl:Thing rdf:about="&lexinfo;commonName">
        <rdf:type rdf:resource="&lexinfo;TermType"/>
        <rdf:type rdf:resource="&owl;NamedIndividual"/>
        <rdfs:label xml:lang="en">common name</rdfs:label>
        <rdfs:label xml:lang="ru">общепринятое название</rdfs:label>
        <rdfs:comment xml:lang="en">A synonym for an international scientific term that is used in general discourse in a given language.</rdfs:comment>
        <rdfs:comment xml:lang="ru">Синоним международного научного термина, который используется в общем употреблении в данном языке.</rdfs:comment>
        <owl:versionInfo>1:0</owl:versionInfo>
        <dc:creator>Wright, Sue Ellen</dc:creator>
        <dcr:datcat rdf:resource="http://www.isocat.org/datcat/DC-328"/>
        <rdfs:isDefinedBy rdf:resource="http://www.lexinfo.net/ontology/2.0/lexinfo"/>
    </owl:Thing>
    


    <!-- http://www.lexinfo.net/ontology/2.0/lexinfo#commonNoun -->

    <owl:Thing rdf:about="&lexinfo;commonNoun">
        <rdf:type rdf:resource="&lexinfo;NounPOS"/>
        <rdf:type rdf:resource="&lexinfo;PartOfSpeech"/>
        <rdf:type rdf:resource="&owl;NamedIndividual"/>
        <rdfs:label xml:lang="en">commonNoun</rdfs:label>
        <rdfs:label xml:lang="ru">имя нарицательное</rdfs:label>
        <rdfs:label xml:lang="en">common noun</rdfs:label>
        <rdfs:label xml:lang="ru">имя нарицательное</rdfs:label>
        <rdfs:comment xml:lang="en">A noun or adjective denoting a class of objects.</rdfs:comment>
        <rdfs:comment xml:lang="ru">Существительное или прилагательное, обозначающее класс объектов.</rdfs:comment>
        <dc:creator>Wright, Sue Ellen</dc:creator>
        <rdfs:comment xml:lang="en">Noun that signifies a non-specific member of a group.</rdfs:comment>
        <rdfs:comment xml:lang="ru">Существительное, которое называет неконкретного члена группы.</rdfs:comment>
        <dc:creator>Francopoulo, Gil</dc:creator>
        <owl:versionInfo>1:0</owl:versionInfo>
        <dcr:datcat rdf:resource="http://www.isocat.org/datcat/DC-1256"/>
        <dcr:datcat rdf:resource="http://www.isocat.org/datcat/DC-385"/>
        <rdfs:isDefinedBy rdf:resource="http://www.lexinfo.net/ontology/2.0/lexinfo"/>
    </owl:Thing>
    


    <!-- http://www.lexinfo.net/ontology/2.0/lexinfo#commonlyUsed -->

    <owl:Thing rdf:about="&lexinfo;commonlyUsed">
        <rdf:type rdf:resource="&lexinfo;Frequency"/>
        <rdf:type rdf:resource="&owl;NamedIndividual"/>
        <rdfs:label xml:lang="en">commonlyUsed</rdfs:label>
        <rdfs:label xml:lang="ru">широкоупотребительное</rdfs:label>
        <rdfs:label xml:lang="en">commonly used</rdfs:label>
        <rdfs:label xml:lang="ru">широкоупотребительное</rdfs:label>
        <dc:creator>Francopoulo, Gil</dc:creator>
        <rdfs:comment xml:lang="en">Said of a term that appears frequently.</rdfs:comment>
        <rdfs:comment xml:lang="ru">О термине, который часто используется.</rdfs:comment>
        <owl:versionInfo>1:0</owl:versionInfo>
        <dc:creator>Wright, Sue Ellen</dc:creator>
        <dcr:datcat rdf:resource="http://www.isocat.org/datcat/DC-1984"/>
        <dcr:datcat rdf:resource="http://www.isocat.org/datcat/DC-234"/>
        <rdfs:isDefinedBy rdf:resource="http://www.lexinfo.net/ontology/2.0/lexinfo"/>
    </owl:Thing>
    


    <!-- http://www.lexinfo.net/ontology/2.0/lexinfo#comparative -->

    <owl:Thing rdf:about="&lexinfo;comparative">
        <rdf:type rdf:resource="&lexinfo;Degree"/>
        <rdf:type rdf:resource="&owl;NamedIndividual"/>
        <rdfs:label xml:lang="en">comparative</rdfs:label>
        <rdfs:label xml:lang="ru">компаратив</rdfs:label>        
        <rdfs:comment xml:lang="en">Comparative is the comparison where only two entites are involved.</rdfs:comment>
        <rdfs:comment xml:lang="ru">Компаратив представляет собой сравнение, в котором участвуют только две сущности.</rdfs:comment>
        <dc:creator>Francopoulo, Gil</dc:creator>
        <owl:versionInfo>1:0</owl:versionInfo>
        <dcr:datcat rdf:resource="http://www.isocat.org/datcat/DC-1421"/>
        <rdfs:isDefinedBy rdf:resource="http://www.lexinfo.net/ontology/2.0/lexinfo"/>
    </owl:Thing>
    


    <!-- http://www.lexinfo.net/ontology/2.0/lexinfo#comparativeParticle -->

    <owl:Thing rdf:about="&lexinfo;comparativeParticle">
        <rdf:type rdf:resource="&lexinfo;PartOfSpeech"/>
        <rdf:type rdf:resource="&lexinfo;ParticlePOS"/>
        <rdf:type rdf:resource="&owl;NamedIndividual"/>
        <rdfs:label xml:lang="en">comparative particle</rdfs:label>
        <rdfs:label xml:lang="ru">сравнительная частица</rdfs:label>        
        <dc:creator>Francopoulo, Gil</dc:creator>
        <rdfs:comment xml:lang="en">Particle used to compare.</rdfs:comment>
        <rdfs:comment xml:lang="ru">Частица, используемая для сравнения.</rdfs:comment>
        <owl:versionInfo>1:0</owl:versionInfo>
        <dcr:datcat rdf:resource="http://www.isocat.org/datcat/DC-1922"/>
        <rdfs:isDefinedBy rdf:resource="http://www.lexinfo.net/ontology/2.0/lexinfo"/>
    </owl:Thing>
    


    <!-- http://www.lexinfo.net/ontology/2.0/lexinfo#compound -->

    <owl:Thing rdf:about="&lexinfo;compound">
        <rdf:type rdf:resource="&lexinfo;TermType"/>
        <rdf:type rdf:resource="&owl;NamedIndividual"/>
        <rdfs:label xml:lang="en">compound</rdfs:label>
        <rdfs:label xml:lang="ru">композит</rdfs:label>        
        <rdfs:comment xml:lang="en">A lexical unit that combines two or sometimes more different words, frequently such that the sense of the new lexical unit is not clearly derivable from the combination of its parts.</rdfs:comment>
        <rdfs:comment xml:lang="ru">Лексическая единица, которая сочетает в себе два или больше разных слова, часто таких, что смысл новой лексической единицы не выводится из сочетания ее частей.</rdfs:comment>
        <owl:versionInfo>1:0</owl:versionInfo>
        <dc:creator>Wright, Sue Ellen</dc:creator>
        <dcr:datcat rdf:resource="http://www.isocat.org/datcat/DC-352"/>
        <rdfs:isDefinedBy rdf:resource="http://www.lexinfo.net/ontology/2.0/lexinfo"/>
    </owl:Thing>
    


    <!-- http://www.lexinfo.net/ontology/2.0/lexinfo#compoundPreposition -->

    <owl:Thing rdf:about="&lexinfo;compoundPreposition">
        <rdf:type rdf:resource="&lexinfo;AdpositionPOS"/>
        <rdf:type rdf:resource="&lexinfo;PartOfSpeech"/>
        <rdf:type rdf:resource="&owl;NamedIndividual"/>
        <rdfs:label xml:lang="en">compound preposition</rdfs:label>
        <rdfs:label xml:lang="ru">сложный предлог</rdfs:label>
        <owl:versionInfo>1:0</owl:versionInfo>
        <dc:creator>Francopoulo, Gil</dc:creator>
        <rdfs:comment xml:lang="en">Preposition that is a aggregation of words</rdfs:comment>
        <rdfs:comment xml:lang="ru">Предлог, представляющий собой совокупность слов</rdfs:comment>
        <dcr:datcat rdf:resource="http://www.isocat.org/datcat/DC-1934"/>
        <rdfs:isDefinedBy rdf:resource="http://www.lexinfo.net/ontology/2.0/lexinfo"/>
    </owl:Thing>
    


    <!-- http://www.lexinfo.net/ontology/2.0/lexinfo#conditional -->

    <owl:Thing rdf:about="&lexinfo;conditional">
        <rdf:type rdf:resource="&lexinfo;VerbFormMood"/>
        <rdf:type rdf:resource="&owl;NamedIndividual"/>
        <rdfs:label xml:lang="en">conditional</rdfs:label>
        <rdfs:label xml:lang="ru">условность</rdfs:label>        
        <owl:versionInfo>1:0</owl:versionInfo>
        <rdfs:comment xml:lang="en">A conditional relation is a logical relation in which the illocutionary act employing one of a pair of propositions is expressed or implied to be true or in force if the other proposition is true.</rdfs:comment>
        <rdfs:comment xml:lang="ru">Условное отношение является логическим отношением, в котором иллокутивный акт, использующий одно из пары утверждений, выражается или подразумевается как истинное или действующее, если другое утверждение истинно.</rdfs:comment>        
        <dc:creator>Francopoulo, Gil</dc:creator>
        <dcr:datcat rdf:resource="http://www.isocat.org/datcat/DC-1258"/>
        <rdfs:isDefinedBy rdf:resource="http://www.lexinfo.net/ontology/2.0/lexinfo"/>
    </owl:Thing>
    


    <!-- http://www.lexinfo.net/ontology/2.0/lexinfo#conditionalParticle -->

    <owl:Thing rdf:about="&lexinfo;conditionalParticle">
        <rdf:type rdf:resource="&lexinfo;PartOfSpeech"/>
        <rdf:type rdf:resource="&lexinfo;ParticlePOS"/>
        <rdf:type rdf:resource="&owl;NamedIndividual"/>
        <rdfs:label xml:lang="en">conditional particule</rdfs:label>
        <rdfs:label xml:lang="ru">условная частица</rdfs:label>        
        <rdfs:comment xml:lang="en">conditional particule</rdfs:comment>
        <rdfs:comment xml:lang="ru">условная частица</rdfs:comment>
        <owl:versionInfo>1:0</owl:versionInfo>
        <dc:creator>Francopoulo, Gil</dc:creator>
        <dcr:datcat rdf:resource="http://www.isocat.org/datcat/DC-2230"/>
        <rdfs:isDefinedBy rdf:resource="http://www.lexinfo.net/ontology/2.0/lexinfo"/>
    </owl:Thing>
    


    <!-- http://www.lexinfo.net/ontology/2.0/lexinfo#conditionalPronoun -->

    <owl:Thing rdf:about="&lexinfo;conditionalPronoun">
        <rdf:type rdf:resource="&lexinfo;PartOfSpeech"/>
        <rdf:type rdf:resource="&lexinfo;PronounPOS"/>
        <rdf:type rdf:resource="&owl;NamedIndividual"/>
        <rdfs:label xml:lang="en">conditional pronoun</rdfs:label>
        <rdfs:label xml:lang="ru">условное местоимение</rdfs:label>        
        <dc:creator>Francopoulo, Gil</dc:creator>
        <rdfs:comment xml:lang="en">conditional pronoun</rdfs:comment>
        <rdfs:comment xml:lang="ru">условное местоимение</rdfs:comment>
        <owl:versionInfo>1:0</owl:versionInfo>
        <dcr:datcat rdf:resource="http://www.isocat.org/datcat/DC-2222"/>
        <rdfs:isDefinedBy rdf:resource="http://www.lexinfo.net/ontology/2.0/lexinfo"/>
    </owl:Thing>
    


    <!-- http://www.lexinfo.net/ontology/2.0/lexinfo#conjunction -->

    <owl:Thing rdf:about="&lexinfo;conjunction">
        <rdf:type rdf:resource="&lexinfo;ConjunctionPOS"/>
        <rdf:type rdf:resource="&lexinfo;PartOfSpeech"/>
        <rdf:type rdf:resource="&owl;NamedIndividual"/>
        <rdfs:label xml:lang="en">conjunction</rdfs:label>
        <rdfs:label xml:lang="ru">союз</rdfs:label>        
        <rdfs:comment xml:lang="en">Word that syntactically links words or constituents, and expresses a semantic relationship between them.</rdfs:comment>
        <rdfs:comment xml:lang="ru">Слово, которое синтаксически связывает слова или составляющие и выражает семантические отношения между ними.</rdfs:comment>        
        <owl:versionInfo>1:0</owl:versionInfo>
        <dc:creator>Francopoulo, Gil</dc:creator>
        <dcr:datcat rdf:resource="http://www.isocat.org/datcat/DC-1260"/>
        <rdfs:isDefinedBy rdf:resource="http://www.lexinfo.net/ontology/2.0/lexinfo"/>
    </owl:Thing>
    


    <!-- http://www.lexinfo.net/ontology/2.0/lexinfo#contraction -->

    <owl:Thing rdf:about="&lexinfo;contraction">
        <rdf:type rdf:resource="&lexinfo;AbbreviatedForm"/>
        <rdf:type rdf:resource="&lexinfo;TermType"/>
        <rdf:type rdf:resource="&owl;NamedIndividual"/>
        <rdfs:label xml:lang="en">contraction</rdfs:label>
        <rdfs:label xml:lang="ru">сокращение</rdfs:label>        
        <rdfs:comment xml:lang="en">A lexical unit formed by a shortening of a word, syllable, or word group by omission of a sound or letter.</rdfs:comment>
        <rdfs:comment xml:lang="ru">Лексическая единица, образованная сокращением слова, слога или группы слов, при котором опускается звук или буква.</rdfs:comment>
        <owl:versionInfo>1:0</owl:versionInfo>
        <dc:creator>Wright, Sue Ellen</dc:creator>
        <dcr:datcat rdf:resource="http://www.isocat.org/datcat/DC-354"/>
        <rdfs:isDefinedBy rdf:resource="http://www.lexinfo.net/ontology/2.0/lexinfo"/>
    </owl:Thing>
    


    <!-- http://www.lexinfo.net/ontology/2.0/lexinfo#coordinatingConjunction -->

    <owl:Thing rdf:about="&lexinfo;coordinatingConjunction">
        <rdf:type rdf:resource="&lexinfo;ConjunctionPOS"/>
        <rdf:type rdf:resource="&lexinfo;PartOfSpeech"/>
        <rdf:type rdf:resource="&owl;NamedIndividual"/>
        <rdfs:label xml:lang="en">coordinating conjunction</rdfs:label>
        <rdfs:label xml:lang="ru">сочинительный союз</rdfs:label>        
        <owl:versionInfo>1:0</owl:versionInfo>
        <rdfs:comment xml:lang="en">Conjunction that links constituents.</rdfs:comment>
        <rdfs:comment xml:lang="ru">Союз, связывающий составляющие.</rdfs:comment>
        <dc:creator>Francopoulo, Gil</dc:creator>
        <dcr:datcat rdf:resource="http://www.isocat.org/datcat/DC-1262"/>
        <rdfs:isDefinedBy rdf:resource="http://www.lexinfo.net/ontology/2.0/lexinfo"/>
    </owl:Thing>
    


    <!-- http://www.lexinfo.net/ontology/2.0/lexinfo#coordinationParticle -->

    <owl:Thing rdf:about="&lexinfo;coordinationParticle">
        <rdf:type rdf:resource="&lexinfo;PartOfSpeech"/>
        <rdf:type rdf:resource="&lexinfo;ParticlePOS"/>
        <rdf:type rdf:resource="&owl;NamedIndividual"/>
        <rdfs:label xml:lang="en">coordination particle</rdfs:label>
        <rdfs:label xml:lang="ru">соединительная частица</rdfs:label>        
        <owl:versionInfo>1:0</owl:versionInfo>
        <dc:creator>Francopoulo, Gil</dc:creator>
        <rdfs:comment xml:lang="en">particle for coordination</rdfs:comment>
        <rdfs:comment xml:lang="ru">частица для согласования</rdfs:comment>
        <dcr:datcat rdf:resource="http://www.isocat.org/datcat/DC-2227"/>
        <rdfs:isDefinedBy rdf:resource="http://www.lexinfo.net/ontology/2.0/lexinfo"/>
    </owl:Thing>
    


    <!-- http://www.lexinfo.net/ontology/2.0/lexinfo#copula -->

    <owl:Thing rdf:about="&lexinfo;copula">
        <rdf:type rdf:resource="&lexinfo;PartOfSpeech"/>
        <rdf:type rdf:resource="&lexinfo;VerbPOS"/>
        <rdf:type rdf:resource="&owl;NamedIndividual"/>
        <rdfs:label xml:lang="en">copula</rdfs:label>
        <rdfs:label xml:lang="ru">связка</rdfs:label>        
        <rdfs:comment xml:lang="en">Special word that combines the subject of a sentence and its description.</rdfs:comment>
        <rdfs:comment xml:lang="ru">Специальное слово, которое соединяет субъект предложения и его описание.</rdfs:comment>
        <owl:versionInfo>1:0</owl:versionInfo>
        <dc:creator>Francopoulo, Gil</dc:creator>
        <dcr:datcat rdf:resource="http://www.isocat.org/datcat/DC-1263"/>
        <rdfs:isDefinedBy rdf:resource="http://www.lexinfo.net/ontology/2.0/lexinfo"/>
    </owl:Thing>
    


    <!-- http://www.lexinfo.net/ontology/2.0/lexinfo#dativeCase -->

    <owl:Thing rdf:about="&lexinfo;dativeCase">
        <rdf:type rdf:resource="&lexinfo;Case"/>
        <rdf:type rdf:resource="&owl;NamedIndividual"/>
        <rdfs:label xml:lang="en">dative case</rdfs:label>
        <rdfs:label xml:lang="ru">дательный падеж</rdfs:label>        
        <owl:versionInfo>1:0</owl:versionInfo>
        <dc:creator>Francopoulo, Gil</dc:creator>
        <rdfs:comment xml:lang="en">Case that expresses an indirect object relationship or a range of meaning similar to that covered by &apos;to&apos; or &apos;for&apos; in English; but there is a great deal of variation between languages in the way this case is used.</rdfs:comment>
        <rdfs:comment xml:lang="ru">Падеж, который выражает косвенное дополнение или диапазон значений, аналогичный тому, который охватывают предлоги &apos;to&apos; или &apos;for&apos; в английском языке (в русском языке: "к", "по"); но в различных языках существуют разные способы использования этого падежа.</rdfs:comment>
        <dcr:datcat rdf:resource="http://www.isocat.org/datcat/DC-1265"/>
        <rdfs:isDefinedBy rdf:resource="http://www.lexinfo.net/ontology/2.0/lexinfo"/>
    </owl:Thing>
    


    <!-- http://www.lexinfo.net/ontology/2.0/lexinfo#deficientVerb -->

    <owl:Thing rdf:about="&lexinfo;deficientVerb">
        <rdf:type rdf:resource="&lexinfo;PartOfSpeech"/>
        <rdf:type rdf:resource="&lexinfo;VerbPOS"/>
        <rdf:type rdf:resource="&owl;NamedIndividual"/>
        <rdfs:label xml:lang="en">deficient verb</rdfs:label>
        <rdfs:label xml:lang="ru">недостаточный глагол</rdfs:label>        
        <owl:versionInfo>1:0</owl:versionInfo>
        <rdfs:comment xml:lang="en">verb lacking certain morphosyntactic properties</rdfs:comment>
        <rdfs:comment xml:lang="ru">глагол, не имеющий определенных морфосинтактических свойств</rdfs:comment>
        <dc:creator>Francopoulo, Gil</dc:creator>
        <dcr:datcat rdf:resource="http://www.isocat.org/datcat/DC-3007"/>
        <rdfs:isDefinedBy rdf:resource="http://www.lexinfo.net/ontology/2.0/lexinfo"/>
    </owl:Thing>
    


    <!-- http://www.lexinfo.net/ontology/2.0/lexinfo#definite -->

    <owl:Thing rdf:about="&lexinfo;definite">
        <rdf:type rdf:resource="&lexinfo;Definiteness"/>
        <rdf:type rdf:resource="&owl;NamedIndividual"/>
        <rdfs:label xml:lang="en">definite</rdfs:label>
        <rdfs:label xml:lang="ru">определенный</rdfs:label>        
        <owl:versionInfo>1:0</owl:versionInfo>
        <dc:creator>Francopoulo, Gil</dc:creator>
        <rdfs:comment xml:lang="en">Value referring to the capacity of identification of an entity.</rdfs:comment>
        <rdfs:comment xml:lang="ru">Значение, относящееся к возможности идентификации объекта.</rdfs:comment>
        <dcr:datcat rdf:resource="http://www.isocat.org/datcat/DC-2004"/>
        <rdfs:isDefinedBy rdf:resource="http://www.lexinfo.net/ontology/2.0/lexinfo"/>
    </owl:Thing>
    


    <!-- http://www.lexinfo.net/ontology/2.0/lexinfo#definiteArticle -->

    <owl:Thing rdf:about="&lexinfo;definiteArticle">
        <rdf:type rdf:resource="&lexinfo;ArticlePOS"/>
        <rdf:type rdf:resource="&lexinfo;DeterminerPOS"/>
        <rdf:type rdf:resource="&lexinfo;PartOfSpeech"/>
        <rdf:type rdf:resource="&owl;NamedIndividual"/>
        <rdfs:label xml:lang="en">definite article</rdfs:label>
        <rdfs:label xml:lang="ru">определенный артикль</rdfs:label>        
        <rdfs:comment xml:lang="en">Article that allows the reference to a specific, identifiable entity (or class of entities).</rdfs:comment>
        <rdfs:comment xml:lang="ru">Артикль, который позволяет указывать на конкретную идентифицируемую сущность (или класс сущностей).</rdfs:comment>
        <owl:versionInfo>1:0</owl:versionInfo>
        <dc:creator>Francopoulo, Gil</dc:creator>
        <dcr:datcat rdf:resource="http://www.isocat.org/datcat/DC-1430"/>
        <rdfs:isDefinedBy rdf:resource="http://www.lexinfo.net/ontology/2.0/lexinfo"/>
    </owl:Thing>
    


    <!-- http://www.lexinfo.net/ontology/2.0/lexinfo#delativeCase -->

    <owl:Thing rdf:about="&lexinfo;delativeCase">
        <rdf:type rdf:resource="&lexinfo;Case"/>
        <rdf:type rdf:resource="&owl;NamedIndividual"/>
        <rdfs:label xml:lang="en">delative case</rdfs:label>
        <rdfs:label xml:lang="ru">верхнеотдалительный падеж</rdfs:label>        
        <rdfs:comment xml:lang="en">Case which expresses motion downward from the referent of the noun it marks.</rdfs:comment>
        <rdfs:comment xml:lang="ru">Падеж, который выражает движение вниз от референта существительного, которое он указывает.</rdfs:comment>
        <dc:creator>Francopoulo, Gil</dc:creator>
        <owl:versionInfo>1:0</owl:versionInfo>
        <dcr:datcat rdf:resource="http://www.isocat.org/datcat/DC-1268"/>
        <rdfs:isDefinedBy rdf:resource="http://www.lexinfo.net/ontology/2.0/lexinfo"/>
    </owl:Thing>
    


    <!-- http://www.lexinfo.net/ontology/2.0/lexinfo#demonstrativeDeterminer -->

    <owl:Thing rdf:about="&lexinfo;demonstrativeDeterminer">
        <rdf:type rdf:resource="&lexinfo;DeterminerPOS"/>
        <rdf:type rdf:resource="&lexinfo;PartOfSpeech"/>
        <rdf:type rdf:resource="&owl;NamedIndividual"/>
        <rdfs:label xml:lang="en">demonstrative determiner</rdfs:label>
        <rdfs:label xml:lang="ru">указательный определитель</rdfs:label>
        <dc:creator>Francopoulo, Gil</dc:creator>
        <owl:versionInfo>1:0</owl:versionInfo>
        <rdfs:comment xml:lang="en">Determiner used to point to an entity in the situation or elsewhere in a sentence.</rdfs:comment>
        <rdfs:comment xml:lang="ru">Определитель, используемый для указания на объект в ситуации или какой-либо части предложения.</rdfs:comment>
        <dcr:datcat rdf:resource="http://www.isocat.org/datcat/DC-1269"/>
        <rdfs:isDefinedBy rdf:resource="http://www.lexinfo.net/ontology/2.0/lexinfo"/>
    </owl:Thing>
    


    <!-- http://www.lexinfo.net/ontology/2.0/lexinfo#demonstrativePronoun -->

    <owl:Thing rdf:about="&lexinfo;demonstrativePronoun">
        <rdf:type rdf:resource="&lexinfo;PartOfSpeech"/>
        <rdf:type rdf:resource="&lexinfo;PronounPOS"/>
        <rdf:type rdf:resource="&owl;NamedIndividual"/>
        <rdfs:label xml:lang="en">demonstrative pronoun</rdfs:label>
        <rdfs:label xml:lang="ru">указательное местоимение</rdfs:label>        
        <dc:creator>Francopoulo, Gil</dc:creator>
        <rdfs:comment xml:lang="en">Pronoun used to point to an entity in the situation or elsewhere in a sentence.</rdfs:comment>
        <rdfs:comment xml:lang="ru">Местоимение, используемое, чтобы указывать на объект в ситуации или какой-либо части предложения.</rdfs:comment>
        <owl:versionInfo>1:0</owl:versionInfo>
        <dcr:datcat rdf:resource="http://www.isocat.org/datcat/DC-1270"/>
        <rdfs:isDefinedBy rdf:resource="http://www.lexinfo.net/ontology/2.0/lexinfo"/>
    </owl:Thing>
    


    <!-- http://www.lexinfo.net/ontology/2.0/lexinfo#deprecatedTerm -->

    <owl:Thing rdf:about="&lexinfo;deprecatedTerm">
        <rdf:type rdf:resource="&lexinfo;NormativeAuthorization"/>
        <rdf:type rdf:resource="&owl;NamedIndividual"/>
        <rdfs:label xml:lang="en">deprecated term</rdfs:label>
        <rdfs:label xml:lang="ru">нерекомендуемый термин</rdfs:label>        
        <rdfs:comment xml:lang="en">A term rated according to the scale of a term acceptability rating as undesired.</rdfs:comment>
        <rdfs:comment xml:lang="ru">Термин, оцененный по шкале приемлемости терминов как  нежелательный.</rdfs:comment>
        <owl:versionInfo>1:0</owl:versionInfo>
        <dc:creator>Wright, Sue Ellen</dc:creator>
        <dcr:datcat rdf:resource="http://www.isocat.org/datcat/DC-378"/>
        <rdfs:isDefinedBy rdf:resource="http://www.lexinfo.net/ontology/2.0/lexinfo"/>
    </owl:Thing>
    


    <!-- http://www.lexinfo.net/ontology/2.0/lexinfo#determiner -->

    <owl:Thing rdf:about="&lexinfo;determiner">
        <rdf:type rdf:resource="&lexinfo;DeterminerPOS"/>
        <rdf:type rdf:resource="&lexinfo;PartOfSpeech"/>
        <rdf:type rdf:resource="&owl;NamedIndividual"/>
        <rdfs:label xml:lang="en">determiner</rdfs:label>
        <rdfs:label xml:lang="ru">определяющее слово</rdfs:label>        
        <dc:creator>Francopoulo, Gil</dc:creator>
        <owl:versionInfo>1:0</owl:versionInfo>
        <rdfs:comment xml:lang="en">Word or affix that belongs to a class of noun modifiers that expresses the reference, including quantity, of a noun.</rdfs:comment>
        <rdfs:comment xml:lang="ru">Слово или аффикс, принадлежащие классу существительных-модификаторов, которые выражают указание на существительное, включая количество.</rdfs:comment>
        <dcr:datcat rdf:resource="http://www.isocat.org/datcat/DC-1272"/>
        <rdfs:isDefinedBy rdf:resource="http://www.lexinfo.net/ontology/2.0/lexinfo"/>
    </owl:Thing>
    


    <!-- http://www.lexinfo.net/ontology/2.0/lexinfo#dialectRegister -->

    <owl:Thing rdf:about="&lexinfo;dialectRegister">
        <rdf:type rdf:resource="&lexinfo;Register"/>
        <rdf:type rdf:resource="&owl;NamedIndividual"/>
        <rdfs:isDefinedBy rdf:resource="http://www.lexinfo.net/ontology/2.0/lexinfo"/>
    </owl:Thing>
    


    <!-- http://www.lexinfo.net/ontology/2.0/lexinfo#diminutiveNoun -->

    <owl:Thing rdf:about="&lexinfo;diminutiveNoun">
        <rdf:type rdf:resource="&lexinfo;NounPOS"/>
        <rdf:type rdf:resource="&lexinfo;PartOfSpeech"/>
        <rdf:type rdf:resource="&owl;NamedIndividual"/>
        <rdfs:label xml:lang="en">diminutive noun</rdfs:label>
        <rdfs:label xml:lang="ru">уменьшительное существительное</rdfs:label>
        <dc:creator>Francopoulo, Gil</dc:creator>
        <owl:versionInfo>1:0</owl:versionInfo>
        <rdfs:comment xml:lang="en">diminutive noun</rdfs:comment>
        <rdfs:comment xml:lang="ru">уменьшительное существительное</rdfs:comment>        
        <dcr:datcat rdf:resource="http://www.isocat.org/datcat/DC-2225"/>
        <rdfs:isDefinedBy rdf:resource="http://www.lexinfo.net/ontology/2.0/lexinfo"/>
    </owl:Thing>
    


    <!-- http://www.lexinfo.net/ontology/2.0/lexinfo#distinctiveParticle -->

    <owl:Thing rdf:about="&lexinfo;distinctiveParticle">
        <rdf:type rdf:resource="&lexinfo;PartOfSpeech"/>
        <rdf:type rdf:resource="&lexinfo;ParticlePOS"/>
        <rdf:type rdf:resource="&owl;NamedIndividual"/>
        <rdfs:label xml:lang="en">distinctive particle</rdfs:label>
        <rdfs:label xml:lang="ru">отличительная частица</rdfs:label>        
        <dc:creator>Francopoulo, Gil</dc:creator>
        <rdfs:comment xml:lang="en">distinctive particle</rdfs:comment>
        <rdfs:comment xml:lang="ru">отличительная частица</rdfs:comment>
        <owl:versionInfo>1:0</owl:versionInfo>
        <dcr:datcat rdf:resource="http://www.isocat.org/datcat/DC-2228"/>
        <rdfs:isDefinedBy rdf:resource="http://www.lexinfo.net/ontology/2.0/lexinfo"/>
    </owl:Thing>
    


    <!-- http://www.lexinfo.net/ontology/2.0/lexinfo#dual -->

    <owl:Thing rdf:about="&lexinfo;dual">
        <rdf:type rdf:resource="&lexinfo;Number"/>
        <rdf:type rdf:resource="&owl;NamedIndividual"/>
        <rdfs:label xml:lang="en">dual</rdfs:label>
        <rdfs:label xml:lang="ru">двойственное</rdfs:label>        
        <dc:creator>Francopoulo, Gil</dc:creator>
        <owl:versionInfo>1:0</owl:versionInfo>
        <dc:creator>Wright, Sue Ellen</dc:creator>
        <rdfs:comment xml:lang="en">The form used in some languages to designate two persons or things.</rdfs:comment>
        <rdfs:comment xml:lang="ru">Форма, используемая в некоторых языках для обозначения двух лиц или вещей.</rdfs:comment>        
        <rdfs:comment xml:lang="en">Form used in some languages to designate two persons or things.</rdfs:comment>
        <rdfs:comment xml:lang="ru">Форма, используемая в некоторых языках для обозначения двух лиц или вещей.</rdfs:comment>
        <dcr:datcat rdf:resource="http://www.isocat.org/datcat/DC-1879"/>
        <dcr:datcat rdf:resource="http://www.isocat.org/datcat/DC-254"/>
        <rdfs:isDefinedBy rdf:resource="http://www.lexinfo.net/ontology/2.0/lexinfo"/>
    </owl:Thing>
    


    <!-- http://www.lexinfo.net/ontology/2.0/lexinfo#elativeCase -->

    <owl:Thing rdf:about="&lexinfo;elativeCase">
        <rdf:type rdf:resource="&lexinfo;Case"/>
        <rdf:type rdf:resource="&owl;NamedIndividual"/>
        <rdfs:label xml:lang="en">elative case</rdfs:label>
        <rdfs:label xml:lang="ru">элатив</rdfs:label>
        <owl:versionInfo>1:0</owl:versionInfo>
        <dc:creator>Francopoulo, Gil</dc:creator>
        <rdfs:comment xml:lang="en">Case which expresses the meaning of motion &apos;away from&apos; from the referent of the noun it marks.</rdfs:comment>
        <rdfs:comment xml:lang="ru">Падеж, обозначающий движение &apos;в сторону от&apos; от референта существительного, на которое он указывает.</rdfs:comment>
        <dcr:datcat rdf:resource="http://www.isocat.org/datcat/DC-1276"/>
        <rdfs:isDefinedBy rdf:resource="http://www.lexinfo.net/ontology/2.0/lexinfo"/>
    </owl:Thing>
    


    <!-- http://www.lexinfo.net/ontology/2.0/lexinfo#emphaticPronoun -->

    <owl:Thing rdf:about="&lexinfo;emphaticPronoun">
        <rdf:type rdf:resource="&lexinfo;PartOfSpeech"/>
        <rdf:type rdf:resource="&lexinfo;PronounPOS"/>
        <rdf:type rdf:resource="&owl;NamedIndividual"/>
        <rdfs:label xml:lang="en">emphatic pronoun</rdfs:label>
        <rdfs:label xml:lang="ru">эмфатическое местоимение</rdfs:label>        
        <dc:creator>Francopoulo, Gil</dc:creator>
        <owl:versionInfo>1:0</owl:versionInfo>
        <rdfs:comment xml:lang="en">An emphatic pronoun is a personal pronoun that is used to emphasize its referent.</rdfs:comment>
        <rdfs:comment xml:lang="ru">Эмфатическое местоимение - это личное местоимение, которое используется, чтобы особо выделить его референт.</rdfs:comment>
        <dcr:datcat rdf:resource="http://www.isocat.org/datcat/DC-1941"/>
        <rdfs:isDefinedBy rdf:resource="http://www.lexinfo.net/ontology/2.0/lexinfo"/>
    </owl:Thing>
    


    <!-- http://www.lexinfo.net/ontology/2.0/lexinfo#entryTerm -->

    <owl:Thing rdf:about="&lexinfo;entryTerm">
        <rdf:type rdf:resource="&lexinfo;TermType"/>
        <rdf:type rdf:resource="&owl;NamedIndividual"/>
        <rdfs:label xml:lang="en">entry term</rdfs:label>
        <rdfs:label xml:lang="ru">заглавный термин</rdfs:label>        
        <rdfs:comment xml:lang="en">A term that heads a terminological entry.</rdfs:comment>
        <rdfs:comment xml:lang="ru">Термин, используемый в качестве основного в терминологической записи.</rdfs:comment>
        <owl:versionInfo>1:0</owl:versionInfo>
        <dc:creator>Wright, Sue Ellen</dc:creator>
        <dcr:datcat rdf:resource="http://www.isocat.org/datcat/DC-316"/>
        <rdfs:isDefinedBy rdf:resource="http://www.lexinfo.net/ontology/2.0/lexinfo"/>
    </owl:Thing>
    


    <!-- http://www.lexinfo.net/ontology/2.0/lexinfo#equation -->

    <owl:Thing rdf:about="&lexinfo;equation">
        <rdf:type rdf:resource="&lexinfo;TermType"/>
        <rdf:type rdf:resource="&owl;NamedIndividual"/>
        <rdfs:label xml:lang="en">equation</rdfs:label>
        <rdfs:label xml:lang="ru">уравнение</rdfs:label>        
        <dc:creator>Wright, Sue Ellen</dc:creator>
        <owl:versionInfo>1:0</owl:versionInfo>
        <rdfs:comment xml:lang="en">An expression used to represent a concept based on a statement that two mathematical expressions are, for instance, equal as identified by the equal sign (=), or assigned to one another by a similar sign.</rdfs:comment>
        <rdfs:comment xml:lang="ru">Выражение, используемое для представления понятия, основанного на утверждении о том, что два математических выражения равны (=) или приписываются друг к другу аналогичным знаком.</rdfs:comment>
        <dcr:datcat rdf:resource="http://www.isocat.org/datcat/DC-326"/>
        <rdfs:isDefinedBy rdf:resource="http://www.lexinfo.net/ontology/2.0/lexinfo"/>
    </owl:Thing>
    


    <!-- http://www.lexinfo.net/ontology/2.0/lexinfo#equativeCase -->

    <owl:Thing rdf:about="&lexinfo;equativeCase">
        <rdf:type rdf:resource="&lexinfo;Case"/>
        <rdf:type rdf:resource="&owl;NamedIndividual"/>
        <rdfs:label xml:lang="en">equative case</rdfs:label>
        <rdfs:label xml:lang="ru">сравнительный падеж</rdfs:label>        
        <dc:creator>Francopoulo, Gil</dc:creator>
        <rdfs:comment xml:lang="en">Case that expresses likeness or identity to the referent of the noun it marks. It can have meaning, such as: &apos;as&apos;, &apos;like&apos;, or &apos;in the capacity of&apos;.</rdfs:comment>
        <rdfs:comment xml:lang="ru">Падеж, выражающий сходство или идентичность с референтом существительного, на которое он указывает. Он может иметь значение, например: &apos;как&apos;, &apos;подобно&apos; или &apos;в качестве&apos;.</rdfs:comment>
        <owl:versionInfo>1:0</owl:versionInfo>
        <dcr:datcat rdf:resource="http://www.isocat.org/datcat/DC-1279"/>
        <rdfs:isDefinedBy rdf:resource="http://www.lexinfo.net/ontology/2.0/lexinfo"/>
    </owl:Thing>
    


    <!-- http://www.lexinfo.net/ontology/2.0/lexinfo#ergativeCase -->

    <owl:Thing rdf:about="&lexinfo;ergativeCase">
        <rdf:type rdf:resource="&lexinfo;Case"/>
        <rdf:type rdf:resource="&owl;NamedIndividual"/>
        <rdfs:label xml:lang="en">ergative case</rdfs:label>
        <rdfs:label xml:lang="ru">эргатив</rdfs:label>        
        <owl:versionInfo>1:0</owl:versionInfo>
        <rdfs:comment xml:lang="en">Case assigned to the subject of a transitive verb as opposed to absolutive case.</rdfs:comment>
        <rdfs:comment xml:lang="ru">Падеж, приписанный субъекту переходного глагола, в противоположность абсолютивному падежу.</rdfs:comment>
        <dc:creator>Francopoulo, Gil</dc:creator>
        <dcr:datcat rdf:resource="http://www.isocat.org/datcat/DC-1280"/>
        <rdfs:isDefinedBy rdf:resource="http://www.lexinfo.net/ontology/2.0/lexinfo"/>
    </owl:Thing>
    


    <!-- http://www.lexinfo.net/ontology/2.0/lexinfo#essiveCase -->

    <owl:Thing rdf:about="&lexinfo;essiveCase">
        <rdf:type rdf:resource="&lexinfo;Case"/>
        <rdf:type rdf:resource="&owl;NamedIndividual"/>
        <rdfs:label xml:lang="en">essive case</rdfs:label>
        <rdfs:label xml:lang="ru">изобразительный падеж</rdfs:label>        
        <rdfs:comment xml:lang="en">Case which expresses a state of being.</rdfs:comment>
        <rdfs:comment xml:lang="ru">Падеж, который выражает состояние.</rdfs:comment>
        <dc:creator>Francopoulo, Gil</dc:creator>
        <owl:versionInfo>1:0</owl:versionInfo>
        <dcr:datcat rdf:resource="http://www.isocat.org/datcat/DC-1281"/>
        <rdfs:isDefinedBy rdf:resource="http://www.lexinfo.net/ontology/2.0/lexinfo"/>
    </owl:Thing>
    


    <!-- http://www.lexinfo.net/ontology/2.0/lexinfo#exclamativeDeterminer -->

    <owl:Thing rdf:about="&lexinfo;exclamativeDeterminer">
        <rdf:type rdf:resource="&lexinfo;DeterminerPOS"/>
        <rdf:type rdf:resource="&lexinfo;PartOfSpeech"/>
        <rdf:type rdf:resource="&owl;NamedIndividual"/>
        <rdfs:label xml:lang="en">exclamative determiner</rdfs:label>
        <rdfs:label xml:lang="ru">восклицательный детерминант</rdfs:label>        
        <rdfs:comment xml:lang="en">Determiner expressing an emotional utterance and marked with a strong intonation.</rdfs:comment>
        <rdfs:comment xml:lang="ru">Детерминант, выражающий эмоциональное высказывание и отмеченный сильной интонацией.</rdfs:comment>
        <owl:versionInfo>1:0</owl:versionInfo>
        <dc:creator>Francopoulo, Gil</dc:creator>
        <dcr:datcat rdf:resource="http://www.isocat.org/datcat/DC-1284"/>
        <rdfs:isDefinedBy rdf:resource="http://www.lexinfo.net/ontology/2.0/lexinfo"/>
    </owl:Thing>
    


    <!-- http://www.lexinfo.net/ontology/2.0/lexinfo#exclamativePoint -->

    <owl:Thing rdf:about="&lexinfo;exclamativePoint">
        <rdf:type rdf:resource="&lexinfo;PartOfSpeech"/>
        <rdf:type rdf:resource="&lexinfo;SymbolPOS"/>
        <rdf:type rdf:resource="&owl;NamedIndividual"/>
        <rdfs:label xml:lang="en">exclamative point</rdfs:label>
        <rdfs:label xml:lang="ru">восклицательный знак</rdfs:label>        
        <owl:versionInfo>1:0</owl:versionInfo>
        <rdfs:comment xml:lang="en">Special sign (!) usually used in writing to mark exclamation.</rdfs:comment>
        <rdfs:comment xml:lang="ru">Специальный знак (!) Обычно используется в письменной форме, чтобы отметить восклицание.</rdfs:comment>
        <dc:creator>Francopoulo, Gil</dc:creator>
        <dcr:datcat rdf:resource="http://www.isocat.org/datcat/DC-1441"/>
        <rdfs:isDefinedBy rdf:resource="http://www.lexinfo.net/ontology/2.0/lexinfo"/>
    </owl:Thing>
    


    <!-- http://www.lexinfo.net/ontology/2.0/lexinfo#exclamativePronoun -->

    <owl:Thing rdf:about="&lexinfo;exclamativePronoun">
        <rdf:type rdf:resource="&lexinfo;PartOfSpeech"/>
        <rdf:type rdf:resource="&lexinfo;PronounPOS"/>
        <rdf:type rdf:resource="&owl;NamedIndividual"/>
        <rdfs:label xml:lang="en">exclamative pronoun</rdfs:label>
        <rdfs:label xml:lang="ru">восклицательное местоимение</rdfs:label>
        <owl:versionInfo>1:0</owl:versionInfo>
        <dc:creator>Francopoulo, Gil</dc:creator>
        <rdfs:comment xml:lang="en">Pronoun marked with an emotional utterance and/or a strong intonation.</rdfs:comment>
        <rdfs:comment xml:lang="ru">Местоимение, помеченное эмоциональным высказыванием и / или сильной интонацией.</rdfs:comment>        
        <dcr:datcat rdf:resource="http://www.isocat.org/datcat/DC-1285"/>
        <rdfs:isDefinedBy rdf:resource="http://www.lexinfo.net/ontology/2.0/lexinfo"/>
    </owl:Thing>
    


    <!-- http://www.lexinfo.net/ontology/2.0/lexinfo#existentialPronoun -->

    <owl:Thing rdf:about="&lexinfo;existentialPronoun">
        <rdf:type rdf:resource="&lexinfo;PartOfSpeech"/>
        <rdf:type rdf:resource="&lexinfo;PronounPOS"/>
        <rdf:type rdf:resource="&owl;NamedIndividual"/>
        <rdfs:label xml:lang="en">existential pronoun</rdfs:label>
        <rdfs:label xml:lang="ru">экзистенциальное местоимение</rdfs:label>        
        <owl:versionInfo>1:0</owl:versionInfo>
        <rdfs:comment xml:lang="en">pronoun that indicates the existence of something or someone</rdfs:comment>
        <rdfs:comment xml:lang="ru">Местоимение, которое указывает на существование чего-либо или кого-либо.</rdfs:comment>
        <dc:creator>Francopoulo, Gil</dc:creator>
        <dcr:datcat rdf:resource="http://www.isocat.org/datcat/DC-3012"/>
        <rdfs:isDefinedBy rdf:resource="http://www.lexinfo.net/ontology/2.0/lexinfo"/>
    </owl:Thing>
    


    <!-- http://www.lexinfo.net/ontology/2.0/lexinfo#expression -->

    <owl:Thing rdf:about="&lexinfo;expression">
        <rdf:type rdf:resource="&lexinfo;TermType"/>
        <rdf:type rdf:resource="&owl;NamedIndividual"/>
        <rdfs:label xml:lang="en">expression</rdfs:label>
        <rdfs:label xml:lang="ru">выражение</rdfs:label>
        <dc:creator>Wright, Sue Ellen</dc:creator>
        <owl:versionInfo>1:0</owl:versionInfo>
        <rdfs:comment xml:lang="en">A significant word or phrase.</rdfs:comment>
        <rdfs:comment xml:lang="ru">Знаменательное слово или словосочетание.</rdfs:comment>
        <dcr:datcat rdf:resource="http://www.isocat.org/datcat/DC-349"/>
        <rdfs:isDefinedBy rdf:resource="http://www.lexinfo.net/ontology/2.0/lexinfo"/>
    </owl:Thing>
    


    <!-- http://www.lexinfo.net/ontology/2.0/lexinfo#facetiousRegister -->

    <owl:Thing rdf:about="&lexinfo;facetiousRegister">
        <rdf:type rdf:resource="&lexinfo;Register"/>
        <rdf:type rdf:resource="&owl;NamedIndividual"/>
        <rdfs:isDefinedBy rdf:resource="http://www.lexinfo.net/ontology/2.0/lexinfo"/>
    </owl:Thing>
    


    <!-- http://www.lexinfo.net/ontology/2.0/lexinfo#feminine -->

    <owl:Thing rdf:about="&lexinfo;feminine">
        <rdf:type rdf:resource="&lexinfo;Gender"/>
        <rdf:type rdf:resource="&owl;NamedIndividual"/>
        <rdfs:label xml:lang="en">feminine</rdfs:label>
        <rdfs:label xml:lang="ru">женский</rdfs:label>        
        <dc:creator>Wright, Sue Ellen</dc:creator>
        <owl:versionInfo>1:0</owl:versionInfo>
        <dc:creator>Francopoulo, Gil</dc:creator>
        <rdfs:comment xml:lang="en">Of, relating to, or constituting the gender that ordinarily includes most words or grammatical forms referring to females.</rdfs:comment>
        <rdfs:comment xml:lang="ru">Об относящемся к полу или составляющем пол, который обычно включает большинство слов или грамматических форм, относящихся к женским особям.</rdfs:comment>
        <dcr:datcat rdf:resource="http://www.isocat.org/datcat/DC-1880"/>
        <dcr:datcat rdf:resource="http://www.isocat.org/datcat/DC-247"/>
        <rdfs:isDefinedBy rdf:resource="http://www.lexinfo.net/ontology/2.0/lexinfo"/>
    </owl:Thing>
    


    <!-- http://www.lexinfo.net/ontology/2.0/lexinfo#finite -->

    <owl:Thing rdf:about="&lexinfo;finite">
        <rdf:type rdf:resource="&lexinfo;Finiteness"/>
        <rdf:type rdf:resource="&owl;NamedIndividual"/>
        <rdfs:label xml:lang="en">finite</rdfs:label>
        <rdfs:label xml:lang="ru">спрягаемый</rdfs:label>        
        <owl:versionInfo>1:0</owl:versionInfo>
        <dc:creator>Francopoulo, Gil</dc:creator>
        <rdfs:comment xml:lang="en">Property applied to a verb form that can occur on its own in an independent sentence.</rdfs:comment>
        <rdfs:comment xml:lang="ru">Свойство, относящееся к форме глагола, которая может использоваться самостоятельно в предложении.</rdfs:comment>
        <dcr:datcat rdf:resource="http://www.isocat.org/datcat/DC-1287"/>
        <rdfs:isDefinedBy rdf:resource="http://www.lexinfo.net/ontology/2.0/lexinfo"/>
    </owl:Thing>
    


    <!-- http://www.lexinfo.net/ontology/2.0/lexinfo#firstPerson -->

    <owl:Thing rdf:about="&lexinfo;firstPerson">
        <rdf:type rdf:resource="&lexinfo;Person"/>
        <rdf:type rdf:resource="&owl;NamedIndividual"/>
        <rdfs:label xml:lang="en">first person</rdfs:label>
        <rdfs:label xml:lang="ru">первое лицо</rdfs:label>        
        <owl:versionInfo>1:0</owl:versionInfo>
        <dc:creator>Francopoulo, Gil</dc:creator>
        <rdfs:comment xml:lang="en">First person deixis is deictic reference that refers to the speaker, or both the speaker and referents grouped with the speaker</rdfs:comment>
        <rdfs:comment xml:lang="ru">Дейксис первого лица указывает непосредственно на говорящего или на говорящего и референтов, объединенных с говорящим.</rdfs:comment>
        <dcr:datcat rdf:resource="http://www.isocat.org/datcat/DC-1288"/>
        <rdfs:isDefinedBy rdf:resource="http://www.lexinfo.net/ontology/2.0/lexinfo"/>
    </owl:Thing>
    


    <!-- http://www.lexinfo.net/ontology/2.0/lexinfo#formalRegister -->

    <owl:Thing rdf:about="&lexinfo;formalRegister">
        <rdf:type rdf:resource="&lexinfo;Register"/>
        <rdf:type rdf:resource="&owl;NamedIndividual"/>
        <rdfs:isDefinedBy rdf:resource="http://www.lexinfo.net/ontology/2.0/lexinfo"/>
    </owl:Thing>
    


    <!-- http://www.lexinfo.net/ontology/2.0/lexinfo#formula -->

    <owl:Thing rdf:about="&lexinfo;formula">
        <rdf:type rdf:resource="&lexinfo;TermType"/>
        <rdf:type rdf:resource="&owl;NamedIndividual"/>
        <rdfs:label xml:lang="en">formula</rdfs:label>
        <rdfs:label xml:lang="ru">формула</rdfs:label>        
        <owl:versionInfo>1:0</owl:versionInfo>
        <dc:creator>Wright, Sue Ellen</dc:creator>
        <dc:creator>Francopoulo, Gil</dc:creator>
        <rdfs:comment xml:lang="en">Figures, symbols or the like used to express a concept briefly, such as a mathematical or chemical formula.</rdfs:comment>
        <rdfs:comment xml:lang="ru">Цифры, символы и другие подобные знаки, используемые для краткого выражения понятия, такого как математическая или химическая формула.</rdfs:comment>
        <dcr:datcat rdf:resource="http://www.isocat.org/datcat/DC-1888"/>
        <dcr:datcat rdf:resource="http://www.isocat.org/datcat/DC-325"/>
        <rdfs:isDefinedBy rdf:resource="http://www.lexinfo.net/ontology/2.0/lexinfo"/>
    </owl:Thing>
    


    <!-- http://www.lexinfo.net/ontology/2.0/lexinfo#fullArticle -->

    <owl:Thing rdf:about="&lexinfo;fullArticle">
        <rdf:type rdf:resource="&lexinfo;Definiteness"/>
        <rdf:type rdf:resource="&owl;NamedIndividual"/>
        <rdfs:label xml:lang="en">full article</rdfs:label>
        <rdfs:label xml:lang="ru">полный артикль</rdfs:label>        
        <rdfs:comment xml:lang="en">For definiteness, when a specific form is the syntactic subject of the clause.</rdfs:comment>
        <rdfs:comment xml:lang="ru">Для определенности, когда конкретная форма является синтаксическим субъектом предложения.</rdfs:comment>
        <owl:versionInfo>1:0</owl:versionInfo>
        <dc:creator>Francopoulo, Gil</dc:creator>
        <dcr:datcat rdf:resource="http://www.isocat.org/datcat/DC-1928"/>
        <rdfs:isDefinedBy rdf:resource="http://www.lexinfo.net/ontology/2.0/lexinfo"/>
    </owl:Thing>
    


    <!-- http://www.lexinfo.net/ontology/2.0/lexinfo#fullForm -->

    <owl:Thing rdf:about="&lexinfo;fullForm">
        <rdf:type rdf:resource="&lexinfo;TermType"/>
        <rdf:type rdf:resource="&owl;NamedIndividual"/>
        <rdfs:label xml:lang="en">full form</rdfs:label>
        <rdfs:label xml:lang="ru">полная форма</rdfs:label>        
        <owl:versionInfo>1:0</owl:versionInfo>
        <rdfs:comment xml:lang="en">The complete presentation of a term or lexeme for which there is an abbreviated form.</rdfs:comment>
        <rdfs:comment xml:lang="ru">Полное представление термина или лексемы, для которых имеется сокращенная форма.</rdfs:comment>
        <dc:creator>Wright, Sue Ellen</dc:creator>
        <dcr:datcat rdf:resource="http://www.isocat.org/datcat/DC-321"/>
        <rdfs:isDefinedBy rdf:resource="http://www.lexinfo.net/ontology/2.0/lexinfo"/>
    </owl:Thing>
    


    <!-- http://www.lexinfo.net/ontology/2.0/lexinfo#fusedPreposition -->

    <owl:Thing rdf:about="&lexinfo;fusedPreposition">
        <rdf:type rdf:resource="&lexinfo;FusedPrepositionPOS"/>
        <rdf:type rdf:resource="&lexinfo;PartOfSpeech"/>
        <rdf:type rdf:resource="&owl;NamedIndividual"/>
        <rdfs:label xml:lang="en">fused preposition</rdfs:label>
        <rdfs:label xml:lang="ru">слитный предлог</rdfs:label>        
        <owl:versionInfo>1:0</owl:versionInfo>
        <dc:creator>Francopoulo, Gil</dc:creator>
        <rdfs:comment xml:lang="en">Preposition that is the result of a morphological merge from at least two words.</rdfs:comment>
        <rdfs:comment xml:lang="ru">Предлог, являющийся результатом морфологического слияния, по меньшей мере, двух слов.</rdfs:comment>
        <dcr:datcat rdf:resource="http://www.isocat.org/datcat/DC-1901"/>
        <rdfs:isDefinedBy rdf:resource="http://www.lexinfo.net/ontology/2.0/lexinfo"/>
    </owl:Thing>
    


    <!-- http://www.lexinfo.net/ontology/2.0/lexinfo#fusedPrepositionDeterminer -->

    <owl:Thing rdf:about="&lexinfo;fusedPrepositionDeterminer">
        <rdf:type rdf:resource="&lexinfo;FusedPrepositionPOS"/>
        <rdf:type rdf:resource="&lexinfo;PartOfSpeech"/>
        <rdf:type rdf:resource="&owl;NamedIndividual"/>
        <rdfs:label xml:lang="en">fused preposition determiner</rdfs:label>
        <rdfs:label xml:lang="ru">определитель слитного предлога</rdfs:label>
        <rdfs:comment xml:lang="en">word resulting from the aggregation of a proposition and a determiner</rdfs:comment>
        <rdfs:comment xml:lang="ru">Слово, образующееся в результате сращения предлога и определителя.</rdfs:comment>
        <dc:creator>Francopoulo, Gil</dc:creator>
        <owl:versionInfo>1:0</owl:versionInfo>
        <dcr:datcat rdf:resource="http://www.isocat.org/datcat/DC-3010"/>
        <rdfs:isDefinedBy rdf:resource="http://www.lexinfo.net/ontology/2.0/lexinfo"/>
    </owl:Thing>
    


    <!-- http://www.lexinfo.net/ontology/2.0/lexinfo#fusedPrepositionPronoun -->

    <owl:Thing rdf:about="&lexinfo;fusedPrepositionPronoun">
        <rdf:type rdf:resource="&lexinfo;FusedPrepositionPOS"/>
        <rdf:type rdf:resource="&lexinfo;PartOfSpeech"/>
        <rdf:type rdf:resource="&owl;NamedIndividual"/>
        <rdfs:label xml:lang="en">fused preposition pronoun</rdfs:label>
        <rdfs:label xml:lang="ru">местоимение слитного предлога</rdfs:label>        
        <owl:versionInfo>1:0</owl:versionInfo>
        <dc:creator>Francopoulo, Gil</dc:creator>
        <rdfs:comment xml:lang="en">word resulting from the aggregation of a preposition and a pronoun</rdfs:comment>
        <rdfs:comment xml:lang="ru">Слово, образующееся в результате сращения предлога и местоимения.</rdfs:comment>
        <dcr:datcat rdf:resource="http://www.isocat.org/datcat/DC-3009"/>
        <rdfs:isDefinedBy rdf:resource="http://www.lexinfo.net/ontology/2.0/lexinfo"/>
    </owl:Thing>
    


    <!-- http://www.lexinfo.net/ontology/2.0/lexinfo#fusedPronounAuxiliary -->

    <owl:Thing rdf:about="&lexinfo;fusedPronounAuxiliary">
        <rdf:type rdf:resource="&lexinfo;PartOfSpeech"/>
        <rdf:type rdf:resource="&lexinfo;PronounPOS"/>
        <rdf:type rdf:resource="&owl;NamedIndividual"/>
        <rdfs:label xml:lang="en">fused pronoun auxiliary</rdfs:label>
        <rdfs:label xml:lang="ru">вспомогательный глагол с местоимением</rdfs:label>        
        <owl:versionInfo>1:0</owl:versionInfo>
        <rdfs:comment xml:lang="en">word resulting from the aggregation of a pronoun and an auxiliary</rdfs:comment>
        <rdfs:comment xml:lang="ru">Слово, появляющееся в результате сращения местоимения и вспомогательного глагола</rdfs:comment>
        <dc:creator>Francopoulo, Gil</dc:creator>
        <dcr:datcat rdf:resource="http://www.isocat.org/datcat/DC-3008"/>
        <rdfs:isDefinedBy rdf:resource="http://www.lexinfo.net/ontology/2.0/lexinfo"/>
    </owl:Thing>
    


    <!-- http://www.lexinfo.net/ontology/2.0/lexinfo#future -->

    <owl:Thing rdf:about="&lexinfo;future">
        <rdf:type rdf:resource="&lexinfo;Tense"/>
        <rdf:type rdf:resource="&owl;NamedIndividual"/>
        <rdfs:label xml:lang="en">future</rdfs:label>
        <rdfs:label xml:lang="ru">будущее</rdfs:label>        
        <rdfs:comment xml:lang="en">Verb tense that indicates action or state of being in the future.</rdfs:comment>
        <rdfs:comment xml:lang="ru">Глагольное время, которое указывает на действие или состояние в будущем.</rdfs:comment>
        <owl:versionInfo>1:0</owl:versionInfo>
        <dc:creator>Francopoulo, Gil</dc:creator>
        <dcr:datcat rdf:resource="http://www.isocat.org/datcat/DC-1291"/>
        <rdfs:isDefinedBy rdf:resource="http://www.lexinfo.net/ontology/2.0/lexinfo"/>
    </owl:Thing>
    


    <!-- http://www.lexinfo.net/ontology/2.0/lexinfo#futureParticle -->

    <owl:Thing rdf:about="&lexinfo;futureParticle">
        <rdf:type rdf:resource="&lexinfo;PartOfSpeech"/>
        <rdf:type rdf:resource="&lexinfo;ParticlePOS"/>
        <rdf:type rdf:resource="&owl;NamedIndividual"/>
        <rdfs:label xml:lang="en">future particle</rdfs:label>
        <rdfs:label xml:lang="ru">частица будущего времени</rdfs:label>        
        <rdfs:comment xml:lang="en">Particle used in order to express future.</rdfs:comment>
        <rdfs:comment xml:lang="ru">Частица используется для выражения будущего времени.</rdfs:comment>
        <dc:creator>Francopoulo, Gil</dc:creator>
        <owl:versionInfo>1:0</owl:versionInfo>
        <dcr:datcat rdf:resource="http://www.isocat.org/datcat/DC-1919"/>
        <rdfs:isDefinedBy rdf:resource="http://www.lexinfo.net/ontology/2.0/lexinfo"/>
    </owl:Thing>
    


    <!-- http://www.lexinfo.net/ontology/2.0/lexinfo#generalAdverb -->

    <owl:Thing rdf:about="&lexinfo;generalAdverb">
        <rdf:type rdf:resource="&lexinfo;AdverbPOS"/>
        <rdf:type rdf:resource="&lexinfo;PartOfSpeech"/>
        <rdf:type rdf:resource="&owl;NamedIndividual"/>
        <rdfs:label xml:lang="en">general adverb</rdfs:label>
        <rdfs:label xml:lang="ru">общее наречие</rdfs:label>        
        <owl:versionInfo>1:0</owl:versionInfo>
        <rdfs:comment xml:lang="en">Adverb belonging to the general class of adverbs</rdfs:comment>
        <rdfs:comment xml:lang="ru">Наречие, принадлежащее к общему классу наречий</rdfs:comment>
        <dc:creator>Francopoulo, Gil</dc:creator>
        <dcr:datcat rdf:resource="http://www.isocat.org/datcat/DC-1435"/>
        <rdfs:isDefinedBy rdf:resource="http://www.lexinfo.net/ontology/2.0/lexinfo"/>
    </owl:Thing>
    


    <!-- http://www.lexinfo.net/ontology/2.0/lexinfo#generalizationWord -->

    <owl:Thing rdf:about="&lexinfo;generalizationWord">
        <rdf:type rdf:resource="&lexinfo;PartOfSpeech"/>
        <rdf:type rdf:resource="&owl;NamedIndividual"/>
        <rdfs:label xml:lang="en">generalization word</rdfs:label>
        <rdfs:label xml:lang="ru">обобщающее слово</rdfs:label>        
        <owl:versionInfo>1:0</owl:versionInfo>
        <dc:creator>Zeman, Dan</dc:creator>
        <rdfs:comment xml:lang="en">A word that does not carry its own meaning but generalizes the meaning of a neighboring word, adding the &amp;quot;etc.&amp;quot; sense.</rdfs:comment>
        <rdfs:comment xml:lang="ru">Слово, которое не имеет своего значения, но обобщает значение соседнего слова, добавляя значение &amp;quot;и т.д.&amp;quot;.</rdfs:comment>
        <dcr:datcat rdf:resource="http://www.isocat.org/datcat/DC-3033"/>
        <rdfs:isDefinedBy rdf:resource="http://www.lexinfo.net/ontology/2.0/lexinfo"/>
    </owl:Thing>
    


    <!-- http://www.lexinfo.net/ontology/2.0/lexinfo#genericNumeral -->

    <owl:Thing rdf:about="&lexinfo;genericNumeral">
        <rdf:type rdf:resource="&lexinfo;NumeralPOS"/>
        <rdf:type rdf:resource="&lexinfo;PartOfSpeech"/>
        <rdf:type rdf:resource="&owl;NamedIndividual"/>
        <rdfs:label xml:lang="en">generic numeral</rdfs:label>
        <rdfs:label xml:lang="ru">обобщённое числительное</rdfs:label>        
        <owl:versionInfo>1:0</owl:versionInfo>
        <rdfs:comment xml:lang="en">A numeral used to indicate the number of sets/kinds of objects.</rdfs:comment>
        <rdfs:comment xml:lang="ru">Числительное, используемое для указания количества групп/видов объектов.</rdfs:comment>        
        <dc:creator>Zeman, Dan</dc:creator>
        <dcr:datcat rdf:resource="http://www.isocat.org/datcat/DC-3022"/>
        <rdfs:isDefinedBy rdf:resource="http://www.lexinfo.net/ontology/2.0/lexinfo"/>
    </owl:Thing>
    


    <!-- http://www.lexinfo.net/ontology/2.0/lexinfo#genitiveCase -->

    <owl:Thing rdf:about="&lexinfo;genitiveCase">
        <rdf:type rdf:resource="&lexinfo;Case"/>
        <rdf:type rdf:resource="&owl;NamedIndividual"/>
        <rdfs:label xml:lang="en">genitive case</rdfs:label>
        <rdfs:label xml:lang="ru">родительный падеж</rdfs:label>        
        <rdfs:comment xml:lang="en">Case which expresses a possessive relationship (e.g. the boy&apos;s book) or some other similarly close connection (e.g. a summer&apos;s day).</rdfs:comment>
        <rdfs:comment xml:lang="ru">Падеж, который выражает  отношение обладания (например, книга мальчика) или другую аналогичную близкую связь (например, летний день).</rdfs:comment>
        <owl:versionInfo>1:0</owl:versionInfo>
        <dc:creator>Francopoulo, Gil</dc:creator>
        <dcr:datcat rdf:resource="http://www.isocat.org/datcat/DC-1293"/>
        <rdfs:isDefinedBy rdf:resource="http://www.lexinfo.net/ontology/2.0/lexinfo"/>
    </owl:Thing>
    


    <!-- http://www.lexinfo.net/ontology/2.0/lexinfo#gerundive -->

    <owl:Thing rdf:about="&lexinfo;gerundive">
        <rdf:type rdf:resource="&lexinfo;VerbFormMood"/>
        <rdf:type rdf:resource="&owl;NamedIndividual"/>
        <rdfs:isDefinedBy rdf:resource="http://www.lexinfo.net/ontology/2.0/lexinfo"/>
    </owl:Thing>
    


    <!-- http://www.lexinfo.net/ontology/2.0/lexinfo#idiom -->

    <owl:Thing rdf:about="&lexinfo;idiom">
        <rdf:type rdf:resource="&lexinfo;TermType"/>
        <rdf:type rdf:resource="&owl;NamedIndividual"/>
        <rdfs:label xml:lang="en">idiom</rdfs:label>
        <rdfs:label xml:lang="ru">идиома</rdfs:label>        
        <rdfs:comment xml:lang="en">A group of words in a fixed order that have a particular meaning that is different from the meanings of each word understood on its own.</rdfs:comment>
        <rdfs:comment xml:lang="ru">Группа слов в фиксированном порядке, которая имеет особое значение, отличное от значений каждого слова, понимаемого отдельно.</rdfs:comment>
        <dc:creator>Wright, Sue Ellen</dc:creator>
        <owl:versionInfo>1:0</owl:versionInfo>
        <dcr:datcat rdf:resource="http://www.isocat.org/datcat/DC-351"/>
        <rdfs:isDefinedBy rdf:resource="http://www.lexinfo.net/ontology/2.0/lexinfo"/>
    </owl:Thing>
    


    <!-- http://www.lexinfo.net/ontology/2.0/lexinfo#illativeCase -->

    <owl:Thing rdf:about="&lexinfo;illativeCase">
        <rdf:type rdf:resource="&lexinfo;Case"/>
        <rdf:type rdf:resource="&owl;NamedIndividual"/>
        <rdfs:label xml:lang="en">illative case</rdfs:label>
        <rdfs:label xml:lang="ru">следственный падеж</rdfs:label>        
        <rdfs:comment xml:lang="en">Case which expresses the meaning of &apos;motion into&apos; or &apos;direction towards&apos; the referent of the noun it marks.</rdfs:comment>
        <rdfs:comment xml:lang="ru">Падеж, который выражает значение &apos;движение в&apos; или &apos;направление к&apos; референта обозначаемого им существительного.</rdfs:comment>
        <owl:versionInfo>1:0</owl:versionInfo>
        <dc:creator>Francopoulo, Gil</dc:creator>
        <dcr:datcat rdf:resource="http://www.isocat.org/datcat/DC-1303"/>
        <rdfs:isDefinedBy rdf:resource="http://www.lexinfo.net/ontology/2.0/lexinfo"/>
    </owl:Thing>
    


    <!-- http://www.lexinfo.net/ontology/2.0/lexinfo#imperative -->

    <owl:Thing rdf:about="&lexinfo;imperative">
        <rdf:type rdf:resource="&lexinfo;Mood"/>
        <rdf:type rdf:resource="&lexinfo;VerbFormMood"/>
        <rdf:type rdf:resource="&owl;NamedIndividual"/>
        <rdfs:label xml:lang="en">imperative</rdfs:label>
        <rdfs:label xml:lang="ru">повелительное</rdfs:label>        
        <dc:creator>Wright, Sue Ellen</dc:creator>
        <rdfs:comment>...</rdfs:comment>
        <owl:versionInfo>1:0</owl:versionInfo>
        <rdfs:comment xml:lang="en">Mood used to express an order.</rdfs:comment>
        <rdfs:comment xml:lang="ru">Наклонение, которое используется для выражения приказа.</rdfs:comment>        
        <dc:creator>Francopoulo, Gil</dc:creator>
        <dcr:datcat rdf:resource="http://www.isocat.org/datcat/DC-1844"/>
        <dcr:datcat rdf:resource="http://www.isocat.org/datcat/DC-369"/>
        <rdfs:isDefinedBy rdf:resource="http://www.lexinfo.net/ontology/2.0/lexinfo"/>
    </owl:Thing>
    


    <!-- http://www.lexinfo.net/ontology/2.0/lexinfo#imperfect -->

    <owl:Thing rdf:about="&lexinfo;imperfect">
        <rdf:type rdf:resource="&lexinfo;Tense"/>
        <rdf:type rdf:resource="&owl;NamedIndividual"/>
        <rdfs:label xml:lang="en">imperfect</rdfs:label>
        <rdfs:label xml:lang="ru">имперфектное</rdfs:label>        
        <rdfs:comment xml:lang="en">Verb tense that refers to action in the past that is incomplete or ongoing.</rdfs:comment>
        <rdfs:comment xml:lang="ru">Время глагола, относящееся к действию в прошлом, которое является незавершенным или продолжающимся.</rdfs:comment>
        <dc:creator>Francopoulo, Gil</dc:creator>
        <owl:versionInfo>1:0</owl:versionInfo>
        <dcr:datcat rdf:resource="http://www.isocat.org/datcat/DC-1304"/>
        <rdfs:isDefinedBy rdf:resource="http://www.lexinfo.net/ontology/2.0/lexinfo"/>
    </owl:Thing>
    


    <!-- http://www.lexinfo.net/ontology/2.0/lexinfo#imperfective -->

    <owl:Thing rdf:about="&lexinfo;imperfective">
        <rdf:type rdf:resource="&lexinfo;Aspect"/>
        <rdf:type rdf:resource="&owl;NamedIndividual"/>
        <rdfs:label xml:lang="en">imperfective</rdfs:label>
        <rdfs:label xml:lang="ru">несовершенный</rdfs:label>        
        <dc:creator>Francopoulo, Gil</dc:creator>
        <owl:versionInfo>1:0</owl:versionInfo>
        <rdfs:comment xml:lang="en">Imperfective aspect is an aspect that expresses an event or state, with respect to its internal structure, instead of expressing it as a simple whole.</rdfs:comment>
        <rdfs:comment xml:lang="ru">Несовершенный вид - это вид, который выражает событие или состояние по отношению к его внутренней структуре, а не выражает его как простое целое.</rdfs:comment>
        <dcr:datcat rdf:resource="http://www.isocat.org/datcat/DC-1305"/>
        <rdfs:isDefinedBy rdf:resource="http://www.lexinfo.net/ontology/2.0/lexinfo"/>
    </owl:Thing>
    


    <!-- http://www.lexinfo.net/ontology/2.0/lexinfo#impersonalPronoun -->

    <owl:Thing rdf:about="&lexinfo;impersonalPronoun">
        <rdf:type rdf:resource="&lexinfo;PartOfSpeech"/>
        <rdf:type rdf:resource="&lexinfo;PronounPOS"/>
        <rdf:type rdf:resource="&owl;NamedIndividual"/>
        <rdfs:label xml:lang="en">impersonal pronoun</rdfs:label>
        <rdfs:label xml:lang="ru">безличное местоимение</rdfs:label>        
        <owl:versionInfo>1:0</owl:versionInfo>
        <dc:creator>Francopoulo, Gil</dc:creator>
        <rdfs:comment xml:lang="en">Pronoun lacking person referent.</rdfs:comment>
        <rdfs:comment xml:lang="ru">Местоимение, в котором отсутствует указание на лицо.</rdfs:comment>
        <dcr:datcat rdf:resource="http://www.isocat.org/datcat/DC-1426"/>
        <rdfs:isDefinedBy rdf:resource="http://www.lexinfo.net/ontology/2.0/lexinfo"/>
    </owl:Thing>
    


    <!-- http://www.lexinfo.net/ontology/2.0/lexinfo#inHouseRegister -->

    <owl:Thing rdf:about="&lexinfo;inHouseRegister">
        <rdf:type rdf:resource="&lexinfo;Register"/>
        <rdf:type rdf:resource="&owl;NamedIndividual"/>
        <rdfs:label xml:lang="en">in house register</rdfs:label>
        <rdfs:label xml:lang="ru">внутренний реестр</rdfs:label>        
        <owl:versionInfo>1:0</owl:versionInfo>
        <dc:creator>Francopoulo, Gil</dc:creator>
        <rdfs:comment xml:lang="en">The register of terms that are company-specific and not readily recognized outside this environment.</rdfs:comment>
        <rdfs:comment xml:lang="ru">Реестр терминов, которые являются специфичными для компании и не легко узнаваемы вне этой среды.</rdfs:comment>
        <dc:creator>Wright, Sue Ellen</dc:creator>
        <rdfs:comment xml:lang="en">Register of terms that are company-specific and not readily recognized outside this environment.</rdfs:comment>
        <rdfs:comment xml:lang="ru">Реестр терминов, которые являются специфичными для компании и не легко узнаваемы вне этой среды.</rdfs:comment>
        <dcr:datcat rdf:resource="http://www.isocat.org/datcat/DC-1993"/>
        <dcr:datcat rdf:resource="http://www.isocat.org/datcat/DC-426"/>
        <rdfs:isDefinedBy rdf:resource="http://www.lexinfo.net/ontology/2.0/lexinfo"/>
    </owl:Thing>
    


    <!-- http://www.lexinfo.net/ontology/2.0/lexinfo#inanimate -->

    <owl:Thing rdf:about="&lexinfo;inanimate">
        <rdf:type rdf:resource="&lexinfo;Animacy"/>
        <rdf:type rdf:resource="&owl;NamedIndividual"/>
        <rdfs:label xml:lang="en">inanimate</rdfs:label>
        <rdfs:label xml:lang="ru">неодушевлённый</rdfs:label>        
        <dc:creator>Francopoulo, Gil</dc:creator>
        <owl:versionInfo>1:0</owl:versionInfo>
        <dc:creator>Wright, Sue Ellen</dc:creator>
        <rdfs:comment xml:lang="en">Perceived as not living.</rdfs:comment>
        <rdfs:comment xml:lang="ru">Воспринимается как неживой.</rdfs:comment>
        <dcr:datcat rdf:resource="http://www.isocat.org/datcat/DC-1952"/>
        <dcr:datcat rdf:resource="http://www.isocat.org/datcat/DC-80"/>
        <rdfs:isDefinedBy rdf:resource="http://www.lexinfo.net/ontology/2.0/lexinfo"/>
    </owl:Thing>
    


    <!-- http://www.lexinfo.net/ontology/2.0/lexinfo#inchoative -->

    <owl:Thing rdf:about="&lexinfo;inchoative">
        <rdf:type rdf:resource="&lexinfo;Aspect"/>
        <rdf:type rdf:resource="&owl;NamedIndividual"/>
        <rdfs:label xml:lang="en">inchoative</rdfs:label>
        <rdfs:label xml:lang="ru">начинательный</rdfs:label>        
        <rdfs:comment xml:lang="en">Aspect that expresses the beginning of an event or state.</rdfs:comment>
        <rdfs:comment xml:lang="ru">Вид, который выражает начало события или состояния.</rdfs:comment>
        <dc:creator>Francopoulo, Gil</dc:creator>
        <owl:versionInfo>1:0</owl:versionInfo>
        <dcr:datcat rdf:resource="http://www.isocat.org/datcat/DC-2002"/>
        <rdfs:isDefinedBy rdf:resource="http://www.lexinfo.net/ontology/2.0/lexinfo"/>
    </owl:Thing>
    


    <!-- http://www.lexinfo.net/ontology/2.0/lexinfo#indefinite -->

    <owl:Thing rdf:about="&lexinfo;indefinite">
        <rdf:type rdf:resource="&lexinfo;Definiteness"/>
        <rdf:type rdf:resource="&owl;NamedIndividual"/>
        <rdfs:label xml:lang="en">indefinite</rdfs:label>
        <rdfs:label xml:lang="ru">неопределенный</rdfs:label>        
        <dc:creator>Francopoulo, Gil</dc:creator>
        <owl:versionInfo>1:0</owl:versionInfo>
        <rdfs:comment xml:lang="en">Value related to an entity in a situation where the identification of this entity is not clear cut.</rdfs:comment>
        <rdfs:comment xml:lang="ru">Значение, связанное с объектом в ситуации, когда идентификация этого объекта нечёткая.</rdfs:comment>
        <dcr:datcat rdf:resource="http://www.isocat.org/datcat/DC-2005"/>
        <rdfs:isDefinedBy rdf:resource="http://www.lexinfo.net/ontology/2.0/lexinfo"/>
    </owl:Thing>
    


    <!-- http://www.lexinfo.net/ontology/2.0/lexinfo#indefiniteArticle -->

    <owl:Thing rdf:about="&lexinfo;indefiniteArticle">
        <rdf:type rdf:resource="&lexinfo;DeterminerPOS"/>
        <rdf:type rdf:resource="&lexinfo;PartOfSpeech"/>
        <rdf:type rdf:resource="&owl;NamedIndividual"/>
        <rdfs:label xml:lang="en">indefinite article</rdfs:label>
        <rdfs:label xml:lang="ru">неопределенный артикль</rdfs:label>        
        <rdfs:comment xml:lang="en">Article not capable of expressing identification.</rdfs:comment>
        <rdfs:comment xml:lang="ru">Артикль, не способный выражать идентификацию.</rdfs:comment>
        <dc:creator>Francopoulo, Gil</dc:creator>
        <owl:versionInfo>1:0</owl:versionInfo>
        <dcr:datcat rdf:resource="http://www.isocat.org/datcat/DC-1308"/>
        <rdfs:isDefinedBy rdf:resource="http://www.lexinfo.net/ontology/2.0/lexinfo"/>
    </owl:Thing>
    


    <!-- http://www.lexinfo.net/ontology/2.0/lexinfo#indefiniteCardinalNumeral -->

    <owl:Thing rdf:about="&lexinfo;indefiniteCardinalNumeral">
        <rdf:type rdf:resource="&lexinfo;NumeralPOS"/>
        <rdf:type rdf:resource="&lexinfo;PartOfSpeech"/>
        <rdf:type rdf:resource="&owl;NamedIndividual"/>
        <rdfs:label xml:lang="en">indefinite cardinal numeral</rdfs:label>
        <rdfs:label xml:lang="ru">неопределённое количественное числительное</rdfs:label>
        <dc:creator>Zeman, Dan</dc:creator>
        <rdfs:comment xml:lang="en">A word used to express imprecise quantity.</rdfs:comment>
        <rdfs:comment xml:lang="ru">Слово, используемое для выражения неточного количества.</rdfs:comment>
        <owl:versionInfo>1:0</owl:versionInfo>
        <dcr:datcat rdf:resource="http://www.isocat.org/datcat/DC-3023"/>
        <rdfs:isDefinedBy rdf:resource="http://www.lexinfo.net/ontology/2.0/lexinfo"/>
    </owl:Thing>
    


    <!-- http://www.lexinfo.net/ontology/2.0/lexinfo#indefiniteDeterminer -->

    <owl:Thing rdf:about="&lexinfo;indefiniteDeterminer">
        <rdf:type rdf:resource="&lexinfo;DeterminerPOS"/>
        <rdf:type rdf:resource="&lexinfo;PartOfSpeech"/>
        <rdf:type rdf:resource="&owl;NamedIndividual"/>
        <rdfs:label xml:lang="en">indefinite determiner</rdfs:label>
        <rdfs:label xml:lang="ru">неопределенный определитель</rdfs:label>        
        <dc:creator>Francopoulo, Gil</dc:creator>
        <rdfs:comment xml:lang="en">Determiner not capable of identification.</rdfs:comment>
        <rdfs:comment xml:lang="ru">Определитель не способный идентифицировать.</rdfs:comment>
        <owl:versionInfo>1:0</owl:versionInfo>
        <dcr:datcat rdf:resource="http://www.isocat.org/datcat/DC-1307"/>
        <rdfs:isDefinedBy rdf:resource="http://www.lexinfo.net/ontology/2.0/lexinfo"/>
    </owl:Thing>
    


    <!-- http://www.lexinfo.net/ontology/2.0/lexinfo#indefiniteMultiplicativeNumeral -->

    <owl:Thing rdf:about="&lexinfo;indefiniteMultiplicativeNumeral">
        <rdf:type rdf:resource="&lexinfo;NumeralPOS"/>
        <rdf:type rdf:resource="&lexinfo;PartOfSpeech"/>
        <rdf:type rdf:resource="&owl;NamedIndividual"/>
        <rdfs:label xml:lang="en">indefinite multiplicative numeral</rdfs:label>
        <rdfs:label xml:lang="ru">неопределённое множественное числительное</rdfs:label>
        <dc:creator>Zeman, Dan</dc:creator>
        <rdfs:comment xml:lang="en">A word indicating imprecise number of times something happened.</rdfs:comment>
        <rdfs:comment xml:lang="ru">Слово, указывающее на то, что действие произошло неточное количество раз.</rdfs:comment>
        <owl:versionInfo>1:0</owl:versionInfo>
        <dcr:datcat rdf:resource="http://www.isocat.org/datcat/DC-3024"/>
        <rdfs:isDefinedBy rdf:resource="http://www.lexinfo.net/ontology/2.0/lexinfo"/>
    </owl:Thing>
    


    <!-- http://www.lexinfo.net/ontology/2.0/lexinfo#indefiniteOrdinalNumeral -->

    <owl:Thing rdf:about="&lexinfo;indefiniteOrdinalNumeral">
        <rdf:type rdf:resource="&lexinfo;NumeralPOS"/>
        <rdf:type rdf:resource="&lexinfo;PartOfSpeech"/>
        <rdf:type rdf:resource="&owl;NamedIndividual"/>
        <rdfs:label xml:lang="en">indefinite ordinal numeral</rdfs:label>
        <rdfs:label xml:lang="ru">неопределённое порядковое числительное</rdfs:label>        
        <rdfs:comment xml:lang="en">A word used to indicate imprecise rank of an object in a sequence.</rdfs:comment>
        <rdfs:comment xml:lang="ru">Слово, используемое для указания неточной порядкового номера объекта в последовательности.</rdfs:comment>
        <dc:creator>Zeman, Dan</dc:creator>
        <owl:versionInfo>1:0</owl:versionInfo>
        <dcr:datcat rdf:resource="http://www.isocat.org/datcat/DC-3025"/>
        <rdfs:isDefinedBy rdf:resource="http://www.lexinfo.net/ontology/2.0/lexinfo"/>
    </owl:Thing>
    


    <!-- http://www.lexinfo.net/ontology/2.0/lexinfo#indefinitePronoun -->

    <owl:Thing rdf:about="&lexinfo;indefinitePronoun">
        <rdf:type rdf:resource="&lexinfo;PartOfSpeech"/>
        <rdf:type rdf:resource="&lexinfo;PronounPOS"/>
        <rdf:type rdf:resource="&owl;NamedIndividual"/>
        <rdfs:label xml:lang="en">indefinite pronoun</rdfs:label>
        <rdfs:label xml:lang="ru">неопределённое местоимение</rdfs:label>        
        <owl:versionInfo>1:0</owl:versionInfo>
        <rdfs:comment xml:lang="en">Pronoun that does not allow reference.</rdfs:comment>
        <rdfs:comment xml:lang="ru">Местоимение, которое не имеет указания.</rdfs:comment>
        <dc:creator>Francopoulo, Gil</dc:creator>
        <dcr:datcat rdf:resource="http://www.isocat.org/datcat/DC-1309"/>
        <rdfs:isDefinedBy rdf:resource="http://www.lexinfo.net/ontology/2.0/lexinfo"/>
    </owl:Thing>
    


    <!-- http://www.lexinfo.net/ontology/2.0/lexinfo#indicative -->

    <owl:Thing rdf:about="&lexinfo;indicative">
        <rdf:type rdf:resource="&lexinfo;Mood"/>
        <rdf:type rdf:resource="&lexinfo;VerbFormMood"/>
        <rdf:type rdf:resource="&owl;NamedIndividual"/>
        <rdfs:label xml:lang="en">indicative</rdfs:label>
        <rdfs:label xml:lang="ru">изъявительное</rdfs:label>        
        <dc:creator>Wright, Sue Ellen</dc:creator>
        <rdfs:comment>...</rdfs:comment>
        <dc:creator>Francopoulo, Gil</dc:creator>
        <rdfs:comment xml:lang="en">Mood value used in the expression of statements and questions.</rdfs:comment>
        <rdfs:comment xml:lang="ru">Наклонение, используемое для выражения утверждений и вопросов.</rdfs:comment>
        <owl:versionInfo>1:0</owl:versionInfo>
        <dcr:datcat rdf:resource="http://www.isocat.org/datcat/DC-1885"/>
        <dcr:datcat rdf:resource="http://www.isocat.org/datcat/DC-367"/>
        <rdfs:isDefinedBy rdf:resource="http://www.lexinfo.net/ontology/2.0/lexinfo"/>
    </owl:Thing>
    


    <!-- http://www.lexinfo.net/ontology/2.0/lexinfo#indifferent -->

    <owl:Thing rdf:about="&lexinfo;indifferent">
        <rdf:type rdf:resource="&lexinfo;ModificationType"/>
        <rdf:type rdf:resource="&owl;NamedIndividual"/>
        <rdfs:label xml:lang="en">indifferent</rdfs:label>
        <rdfs:label xml:lang="ru">нейтральный</rdfs:label>        
        <rdfs:comment xml:lang="en">Markup to express that there is not any pertinence.</rdfs:comment>
        <rdfs:comment xml:lang="ru">Разметка, указывающая на то, что отсутствует релевантность.</rdfs:comment>
        <owl:versionInfo>1:0</owl:versionInfo>
        <dc:creator>Francopoulo, Gil</dc:creator>
        <dcr:datcat rdf:resource="http://www.isocat.org/datcat/DC-1944"/>
        <rdfs:isDefinedBy rdf:resource="http://www.lexinfo.net/ontology/2.0/lexinfo"/>
    </owl:Thing>
    


    <!-- http://www.lexinfo.net/ontology/2.0/lexinfo#inessiveCase -->

    <owl:Thing rdf:about="&lexinfo;inessiveCase">
        <rdf:type rdf:resource="&lexinfo;Case"/>
        <rdf:type rdf:resource="&owl;NamedIndividual"/>
        <rdfs:label xml:lang="en">inessive case</rdfs:label>
        <rdfs:label xml:lang="ru">инессив</rdfs:label>        
        <rdfs:comment xml:lang="en">Case which expresses the meaning of location or position within a place.</rdfs:comment>
        <rdfs:comment xml:lang="ru">Падеж, который выражает значение местоположения или положения в пределах места.</rdfs:comment>
        <dc:creator>Francopoulo, Gil</dc:creator>
        <owl:versionInfo>1:0</owl:versionInfo>
        <dcr:datcat rdf:resource="http://www.isocat.org/datcat/DC-1311"/>
        <rdfs:isDefinedBy rdf:resource="http://www.lexinfo.net/ontology/2.0/lexinfo"/>
    </owl:Thing>
    


    <!-- http://www.lexinfo.net/ontology/2.0/lexinfo#infinitive -->

    <owl:Thing rdf:about="&lexinfo;infinitive">
        <rdf:type rdf:resource="&lexinfo;VerbFormMood"/>
        <rdf:type rdf:resource="&owl;NamedIndividual"/>
        <rdfs:label xml:lang="en">infinitive</rdfs:label>
        <rdfs:label xml:lang="ru">инфинитив</rdfs:label>        
        <dc:creator>Francopoulo, Gil</dc:creator>
        <owl:versionInfo>1:0</owl:versionInfo>
        <rdfs:comment xml:lang="en">Mood cited as unmarked or base form.</rdfs:comment>
        <rdfs:comment xml:lang="ru">Наклонение, обозначенное как немаркированная или начальная форма.</rdfs:comment>
        <dcr:datcat rdf:resource="http://www.isocat.org/datcat/DC-1312"/>
        <rdfs:isDefinedBy rdf:resource="http://www.lexinfo.net/ontology/2.0/lexinfo"/>
    </owl:Thing>
    


    <!-- http://www.lexinfo.net/ontology/2.0/lexinfo#infinitiveParticle -->

    <owl:Thing rdf:about="&lexinfo;infinitiveParticle">
        <rdf:type rdf:resource="&lexinfo;PartOfSpeech"/>
        <rdf:type rdf:resource="&lexinfo;ParticlePOS"/>
        <rdf:type rdf:resource="&owl;NamedIndividual"/>
        <rdfs:label xml:lang="en">infinitive particle</rdfs:label>
        <rdfs:label xml:lang="ru">инфинитивная частица</rdfs:label>        
        <rdfs:comment xml:lang="en">Particle used to express infinitive.</rdfs:comment>
        <rdfs:comment xml:lang="ru">Частица, используемая для выражения инфинитива.</rdfs:comment>
        <dc:creator>Francopoulo, Gil</dc:creator>
        <owl:versionInfo>1:0</owl:versionInfo>
        <dcr:datcat rdf:resource="http://www.isocat.org/datcat/DC-1896"/>
        <rdfs:isDefinedBy rdf:resource="http://www.lexinfo.net/ontology/2.0/lexinfo"/>
    </owl:Thing>
    


    <!-- http://www.lexinfo.net/ontology/2.0/lexinfo#infix -->

    <owl:Thing rdf:about="&lexinfo;infix">
        <rdf:type rdf:resource="&lexinfo;TermElement"/>
        <rdf:type rdf:resource="&owl;NamedIndividual"/>
        <rdfs:isDefinedBy rdf:resource="http://www.lexinfo.net/ontology/2.0/lexinfo"/>
    </owl:Thing>
    


    <!-- http://www.lexinfo.net/ontology/2.0/lexinfo#inflectionElement -->

    <owl:Thing rdf:about="&lexinfo;inflectionElement">
        <rdf:type rdf:resource="&lexinfo;TermElement"/>
        <rdf:type rdf:resource="&owl;NamedIndividual"/>
        <rdfs:label xml:lang="en">inflectionElement</rdfs:label>
        <rdfs:label xml:lang="ru">флексия</rdfs:label>        
        <dc:creator>Wright, Sue Ellen</dc:creator>
        <owl:versionInfo>1:0</owl:versionInfo>
        <rdfs:comment xml:lang="en">An element of language used to change the form of a word (noun, adjective) by declension, and (verbs) by conjugation.</rdfs:comment>
        <rdfs:comment xml:lang="ru">Элемент языка, используемый для изменения формы слова (существительного, прилагательного) по склонению и (глаголов)  по спряжению.</rdfs:comment>
        <dcr:datcat rdf:resource="http://www.isocat.org/datcat/DC-292"/>
        <rdfs:isDefinedBy rdf:resource="http://www.lexinfo.net/ontology/2.0/lexinfo"/>
    </owl:Thing>
    


    <!-- http://www.lexinfo.net/ontology/2.0/lexinfo#infrequentlyUsed -->

    <owl:Thing rdf:about="&lexinfo;infrequentlyUsed">
        <rdf:type rdf:resource="&lexinfo;Frequency"/>
        <rdf:type rdf:resource="&owl;NamedIndividual"/>
        <rdfs:label xml:lang="en">infrequentlyUsed</rdfs:label>
        <rdfs:label xml:lang="ru">нечастоиспользуемый</rdfs:label>        
        <rdfs:label xml:lang="en">infrequently used</rdfs:label>
        <rdfs:label xml:lang="ru">нечастоиспользуемый</rdfs:label>
        <rdfs:comment xml:lang="en">Said of a term that does not appear frequently.</rdfs:comment>
        <rdfs:comment xml:lang="ru">О термине, который не часто используется.</rdfs:comment>        
        <dc:creator>Francopoulo, Gil</dc:creator>
        <dc:creator>Wright, Sue Ellen</dc:creator>
        <owl:versionInfo>1:0</owl:versionInfo>
        <dcr:datcat rdf:resource="http://www.isocat.org/datcat/DC-1985"/>
        <dcr:datcat rdf:resource="http://www.isocat.org/datcat/DC-235"/>
        <rdfs:isDefinedBy rdf:resource="http://www.lexinfo.net/ontology/2.0/lexinfo"/>
    </owl:Thing>
    


    <!-- http://www.lexinfo.net/ontology/2.0/lexinfo#initialism -->

    <owl:Thing rdf:about="&lexinfo;initialism">
        <rdf:type rdf:resource="&lexinfo;AbbreviatedForm"/>
        <rdf:type rdf:resource="&lexinfo;TermType"/>
        <rdf:type rdf:resource="&owl;NamedIndividual"/>
        <rdfs:label xml:lang="en">initialism</rdfs:label>
        <rdfs:label xml:lang="ru">инициал</rdfs:label>        
        <dc:creator>Wright, Sue Ellen</dc:creator>
        <owl:versionInfo>1:0</owl:versionInfo>
        <rdfs:comment xml:lang="en">An abbreviation made up of the initial letters of the components of the full form of the designation or from syllables of the full form and pronounced letter by letter.</rdfs:comment>
        <rdfs:comment xml:lang="ru">Аббревиатура, состоящая из начальных букв компонентов полной формы обозначения или из слогов полной формы. Произносится по буквам.</rdfs:comment>        
        <dcr:datcat rdf:resource="http://www.isocat.org/datcat/DC-333"/>
        <rdfs:isDefinedBy rdf:resource="http://www.lexinfo.net/ontology/2.0/lexinfo"/>
    </owl:Thing>
    


    <!-- http://www.lexinfo.net/ontology/2.0/lexinfo#instrumentalCase -->

    <owl:Thing rdf:about="&lexinfo;instrumentalCase">
        <rdf:type rdf:resource="&lexinfo;Case"/>
        <rdf:type rdf:resource="&owl;NamedIndividual"/>
        <rdfs:label xml:lang="en">instrumental case</rdfs:label>
        <rdfs:label xml:lang="ru">творительный падеж</rdfs:label>        
        <owl:versionInfo>1:0</owl:versionInfo>
        <dc:creator>Francopoulo, Gil</dc:creator>
        <rdfs:comment xml:lang="en">Case indicating that the referent of the noun it marks is the means of the accomplishment of the action expressed by the clause.</rdfs:comment>
        <rdfs:comment xml:lang="ru">Падеж, указывающий, что референт отмеченного им существительного, является средством совершения действия, выраженного в предложении.</rdfs:comment>
        <dcr:datcat rdf:resource="http://www.isocat.org/datcat/DC-1316"/>
        <rdfs:isDefinedBy rdf:resource="http://www.lexinfo.net/ontology/2.0/lexinfo"/>
    </owl:Thing>
    


    <!-- http://www.lexinfo.net/ontology/2.0/lexinfo#interjection -->

    <owl:Thing rdf:about="&lexinfo;interjection">
        <rdf:type rdf:resource="&lexinfo;PartOfSpeech"/>
        <rdf:type rdf:resource="&owl;NamedIndividual"/>
        <rdfs:label xml:lang="en">interjection</rdfs:label>
        <rdfs:label xml:lang="ru">междометие</rdfs:label>        
        <owl:versionInfo>1:0</owl:versionInfo>
        <dc:creator>Francopoulo, Gil</dc:creator>
        <rdfs:comment xml:lang="en">Word or sound that expresses an emotion.</rdfs:comment>
        <rdfs:comment xml:lang="ru">Слово или звук, выражающий эмоции.</rdfs:comment>
        <dcr:datcat rdf:resource="http://www.isocat.org/datcat/DC-1318"/>
        <rdfs:isDefinedBy rdf:resource="http://www.lexinfo.net/ontology/2.0/lexinfo"/>
    </owl:Thing>
    


    <!-- http://www.lexinfo.net/ontology/2.0/lexinfo#internationalScientificTerm -->

    <owl:Thing rdf:about="&lexinfo;internationalScientificTerm">
        <rdf:type rdf:resource="&lexinfo;TermType"/>
        <rdf:type rdf:resource="&owl;NamedIndividual"/>
        <rdfs:label xml:lang="en">international scientific term</rdfs:label>
        <rdfs:label xml:lang="ru">международный научный термин</rdfs:label>        
        <rdfs:comment xml:lang="en">A term that is part of an international scientific nomenclature as adopted by an appropriate scientific body.</rdfs:comment>
        <rdfs:comment xml:lang="ru">Термин, который является частью международной научной номенклатуры, принятой соответствующим научным органом.</rdfs:comment>
        <dc:creator>Wright, Sue Ellen</dc:creator>
        <owl:versionInfo>1:0</owl:versionInfo>
        <dcr:datcat rdf:resource="http://www.isocat.org/datcat/DC-319"/>
        <rdfs:isDefinedBy rdf:resource="http://www.lexinfo.net/ontology/2.0/lexinfo"/>
    </owl:Thing>
    


    <!-- http://www.lexinfo.net/ontology/2.0/lexinfo#internationalism -->

    <owl:Thing rdf:about="&lexinfo;internationalism">
        <rdf:type rdf:resource="&lexinfo;TermType"/>
        <rdf:type rdf:resource="&owl;NamedIndividual"/>
        <rdfs:label xml:lang="en">internationalism</rdfs:label>
        <rdfs:label xml:lang="ru">интернационализм</rdfs:label>        
        <dc:creator>Wright, Sue Ellen</dc:creator>
        <owl:versionInfo>1:0</owl:versionInfo>
        <rdfs:comment xml:lang="en">A term that has the same or nearly identical orthographic or phonemic form in many languages.</rdfs:comment>
        <rdfs:comment xml:lang="ru">Термин, который имеет ту же или почти идентичную орфографическую или фонематическую форму во многих языках.</rdfs:comment>
        <dcr:datcat rdf:resource="http://www.isocat.org/datcat/DC-320"/>
        <rdfs:isDefinedBy rdf:resource="http://www.lexinfo.net/ontology/2.0/lexinfo"/>
    </owl:Thing>
    


    <!-- http://www.lexinfo.net/ontology/2.0/lexinfo#interrogativeCardinalNumeral -->

    <owl:Thing rdf:about="&lexinfo;interrogativeCardinalNumeral">
        <rdf:type rdf:resource="&lexinfo;NumeralPOS"/>
        <rdf:type rdf:resource="&lexinfo;PartOfSpeech"/>
        <rdf:type rdf:resource="&owl;NamedIndividual"/>
        <rdfs:label xml:lang="en">interrogative cardinal numeral</rdfs:label>
        <rdfs:label xml:lang="ru">вопросительное количественное числительное</rdfs:label>        
        <dc:creator>Zeman, Dan</dc:creator>
        <rdfs:comment xml:lang="en">An interrogative/relative word used to ask about quantity.</rdfs:comment>
        <rdfs:comment xml:lang="ru">Вопросительное / относительное слово, которое используется для задания вопроса о количестве.</rdfs:comment>
        <owl:versionInfo>1:0</owl:versionInfo>
        <dcr:datcat rdf:resource="http://www.isocat.org/datcat/DC-3018"/>
        <rdfs:isDefinedBy rdf:resource="http://www.lexinfo.net/ontology/2.0/lexinfo"/>
    </owl:Thing>
    


    <!-- http://www.lexinfo.net/ontology/2.0/lexinfo#interrogativeDeterminer -->

    <owl:Thing rdf:about="&lexinfo;interrogativeDeterminer">
        <rdf:type rdf:resource="&lexinfo;DeterminerPOS"/>
        <rdf:type rdf:resource="&lexinfo;PartOfSpeech"/>
        <rdf:type rdf:resource="&owl;NamedIndividual"/>
        <rdfs:label xml:lang="en">interrogative determiner</rdfs:label>
        <rdfs:label xml:lang="ru">вопросительный определитель</rdfs:label>        
        <owl:versionInfo>1:0</owl:versionInfo>
        <dc:creator>Francopoulo, Gil</dc:creator>
        <rdfs:comment xml:lang="en">Determiner used to express a question.</rdfs:comment>
        <rdfs:comment xml:lang="ru">Определитель, используемый для выражения вопроса.</rdfs:comment>
        <dcr:datcat rdf:resource="http://www.isocat.org/datcat/DC-1320"/>
        <rdfs:isDefinedBy rdf:resource="http://www.lexinfo.net/ontology/2.0/lexinfo"/>
    </owl:Thing>
    


    <!-- http://www.lexinfo.net/ontology/2.0/lexinfo#interrogativeMultiplicativeNumeral -->

    <owl:Thing rdf:about="&lexinfo;interrogativeMultiplicativeNumeral">
        <rdf:type rdf:resource="&lexinfo;NumeralPOS"/>
        <rdf:type rdf:resource="&lexinfo;PartOfSpeech"/>
        <rdf:type rdf:resource="&owl;NamedIndividual"/>
        <rdfs:label xml:lang="en">interrogative multiplicative numeral</rdfs:label>
        <rdfs:label xml:lang="ru">вопросительное множественное числительное</rdfs:label>
        <owl:versionInfo>1:0</owl:versionInfo>
        <rdfs:comment xml:lang="en">An interrogative/relative word used to ask about the number of times something happened.</rdfs:comment>
        <rdfs:comment xml:lang="ru">Вопросительное / относительное слово используемое, чтобы спросить, сколько раз что-либо произошло.</rdfs:comment>
        <dc:creator>Zeman, Dan</dc:creator>
        <dcr:datcat rdf:resource="http://www.isocat.org/datcat/DC-3021"/>
        <rdfs:isDefinedBy rdf:resource="http://www.lexinfo.net/ontology/2.0/lexinfo"/>
    </owl:Thing>
    


    <!-- http://www.lexinfo.net/ontology/2.0/lexinfo#interrogativeOrdinalNumeral -->

    <owl:Thing rdf:about="&lexinfo;interrogativeOrdinalNumeral">
        <rdf:type rdf:resource="&lexinfo;NumeralPOS"/>
        <rdf:type rdf:resource="&lexinfo;PartOfSpeech"/>
        <rdf:type rdf:resource="&owl;NamedIndividual"/>
        <rdfs:label xml:lang="en">interrogative ordinal numeral</rdfs:label>
        <rdfs:label xml:lang="ru">вопросительное порядковое числительное</rdfs:label>        
        <dc:creator>Zeman, Dan</dc:creator>
        <rdfs:comment xml:lang="en">An interrogative/relative word used to ask about numeric ranking.</rdfs:comment>
        <rdfs:comment xml:lang="ru">Вопросительное / относительное слово, используемое для запроса о порядковом номере.</rdfs:comment>
        <owl:versionInfo>1:0</owl:versionInfo>
        <dcr:datcat rdf:resource="http://www.isocat.org/datcat/DC-3019"/>
        <rdfs:isDefinedBy rdf:resource="http://www.lexinfo.net/ontology/2.0/lexinfo"/>
    </owl:Thing>
    


    <!-- http://www.lexinfo.net/ontology/2.0/lexinfo#interrogativeParticle -->

    <owl:Thing rdf:about="&lexinfo;interrogativeParticle">
        <rdf:type rdf:resource="&lexinfo;PartOfSpeech"/>
        <rdf:type rdf:resource="&lexinfo;ParticlePOS"/>
        <rdf:type rdf:resource="&owl;NamedIndividual"/>
        <rdfs:label xml:lang="en">interrogative particle</rdfs:label>
        <rdfs:label xml:lang="ru">вопросительная частица</rdfs:label>
        <owl:versionInfo>1:0</owl:versionInfo>
        <dc:creator>Francopoulo, Gil</dc:creator>
        <rdfs:comment xml:lang="en">Particle used to express a question.</rdfs:comment>
        <rdfs:comment xml:lang="ru">Частица, используемая для выражения вопроса.</rdfs:comment>
        <dcr:datcat rdf:resource="http://www.isocat.org/datcat/DC-1921"/>
        <rdfs:isDefinedBy rdf:resource="http://www.lexinfo.net/ontology/2.0/lexinfo"/>
    </owl:Thing>
    


    <!-- http://www.lexinfo.net/ontology/2.0/lexinfo#interrogativePronoun -->

    <owl:Thing rdf:about="&lexinfo;interrogativePronoun">
        <rdf:type rdf:resource="&lexinfo;PartOfSpeech"/>
        <rdf:type rdf:resource="&lexinfo;PronounPOS"/>
        <rdf:type rdf:resource="&owl;NamedIndividual"/>
        <rdfs:label xml:lang="en">interrogative pronoun</rdfs:label>
        <rdfs:label xml:lang="ru">вопросительное местоимение</rdfs:label>        
        <dc:creator>Francopoulo, Gil</dc:creator>
        <owl:versionInfo>1:0</owl:versionInfo>
        <rdfs:comment xml:lang="en">Pronoun used to express a question.</rdfs:comment>
        <rdfs:comment xml:lang="ru">Местоимение, используемое для выражения вопроса.</rdfs:comment>
        <dcr:datcat rdf:resource="http://www.isocat.org/datcat/DC-1321"/>
        <rdfs:isDefinedBy rdf:resource="http://www.lexinfo.net/ontology/2.0/lexinfo"/>
    </owl:Thing>
    


    <!-- http://www.lexinfo.net/ontology/2.0/lexinfo#interrogativeRelativePronoun -->

    <owl:Thing rdf:about="&lexinfo;interrogativeRelativePronoun">
        <rdf:type rdf:resource="&lexinfo;PartOfSpeech"/>
        <rdf:type rdf:resource="&owl;NamedIndividual"/>
        <rdfs:label xml:lang="en">interrogative relative pronoun</rdfs:label>
        <rdfs:label xml:lang="ru">вопросительное относительное местоимение</rdfs:label>        
        <dc:creator>Francopoulo, Gil</dc:creator>
        <owl:versionInfo>1:0</owl:versionInfo>
        <rdfs:comment xml:lang="en">pronoun which may act as a relative pronoun or an interrogative one</rdfs:comment>
        <rdfs:comment xml:lang="ru">Местоимение, которое может функкционировать как относительное местоимение или вопросительное местоимение</rdfs:comment>
        <dcr:datcat rdf:resource="http://www.isocat.org/datcat/DC-3016"/>
        <rdfs:isDefinedBy rdf:resource="http://www.lexinfo.net/ontology/2.0/lexinfo"/>
    </owl:Thing>
    


    <!-- http://www.lexinfo.net/ontology/2.0/lexinfo#invertedComma -->

    <owl:Thing rdf:about="&lexinfo;invertedComma">
        <rdf:type rdf:resource="&lexinfo;PartOfSpeech"/>
        <rdf:type rdf:resource="&lexinfo;SymbolPOS"/>
        <rdf:type rdf:resource="&owl;NamedIndividual"/>
        <rdfs:label xml:lang="en">inverted comma</rdfs:label>
        <rdfs:label xml:lang="ru">кавычка</rdfs:label>
        <rdfs:comment xml:lang="en">Inverted comma.</rdfs:comment>
        <rdfs:comment xml:lang="ru">Кавычка</rdfs:comment>
        <dc:creator>Francopoulo, Gil</dc:creator>
        <owl:versionInfo>1:0</owl:versionInfo>
        <dcr:datcat rdf:resource="http://www.isocat.org/datcat/DC-1443"/>
        <rdfs:isDefinedBy rdf:resource="http://www.lexinfo.net/ontology/2.0/lexinfo"/>
    </owl:Thing>
    


    <!-- http://www.lexinfo.net/ontology/2.0/lexinfo#ironicRegister -->

    <owl:Thing rdf:about="&lexinfo;ironicRegister">
        <rdf:type rdf:resource="&lexinfo;Register"/>
        <rdf:type rdf:resource="&owl;NamedIndividual"/>
        <rdfs:isDefinedBy rdf:resource="http://www.lexinfo.net/ontology/2.0/lexinfo"/>
    </owl:Thing>
    


    <!-- http://www.lexinfo.net/ontology/2.0/lexinfo#irreflexivePersonalPronoun -->

    <owl:Thing rdf:about="&lexinfo;irreflexivePersonalPronoun">
        <rdf:type rdf:resource="&lexinfo;PartOfSpeech"/>
        <rdf:type rdf:resource="&lexinfo;PronounPOS"/>
        <rdf:type rdf:resource="&owl;NamedIndividual"/>
        <rdfs:label xml:lang="en">irreflexive personal pronoun</rdfs:label>
        <rdfs:label xml:lang="ru">невозвратное личное местоимение</rdfs:label>        
        <owl:versionInfo>1:0</owl:versionInfo>
        <dc:creator>Francopoulo, Gil</dc:creator>
        <rdfs:comment xml:lang="en">personal pronoun which is not reflexive</rdfs:comment>
        <rdfs:comment xml:lang="ru">Личное местоимение, которое не может быть возвратным</rdfs:comment>
        <dcr:datcat rdf:resource="http://www.isocat.org/datcat/DC-3013"/>
        <rdfs:isDefinedBy rdf:resource="http://www.lexinfo.net/ontology/2.0/lexinfo"/>
    </owl:Thing>
    


    <!-- http://www.lexinfo.net/ontology/2.0/lexinfo#lativeCase -->

    <owl:Thing rdf:about="&lexinfo;lativeCase">
        <rdf:type rdf:resource="&lexinfo;Case"/>
        <rdf:type rdf:resource="&owl;NamedIndividual"/>
        <rdfs:label xml:lang="en">lative case</rdfs:label>
        <rdfs:label xml:lang="ru">латив</rdfs:label>        
        <dc:creator>Francopoulo, Gil</dc:creator>
        <rdfs:comment xml:lang="en">Case which expresses motion to a location.</rdfs:comment>
        <rdfs:comment xml:lang="ru">Падеж, который обозначает "движение к местоположению".</rdfs:comment>
        <owl:versionInfo>1:0</owl:versionInfo>
        <dcr:datcat rdf:resource="http://www.isocat.org/datcat/DC-1323"/>
        <rdfs:isDefinedBy rdf:resource="http://www.lexinfo.net/ontology/2.0/lexinfo"/>
    </owl:Thing>
    


    <!-- http://www.lexinfo.net/ontology/2.0/lexinfo#legalTerm -->

    <owl:Thing rdf:about="&lexinfo;legalTerm">
        <rdf:type rdf:resource="&lexinfo;NormativeAuthorization"/>
        <rdf:type rdf:resource="&owl;NamedIndividual"/>
        <rdfs:label xml:lang="en">legal term</rdfs:label>
        <rdfs:label xml:lang="ru">юридический термин</rdfs:label>        
        <owl:versionInfo>1:0</owl:versionInfo>
        <rdfs:comment xml:lang="en">A term that is legally defined and used in legally binding documents.</rdfs:comment>
        <rdfs:comment xml:lang="ru">Термин, который определяется юридически и используется в юридических документах.</rdfs:comment>
        <dc:creator>Wright, Sue Ellen</dc:creator>
        <dcr:datcat rdf:resource="http://www.isocat.org/datcat/DC-380"/>
        <rdfs:isDefinedBy rdf:resource="http://www.lexinfo.net/ontology/2.0/lexinfo"/>
    </owl:Thing>
    


    <!-- http://www.lexinfo.net/ontology/2.0/lexinfo#letter -->

    <owl:Thing rdf:about="&lexinfo;letter">
        <rdf:type rdf:resource="&lexinfo;SymbolPOS"/>
        <rdf:type rdf:resource="&owl;NamedIndividual"/>
        <rdfs:isDefinedBy rdf:resource="http://www.lexinfo.net/ontology/2.0/lexinfo"/>
    </owl:Thing>
    


    <!-- http://www.lexinfo.net/ontology/2.0/lexinfo#lightVerb -->

    <owl:Thing rdf:about="&lexinfo;lightVerb">
        <rdf:type rdf:resource="&lexinfo;PartOfSpeech"/>
        <rdf:type rdf:resource="&lexinfo;VerbPOS"/>
        <rdf:type rdf:resource="&owl;NamedIndividual"/>
        <rdfs:label xml:lang="en">light verb</rdfs:label>
        <rdfs:label xml:lang="ru">ослабленный глагол</rdfs:label>        
        <owl:versionInfo>1:0</owl:versionInfo>
        <rdfs:comment xml:lang="en">verb participating in a complex predication that has little semantic content of its own.</rdfs:comment>
        <rdfs:comment xml:lang="ru">Глагол, входящий в состав составных сказуемых и имеющий ослабленную семантику</rdfs:comment>
        <dc:creator>Francopoulo, Gil</dc:creator>
        <dcr:datcat rdf:resource="http://www.isocat.org/datcat/DC-3003"/>
        <rdfs:isDefinedBy rdf:resource="http://www.lexinfo.net/ontology/2.0/lexinfo"/>
    </owl:Thing>
    


    <!-- http://www.lexinfo.net/ontology/2.0/lexinfo#locativeCase -->

    <owl:Thing rdf:about="&lexinfo;locativeCase">
        <rdf:type rdf:resource="&lexinfo;Case"/>
        <rdf:type rdf:resource="&owl;NamedIndividual"/>
        <rdfs:label xml:lang="en">locative case</rdfs:label>
        <rdfs:label xml:lang="ru">местный падеж</rdfs:label>        
        <owl:versionInfo>1:0</owl:versionInfo>
        <dc:creator>Francopoulo, Gil</dc:creator>
        <rdfs:comment xml:lang="en">Case that indicates a final location of action or a time of the action.</rdfs:comment>
        <rdfs:comment xml:lang="ru">Падеж, указывающий на конечное место действия или время действия.</rdfs:comment>
        <dcr:datcat rdf:resource="http://www.isocat.org/datcat/DC-1326"/>
        <rdfs:isDefinedBy rdf:resource="http://www.lexinfo.net/ontology/2.0/lexinfo"/>
    </owl:Thing>
    


    <!-- http://www.lexinfo.net/ontology/2.0/lexinfo#logicalExpression -->

    <owl:Thing rdf:about="&lexinfo;logicalExpression">
        <rdf:type rdf:resource="&lexinfo;TermType"/>
        <rdf:type rdf:resource="&owl;NamedIndividual"/>
        <rdfs:label xml:lang="en">logical expression</rdfs:label>
        <rdfs:label xml:lang="ru">логическое выражение</rdfs:label>        
        <owl:versionInfo>1:0</owl:versionInfo>
        <rdfs:comment xml:lang="en">An expression used to represent a concept based on mathematical or logical relations, such as statements of inequality, set relationships, boolean operations, and the like.</rdfs:comment>
        <rdfs:comment xml:lang="ru">Выражение, используемое для представления понятия, основанного на математических или логических отношениях таких, как утверждения неравенства, множество отношений, булевы операции и т.п.</rdfs:comment>
        <dc:creator>Wright, Sue Ellen</dc:creator>
        <dcr:datcat rdf:resource="http://www.isocat.org/datcat/DC-327"/>
        <rdfs:isDefinedBy rdf:resource="http://www.lexinfo.net/ontology/2.0/lexinfo"/>
    </owl:Thing>
    


    <!-- http://www.lexinfo.net/ontology/2.0/lexinfo#mainVerb -->

    <owl:Thing rdf:about="&lexinfo;mainVerb">
        <rdf:type rdf:resource="&lexinfo;PartOfSpeech"/>
        <rdf:type rdf:resource="&lexinfo;VerbPOS"/>
        <rdf:type rdf:resource="&owl;NamedIndividual"/>
        <rdfs:label xml:lang="en">main verb</rdfs:label>
        <rdfs:label xml:lang="ru">смысловой глагол</rdfs:label>
        <owl:versionInfo>1:0</owl:versionInfo>
        <dc:creator>Francopoulo, Gil</dc:creator>
        <rdfs:comment xml:lang="en">Main verb in contrast to a modal or an auxiliary.</rdfs:comment>
        <rdfs:comment xml:lang="ru">Смысловой глагол в противоположность модальному или вспомогательному глаголу.</rdfs:comment>        
        <dcr:datcat rdf:resource="http://www.isocat.org/datcat/DC-1400"/>
        <rdfs:isDefinedBy rdf:resource="http://www.lexinfo.net/ontology/2.0/lexinfo"/>
    </owl:Thing>
    


    <!-- http://www.lexinfo.net/ontology/2.0/lexinfo#masculine -->

    <owl:Thing rdf:about="&lexinfo;masculine">
        <rdf:type rdf:resource="&lexinfo;Gender"/>
        <rdf:type rdf:resource="&owl;NamedIndividual"/>
        <rdfs:label xml:lang="en">masculine</rdfs:label>
        <rdfs:label xml:lang="ru">мужской</rdfs:label>        
        <owl:versionInfo>1:0</owl:versionInfo>
        <rdfs:comment xml:lang="en">Of, relating to, or constituting the gender that ordinarily includes most words or grammatical forms referring to males.</rdfs:comment>
        <rdfs:comment xml:lang="ru">Об относящемся к или о составляющем род, который обычно включает большинство слов или грамматических форм, обозначающих мужских особей.</rdfs:comment>
        <dc:creator>Francopoulo, Gil</dc:creator>
        <dc:creator>Wright, Sue Ellen</dc:creator>
        <dcr:datcat rdf:resource="http://www.isocat.org/datcat/DC-1883"/>
        <dcr:datcat rdf:resource="http://www.isocat.org/datcat/DC-246"/>
        <rdfs:isDefinedBy rdf:resource="http://www.lexinfo.net/ontology/2.0/lexinfo"/>
    </owl:Thing>
    


    <!-- http://www.lexinfo.net/ontology/2.0/lexinfo#massNoun -->

    <owl:Thing rdf:about="&lexinfo;massNoun">
        <rdf:type rdf:resource="&lexinfo;Number"/>
        <rdf:type rdf:resource="&owl;NamedIndividual"/>
        <rdfs:label xml:lang="en">massNoun</rdfs:label>
        <rdfs:label xml:lang="ru">неисчисляемое существительное</rdfs:label>
        <rdfs:label xml:lang="en">mass noun</rdfs:label>
        <rdfs:label xml:lang="ru">неисчисляемое существительное</rdfs:label>
        <owl:versionInfo>1:0</owl:versionInfo>
        <dc:creator>Wright, Sue Ellen</dc:creator>
        <rdfs:comment xml:lang="en">Designation of a term or word that is not countable and cannot generally be used with the indefinite article or in the plural.</rdfs:comment>
        <rdfs:comment xml:lang="ru">Обозначение для термина или слова, не являющегося исчисляемым, и которое не может быть использовано с неопредленным артиклем или во множественном числе.</rdfs:comment>        
        <dc:creator>Francopoulo, Gil</dc:creator>
        <dcr:datcat rdf:resource="http://www.isocat.org/datcat/DC-2277"/>
        <dcr:datcat rdf:resource="http://www.isocat.org/datcat/DC-255"/>
        <rdfs:isDefinedBy rdf:resource="http://www.lexinfo.net/ontology/2.0/lexinfo"/>
    </owl:Thing>
    


    <!-- http://www.lexinfo.net/ontology/2.0/lexinfo#middleVoice -->

    <owl:Thing rdf:about="&lexinfo;middleVoice">
        <rdf:type rdf:resource="&lexinfo;Voice"/>
        <rdf:type rdf:resource="&owl;NamedIndividual"/>
        <rdfs:label xml:lang="en">middle voice</rdfs:label>
        <rdfs:label xml:lang="ru">медиальный залог</rdfs:label>        
        <dc:creator>Francopoulo, Gil</dc:creator>
        <rdfs:comment xml:lang="en">Value for middle voice that expresses that the subject is both the agent and object, or that the subject is separate from the agent or that the receiver is the agent him/herself.</rdfs:comment>
        <rdfs:comment xml:lang="ru">Означает, что подлежащее является одновременно исполнителем (субъектом) и объектом,  или что  исполнитель (субъект) отделен от объекта, или что получатель и является исполнителем (субъектом).</rdfs:comment>
        <owl:versionInfo>1:0</owl:versionInfo>
        <dcr:datcat rdf:resource="http://www.isocat.org/datcat/DC-1983"/>
        <rdfs:isDefinedBy rdf:resource="http://www.lexinfo.net/ontology/2.0/lexinfo"/>
    </owl:Thing>
    


    <!-- http://www.lexinfo.net/ontology/2.0/lexinfo#modal -->

    <owl:Thing rdf:about="&lexinfo;modal">
        <rdf:type rdf:resource="&lexinfo;PartOfSpeech"/>
        <rdf:type rdf:resource="&lexinfo;VerbPOS"/>
        <rdf:type rdf:resource="&owl;NamedIndividual"/>
        <rdfs:label xml:lang="en">modal</rdfs:label>
        <rdfs:label xml:lang="ru">модальный</rdfs:label>        
        <owl:versionInfo>1:0</owl:versionInfo>
        <dc:creator>Francopoulo, Gil</dc:creator>
        <rdfs:comment xml:lang="en">Verb form that is usually used with another verb to express ideas such as possibilities, permission, or intention.</rdfs:comment>
        <rdfs:comment xml:lang="ru">Глагольная форма, которая обычно используется с другим глаголом, для выражения возможности, разрешения или намерения.</rdfs:comment>        
        <dcr:datcat rdf:resource="http://www.isocat.org/datcat/DC-1329"/>
        <rdfs:isDefinedBy rdf:resource="http://www.lexinfo.net/ontology/2.0/lexinfo"/>
    </owl:Thing>
    


    <!-- http://www.lexinfo.net/ontology/2.0/lexinfo#modern -->

    <owl:Thing rdf:about="&lexinfo;modern">
        <rdf:type rdf:resource="&lexinfo;Dating"/>
        <rdf:type rdf:resource="&owl;NamedIndividual"/>
        <rdfs:label xml:lang="en">modern</rdfs:label>
        <rdfs:label xml:lang="ru">современный</rdfs:label>        
        <dc:creator>Francopoulo, Gil</dc:creator>
        <owl:versionInfo>1:0</owl:versionInfo>
        <rdfs:comment xml:lang="en">Currently in use.</rdfs:comment>
        <rdfs:comment xml:lang="ru">Используется в настоящее время.</rdfs:comment>
        <dcr:datcat rdf:resource="http://www.isocat.org/datcat/DC-1962"/>
        <rdfs:isDefinedBy rdf:resource="http://www.lexinfo.net/ontology/2.0/lexinfo"/>
    </owl:Thing>
    


    <!-- http://www.lexinfo.net/ontology/2.0/lexinfo#morphologicalElement -->

    <owl:Thing rdf:about="&lexinfo;morphologicalElement">
        <rdf:type rdf:resource="&lexinfo;TermElement"/>
        <rdf:type rdf:resource="&owl;NamedIndividual"/>
        <rdfs:label xml:lang="en">morphological element</rdfs:label>
        <rdfs:label xml:lang="ru">морфологический элемент</rdfs:label>
        <dc:creator>Wright, Sue Ellen</dc:creator>
        <owl:versionInfo>1:0</owl:versionInfo>
        <rdfs:comment xml:lang="en">Unit resulting from the division of words into their smallest meaningful parts.
Note: moved to lexeme element from being an independent element; note that this is currently an independent element in 12620</rdfs:comment>
        <rdfs:comment xml:lang="ru">Элемент, являющийся результатом деления слова на наименьшие значимые части.
Замечание: перенесен в категорию “элемент лексемы”  из категории “независимая лексема”; обратите внимание, сейчас это независимый элемент в 12620.</rdfs:comment>
        <dcr:datcat rdf:resource="http://www.isocat.org/datcat/DC-300"/>
        <rdfs:isDefinedBy rdf:resource="http://www.lexinfo.net/ontology/2.0/lexinfo"/>
    </owl:Thing>
    


    <!-- http://www.lexinfo.net/ontology/2.0/lexinfo#multiplicativeNumeral -->

    <owl:Thing rdf:about="&lexinfo;multiplicativeNumeral">
        <rdf:type rdf:resource="&lexinfo;NumeralPOS"/>
        <rdf:type rdf:resource="&lexinfo;PartOfSpeech"/>
        <rdf:type rdf:resource="&owl;NamedIndividual"/>
        <rdfs:label xml:lang="en">multiplicative numeral</rdfs:label>
        <rdfs:label xml:lang="ru">множественное числительное</rdfs:label>        
        <owl:versionInfo>1:0</owl:versionInfo>
        <rdfs:comment xml:lang="en">A word that expresses the number of times something happened.</rdfs:comment>
        <rdfs:comment xml:lang="ru">Слово, которое выражает, сколько раз что-либо происходит.</rdfs:comment>
        <dc:creator>Zeman, Dan</dc:creator>
        <dcr:datcat rdf:resource="http://www.isocat.org/datcat/DC-3020"/>
        <rdfs:isDefinedBy rdf:resource="http://www.lexinfo.net/ontology/2.0/lexinfo"/>
    </owl:Thing>
    


    <!-- http://www.lexinfo.net/ontology/2.0/lexinfo#negativeParticle -->

    <owl:Thing rdf:about="&lexinfo;negativeParticle">
        <rdf:type rdf:resource="&lexinfo;PartOfSpeech"/>
        <rdf:type rdf:resource="&lexinfo;ParticlePOS"/>
        <rdf:type rdf:resource="&owl;NamedIndividual"/>
        <rdfs:label xml:lang="en">negative particle</rdfs:label>
        <rdfs:label xml:lang="ru">отрицательная частица</rdfs:label>        
        <owl:versionInfo>1:0</owl:versionInfo>
        <dc:creator>Francopoulo, Gil</dc:creator>
        <rdfs:comment xml:lang="en">Particle used to express negation.</rdfs:comment>
        <rdfs:comment xml:lang="ru">Частица, используемая для выражения отрицания.</rdfs:comment>
        <dcr:datcat rdf:resource="http://www.isocat.org/datcat/DC-1894"/>
        <rdfs:isDefinedBy rdf:resource="http://www.lexinfo.net/ontology/2.0/lexinfo"/>
    </owl:Thing>
    


    <!-- http://www.lexinfo.net/ontology/2.0/lexinfo#negativePronoun -->

    <owl:Thing rdf:about="&lexinfo;negativePronoun">
        <rdf:type rdf:resource="&lexinfo;PartOfSpeech"/>
        <rdf:type rdf:resource="&lexinfo;PronounPOS"/>
        <rdf:type rdf:resource="&owl;NamedIndividual"/>
        <rdfs:label xml:lang="en">negative pronoun</rdfs:label>
        <rdfs:label xml:lang="ru">отрицательное местоимение</rdfs:label>        
        <rdfs:comment xml:lang="en">Pronoun used in a context of a negation or for expressing a negation.</rdfs:comment>
        <rdfs:comment xml:lang="ru">Местоимение, используемое в контексте отрицания или для выражения отрицания.</rdfs:comment>
        <dc:creator>Francopoulo, Gil</dc:creator>
        <owl:versionInfo>1:0</owl:versionInfo>
        <dcr:datcat rdf:resource="http://www.isocat.org/datcat/DC-1925"/>
        <rdfs:isDefinedBy rdf:resource="http://www.lexinfo.net/ontology/2.0/lexinfo"/>
    </owl:Thing>
    


    <!-- http://www.lexinfo.net/ontology/2.0/lexinfo#neuter -->

    <owl:Thing rdf:about="&lexinfo;neuter">
        <rdf:type rdf:resource="&lexinfo;Gender"/>
        <rdf:type rdf:resource="&owl;NamedIndividual"/>
        <rdfs:label xml:lang="en">neuter</rdfs:label>
        <rdfs:label xml:lang="ru">средний</rdfs:label>        
        <owl:versionInfo>1:0</owl:versionInfo>
        <dc:creator>Francopoulo, Gil</dc:creator>
        <dc:creator>Wright, Sue Ellen</dc:creator>
        <rdfs:comment xml:lang="en">Of, relating to, or constituting the gender that ordinarily includes most words or grammatical forms referring to objects that are not characterized as male or female.</rdfs:comment>
        <rdfs:comment xml:lang="ru">Об относящемся к или о составляющем род, который обычно включает большинство слов или грамматических форм, указывающих на объекты, которые не характеризуются как относящиеся мужскому или женскому полу.</rdfs:comment>
        <dcr:datcat rdf:resource="http://www.isocat.org/datcat/DC-1884"/>
        <dcr:datcat rdf:resource="http://www.isocat.org/datcat/DC-248"/>
        <rdfs:isDefinedBy rdf:resource="http://www.lexinfo.net/ontology/2.0/lexinfo"/>
    </owl:Thing>
    


    <!-- http://www.lexinfo.net/ontology/2.0/lexinfo#neutralRegister -->

    <owl:Thing rdf:about="&lexinfo;neutralRegister">
        <rdf:type rdf:resource="&lexinfo;Register"/>
        <rdf:type rdf:resource="&owl;NamedIndividual"/>
        <rdfs:label xml:lang="en">neutral register</rdfs:label>
        <rdfs:label xml:lang="ru">нейтральный реестр</rdfs:label>        
        <rdfs:comment xml:lang="en">The register appropriate to general texts or discourse.</rdfs:comment>
        <rdfs:comment xml:lang="ru">Реестр, соответствующий общим текстам или речи.</rdfs:comment>
        <owl:versionInfo>1:0</owl:versionInfo>
        <dc:creator>Wright, Sue Ellen</dc:creator>
        <dc:creator>Francopoulo, Gil</dc:creator>
        <dcr:datcat rdf:resource="http://www.isocat.org/datcat/DC-1999"/>
        <dcr:datcat rdf:resource="http://www.isocat.org/datcat/DC-424"/>
        <rdfs:isDefinedBy rdf:resource="http://www.lexinfo.net/ontology/2.0/lexinfo"/>
    </owl:Thing>
    


    <!-- http://www.lexinfo.net/ontology/2.0/lexinfo#no -->

    <owl:Thing rdf:about="&lexinfo;no">
        <rdf:type rdf:resource="&lexinfo;Cliticness"/>
        <rdf:type rdf:resource="&lexinfo;Negative"/>
        <rdf:type rdf:resource="&owl;NamedIndividual"/>
        <rdfs:label xml:lang="en">no</rdfs:label>
        <rdfs:label xml:lang="ru">нет</rdfs:label>        
        <dc:creator>Francopoulo, Gil</dc:creator>
        <owl:versionInfo>1:0</owl:versionInfo>
        <rdfs:comment xml:lang="en">Value for negation.</rdfs:comment>
        <rdfs:comment xml:lang="ru">Значение отрицания.</rdfs:comment>
        <dcr:datcat rdf:resource="http://www.isocat.org/datcat/DC-1905"/>
        <rdfs:isDefinedBy rdf:resource="http://www.lexinfo.net/ontology/2.0/lexinfo"/>
    </owl:Thing>
    


    <!-- http://www.lexinfo.net/ontology/2.0/lexinfo#nominativeCase -->

    <owl:Thing rdf:about="&lexinfo;nominativeCase">
        <rdf:type rdf:resource="&lexinfo;Case"/>
        <rdf:type rdf:resource="&owl;NamedIndividual"/>
        <rdfs:label xml:lang="en">nominative case</rdfs:label>
        <rdfs:label xml:lang="ru">именительный падеж</rdfs:label>        
        <dc:creator>Francopoulo, Gil</dc:creator>
        <rdfs:comment xml:lang="en">Case used to indicate the subject of a verb.</rdfs:comment>
        <rdfs:comment xml:lang="ru">Падеж, используемый для обозначения подлежащего.</rdfs:comment>
        <owl:versionInfo>1:0</owl:versionInfo>
        <dcr:datcat rdf:resource="http://www.isocat.org/datcat/DC-1331"/>
        <rdfs:isDefinedBy rdf:resource="http://www.lexinfo.net/ontology/2.0/lexinfo"/>
    </owl:Thing>
    


    <!-- http://www.lexinfo.net/ontology/2.0/lexinfo#nonFinite -->

    <owl:Thing rdf:about="&lexinfo;nonFinite">
        <rdf:type rdf:resource="&lexinfo;Finiteness"/>
        <rdf:type rdf:resource="&owl;NamedIndividual"/>
        <rdfs:label xml:lang="en">non-finite</rdfs:label>
        <rdfs:label xml:lang="ru">неспрягаемый</rdfs:label>        
        <rdfs:comment xml:lang="en">Property related for verb forms occurring on their own only in dependent clauses and lacking tense and mood contrasts.</rdfs:comment>
        <rdfs:comment xml:lang="ru">Свойство, относящееся к глаголам, которые самостоятельно употребляются только в придаточных предложениях и не имеют отличия в отнесенности ко времени и наклонению.</rdfs:comment>
        <dc:creator>Francopoulo, Gil</dc:creator>
        <owl:versionInfo>1:0</owl:versionInfo>
        <dcr:datcat rdf:resource="http://www.isocat.org/datcat/DC-1332"/>
        <rdfs:isDefinedBy rdf:resource="http://www.lexinfo.net/ontology/2.0/lexinfo"/>
    </owl:Thing>
    


    <!-- http://www.lexinfo.net/ontology/2.0/lexinfo#noun -->

    <owl:Thing rdf:about="&lexinfo;noun">
        <rdf:type rdf:resource="&lexinfo;NounPOS"/>
        <rdf:type rdf:resource="&lexinfo;PartOfSpeech"/>
        <rdf:type rdf:resource="&owl;NamedIndividual"/>
        <rdfs:label xml:lang="en">noun</rdfs:label>
        <rdfs:label xml:lang="ru">имя существительное</rdfs:label>        
        <rdfs:comment xml:lang="en">Part of speech used to express the name of a person, place, action or thing.</rdfs:comment>
        <rdfs:comment xml:lang="ru">Часть речи, используемая для выражения наименования лица, места, действия или вещи.</rdfs:comment>
        <owl:versionInfo>1:0</owl:versionInfo>
        <dc:creator>Francopoulo, Gil</dc:creator>
        <dcr:datcat rdf:resource="http://www.isocat.org/datcat/DC-1333"/>
        <rdfs:isDefinedBy rdf:resource="http://www.lexinfo.net/ontology/2.0/lexinfo"/>
    </owl:Thing>
    


    <!-- http://www.lexinfo.net/ontology/2.0/lexinfo#nucleus -->

    <owl:Thing rdf:about="&lexinfo;nucleus">
        <rdf:type rdf:resource="&lexinfo;TermType"/>
        <rdf:type rdf:resource="&owl;NamedIndividual"/>
        <rdfs:label xml:lang="en">nucleus</rdfs:label>
        <rdfs:label xml:lang="ru">ядро</rdfs:label>        
        <owl:versionInfo>1:0</owl:versionInfo>
        <rdfs:comment xml:lang="en">The component of a multiword or multi-morphemic compound term that is determined or modified by the other components making up the term.</rdfs:comment>
        <rdfs:comment xml:lang="ru">Компонент составного термина, состоящего из нескольких слов или морфем, который определяется другими компонентами, входящими в состав термина.</rdfs:comment>
        <dc:creator>Wright, Sue Ellen</dc:creator>
        <dcr:datcat rdf:resource="http://www.isocat.org/datcat/DC-357"/>
        <rdfs:isDefinedBy rdf:resource="http://www.lexinfo.net/ontology/2.0/lexinfo"/>
    </owl:Thing>
    


    <!-- http://www.lexinfo.net/ontology/2.0/lexinfo#numeral -->

    <owl:Thing rdf:about="&lexinfo;numeral">
        <rdf:type rdf:resource="&lexinfo;NumeralPOS"/>
        <rdf:type rdf:resource="&lexinfo;PartOfSpeech"/>
        <rdf:type rdf:resource="&owl;NamedIndividual"/>
        <rdfs:label xml:lang="en">numeral</rdfs:label>
        <rdfs:label xml:lang="ru">имя числительное</rdfs:label>        
        <owl:versionInfo>1:0</owl:versionInfo>
        <dc:creator>Francopoulo, Gil</dc:creator>
        <rdfs:comment xml:lang="en">Part of speech that expresses a number or the relation to a number.</rdfs:comment>
        <rdfs:comment xml:lang="ru">Часть речи, выражающая число или отношение к числу.</rdfs:comment>
        <dcr:datcat rdf:resource="http://www.isocat.org/datcat/DC-1334"/>
        <rdfs:isDefinedBy rdf:resource="http://www.lexinfo.net/ontology/2.0/lexinfo"/>
    </owl:Thing>
    


    <!-- http://www.lexinfo.net/ontology/2.0/lexinfo#numeralFraction -->

    <owl:Thing rdf:about="&lexinfo;numeralFraction">
        <rdf:type rdf:resource="&lexinfo;NumeralPOS"/>
        <rdf:type rdf:resource="&lexinfo;PartOfSpeech"/>
        <rdf:type rdf:resource="&owl;NamedIndividual"/>
        <rdfs:label xml:lang="en">numeral fraction</rdfs:label>
        <rdfs:label xml:lang="ru">дробь</rdfs:label>        
        <dc:creator>Zeman, Dan</dc:creator>
        <rdfs:comment xml:lang="en">Word used to denote the denominator of a fraction.</rdfs:comment>
        <rdfs:comment xml:lang="ru">Слово, используемое для обозначения знаменателя дроби.</rdfs:comment>
        <owl:versionInfo>1:0</owl:versionInfo>
        <dcr:datcat rdf:resource="http://www.isocat.org/datcat/DC-3026"/>
        <rdfs:isDefinedBy rdf:resource="http://www.lexinfo.net/ontology/2.0/lexinfo"/>
    </owl:Thing>
    


    <!-- http://www.lexinfo.net/ontology/2.0/lexinfo#obliqueCase -->

    <owl:Thing rdf:about="&lexinfo;obliqueCase">
        <rdf:type rdf:resource="&lexinfo;Case"/>
        <rdf:type rdf:resource="&owl;NamedIndividual"/>
        <rdfs:label xml:lang="en">oblique case</rdfs:label>
        <rdfs:label xml:lang="ru">косвенный падеж</rdfs:label>        
        <dc:creator>Francopoulo, Gil</dc:creator>
        <owl:versionInfo>1:0</owl:versionInfo>
        <rdfs:comment xml:lang="en">Case that is used when a noun is the object of a verb or a proposition, except for nominative and vocative case.</rdfs:comment>
        <rdfs:comment xml:lang="ru">Падеж, используемый когда существительное является объектом глагола, кроме именительного и звательного падежей.</rdfs:comment>
        <dcr:datcat rdf:resource="http://www.isocat.org/datcat/DC-1336"/>
        <rdfs:isDefinedBy rdf:resource="http://www.lexinfo.net/ontology/2.0/lexinfo"/>
    </owl:Thing>
    


    <!-- http://www.lexinfo.net/ontology/2.0/lexinfo#obsoleteForm -->

    <owl:Thing rdf:about="&lexinfo;obsoleteForm">
        <rdf:type rdf:resource="&lexinfo;TemporalQualifier"/>
        <rdf:type rdf:resource="&owl;NamedIndividual"/>
        <rdfs:label xml:lang="en">obsolete form</rdfs:label>
        <rdfs:label xml:lang="ru">архаичная форма</rdfs:label>        
        <rdfs:comment xml:lang="en">A term or lexeme which is no longer in common use.</rdfs:comment>
        <rdfs:comment xml:lang="ru">Термин или лексема, которые больше не являются общеупотребительными.</rdfs:comment>
        <dc:creator>Wright, Sue Ellen</dc:creator>
        <owl:versionInfo>1:0</owl:versionInfo>
        <dcr:datcat rdf:resource="http://www.isocat.org/datcat/DC-506"/>
        <rdfs:isDefinedBy rdf:resource="http://www.lexinfo.net/ontology/2.0/lexinfo"/>
    </owl:Thing>
    


    <!-- http://www.lexinfo.net/ontology/2.0/lexinfo#old -->

    <owl:Thing rdf:about="&lexinfo;old">
        <rdf:type rdf:resource="&lexinfo;Dating"/>
        <rdf:type rdf:resource="&owl;NamedIndividual"/>
        <rdfs:label xml:lang="en">old</rdfs:label>
        <rdfs:label xml:lang="ru">старый</rdfs:label>        
        <rdfs:comment xml:lang="en">Used in the past.</rdfs:comment>
        <rdfs:comment xml:lang="ru">Используемый в прошлом.</rdfs:comment>
        <owl:versionInfo>1:0</owl:versionInfo>
        <dc:creator>Francopoulo, Gil</dc:creator>
        <dcr:datcat rdf:resource="http://www.isocat.org/datcat/DC-1961"/>
        <rdfs:isDefinedBy rdf:resource="http://www.lexinfo.net/ontology/2.0/lexinfo"/>
    </owl:Thing>
    


    <!-- http://www.lexinfo.net/ontology/2.0/lexinfo#openParenthesis -->

    <owl:Thing rdf:about="&lexinfo;openParenthesis">
        <rdf:type rdf:resource="&lexinfo;PartOfSpeech"/>
        <rdf:type rdf:resource="&lexinfo;SymbolPOS"/>
        <rdf:type rdf:resource="&owl;NamedIndividual"/>
        <rdfs:label xml:lang="en">open parenthesis</rdfs:label>
        <rdfs:label xml:lang="ru">открывающая скобка</rdfs:label>        
        <dc:creator>Francopoulo, Gil</dc:creator>
        <rdfs:comment xml:lang="en">Beginning of a pair of parenthesis.</rdfs:comment>
        <rdfs:comment xml:lang="ru">Начальная скобка в паре круглых скобок.</rdfs:comment>
        <owl:versionInfo>1:0</owl:versionInfo>
        <dcr:datcat rdf:resource="http://www.isocat.org/datcat/DC-1442"/>
        <rdfs:isDefinedBy rdf:resource="http://www.lexinfo.net/ontology/2.0/lexinfo"/>
    </owl:Thing>
    


    <!-- http://www.lexinfo.net/ontology/2.0/lexinfo#optionalElement -->

    <owl:Thing rdf:about="&lexinfo;optionalElement">
        <rdf:type rdf:resource="&lexinfo;TermElement"/>
        <rdf:type rdf:resource="&owl;NamedIndividual"/>
        <rdfs:label xml:lang="en">optionalElement</rdfs:label>
        <rdfs:label xml:lang="ru">дополнительный элемент</rdfs:label>        
        <dc:creator>Wright, Sue Ellen</dc:creator>
        <owl:versionInfo>1:0</owl:versionInfo>
        <rdfs:comment xml:lang="en">1951: An optional part of a headword.
1951; examples? The question arises whether these are true options or whether the options reflect synonyms or hyponyms (e.g., barrage, barrage de retenue). The question is not whether 1951 should use this markup, but rather how to map this markup in a global environment.</rdfs:comment>
        <rdfs:comment xml:lang="ru">1951: Дополнительная часть заглавного слова.
Возникает вопрос, являются эти варианты истинными или отражают ли данные варианты синонимы или гипонимы (например, заграждение (barrage), заграждение для удержания (barrage de retenue). Вопрос заключается не в том, должен ли 1951 использовать эту разметку, а в том, как отразить данную разметку в глобальном  масштабе.</rdfs:comment>
        <dcr:datcat rdf:resource="http://www.isocat.org/datcat/DC-299"/>
        <rdfs:isDefinedBy rdf:resource="http://www.lexinfo.net/ontology/2.0/lexinfo"/>
    </owl:Thing>
    


    <!-- http://www.lexinfo.net/ontology/2.0/lexinfo#ordinalAdjective -->

    <owl:Thing rdf:about="&lexinfo;ordinalAdjective">
        <rdf:type rdf:resource="&lexinfo;AdjectivePOS"/>
        <rdf:type rdf:resource="&lexinfo;PartOfSpeech"/>
        <rdf:type rdf:resource="&owl;NamedIndividual"/>
        <rdfs:label xml:lang="en">ordinal adjective</rdfs:label>
        <rdfs:label xml:lang="ru">порядковое прилагательное</rdfs:label>        
        <rdfs:comment xml:lang="en">Adjective/numeral/number expressing a numeric ranking.</rdfs:comment>
        <rdfs:comment xml:lang="ru">Прилагательное/числительное/число, выражающее числовой порядок.</rdfs:comment>
        <dc:creator>Francopoulo, Gil</dc:creator>
        <owl:versionInfo>1:0</owl:versionInfo>
        <dcr:datcat rdf:resource="http://www.isocat.org/datcat/DC-1338"/>
        <rdfs:isDefinedBy rdf:resource="http://www.lexinfo.net/ontology/2.0/lexinfo"/>
    </owl:Thing>
    


    <!-- http://www.lexinfo.net/ontology/2.0/lexinfo#otherAnimacy -->

    <owl:Thing rdf:about="&lexinfo;otherAnimacy">
        <rdf:type rdf:resource="&lexinfo;Animacy"/>
        <rdf:type rdf:resource="&owl;NamedIndividual"/>
        <rdfs:label xml:lang="en">otherAnimacy</rdfs:label>
        <rdfs:label xml:lang="ru">другая одушевленность</rdfs:label>        
        <rdfs:label xml:lang="en">other animacy</rdfs:label>
        <rdfs:label xml:lang="ru">другая одушевленность</rdfs:label>        
        <owl:versionInfo>1:0</owl:versionInfo>
        <dc:creator>Francopoulo, Gil</dc:creator>
        <dc:creator>Wright, Sue Ellen</dc:creator>
        <rdfs:comment xml:lang="en">Perceived as related to animacy, but without specific reference to the previous items.</rdfs:comment>
        <rdfs:comment xml:lang="ru">Воспринимаемый как связанный с одушевленностью, но без специфического указания на предыдущие единицы.</rdfs:comment>        
        <dcr:datcat rdf:resource="http://www.isocat.org/datcat/DC-1953"/>
        <dcr:datcat rdf:resource="http://www.isocat.org/datcat/DC-81"/>
        <rdfs:isDefinedBy rdf:resource="http://www.lexinfo.net/ontology/2.0/lexinfo"/>
    </owl:Thing>
    


    <!-- http://www.lexinfo.net/ontology/2.0/lexinfo#otherGender -->

    <owl:Thing rdf:about="&lexinfo;otherGender">
        <rdf:type rdf:resource="&lexinfo;Gender"/>
        <rdf:type rdf:resource="&owl;NamedIndividual"/>
        <rdfs:label xml:lang="en">otherGender</rdfs:label>
        <rdfs:label xml:lang="ru">другой род</rdfs:label>        
        <dc:creator>Wright, Sue Ellen</dc:creator>
        <owl:versionInfo>1:0</owl:versionInfo>
        <rdfs:comment xml:lang="en">A grammatical category that indicates grammatical relationships between words in sentences.</rdfs:comment>
        <rdfs:comment xml:lang="ru">Грамматическая категория, указывающая на грамматические отношения между словами в предложении.</rdfs:comment>        
        <dcr:datcat rdf:resource="http://www.isocat.org/datcat/DC-249"/>
        <rdfs:isDefinedBy rdf:resource="http://www.lexinfo.net/ontology/2.0/lexinfo"/>
    </owl:Thing>
    


    <!-- http://www.lexinfo.net/ontology/2.0/lexinfo#otherNumber -->

    <owl:Thing rdf:about="&lexinfo;otherNumber">
        <rdf:type rdf:resource="&lexinfo;Number"/>
        <rdf:type rdf:resource="&owl;NamedIndividual"/>
        <rdfs:label xml:lang="en">otherNumber</rdfs:label>
        <rdfs:label xml:lang="ru">другое число</rdfs:label>        
        <owl:versionInfo>1:0</owl:versionInfo>
        <dc:creator>Wright, Sue Ellen</dc:creator>
        <rdfs:comment xml:lang="en">Designation used to classify number-related grammatical information that can differ from the standard European classifications cited above.</rdfs:comment>
        <rdfs:comment xml:lang="ru">Обозначение, используемое для классификации грамматической информации, связанной с числом, которая может отличаться от стандартной европейских классов, приведенных выше.</rdfs:comment>
        <dcr:datcat rdf:resource="http://www.isocat.org/datcat/DC-256"/>
        <rdfs:isDefinedBy rdf:resource="http://www.lexinfo.net/ontology/2.0/lexinfo"/>
    </owl:Thing>
    


    <!-- http://www.lexinfo.net/ontology/2.0/lexinfo#outdatedForm -->

    <owl:Thing rdf:about="&lexinfo;outdatedForm">
        <rdf:type rdf:resource="&lexinfo;TemporalQualifier"/>
        <rdf:type rdf:resource="&owl;NamedIndividual"/>
        <rdfs:label xml:lang="en">outdated form</rdfs:label>
        <rdfs:label xml:lang="ru">устаревшая форма</rdfs:label>        
        <owl:versionInfo>1:0</owl:versionInfo>
        <rdfs:comment xml:lang="en">A term or lexeme that has fallen from fashion, but the meaning of which is readily recognizable.</rdfs:comment>
        <rdfs:comment xml:lang="ru">Термин или лексема, вышедшая из употребления, но легко узнаваемая.</rdfs:comment>
        <dc:creator>Wright, Sue Ellen</dc:creator>
        <dcr:datcat rdf:resource="http://www.isocat.org/datcat/DC-505"/>
        <rdfs:isDefinedBy rdf:resource="http://www.lexinfo.net/ontology/2.0/lexinfo"/>
    </owl:Thing>
    


    <!-- http://www.lexinfo.net/ontology/2.0/lexinfo#partNumber -->

    <owl:Thing rdf:about="&lexinfo;partNumber">
        <rdf:type rdf:resource="&lexinfo;TermType"/>
        <rdf:type rdf:resource="&owl;NamedIndividual"/>
        <rdfs:label xml:lang="en">part number</rdfs:label>
        <rdfs:label xml:lang="ru">номер детали</rdfs:label>        
        <rdfs:comment xml:lang="en">A unique alphanumeric designation assigned to an object in a manufacturing system.</rdfs:comment>
        <rdfs:comment xml:lang="ru">Уникальное буквенно-числовое обозначение, приписанное объекту в производственной системе.</rdfs:comment>        
        <owl:versionInfo>1:0</owl:versionInfo>
        <dc:creator>Wright, Sue Ellen</dc:creator>
        <dcr:datcat rdf:resource="http://www.isocat.org/datcat/DC-338"/>
        <rdfs:isDefinedBy rdf:resource="http://www.lexinfo.net/ontology/2.0/lexinfo"/>
    </owl:Thing>
    


    <!-- http://www.lexinfo.net/ontology/2.0/lexinfo#participle -->

    <owl:Thing rdf:about="&lexinfo;participle">
        <rdf:type rdf:resource="&lexinfo;VerbFormMood"/>
        <rdf:type rdf:resource="&owl;NamedIndividual"/>
        <rdfs:label xml:lang="en">participle</rdfs:label>
        <rdfs:label xml:lang="ru">причастие</rdfs:label>        
        <dc:creator>Francopoulo, Gil</dc:creator>
        <owl:versionInfo>1:0</owl:versionInfo>
        <rdfs:comment xml:lang="en">Term referring to a word derived from a verb and used as an adjective.</rdfs:comment>
        <rdfs:comment xml:lang="ru">Термин, относящийся к слову, производному от глагола и используемому как прилагательное.</rdfs:comment>        
        <dcr:datcat rdf:resource="http://www.isocat.org/datcat/DC-1341"/>
        <rdfs:isDefinedBy rdf:resource="http://www.lexinfo.net/ontology/2.0/lexinfo"/>
    </owl:Thing>
    


    <!-- http://www.lexinfo.net/ontology/2.0/lexinfo#participleAdjective -->

    <owl:Thing rdf:about="&lexinfo;participleAdjective">
        <rdf:type rdf:resource="&lexinfo;AdjectivePOS"/>
        <rdf:type rdf:resource="&lexinfo;PartOfSpeech"/>
        <rdf:type rdf:resource="&owl;NamedIndividual"/>
        <rdfs:label xml:lang="en">participle adjective</rdfs:label>
        <rdfs:label xml:lang="ru">отглагольное прилагательное</rdfs:label>        
        <rdfs:comment xml:lang="en">Adjective based on a verb.</rdfs:comment>
        <rdfs:comment xml:lang="ru">Прилагательное, образованное от глагола.</rdfs:comment>
        <owl:versionInfo>1:0</owl:versionInfo>
        <dc:creator>Francopoulo, Gil</dc:creator>
        <dcr:datcat rdf:resource="http://www.isocat.org/datcat/DC-1598"/>
        <rdfs:isDefinedBy rdf:resource="http://www.lexinfo.net/ontology/2.0/lexinfo"/>
    </owl:Thing>
    


    <!-- http://www.lexinfo.net/ontology/2.0/lexinfo#particle -->

    <owl:Thing rdf:about="&lexinfo;particle">
        <rdf:type rdf:resource="&lexinfo;PartOfSpeech"/>
        <rdf:type rdf:resource="&lexinfo;ParticlePOS"/>
        <rdf:type rdf:resource="&owl;NamedIndividual"/>
        <rdfs:label xml:lang="en">particle</rdfs:label>
        <rdfs:label xml:lang="ru">частица</rdfs:label>        
        <owl:versionInfo>1:0</owl:versionInfo>
        <dc:creator>Francopoulo, Gil</dc:creator>
        <rdfs:comment xml:lang="en">Word that does not belong to one of the main classes of words, is invariable in form, and typically has grammatical or pragmatic meaning.</rdfs:comment>
        <rdfs:comment xml:lang="ru">Неизменяемое слово, не принадлежащее  ни к одной  значимых частей речи и обычно имеющее грамматическое или прагматическое значение.</rdfs:comment>
        <dcr:datcat rdf:resource="http://www.isocat.org/datcat/DC-1342"/>
        <rdfs:isDefinedBy rdf:resource="http://www.lexinfo.net/ontology/2.0/lexinfo"/>
    </owl:Thing>
    


    <!-- http://www.lexinfo.net/ontology/2.0/lexinfo#partitiveArticle -->

    <owl:Thing rdf:about="&lexinfo;partitiveArticle">
        <rdf:type rdf:resource="&lexinfo;ArticlePOS"/>
        <rdf:type rdf:resource="&lexinfo;PartOfSpeech"/>
        <rdf:type rdf:resource="&owl;NamedIndividual"/>
        <rdfs:label xml:lang="en">partitive article</rdfs:label>
        <rdfs:label xml:lang="ru">партитивный артикль</rdfs:label>        
        <owl:versionInfo>1:0</owl:versionInfo>
        <rdfs:comment xml:lang="en">Article expressing a part or quantity.</rdfs:comment>
        <rdfs:comment xml:lang="ru">Артикль, выражающий часть или количество.</rdfs:comment>
        <dc:creator>Francopoulo, Gil</dc:creator>
        <dcr:datcat rdf:resource="http://www.isocat.org/datcat/DC-1898"/>
        <rdfs:isDefinedBy rdf:resource="http://www.lexinfo.net/ontology/2.0/lexinfo"/>
    </owl:Thing>
    


    <!-- http://www.lexinfo.net/ontology/2.0/lexinfo#partitiveCase -->

    <owl:Thing rdf:about="&lexinfo;partitiveCase">
        <rdf:type rdf:resource="&lexinfo;Case"/>
        <rdf:type rdf:resource="&owl;NamedIndividual"/>
        <rdfs:label xml:lang="en">partitive case</rdfs:label>
        <rdfs:label xml:lang="ru">партитивный падеж</rdfs:label>        
        <dc:creator>Francopoulo, Gil</dc:creator>
        <owl:versionInfo>1:0</owl:versionInfo>
        <rdfs:comment xml:lang="en">Case that expresses the partial nature of the referent of the noun it marks, as opposed to expressing the whole unit or class of which the referent is a part.</rdfs:comment>
        <rdfs:comment xml:lang="ru">Падеж, выражающий неполную природу референта указываемого им существительного, в противоположность выражению целой единицы или класса, частью которого  является референт.</rdfs:comment>
        <dcr:datcat rdf:resource="http://www.isocat.org/datcat/DC-2003"/>
        <rdfs:isDefinedBy rdf:resource="http://www.lexinfo.net/ontology/2.0/lexinfo"/>
    </owl:Thing>
    


    <!-- http://www.lexinfo.net/ontology/2.0/lexinfo#passiveVoice -->

    <owl:Thing rdf:about="&lexinfo;passiveVoice">
        <rdf:type rdf:resource="&lexinfo;Voice"/>
        <rdf:type rdf:resource="&owl;NamedIndividual"/>
        <rdfs:label xml:lang="en">passive voice</rdfs:label>
        <rdfs:label xml:lang="ru">страдательный залог</rdfs:label>        
        <rdfs:comment xml:lang="en">Term referring to a situation where the grammatical subject is typically the recipient or goal of the action denoted by the verb.</rdfs:comment>
        <rdfs:comment xml:lang="ru">Термин, относящийся к ситуации, где грамматическое подлежащее обычно является реципиентом или целью действия, обозначаемого глаголом.</rdfs:comment>
        <dc:creator>Francopoulo, Gil</dc:creator>
        <owl:versionInfo>1:0</owl:versionInfo>
        <dcr:datcat rdf:resource="http://www.isocat.org/datcat/DC-1346"/>
        <rdfs:isDefinedBy rdf:resource="http://www.lexinfo.net/ontology/2.0/lexinfo"/>
    </owl:Thing>
    


    <!-- http://www.lexinfo.net/ontology/2.0/lexinfo#past -->

    <owl:Thing rdf:about="&lexinfo;past">
        <rdf:type rdf:resource="&lexinfo;Tense"/>
        <rdf:type rdf:resource="&owl;NamedIndividual"/>
        <rdfs:label xml:lang="en">past</rdfs:label>
        <rdfs:label xml:lang="ru">прошедшее</rdfs:label>        
        <rdfs:comment xml:lang="en">Past tense is an absolute tense that refers to a time before the moment of utterance.</rdfs:comment>
        <rdfs:comment xml:lang="ru">Прошедшее время является абсолютным временем, которое обозначает время, предшествующее моменту высказывания.</rdfs:comment>        
        <dc:creator>Francopoulo, Gil</dc:creator>
        <owl:versionInfo>1:0</owl:versionInfo>
        <dcr:datcat rdf:resource="http://www.isocat.org/datcat/DC-1347"/>
        <rdfs:isDefinedBy rdf:resource="http://www.lexinfo.net/ontology/2.0/lexinfo"/>
    </owl:Thing>
    


    <!-- http://www.lexinfo.net/ontology/2.0/lexinfo#pastParticipleAdjective -->

    <owl:Thing rdf:about="&lexinfo;pastParticipleAdjective">
        <rdf:type rdf:resource="&lexinfo;AdjectivePOS"/>
        <rdf:type rdf:resource="&lexinfo;PartOfSpeech"/>
        <rdf:type rdf:resource="&owl;NamedIndividual"/>
        <rdfs:label xml:lang="en">past participle adjective</rdfs:label>
        <rdfs:label xml:lang="ru">прилагательное от причастия прошедшего времени</rdfs:label>        
        <dc:creator>Francopoulo, Gil</dc:creator>
        <owl:versionInfo>1:0</owl:versionInfo>
        <rdfs:comment xml:lang="en">Adjective based on a past participle.</rdfs:comment>
        <rdfs:comment xml:lang="ru">Прилагательное, основанное на причастии прошедшего времени.</rdfs:comment>        
        <dcr:datcat rdf:resource="http://www.isocat.org/datcat/DC-1596"/>
        <rdfs:isDefinedBy rdf:resource="http://www.lexinfo.net/ontology/2.0/lexinfo"/>
    </owl:Thing>
    


    <!-- http://www.lexinfo.net/ontology/2.0/lexinfo#paucal -->

    <owl:Thing rdf:about="&lexinfo;paucal">
        <rdf:type rdf:resource="&lexinfo;Number"/>
        <rdf:type rdf:resource="&owl;NamedIndividual"/>
        <rdfs:label xml:lang="en">paucal</rdfs:label>
        <rdfs:label xml:lang="ru">несколько</rdfs:label>        
        <rdfs:comment xml:lang="en">Number that specifies &apos;a few&apos; things.</rdfs:comment>
        <rdfs:comment xml:lang="ru">Число, указывающее на несколько вещей.</rdfs:comment>
        <dc:creator>Francopoulo, Gil</dc:creator>
        <owl:versionInfo>1:0</owl:versionInfo>
        <dcr:datcat rdf:resource="http://www.isocat.org/datcat/DC-1350"/>
        <rdfs:isDefinedBy rdf:resource="http://www.lexinfo.net/ontology/2.0/lexinfo"/>
    </owl:Thing>
    


    <!-- http://www.lexinfo.net/ontology/2.0/lexinfo#perfective -->

    <owl:Thing rdf:about="&lexinfo;perfective">
        <rdf:type rdf:resource="&lexinfo;Aspect"/>
        <rdf:type rdf:resource="&owl;NamedIndividual"/>
        <rdfs:label xml:lang="en">perfective</rdfs:label>
        <rdfs:label xml:lang="ru">совершенный</rdfs:label>        
        <dc:creator>Francopoulo, Gil</dc:creator>
        <owl:versionInfo>1:0</owl:versionInfo>
        <rdfs:comment xml:lang="en">Perfective aspect is an aspect that expresses a temporal view of an event or state as a simple whole, apart from the consideration of the internal structure of the time in which it occurs.</rdfs:comment>
        <rdfs:comment xml:lang="ru">Совершенный вид представляет собой вид, выражающий темпоральный вид события или состояния как простое целое, отдельно от рассмотрения внутренней структуры времени, в которое оно происходит.</rdfs:comment>
        <dcr:datcat rdf:resource="http://www.isocat.org/datcat/DC-1352"/>
        <rdfs:isDefinedBy rdf:resource="http://www.lexinfo.net/ontology/2.0/lexinfo"/>
    </owl:Thing>
    


    <!-- http://www.lexinfo.net/ontology/2.0/lexinfo#personal -->

    <owl:Thing rdf:about="&lexinfo;personal">
        <rdf:type rdf:resource="&lexinfo;ReferentType"/>
        <rdf:type rdf:resource="&owl;NamedIndividual"/>
        <rdfs:label xml:lang="en">personal</rdfs:label>
        <rdfs:label xml:lang="ru">личное</rdfs:label>        
        <dc:creator>Francopoulo, Gil</dc:creator>
        <owl:versionInfo>1:0</owl:versionInfo>
        <rdfs:comment xml:lang="en">Property that refers to the person.</rdfs:comment>
        <rdfs:comment xml:lang="ru">Свойство, относящееся к лицу.</rdfs:comment>        
        <dcr:datcat rdf:resource="http://www.isocat.org/datcat/DC-1946"/>
        <rdfs:isDefinedBy rdf:resource="http://www.lexinfo.net/ontology/2.0/lexinfo"/>
    </owl:Thing>
    


    <!-- http://www.lexinfo.net/ontology/2.0/lexinfo#personalPronoun -->

    <owl:Thing rdf:about="&lexinfo;personalPronoun">
        <rdf:type rdf:resource="&lexinfo;PartOfSpeech"/>
        <rdf:type rdf:resource="&lexinfo;PronounPOS"/>
        <rdf:type rdf:resource="&owl;NamedIndividual"/>
        <rdfs:label xml:lang="en">personal pronoun</rdfs:label>
        <rdfs:label xml:lang="ru">личное местоимение</rdfs:label>        
        <dc:creator>Francopoulo, Gil</dc:creator>
        <rdfs:comment xml:lang="en">Pronoun referring a person.</rdfs:comment>
        <rdfs:comment xml:lang="ru">Местоимение, относящееся к лицу.</rdfs:comment>        
        <owl:versionInfo>1:0</owl:versionInfo>
        <dcr:datcat rdf:resource="http://www.isocat.org/datcat/DC-1463"/>
        <rdfs:isDefinedBy rdf:resource="http://www.lexinfo.net/ontology/2.0/lexinfo"/>
    </owl:Thing>
    


    <!-- http://www.lexinfo.net/ontology/2.0/lexinfo#phraseologicalUnit -->

    <owl:Thing rdf:about="&lexinfo;phraseologicalUnit">
        <rdf:type rdf:resource="&lexinfo;TermType"/>
        <rdf:type rdf:resource="&owl;NamedIndividual"/>
        <rdfs:label xml:lang="en">phraseological unit</rdfs:label>
        <rdfs:label xml:lang="ru">фразеологическая единица</rdfs:label>        
        <dc:creator>Wright, Sue Ellen</dc:creator>
        <owl:versionInfo>1:0</owl:versionInfo>
        <rdfs:comment xml:lang="en">Any group of two or more words that form a unit, the meaning of which frequently cannot be deduced based on the combined sense of the words making up the phrase.</rdfs:comment>
        <rdfs:comment xml:lang="ru">Любое сочетание, состоящее из двух или более слов, образующих единство, значение которого часто не может быть выведено, на основании общего смысла слов, составляющих сочетание.</rdfs:comment>
        <dcr:datcat rdf:resource="http://www.isocat.org/datcat/DC-339"/>
        <rdfs:isDefinedBy rdf:resource="http://www.lexinfo.net/ontology/2.0/lexinfo"/>
    </owl:Thing>
    


    <!-- http://www.lexinfo.net/ontology/2.0/lexinfo#plainVerb -->

    <owl:Thing rdf:about="&lexinfo;plainVerb">
        <rdf:type rdf:resource="&lexinfo;PartOfSpeech"/>
        <rdf:type rdf:resource="&lexinfo;VerbPOS"/>
        <rdf:type rdf:resource="&owl;NamedIndividual"/>
        <rdfs:label xml:lang="en">plain verb</rdfs:label>
        <rdfs:label xml:lang="ru">простой глагол</rdfs:label>
        <dc:creator>Francopoulo, Gil</dc:creator>
        <owl:versionInfo>1:0</owl:versionInfo>
        <rdfs:comment xml:lang="en">verb which has its own semantics</rdfs:comment>
        <rdfs:comment xml:lang="ru">Глагол со своей собственной семантикой.</rdfs:comment>
        <dcr:datcat rdf:resource="http://www.isocat.org/datcat/DC-3004"/>
        <rdfs:isDefinedBy rdf:resource="http://www.lexinfo.net/ontology/2.0/lexinfo"/>
    </owl:Thing>
    


    <!-- http://www.lexinfo.net/ontology/2.0/lexinfo#plural -->

    <owl:Thing rdf:about="&lexinfo;plural">
        <rdf:type rdf:resource="&lexinfo;Number"/>
        <rdf:type rdf:resource="&owl;NamedIndividual"/>
        <rdfs:label xml:lang="en">plural</rdfs:label>
        <rdfs:label xml:lang="ru">множественное</rdfs:label>        
        <rdfs:comment xml:lang="en">The form of a term or word (usually of a noun) used to designate more than one object.</rdfs:comment>
        <rdfs:comment xml:lang="ru">Форма термина или слова (обычно существительного), используемого для обозначения более чем одного объекта.</rdfs:comment>
        <rdfs:comment xml:lang="en">Value that expresses more than one element.</rdfs:comment>
        <rdfs:comment xml:lang="ru">Значение, выражающее, что элементов больше, чем один.</rdfs:comment>        
        <dc:creator>Wright, Sue Ellen</dc:creator>
        <owl:versionInfo>1:0</owl:versionInfo>
        <dc:creator>Francopoulo, Gil</dc:creator>
        <dcr:datcat rdf:resource="http://www.isocat.org/datcat/DC-1354"/>
        <dcr:datcat rdf:resource="http://www.isocat.org/datcat/DC-253"/>
        <rdfs:isDefinedBy rdf:resource="http://www.lexinfo.net/ontology/2.0/lexinfo"/>
    </owl:Thing>
    


    <!-- http://www.lexinfo.net/ontology/2.0/lexinfo#point -->

    <owl:Thing rdf:about="&lexinfo;point">
        <rdf:type rdf:resource="&lexinfo;PartOfSpeech"/>
        <rdf:type rdf:resource="&lexinfo;SymbolPOS"/>
        <rdf:type rdf:resource="&owl;NamedIndividual"/>
        <rdfs:label xml:lang="en">point</rdfs:label>
        <rdfs:label xml:lang="ru">точка</rdfs:label>        
        <rdfs:comment xml:lang="en">Sign (.) used to expresses the end of a sentence or an abbreviation.</rdfs:comment>
        <rdfs:comment xml:lang="ru">Знак (.), используемый для обозначения конца предложения или аббревиатуры.</rdfs:comment>
        <owl:versionInfo>1:0</owl:versionInfo>
        <dc:creator>Francopoulo, Gil</dc:creator>
        <dcr:datcat rdf:resource="http://www.isocat.org/datcat/DC-1445"/>
        <rdfs:isDefinedBy rdf:resource="http://www.lexinfo.net/ontology/2.0/lexinfo"/>
    </owl:Thing>
    


    <!-- http://www.lexinfo.net/ontology/2.0/lexinfo#positive -->

    <owl:Thing rdf:about="&lexinfo;positive">
        <rdf:type rdf:resource="&lexinfo;Degree"/>
        <rdf:type rdf:resource="&owl;NamedIndividual"/>
        <rdfs:label xml:lang="en">positive</rdfs:label>
        <rdfs:label xml:lang="ru">положительная</rdfs:label>        
        <dc:creator>Francopoulo, Gil</dc:creator>
        <owl:versionInfo>1:0</owl:versionInfo>
        <rdfs:comment xml:lang="en">Value used in a comparison relationship when no comparison is involved.</rdfs:comment>
        <rdfs:comment xml:lang="ru">Значение, используемое в отношениях сравнения, когда не подразумевается сравнение.</rdfs:comment>        
        <dcr:datcat rdf:resource="http://www.isocat.org/datcat/DC-1420"/>
        <rdfs:isDefinedBy rdf:resource="http://www.lexinfo.net/ontology/2.0/lexinfo"/>
    </owl:Thing>
    


    <!-- http://www.lexinfo.net/ontology/2.0/lexinfo#possessive -->

    <owl:Thing rdf:about="&lexinfo;possessive">
        <rdf:type rdf:resource="&lexinfo;ReferentType"/>
        <rdf:type rdf:resource="&owl;NamedIndividual"/>
        <rdfs:label xml:lang="en">possessive</rdfs:label>
        <rdfs:label xml:lang="ru">притяжательное</rdfs:label>        
        <owl:versionInfo>1:0</owl:versionInfo>
        <rdfs:comment xml:lang="en">Relative to the possession or association.</rdfs:comment>
        <rdfs:comment xml:lang="ru">Относящееся к обладанию или связи.</rdfs:comment>
        <dc:creator>Francopoulo, Gil</dc:creator>
        <dcr:datcat rdf:resource="http://www.isocat.org/datcat/DC-1355"/>
        <rdfs:isDefinedBy rdf:resource="http://www.lexinfo.net/ontology/2.0/lexinfo"/>
    </owl:Thing>
    


    <!-- http://www.lexinfo.net/ontology/2.0/lexinfo#possessiveAdjective -->

    <owl:Thing rdf:about="&lexinfo;possessiveAdjective">
        <rdf:type rdf:resource="&lexinfo;AdjectivePOS"/>
        <rdf:type rdf:resource="&lexinfo;PartOfSpeech"/>
        <rdf:type rdf:resource="&owl;NamedIndividual"/>
        <rdfs:label xml:lang="en">possessive adjective</rdfs:label>
        <rdfs:label xml:lang="ru">притяжательное прилагательное</rdfs:label>        
        <owl:versionInfo>1:0</owl:versionInfo>
        <rdfs:comment xml:lang="en">An adjective derived from a noun and denoting possession by the object described by the noun.</rdfs:comment>
        <rdfs:comment xml:lang="ru">Прилагательное, образованное от существительного и обозначающее обладание объектом, выраженным существительным.</rdfs:comment>
        <dc:creator>Zeman, Dan</dc:creator>
        <dcr:datcat rdf:resource="http://www.isocat.org/datcat/DC-3017"/>
        <rdfs:isDefinedBy rdf:resource="http://www.lexinfo.net/ontology/2.0/lexinfo"/>
    </owl:Thing>
    


    <!-- http://www.lexinfo.net/ontology/2.0/lexinfo#possessiveDeterminer -->

    <owl:Thing rdf:about="&lexinfo;possessiveDeterminer">
        <rdf:type rdf:resource="&lexinfo;DeterminerPOS"/>
        <rdf:type rdf:resource="&lexinfo;PartOfSpeech"/>
        <rdf:type rdf:resource="&owl;NamedIndividual"/>
        <rdfs:label xml:lang="en">possessive determiner</rdfs:label>
        <rdfs:label xml:lang="ru">определитель притяжательности</rdfs:label>        
        <dc:creator>Francopoulo, Gil</dc:creator>
        <rdfs:comment xml:lang="en">Determiner that expresses ownership.</rdfs:comment>
        <rdfs:comment xml:lang="ru">Определитель, выражающий обладание.</rdfs:comment>        
        <owl:versionInfo>1:0</owl:versionInfo>
        <dcr:datcat rdf:resource="http://www.isocat.org/datcat/DC-1357"/>
        <rdfs:isDefinedBy rdf:resource="http://www.lexinfo.net/ontology/2.0/lexinfo"/>
    </owl:Thing>
    


    <!-- http://www.lexinfo.net/ontology/2.0/lexinfo#possessiveParticle -->

    <owl:Thing rdf:about="&lexinfo;possessiveParticle">
        <rdf:type rdf:resource="&lexinfo;PartOfSpeech"/>
        <rdf:type rdf:resource="&lexinfo;ParticlePOS"/>
        <rdf:type rdf:resource="&owl;NamedIndividual"/>
        <rdfs:label xml:lang="en">possessive particle</rdfs:label>
        <rdfs:label xml:lang="ru">притяжательная частица</rdfs:label>        
        <rdfs:comment xml:lang="en">Particle expressing ownship.</rdfs:comment>
        <rdfs:comment xml:lang="ru">Частица, выражающая обладание.</rdfs:comment>        
        <owl:versionInfo>1:0</owl:versionInfo>
        <dc:creator>Francopoulo, Gil</dc:creator>
        <dcr:datcat rdf:resource="http://www.isocat.org/datcat/DC-1895"/>
        <rdfs:isDefinedBy rdf:resource="http://www.lexinfo.net/ontology/2.0/lexinfo"/>
    </owl:Thing>
    


    <!-- http://www.lexinfo.net/ontology/2.0/lexinfo#possessivePronoun -->

    <owl:Thing rdf:about="&lexinfo;possessivePronoun">
        <rdf:type rdf:resource="&lexinfo;PartOfSpeech"/>
        <rdf:type rdf:resource="&lexinfo;PronounPOS"/>
        <rdf:type rdf:resource="&owl;NamedIndividual"/>
        <rdfs:label xml:lang="en">possessive pronoun</rdfs:label>
        <rdfs:label xml:lang="ru">притяжательное местоимение</rdfs:label>        
        <rdfs:comment xml:lang="en">Pronoun that expresses ownership and relationships like ownership, such as kinship, and other forms of association.</rdfs:comment>
        <rdfs:comment xml:lang="ru">Местоимение, выражающее обладание или отношение, похожее на обладание такое, как родство и другие формы связи.</rdfs:comment>
        <owl:versionInfo>1:0</owl:versionInfo>
        <dc:creator>Francopoulo, Gil</dc:creator>
        <dcr:datcat rdf:resource="http://www.isocat.org/datcat/DC-1359"/>
        <rdfs:isDefinedBy rdf:resource="http://www.lexinfo.net/ontology/2.0/lexinfo"/>
    </owl:Thing>
    


    <!-- http://www.lexinfo.net/ontology/2.0/lexinfo#possessiveRelativePronoun -->

    <owl:Thing rdf:about="&lexinfo;possessiveRelativePronoun">
        <rdf:type rdf:resource="&lexinfo;PartOfSpeech"/>
        <rdf:type rdf:resource="&lexinfo;PronounPOS"/>
        <rdf:type rdf:resource="&owl;NamedIndividual"/>
        <rdfs:label xml:lang="en">possessive relative pronoun</rdfs:label>
        <rdfs:label xml:lang="ru">притяжательное относительное местоимение</rdfs:label>        
        <rdfs:comment xml:lang="en">A relative pronoun whose antecedent is the possessor of the subject or object in the relative clause.</rdfs:comment>
        <rdfs:comment xml:lang="ru">Относительное местоимение, чей антецедент является обладателем субъекта или объекта в относительном придаточном предложении.</rdfs:comment>        
        <dc:creator>Zeman, Dan</dc:creator>
        <owl:versionInfo>1:0</owl:versionInfo>
        <dcr:datcat rdf:resource="http://www.isocat.org/datcat/DC-3005"/>
        <rdfs:isDefinedBy rdf:resource="http://www.lexinfo.net/ontology/2.0/lexinfo"/>
    </owl:Thing>
    


    <!-- http://www.lexinfo.net/ontology/2.0/lexinfo#postModifier -->

    <owl:Thing rdf:about="&lexinfo;postModifier">
        <rdf:type rdf:resource="&lexinfo;ModificationType"/>
        <rdf:type rdf:resource="&owl;NamedIndividual"/>
        <rdfs:label xml:lang="en">post modifier</rdfs:label>
        <rdfs:label xml:lang="ru">определение в постпозиции</rdfs:label>        
        <rdfs:comment xml:lang="en">Situation where the modifier is after the modified.</rdfs:comment>
        <rdfs:comment xml:lang="ru">Ситуация, в которой определение стоит после определяемого.</rdfs:comment>
        <dc:creator>Francopoulo, Gil</dc:creator>
        <owl:versionInfo>1:0</owl:versionInfo>
        <dcr:datcat rdf:resource="http://www.isocat.org/datcat/DC-1945"/>
        <rdfs:isDefinedBy rdf:resource="http://www.lexinfo.net/ontology/2.0/lexinfo"/>
    </owl:Thing>
    


    <!-- http://www.lexinfo.net/ontology/2.0/lexinfo#postposition -->

    <owl:Thing rdf:about="&lexinfo;postposition">
        <rdf:type rdf:resource="&lexinfo;AdpositionPOS"/>
        <rdf:type rdf:resource="&lexinfo;PartOfSpeech"/>
        <rdf:type rdf:resource="&owl;NamedIndividual"/>
        <rdfs:label xml:lang="en">postposition</rdfs:label>
        <rdfs:label xml:lang="ru">постпозиция</rdfs:label>        
        <rdfs:comment xml:lang="en">Adposition that appears at the end of the noun phrase.</rdfs:comment>
        <rdfs:comment xml:lang="ru">Предлог, стоящий в конце именной группы.</rdfs:comment>
        <owl:versionInfo>1:0</owl:versionInfo>
        <dc:creator>Francopoulo, Gil</dc:creator>
        <dcr:datcat rdf:resource="http://www.isocat.org/datcat/DC-1360"/>
        <rdfs:isDefinedBy rdf:resource="http://www.lexinfo.net/ontology/2.0/lexinfo"/>
    </owl:Thing>
    


    <!-- http://www.lexinfo.net/ontology/2.0/lexinfo#preModifier -->

    <owl:Thing rdf:about="&lexinfo;preModifier">
        <rdf:type rdf:resource="&lexinfo;ModificationType"/>
        <rdf:type rdf:resource="&owl;NamedIndividual"/>
        <rdfs:label xml:lang="en">premodifier</rdfs:label>
        <rdfs:label xml:lang="ru">определение в препозиции</rdfs:label>        
        <owl:versionInfo>1:0</owl:versionInfo>
        <rdfs:comment xml:lang="en">Situation where the modifier is before the modified.</rdfs:comment>
        <rdfs:comment xml:lang="ru">Ситуация, в которой определение стоит перед определяемым.</rdfs:comment>
        <dc:creator>Francopoulo, Gil</dc:creator>
        <dcr:datcat rdf:resource="http://www.isocat.org/datcat/DC-1943"/>
        <rdfs:isDefinedBy rdf:resource="http://www.lexinfo.net/ontology/2.0/lexinfo"/>
    </owl:Thing>
    


    <!-- http://www.lexinfo.net/ontology/2.0/lexinfo#preferredTerm -->

    <owl:Thing rdf:about="&lexinfo;preferredTerm">
        <rdf:type rdf:resource="&lexinfo;NormativeAuthorization"/>
        <rdf:type rdf:resource="&owl;NamedIndividual"/>
        <rdfs:label xml:lang="en">preferred term</rdfs:label>
        <rdfs:label xml:lang="ru">предпочтительный термин</rdfs:label>        
        <dc:creator>Wright, Sue Ellen</dc:creator>
        <owl:versionInfo>1:0</owl:versionInfo>
        <rdfs:comment xml:lang="en">A term rated according to the scale of a term acceptability rating as the primary term for a given concept.</rdfs:comment>
        <rdfs:comment xml:lang="ru">Термин, который по шкале приемлемости терминов расценивается как первоочередной для данного понятия.</rdfs:comment>
        <dcr:datcat rdf:resource="http://www.isocat.org/datcat/DC-376"/>
        <rdfs:isDefinedBy rdf:resource="http://www.lexinfo.net/ontology/2.0/lexinfo"/>
    </owl:Thing>
    


    <!-- http://www.lexinfo.net/ontology/2.0/lexinfo#prefix -->

    <owl:Thing rdf:about="&lexinfo;prefix">
        <rdf:type rdf:resource="&lexinfo;TermElement"/>
        <rdf:type rdf:resource="&owl;NamedIndividual"/>
        <rdfs:isDefinedBy rdf:resource="http://www.lexinfo.net/ontology/2.0/lexinfo"/>
    </owl:Thing>
    


    <!-- http://www.lexinfo.net/ontology/2.0/lexinfo#preposition -->

    <owl:Thing rdf:about="&lexinfo;preposition">
        <rdf:type rdf:resource="&lexinfo;AdpositionPOS"/>
        <rdf:type rdf:resource="&lexinfo;PartOfSpeech"/>
        <rdf:type rdf:resource="&owl;NamedIndividual"/>
        <rdfs:label xml:lang="en">preposition</rdfs:label>
        <rdfs:label xml:lang="ru">предлог</rdfs:label>        
        <dc:creator>Francopoulo, Gil</dc:creator>
        <rdfs:comment xml:lang="en">Adposition placed at the beginning of a noun phrase.</rdfs:comment>
        <rdfs:comment xml:lang="ru">Предлог, поставленный в начало именной фразы.</rdfs:comment>        
        <owl:versionInfo>1:0</owl:versionInfo>
        <dcr:datcat rdf:resource="http://www.isocat.org/datcat/DC-1366"/>
        <rdfs:isDefinedBy rdf:resource="http://www.lexinfo.net/ontology/2.0/lexinfo"/>
    </owl:Thing>
    


    <!-- http://www.lexinfo.net/ontology/2.0/lexinfo#prepositionalAdverb -->

    <owl:Thing rdf:about="&lexinfo;prepositionalAdverb">
        <rdf:type rdf:resource="&lexinfo;AdverbPOS"/>
        <rdf:type rdf:resource="&lexinfo;PartOfSpeech"/>
        <rdf:type rdf:resource="&owl;NamedIndividual"/>
        <rdfs:label xml:lang="en">prepositional adverb</rdfs:label>
        <rdfs:label xml:lang="ru">наречие в препозиции</rdfs:label>        
        <owl:versionInfo>1:0</owl:versionInfo>
        <dc:creator>Francopoulo, Gil</dc:creator>
        <rdfs:comment xml:lang="en">adverb which is very similar in its form to a preposition</rdfs:comment>
        <rdfs:comment xml:lang="ru">Наречие, по своей форме очень схожее с предлогом.</rdfs:comment>        
        <dcr:datcat rdf:resource="http://www.isocat.org/datcat/DC-3000"/>
        <rdfs:isDefinedBy rdf:resource="http://www.lexinfo.net/ontology/2.0/lexinfo"/>
    </owl:Thing>
    


    <!-- http://www.lexinfo.net/ontology/2.0/lexinfo#present -->

    <owl:Thing rdf:about="&lexinfo;present">
        <rdf:type rdf:resource="&lexinfo;Tense"/>
        <rdf:type rdf:resource="&owl;NamedIndividual"/>
        <rdfs:label xml:lang="en">present</rdfs:label>
        <rdfs:label xml:lang="ru">настоящее</rdfs:label>        
        <dc:creator>Francopoulo, Gil</dc:creator>
        <rdfs:comment xml:lang="en">Verb tense that indicates action or state of being in the present.</rdfs:comment>
        <rdfs:comment xml:lang="ru">Время глагола, обозначающее действие или состояние присутствия в настоящем.</rdfs:comment>
        <owl:versionInfo>1:0</owl:versionInfo>
        <dcr:datcat rdf:resource="http://www.isocat.org/datcat/DC-1367"/>
        <rdfs:isDefinedBy rdf:resource="http://www.lexinfo.net/ontology/2.0/lexinfo"/>
    </owl:Thing>
    


    <!-- http://www.lexinfo.net/ontology/2.0/lexinfo#presentParticipleAdjective -->

    <owl:Thing rdf:about="&lexinfo;presentParticipleAdjective">
        <rdf:type rdf:resource="&lexinfo;AdjectivePOS"/>
        <rdf:type rdf:resource="&lexinfo;PartOfSpeech"/>
        <rdf:type rdf:resource="&owl;NamedIndividual"/>
        <rdfs:label xml:lang="en">present participle adjective</rdfs:label>
        <rdfs:label xml:lang="ru">прилагательное от причастия настоящего времени</rdfs:label>        
        <rdfs:comment xml:lang="en">Adjective based on a present participle.</rdfs:comment>
        <rdfs:comment xml:lang="ru">Прилагательное, образованное от причастия настоящего времени.</rdfs:comment>
        <dc:creator>Francopoulo, Gil</dc:creator>
        <owl:versionInfo>1:0</owl:versionInfo>
        <dcr:datcat rdf:resource="http://www.isocat.org/datcat/DC-1597"/>
        <rdfs:isDefinedBy rdf:resource="http://www.lexinfo.net/ontology/2.0/lexinfo"/>
    </owl:Thing>
    


    <!-- http://www.lexinfo.net/ontology/2.0/lexinfo#presentativePronoun -->

    <owl:Thing rdf:about="&lexinfo;presentativePronoun">
        <rdf:type rdf:resource="&lexinfo;PartOfSpeech"/>
        <rdf:type rdf:resource="&lexinfo;PronounPOS"/>
        <rdf:type rdf:resource="&owl;NamedIndividual"/>
        <rdfs:label xml:lang="en">presentative pronoun</rdfs:label>
        <rdfs:label xml:lang="ru">презентативное местоимение</rdfs:label>        
        <owl:versionInfo>1:0</owl:versionInfo>
        <dc:creator>Francopoulo, Gil</dc:creator>
        <rdfs:comment xml:lang="en">pronoun that identify the current locative or temporal situation</rdfs:comment>
        <rdfs:comment xml:lang="ru">Местоимение, обозначающее текущую локативную или темпоральную ситуацию.</rdfs:comment>
        <dcr:datcat rdf:resource="http://www.isocat.org/datcat/DC-3015"/>
        <rdfs:isDefinedBy rdf:resource="http://www.lexinfo.net/ontology/2.0/lexinfo"/>
    </owl:Thing>
    


    <!-- http://www.lexinfo.net/ontology/2.0/lexinfo#preterite -->

    <owl:NamedIndividual rdf:about="&lexinfo;preterite">
        <rdf:type rdf:resource="&lexinfo;Tense"/>
        <rdfs:comment xml:lang="en">The simple past or preterite as distinct from the perfect form, e.g,, &quot;showed&quot; not &quot;shown&quot;</rdfs:comment>
        <rdfs:comment xml:lang="ru">Настоящее простое или претерит, как отдельная форма перфектной формы, например, &quot;showed&quot; (показал), а не &quot;shown&quot;(показанный).</rdfs:comment>
    </owl:NamedIndividual>
    


    <!-- http://www.lexinfo.net/ontology/2.0/lexinfo#productName -->

    <owl:Thing rdf:about="&lexinfo;productName">
        <rdf:type rdf:resource="&lexinfo;TermType"/>
        <rdf:type rdf:resource="&owl;NamedIndividual"/>
        <rdfs:label xml:lang="en">productName</rdfs:label>
        <rdfs:label xml:lang="ru">название продукта</rdfs:label>        
        <owl:versionInfo>1:0</owl:versionInfo>
        <rdfs:comment xml:lang="en">An attribute assigned to a term indicating that that term is the official designator for a product.</rdfs:comment>
        <rdfs:comment xml:lang="ru">Определение, приписанное термину, указывающее на то, что данный термин является официальным десигнатором термина.</rdfs:comment>
        <dc:creator>Wright, Sue Ellen</dc:creator>
        <dcr:datcat rdf:resource="http://www.isocat.org/datcat/DC-346"/>
        <rdfs:isDefinedBy rdf:resource="http://www.lexinfo.net/ontology/2.0/lexinfo"/>
    </owl:Thing>
    


    <!-- http://www.lexinfo.net/ontology/2.0/lexinfo#prolativeCase -->

    <owl:Thing rdf:about="&lexinfo;prolativeCase">
        <rdf:type rdf:resource="&lexinfo;Case"/>
        <rdf:type rdf:resource="&owl;NamedIndividual"/>
        <rdfs:label xml:lang="en">prolative case</rdfs:label>
        <rdfs:label xml:lang="ru">пролатив</rdfs:label>
        <dc:creator>Francopoulo, Gil</dc:creator>
        <rdfs:comment xml:lang="en">Case for a noun or a pronoun that expresses motion within a place or a period of time needed for an event.</rdfs:comment>
        <rdfs:comment xml:lang="ru">Падеж существительного или местоимения, который выражает движение внутри места или периода времени, необходимого для события.</rdfs:comment>        
        <owl:versionInfo>1:0</owl:versionInfo>
        <dcr:datcat rdf:resource="http://www.isocat.org/datcat/DC-1368"/>
        <rdfs:isDefinedBy rdf:resource="http://www.lexinfo.net/ontology/2.0/lexinfo"/>
    </owl:Thing>
    


    <!-- http://www.lexinfo.net/ontology/2.0/lexinfo#pronominalAdverb -->

    <owl:Thing rdf:about="&lexinfo;pronominalAdverb">
        <rdf:type rdf:resource="&lexinfo;AdverbPOS"/>
        <rdf:type rdf:resource="&lexinfo;PartOfSpeech"/>
        <rdf:type rdf:resource="&owl;NamedIndividual"/>
        <rdfs:label xml:lang="en">pronominal adverb</rdfs:label>
        <rdfs:label xml:lang="ru">местоименное наречие</rdfs:label>        
        <dc:creator>Francopoulo, Gil</dc:creator>
        <owl:versionInfo>1:0</owl:versionInfo>
        <rdfs:comment xml:lang="en">adverb formed in replacement of a preposition and a pronoun</rdfs:comment>
        <rdfs:comment xml:lang="ru">Наречие, образованное для замещения предлога и местоимения.</rdfs:comment>        
        <dcr:datcat rdf:resource="http://www.isocat.org/datcat/DC-2998"/>
        <rdfs:isDefinedBy rdf:resource="http://www.lexinfo.net/ontology/2.0/lexinfo"/>
    </owl:Thing>
    


    <!-- http://www.lexinfo.net/ontology/2.0/lexinfo#pronoun -->

    <owl:Thing rdf:about="&lexinfo;pronoun">
        <rdf:type rdf:resource="&lexinfo;PartOfSpeech"/>
        <rdf:type rdf:resource="&lexinfo;PronounPOS"/>
        <rdf:type rdf:resource="&owl;NamedIndividual"/>
        <rdfs:label xml:lang="en">pronoun</rdfs:label>
        <rdfs:label xml:lang="ru">местоимение</rdfs:label>        
        <dc:creator>Francopoulo, Gil</dc:creator>
        <owl:versionInfo>1:0</owl:versionInfo>
        <rdfs:comment xml:lang="en">Word used in place of a noun or a noun phrase.</rdfs:comment>
        <rdfs:comment xml:lang="ru">Слово, используемое на месте существительного или именной группы.</rdfs:comment>
        <dcr:datcat rdf:resource="http://www.isocat.org/datcat/DC-1370"/>
        <rdfs:isDefinedBy rdf:resource="http://www.lexinfo.net/ontology/2.0/lexinfo"/>
    </owl:Thing>
    


    <!-- http://www.lexinfo.net/ontology/2.0/lexinfo#properNoun -->

    <owl:Thing rdf:about="&lexinfo;properNoun">
        <rdf:type rdf:resource="&lexinfo;NounPOS"/>
        <rdf:type rdf:resource="&lexinfo;PartOfSpeech"/>
        <rdf:type rdf:resource="&owl;NamedIndividual"/>
        <rdfs:label xml:lang="en">properNoun</rdfs:label>
        <rdfs:label xml:lang="ru">имя собственное</rdfs:label>
        <rdfs:label xml:lang="en">proper noun</rdfs:label>
        <rdfs:label xml:lang="ru">имя собственное</rdfs:label>        
        <dc:creator>Wright, Sue Ellen</dc:creator>
        <owl:versionInfo>1:0</owl:versionInfo>
        <rdfs:comment xml:lang="en">Noun that is the name of a specific individual, place, or object.</rdfs:comment>
        <rdfs:comment xml:lang="ru">Существительное для называния конкретного (отдельно взятого) индивида, места или объекта.</rdfs:comment>
        <rdfs:comment xml:lang="en">A noun or adjective denoting a single object.</rdfs:comment>
        <rdfs:comment xml:lang="ru">Существительное или прилагательное для обозначения единичного объекта.</rdfs:comment>
        <dc:creator>Francopoulo, Gil</dc:creator>
        <dcr:datcat rdf:resource="http://www.isocat.org/datcat/DC-1371"/>
        <dcr:datcat rdf:resource="http://www.isocat.org/datcat/DC-384"/>
        <rdfs:isDefinedBy rdf:resource="http://www.lexinfo.net/ontology/2.0/lexinfo"/>
    </owl:Thing>
    


    <!-- http://www.lexinfo.net/ontology/2.0/lexinfo#proverb -->

    <owl:Thing rdf:about="&lexinfo;proverb">
        <rdf:type rdf:resource="&lexinfo;TermType"/>
        <rdf:type rdf:resource="&owl;NamedIndividual"/>
        <rdfs:label xml:lang="en">proverb</rdfs:label>
        <rdfs:label xml:lang="ru">пословица</rdfs:label>
        <owl:versionInfo>1:0</owl:versionInfo>
        <rdfs:comment xml:lang="en">A brief popular axiom or saying.</rdfs:comment>
        <rdfs:comment xml:lang="ru">Краткая, широко используемая аксиома или высказывание.</rdfs:comment>
        <dc:creator>Wright, Sue Ellen</dc:creator>
        <dcr:datcat rdf:resource="http://www.isocat.org/datcat/DC-353"/>
        <rdfs:isDefinedBy rdf:resource="http://www.lexinfo.net/ontology/2.0/lexinfo"/>
    </owl:Thing>
    


    <!-- http://www.lexinfo.net/ontology/2.0/lexinfo#punctuation -->

    <owl:Thing rdf:about="&lexinfo;punctuation">
        <rdf:type rdf:resource="&lexinfo;PartOfSpeech"/>
        <rdf:type rdf:resource="&lexinfo;SymbolPOS"/>
        <rdf:type rdf:resource="&owl;NamedIndividual"/>
        <rdfs:label xml:lang="en">punctuation</rdfs:label>
        <rdfs:label xml:lang="ru">пунктуация</rdfs:label>        
        <rdfs:comment xml:lang="en">Graphical mark used either at word level to indicate an abbreviation or at a text level to separate phrases or sentences.</rdfs:comment>
        <rdfs:comment xml:lang="ru">Графический знак, используемый на уровне слов для обозначения аббревиатуры, или на уровне текста для обозначения отдельных групп (словосочетаний) или предложений.</rdfs:comment>        
        <dc:creator>Francopoulo, Gil</dc:creator>
        <owl:versionInfo>1:0</owl:versionInfo>
        <dcr:datcat rdf:resource="http://www.isocat.org/datcat/DC-1372"/>
        <rdfs:isDefinedBy rdf:resource="http://www.lexinfo.net/ontology/2.0/lexinfo"/>
    </owl:Thing>
    


    <!-- http://www.lexinfo.net/ontology/2.0/lexinfo#quadrial -->

    <owl:Thing rdf:about="&lexinfo;quadrial">
        <rdf:type rdf:resource="&lexinfo;Number"/>
        <rdf:type rdf:resource="&owl;NamedIndividual"/>
        <rdfs:label xml:lang="en">quadrial</rdfs:label>
        <rdfs:label xml:lang="ru">квадратичный</rdfs:label>        
        <dc:creator>Francopoulo, Gil</dc:creator>
        <owl:versionInfo>1:0</owl:versionInfo>
        <rdfs:comment xml:lang="en">Property related to four elements.</rdfs:comment>
        <rdfs:comment xml:lang="ru">Свойство, относящееся к четырем элементам.</rdfs:comment>        
        <dcr:datcat rdf:resource="http://www.isocat.org/datcat/DC-2000"/>
        <rdfs:isDefinedBy rdf:resource="http://www.lexinfo.net/ontology/2.0/lexinfo"/>
    </owl:Thing>
    


    <!-- http://www.lexinfo.net/ontology/2.0/lexinfo#qualifierAdjective -->

    <owl:Thing rdf:about="&lexinfo;qualifierAdjective">
        <rdf:type rdf:resource="&lexinfo;AdjectivePOS"/>
        <rdf:type rdf:resource="&lexinfo;PartOfSpeech"/>
        <rdf:type rdf:resource="&owl;NamedIndividual"/>
        <rdfs:label xml:lang="en">qualifier adjective</rdfs:label>
        <rdfs:label xml:lang="ru">качественное прилагательное</rdfs:label>        
        <owl:versionInfo>1:0</owl:versionInfo>
        <dc:creator>Francopoulo, Gil</dc:creator>
        <rdfs:comment xml:lang="en">Adjective used to qualify.</rdfs:comment>
        <rdfs:comment xml:lang="ru">Прилагательное, используемое для определения.</rdfs:comment>
        <dcr:datcat rdf:resource="http://www.isocat.org/datcat/DC-1477"/>
        <rdfs:isDefinedBy rdf:resource="http://www.lexinfo.net/ontology/2.0/lexinfo"/>
    </owl:Thing>
    


    <!-- http://www.lexinfo.net/ontology/2.0/lexinfo#questionMark -->

    <owl:Thing rdf:about="&lexinfo;questionMark">
        <rdf:type rdf:resource="&lexinfo;PartOfSpeech"/>
        <rdf:type rdf:resource="&lexinfo;SymbolPOS"/>
        <rdf:type rdf:resource="&owl;NamedIndividual"/>
        <rdfs:label xml:lang="en">question mark</rdfs:label>
        <rdfs:label xml:lang="ru">вопросительный знак</rdfs:label>        
        <dc:creator>Francopoulo, Gil</dc:creator>
        <rdfs:comment xml:lang="en">Sign used to express a question.</rdfs:comment>
        <rdfs:comment xml:lang="ru">Знак, используемый для выражения вопроса.</rdfs:comment>
        <owl:versionInfo>1:0</owl:versionInfo>
        <dcr:datcat rdf:resource="http://www.isocat.org/datcat/DC-1444"/>
        <rdfs:isDefinedBy rdf:resource="http://www.lexinfo.net/ontology/2.0/lexinfo"/>
    </owl:Thing>
    


    <!-- http://www.lexinfo.net/ontology/2.0/lexinfo#radical -->

    <owl:Thing rdf:about="&lexinfo;radical">
        <rdf:type rdf:resource="&lexinfo;TermElement"/>
        <rdf:type rdf:resource="&owl;NamedIndividual"/>
        <rdfs:label xml:lang="en">radical</rdfs:label>
        <rdfs:label xml:lang="ru">корень</rdfs:label>        
        <rdfs:comment xml:lang="en">A basic identifiable component of every CJKV character, often found on the left side of the character, that sometimes gives a rough indication of meaning and is used for collating lexical and terminological resources.</rdfs:comment>
        <rdfs:comment xml:lang="ru">Основной опознаваемый компонент каждого китайского, японского, корейского или вьетнамского иероглифа, обычно располагающийся с левой стороны от иероглифа, который иногда дает приближенное указание значения и используется для сопоставления лексических и терминологических ресурсов.</rdfs:comment>
        <dc:creator>Wright, Sue Ellen</dc:creator>
        <owl:versionInfo>1:0</owl:versionInfo>
        <dcr:datcat rdf:resource="http://www.isocat.org/datcat/DC-296"/>
        <rdfs:isDefinedBy rdf:resource="http://www.lexinfo.net/ontology/2.0/lexinfo"/>
    </owl:Thing>
    


    <!-- http://www.lexinfo.net/ontology/2.0/lexinfo#rarelyUsed -->

    <owl:Thing rdf:about="&lexinfo;rarelyUsed">
        <rdf:type rdf:resource="&lexinfo;Frequency"/>
        <rdf:type rdf:resource="&owl;NamedIndividual"/>
        <rdfs:label xml:lang="en">rarelyUsed</rdfs:label>
        <rdfs:label xml:lang="ru">редкоиспользуемый</rdfs:label>        
        <rdfs:label xml:lang="en">rarely used</rdfs:label>
        <rdfs:label xml:lang="ru">редкоиспользуемый</rdfs:label>
        <dc:creator>Francopoulo, Gil</dc:creator>
        <rdfs:comment xml:lang="en">Said of a term that is almost never used.</rdfs:comment>
        <rdfs:comment xml:lang="ru">Говорится о термине, который практически никогда не используется.</rdfs:comment>
        <dc:creator>Wright, Sue Ellen</dc:creator>
        <owl:versionInfo>1:0</owl:versionInfo>
        <dcr:datcat rdf:resource="http://www.isocat.org/datcat/DC-1986"/>
        <dcr:datcat rdf:resource="http://www.isocat.org/datcat/DC-236"/>
        <rdfs:isDefinedBy rdf:resource="http://www.lexinfo.net/ontology/2.0/lexinfo"/>
    </owl:Thing>
    


    <!-- http://www.lexinfo.net/ontology/2.0/lexinfo#reciprocalPronoun -->

    <owl:Thing rdf:about="&lexinfo;reciprocalPronoun">
        <rdf:type rdf:resource="&lexinfo;PartOfSpeech"/>
        <rdf:type rdf:resource="&lexinfo;PronounPOS"/>
        <rdf:type rdf:resource="&owl;NamedIndividual"/>
        <rdfs:label xml:lang="en">reciprocal pronoun</rdfs:label>
        <rdfs:label xml:lang="ru">взаимное местоимение</rdfs:label>        
        <dc:creator>Francopoulo, Gil</dc:creator>
        <owl:versionInfo>1:0</owl:versionInfo>
        <rdfs:comment xml:lang="en">Pronoun expressing mutual relationship.</rdfs:comment>
        <rdfs:comment xml:lang="ru">Местоимение, выражающее взаимные отношения.</rdfs:comment>        
        <dcr:datcat rdf:resource="http://www.isocat.org/datcat/DC-1924"/>
        <rdfs:isDefinedBy rdf:resource="http://www.lexinfo.net/ontology/2.0/lexinfo"/>
    </owl:Thing>
    


    <!-- http://www.lexinfo.net/ontology/2.0/lexinfo#reflexiveDeterminer -->

    <owl:Thing rdf:about="&lexinfo;reflexiveDeterminer">
        <rdf:type rdf:resource="&lexinfo;DeterminerPOS"/>
        <rdf:type rdf:resource="&lexinfo;PartOfSpeech"/>
        <rdf:type rdf:resource="&owl;NamedIndividual"/>
        <rdfs:label xml:lang="en">reflexive adjective</rdfs:label>
        <rdfs:label xml:lang="ru">возвратное прилагательное</rdfs:label>
        <dc:creator>Francopoulo, Gil</dc:creator>
        <rdfs:comment xml:lang="en">Determiner that refers to the same entity.</rdfs:comment>
        <rdfs:comment xml:lang="ru">Определитель, который ссылается на одну и ту же сущность.</rdfs:comment>        
        <owl:versionInfo>1:0</owl:versionInfo>
        <dcr:datcat rdf:resource="http://www.isocat.org/datcat/DC-1377"/>
        <rdfs:isDefinedBy rdf:resource="http://www.lexinfo.net/ontology/2.0/lexinfo"/>
    </owl:Thing>
    


    <!-- http://www.lexinfo.net/ontology/2.0/lexinfo#reflexivePersonalPronoun -->

    <owl:Thing rdf:about="&lexinfo;reflexivePersonalPronoun">
        <rdf:type rdf:resource="&lexinfo;PartOfSpeech"/>
        <rdf:type rdf:resource="&lexinfo;PronounPOS"/>
        <rdf:type rdf:resource="&owl;NamedIndividual"/>
        <rdfs:label xml:lang="en">reflexive personal pronoun</rdfs:label>
        <rdfs:label xml:lang="ru">возвратное личное местоимение</rdfs:label>        
        <dc:creator>Francopoulo, Gil</dc:creator>
        <rdfs:comment xml:lang="en">personal pronoun which is reflexive</rdfs:comment>
        <rdfs:comment xml:lang="ru">Личное местоимение, являющееся возвратным.</rdfs:comment>
        <owl:versionInfo>1:0</owl:versionInfo>
        <dcr:datcat rdf:resource="http://www.isocat.org/datcat/DC-3014"/>
        <rdfs:isDefinedBy rdf:resource="http://www.lexinfo.net/ontology/2.0/lexinfo"/>
    </owl:Thing>
    


    <!-- http://www.lexinfo.net/ontology/2.0/lexinfo#reflexivePossessivePronoun -->

    <owl:Thing rdf:about="&lexinfo;reflexivePossessivePronoun">
        <rdf:type rdf:resource="&lexinfo;PartOfSpeech"/>
        <rdf:type rdf:resource="&lexinfo;PronounPOS"/>
        <rdf:type rdf:resource="&owl;NamedIndividual"/>
        <rdfs:label xml:lang="en">reflexive possessive pronoun</rdfs:label>
        <rdfs:label xml:lang="ru">возвратное притяжательное местоимение</rdfs:label>        
        <dc:creator>Zeman, Dan</dc:creator>
        <rdfs:comment xml:lang="en">A possessive pronoun that refers to the subject as the possessor.</rdfs:comment>
        <rdfs:comment xml:lang="ru">Притяжательное местоимение, которое имеет отношение к субъекту как обладателю.</rdfs:comment>
        <owl:versionInfo>1:0</owl:versionInfo>
        <dcr:datcat rdf:resource="http://www.isocat.org/datcat/DC-3001"/>
        <rdfs:isDefinedBy rdf:resource="http://www.lexinfo.net/ontology/2.0/lexinfo"/>
    </owl:Thing>
    


    <!-- http://www.lexinfo.net/ontology/2.0/lexinfo#regulatedTerm -->

    <owl:Thing rdf:about="&lexinfo;regulatedTerm">
        <rdf:type rdf:resource="&lexinfo;NormativeAuthorization"/>
        <rdf:type rdf:resource="&owl;NamedIndividual"/>
        <rdfs:label xml:lang="en">regulated term</rdfs:label>
        <rdfs:label xml:lang="ru">нормативный термин</rdfs:label>        
        <rdfs:comment xml:lang="en">A term defined by law or government regulation.</rdfs:comment>
        <rdfs:comment xml:lang="ru">Термин, определенный законом или государственным регулированием.</rdfs:comment>
        <owl:versionInfo>1:0</owl:versionInfo>
        <dc:creator>Wright, Sue Ellen</dc:creator>
        <dcr:datcat rdf:resource="http://www.isocat.org/datcat/DC-381"/>
        <rdfs:isDefinedBy rdf:resource="http://www.lexinfo.net/ontology/2.0/lexinfo"/>
    </owl:Thing>
    


    <!-- http://www.lexinfo.net/ontology/2.0/lexinfo#relationNoun -->

    <owl:Thing rdf:about="&lexinfo;relationNoun">
        <rdf:type rdf:resource="&lexinfo;NounPOS"/>
        <rdf:type rdf:resource="&lexinfo;PartOfSpeech"/>
        <rdf:type rdf:resource="&owl;NamedIndividual"/>
        <rdfs:label xml:lang="en">relation noun</rdfs:label>
        <rdfs:label xml:lang="ru">родственное существительное</rdfs:label>        
        <dc:creator>Francopoulo, Gil</dc:creator>
        <rdfs:comment xml:lang="en">relation noun</rdfs:comment>
        <rdfs:comment xml:lang="ru">родственное существительное</rdfs:comment>        
        <owl:versionInfo>1:0</owl:versionInfo>
        <dcr:datcat rdf:resource="http://www.isocat.org/datcat/DC-2226"/>
        <rdfs:isDefinedBy rdf:resource="http://www.lexinfo.net/ontology/2.0/lexinfo"/>
    </owl:Thing>
    


    <!-- http://www.lexinfo.net/ontology/2.0/lexinfo#relativeDeterminer -->

    <owl:Thing rdf:about="&lexinfo;relativeDeterminer">
        <rdf:type rdf:resource="&lexinfo;DeterminerPOS"/>
        <rdf:type rdf:resource="&lexinfo;PartOfSpeech"/>
        <rdf:type rdf:resource="&owl;NamedIndividual"/>
        <rdfs:label xml:lang="en">relative determiner</rdfs:label>
        <rdfs:label xml:lang="ru">относительный определитель</rdfs:label>        
        <dc:creator>Francopoulo, Gil</dc:creator>
        <owl:versionInfo>1:0</owl:versionInfo>
        <rdfs:comment xml:lang="en">Determiner related to a referent.</rdfs:comment>
        <rdfs:comment xml:lang="ru">Определитель, связанный с референтом.</rdfs:comment>
        <dcr:datcat rdf:resource="http://www.isocat.org/datcat/DC-1379"/>
        <rdfs:isDefinedBy rdf:resource="http://www.lexinfo.net/ontology/2.0/lexinfo"/>
    </owl:Thing>
    


    <!-- http://www.lexinfo.net/ontology/2.0/lexinfo#relativeParticle -->

    <owl:Thing rdf:about="&lexinfo;relativeParticle">
        <rdf:type rdf:resource="&lexinfo;PartOfSpeech"/>
        <rdf:type rdf:resource="&lexinfo;ParticlePOS"/>
        <rdf:type rdf:resource="&owl;NamedIndividual"/>
        <rdfs:label xml:lang="en">relative particle</rdfs:label>
        <rdfs:label xml:lang="ru">относительная частица</rdfs:label>        
        <owl:versionInfo>1:0</owl:versionInfo>
        <dc:creator>Francopoulo, Gil</dc:creator>
        <rdfs:comment xml:lang="en">relative particle</rdfs:comment>
        <rdfs:comment xml:lang="ru">относительная частица</rdfs:comment>
        <dcr:datcat rdf:resource="http://www.isocat.org/datcat/DC-2229"/>
        <rdfs:isDefinedBy rdf:resource="http://www.lexinfo.net/ontology/2.0/lexinfo"/>
    </owl:Thing>
    


    <!-- http://www.lexinfo.net/ontology/2.0/lexinfo#relativePronoun -->

    <owl:Thing rdf:about="&lexinfo;relativePronoun">
        <rdf:type rdf:resource="&lexinfo;PartOfSpeech"/>
        <rdf:type rdf:resource="&lexinfo;PronounPOS"/>
        <rdf:type rdf:resource="&owl;NamedIndividual"/>
        <rdfs:label xml:lang="en">relative pronoun</rdfs:label>
        <rdfs:label xml:lang="ru">относительное местоимение</rdfs:label>
        <rdfs:comment xml:lang="en">Pronoun which introduces a relative clause and refers to something that has been said before.</rdfs:comment>
        <rdfs:comment xml:lang="ru">Местоимение, которое вводит придаточное предложение и указывает на то, что было сказано ранее.</rdfs:comment>        
        <dc:creator>Francopoulo, Gil</dc:creator>
        <owl:versionInfo>1:0</owl:versionInfo>
        <dcr:datcat rdf:resource="http://www.isocat.org/datcat/DC-1380"/>
        <rdfs:isDefinedBy rdf:resource="http://www.lexinfo.net/ontology/2.0/lexinfo"/>
    </owl:Thing>
    


    <!-- http://www.lexinfo.net/ontology/2.0/lexinfo#secondPerson -->

    <owl:Thing rdf:about="&lexinfo;secondPerson">
        <rdf:type rdf:resource="&lexinfo;Person"/>
        <rdf:type rdf:resource="&owl;NamedIndividual"/>
        <rdfs:label xml:lang="en">second person</rdfs:label>
        <rdfs:label xml:lang="ru">второе лицо</rdfs:label>        
        <dc:creator>Francopoulo, Gil</dc:creator>
        <rdfs:comment xml:lang="en">Second person deixis is deictic reference to a person or persons identified as addressee.</rdfs:comment>
        <rdfs:comment xml:lang="ru">Указание второго лица является ссылкой на человека или лиц, указанных в качестве адресата.</rdfs:comment>
        <owl:versionInfo>1:0</owl:versionInfo>
        <dcr:datcat rdf:resource="http://www.isocat.org/datcat/DC-1384"/>
        <rdfs:isDefinedBy rdf:resource="http://www.lexinfo.net/ontology/2.0/lexinfo"/>
    </owl:Thing>
    


    <!-- http://www.lexinfo.net/ontology/2.0/lexinfo#semiColon -->

    <owl:Thing rdf:about="&lexinfo;semiColon">
        <rdf:type rdf:resource="&lexinfo;PartOfSpeech"/>
        <rdf:type rdf:resource="&lexinfo;SymbolPOS"/>
        <rdf:type rdf:resource="&owl;NamedIndividual"/>
        <rdfs:label xml:lang="en">semi-colon</rdfs:label>
        <rdfs:label xml:lang="ru">Точка с запятой</rdfs:label>        
        <rdfs:comment xml:lang="en">Sign (;) usually used to separate phrases.</rdfs:comment>
        <rdfs:comment xml:lang="ru">Знак (;), обычно используемый для отделения предложений.</rdfs:comment>        
        <owl:versionInfo>1:0</owl:versionInfo>
        <dc:creator>Francopoulo, Gil</dc:creator>
        <dcr:datcat rdf:resource="http://www.isocat.org/datcat/DC-1446"/>
        <rdfs:isDefinedBy rdf:resource="http://www.lexinfo.net/ontology/2.0/lexinfo"/>
    </owl:Thing>
    


    <!-- http://www.lexinfo.net/ontology/2.0/lexinfo#setPhrase -->

    <owl:Thing rdf:about="&lexinfo;setPhrase">
        <rdf:type rdf:resource="&lexinfo;TermType"/>
        <rdf:type rdf:resource="&owl;NamedIndividual"/>
        <rdfs:label xml:lang="en">set phrase</rdfs:label>
        <rdfs:label xml:lang="ru">устойчивое словосочетание</rdfs:label>        
        <owl:versionInfo>1:0</owl:versionInfo>
        <dc:creator>Wright, Sue Ellen</dc:creator>
        <rdfs:comment xml:lang="en">A fixed, lexicalized phrase.</rdfs:comment>
        <rdfs:comment xml:lang="ru">Устойчивое ​​лексикализованное словосочетание.</rdfs:comment>
        <dcr:datcat rdf:resource="http://www.isocat.org/datcat/DC-341"/>
        <rdfs:isDefinedBy rdf:resource="http://www.lexinfo.net/ontology/2.0/lexinfo"/>
    </owl:Thing>
    


    <!-- http://www.lexinfo.net/ontology/2.0/lexinfo#shortArticle -->

    <owl:Thing rdf:about="&lexinfo;shortArticle">
        <rdf:type rdf:resource="&lexinfo;Definiteness"/>
        <rdf:type rdf:resource="&owl;NamedIndividual"/>
        <rdfs:label xml:lang="en">short article</rdfs:label>
        <rdfs:label xml:lang="ru">Краткий артикль</rdfs:label>        
        <rdfs:comment xml:lang="en">For definiteness, when a specific form is not the syntactic subject of the clause.</rdfs:comment>
        <rdfs:comment xml:lang="ru">Для определенности, когда конкретная форма не является синтаксическим субъектом предложения.</rdfs:comment>
        <dc:creator>Francopoulo, Gil</dc:creator>
        <owl:versionInfo>1:0</owl:versionInfo>
        <dcr:datcat rdf:resource="http://www.isocat.org/datcat/DC-1927"/>
        <rdfs:isDefinedBy rdf:resource="http://www.lexinfo.net/ontology/2.0/lexinfo"/>
    </owl:Thing>
    


    <!-- http://www.lexinfo.net/ontology/2.0/lexinfo#shortForm -->

    <owl:Thing rdf:about="&lexinfo;shortForm">
        <rdf:type rdf:resource="&lexinfo;TermType"/>
        <rdf:type rdf:resource="&owl;NamedIndividual"/>
        <rdfs:label xml:lang="en">short form</rdfs:label>
        <rdfs:label xml:lang="ru">краткая форма</rdfs:label>        
        <owl:versionInfo>1:0</owl:versionInfo>
        <rdfs:comment xml:lang="en">A variant of a multiword term or lexeme that includes fewer words than the full form.</rdfs:comment>
        <rdfs:comment xml:lang="ru">Вариант многословного термина или лексемы, который содержит меньше слов, чем полная форма.</rdfs:comment>        
        <dc:creator>Wright, Sue Ellen</dc:creator>
        <dcr:datcat rdf:resource="http://www.isocat.org/datcat/DC-332"/>
        <rdfs:isDefinedBy rdf:resource="http://www.lexinfo.net/ontology/2.0/lexinfo"/>
    </owl:Thing>
    


    <!-- http://www.lexinfo.net/ontology/2.0/lexinfo#singular -->

    <owl:Thing rdf:about="&lexinfo;singular">
        <rdf:type rdf:resource="&lexinfo;Number"/>
        <rdf:type rdf:resource="&owl;NamedIndividual"/>
        <rdfs:label xml:lang="en">singular</rdfs:label>
        <rdfs:label xml:lang="ru">единственное</rdfs:label>        
        <rdfs:comment xml:lang="en">The form of a term or word (usually of a noun) used to designate one object.</rdfs:comment>
        <rdfs:comment xml:lang="ru">Форма термина или слова (обычно существительного), используемого для обозначения одного объекта.</rdfs:comment>
        <dc:creator>Wright, Sue Ellen</dc:creator>
        <rdfs:comment xml:lang="en">Value that expresses one element.</rdfs:comment>
        <rdfs:comment xml:lang="ru">Значение, показывающее, что предмет один.</rdfs:comment>
        <dc:creator>Francopoulo, Gil</dc:creator>
        <owl:versionInfo>1:0</owl:versionInfo>
        <dcr:datcat rdf:resource="http://www.isocat.org/datcat/DC-1387"/>
        <dcr:datcat rdf:resource="http://www.isocat.org/datcat/DC-252"/>
        <rdfs:isDefinedBy rdf:resource="http://www.lexinfo.net/ontology/2.0/lexinfo"/>
    </owl:Thing>
    


    <!-- http://www.lexinfo.net/ontology/2.0/lexinfo#sku -->

    <owl:Thing rdf:about="&lexinfo;sku">
        <rdf:type rdf:resource="&lexinfo;TermType"/>
        <rdf:type rdf:resource="&owl;NamedIndividual"/>
        <rdfs:label xml:lang="en">sku</rdfs:label>
        <rdfs:label xml:lang="ru">артикул</rdfs:label>        
        <owl:versionInfo>1:0</owl:versionInfo>
        <rdfs:comment xml:lang="en">An inventory item identified by a unique alphanumeric designation assigned to an object in an inventory control system.</rdfs:comment>
        <rdfs:comment xml:lang="ru">Учётная единица, идентифицируемая уникальным буквенно-цифровым обозначением, приписанным объекту в системе контроля материально-технических запасов.</rdfs:comment>        
        <dc:creator>Wright, Sue Ellen</dc:creator>
        <dcr:datcat rdf:resource="http://www.isocat.org/datcat/DC-337"/>
        <rdfs:isDefinedBy rdf:resource="http://www.lexinfo.net/ontology/2.0/lexinfo"/>
    </owl:Thing>
    


    <!-- http://www.lexinfo.net/ontology/2.0/lexinfo#slangRegister -->

    <owl:Thing rdf:about="&lexinfo;slangRegister">
        <rdf:type rdf:resource="&lexinfo;Register"/>
        <rdf:type rdf:resource="&owl;NamedIndividual"/>
        <rdfs:label xml:lang="en">slang register</rdfs:label>
        <rdfs:label xml:lang="ru">реестр слэнга</rdfs:label>        
        <owl:versionInfo>1:0</owl:versionInfo>
        <rdfs:comment xml:lang="en">An extremely informal register of a word, term, or text that is used in spoken and everyday language and less commonly in documents.</rdfs:comment>
        <rdfs:comment xml:lang="ru">Неофициальный реестр слов, терминов или текстов, которые используются в устной обиходно-разговорной речи и реже в документах.</rdfs:comment>
        <dc:creator>Wright, Sue Ellen</dc:creator>
        <dc:creator>Francopoulo, Gil</dc:creator>
        <dcr:datcat rdf:resource="http://www.isocat.org/datcat/DC-1995"/>
        <dcr:datcat rdf:resource="http://www.isocat.org/datcat/DC-428"/>
        <rdfs:isDefinedBy rdf:resource="http://www.lexinfo.net/ontology/2.0/lexinfo"/>
    </owl:Thing>
    


    <!-- http://www.lexinfo.net/ontology/2.0/lexinfo#slash -->

    <owl:Thing rdf:about="&lexinfo;slash">
        <rdf:type rdf:resource="&lexinfo;PartOfSpeech"/>
        <rdf:type rdf:resource="&lexinfo;SymbolPOS"/>
        <rdf:type rdf:resource="&owl;NamedIndividual"/>
        <rdfs:label xml:lang="en">slash</rdfs:label>
        <rdfs:label xml:lang="ru">косая черта</rdfs:label>        
        <dc:creator>Francopoulo, Gil</dc:creator>
        <rdfs:comment xml:lang="en">The punctuation sign /</rdfs:comment>
        <rdfs:comment xml:lang="ru">Пунктуационный знак /</rdfs:comment>
        <owl:versionInfo>1:0</owl:versionInfo>
        <dcr:datcat rdf:resource="http://www.isocat.org/datcat/DC-1437"/>
        <rdfs:isDefinedBy rdf:resource="http://www.lexinfo.net/ontology/2.0/lexinfo"/>
    </owl:Thing>
    


    <!-- http://www.lexinfo.net/ontology/2.0/lexinfo#sociativeCase -->

    <owl:Thing rdf:about="&lexinfo;sociativeCase">
        <rdf:type rdf:resource="&lexinfo;Case"/>
        <rdf:type rdf:resource="&owl;NamedIndividual"/>
        <rdfs:label xml:lang="en">sociative case</rdfs:label>
        <rdfs:label xml:lang="ru">социатив</rdfs:label>        
        <dc:creator>Francopoulo, Gil</dc:creator>
        <rdfs:comment xml:lang="en">Case related to the person in whose company the action is carried out, or to any belongings of people which take part in the action.</rdfs:comment>
        <rdfs:comment xml:lang="ru">Падеж, связанный с лицом, в компании которого осуществляется действие, или с любыми вещами, принадлежащими людям, которые принимают участие в действии.</rdfs:comment>        
        <owl:versionInfo>1:0</owl:versionInfo>
        <dcr:datcat rdf:resource="http://www.isocat.org/datcat/DC-1388"/>
        <rdfs:isDefinedBy rdf:resource="http://www.lexinfo.net/ontology/2.0/lexinfo"/>
    </owl:Thing>
    


    <!-- http://www.lexinfo.net/ontology/2.0/lexinfo#standardText -->

    <owl:Thing rdf:about="&lexinfo;standardText">
        <rdf:type rdf:resource="&lexinfo;TermType"/>
        <rdf:type rdf:resource="&owl;NamedIndividual"/>
        <rdfs:label xml:lang="en">standard text</rdfs:label>
        <rdfs:label xml:lang="ru">стандартное выражение</rdfs:label>        
        <owl:versionInfo>1:0</owl:versionInfo>
        <dc:creator>Wright, Sue Ellen</dc:creator>
        <rdfs:comment xml:lang="en">A fixed chunk of recurring text.</rdfs:comment>
        <rdfs:comment xml:lang="ru">Фиксированная часть повторяющегося текста.</rdfs:comment>        
        <dcr:datcat rdf:resource="http://www.isocat.org/datcat/DC-343"/>
        <rdfs:isDefinedBy rdf:resource="http://www.lexinfo.net/ontology/2.0/lexinfo"/>
    </owl:Thing>
    


    <!-- http://www.lexinfo.net/ontology/2.0/lexinfo#standardizedTerm -->

    <owl:Thing rdf:about="&lexinfo;standardizedTerm">
        <rdf:type rdf:resource="&lexinfo;NormativeAuthorization"/>
        <rdf:type rdf:resource="&owl;NamedIndividual"/>
        <rdfs:label xml:lang="en">standardized term</rdfs:label>
        <rdfs:label xml:lang="ru">стандартный термин</rdfs:label>        
        <rdfs:comment xml:lang="en">A term that has been standardized by a standardizing body.</rdfs:comment>
        <rdfs:comment xml:lang="ru">Термин, стандартизованный соответствующим органом.</rdfs:comment>
        <owl:versionInfo>1:0</owl:versionInfo>
        <dc:creator>Wright, Sue Ellen</dc:creator>
        <dcr:datcat rdf:resource="http://www.isocat.org/datcat/DC-375"/>
        <rdfs:isDefinedBy rdf:resource="http://www.lexinfo.net/ontology/2.0/lexinfo"/>
    </owl:Thing>
    


    <!-- http://www.lexinfo.net/ontology/2.0/lexinfo#string -->

    <owl:Thing rdf:about="&lexinfo;string">
        <rdf:type rdf:resource="&lexinfo;TermType"/>
        <rdf:type rdf:resource="&owl;NamedIndividual"/>
        <rdfs:label xml:lang="en">string</rdfs:label>
        <rdfs:label xml:lang="ru">строка</rdfs:label>        
        <rdfs:comment xml:lang="en">A chunk of text used in a software interface, documentation, help file, or the like.</rdfs:comment>
        <rdfs:comment xml:lang="ru">Часть текста, использованная в программном интерфейсе, документации, справочном файле и т.п.</rdfs:comment>
        <owl:versionInfo>1:0</owl:versionInfo>
        <dc:creator>Wright, Sue Ellen</dc:creator>
        <dcr:datcat rdf:resource="http://www.isocat.org/datcat/DC-344"/>
        <rdfs:isDefinedBy rdf:resource="http://www.lexinfo.net/ontology/2.0/lexinfo"/>
    </owl:Thing>
    


    <!-- http://www.lexinfo.net/ontology/2.0/lexinfo#stringCategory -->

    <owl:Thing rdf:about="&lexinfo;stringCategory">
        <rdf:type rdf:resource="&lexinfo;TermType"/>
        <rdf:type rdf:resource="&owl;NamedIndividual"/>
        <rdfs:label xml:lang="en">stringCategory</rdfs:label>
        <rdfs:label xml:lang="ru">категория строки</rdfs:label>        
        <dc:creator>Wright, Sue Ellen</dc:creator>
        <rdfs:comment xml:lang="en">A type value assigned to a string.</rdfs:comment>
        <rdfs:comment xml:lang="ru">Значение типа, присвоенное строке.</rdfs:comment>
        <owl:versionInfo>1:0</owl:versionInfo>
        <dcr:datcat rdf:resource="http://www.isocat.org/datcat/DC-345"/>
        <rdfs:isDefinedBy rdf:resource="http://www.lexinfo.net/ontology/2.0/lexinfo"/>
    </owl:Thing>
    


    <!-- http://www.lexinfo.net/ontology/2.0/lexinfo#strongPersonalPronoun -->

    <owl:Thing rdf:about="&lexinfo;strongPersonalPronoun">
        <rdf:type rdf:resource="&lexinfo;PartOfSpeech"/>
        <rdf:type rdf:resource="&lexinfo;PronounPOS"/>
        <rdf:type rdf:resource="&owl;NamedIndividual"/>
        <rdfs:label xml:lang="en">strong personal pronoun</rdfs:label>
        <rdfs:label xml:lang="ru">Сильное личное местоимение</rdfs:label>        
        <dc:creator>Francopoulo, Gil</dc:creator>
        <owl:versionInfo>1:0</owl:versionInfo>
        <rdfs:comment xml:lang="en">Personal pronoun that can occupy the position after a preposition and/or reinforce a weak personal pronoun.</rdfs:comment>
        <rdfs:comment xml:lang="ru">Личное местоимение, которое может занимать место после предлога и / или усиливать слабое личное местоимение.</rdfs:comment>
        <dcr:datcat rdf:resource="http://www.isocat.org/datcat/DC-1390"/>
        <rdfs:isDefinedBy rdf:resource="http://www.lexinfo.net/ontology/2.0/lexinfo"/>
    </owl:Thing>
    


    <!-- http://www.lexinfo.net/ontology/2.0/lexinfo#subjunctive -->

    <owl:Thing rdf:about="&lexinfo;subjunctive">
        <rdf:type rdf:resource="&lexinfo;Mood"/>
        <rdf:type rdf:resource="&lexinfo;VerbFormMood"/>
        <rdf:type rdf:resource="&owl;NamedIndividual"/>
        <rdfs:label xml:lang="en">subjunctive</rdfs:label>
        <rdfs:label xml:lang="ru">сослагательное</rdfs:label>        
        <rdfs:comment>...</rdfs:comment>
        <dc:creator>Francopoulo, Gil</dc:creator>
        <dc:creator>Wright, Sue Ellen</dc:creator>
        <rdfs:comment xml:lang="en">Mood often used to express uncertainty, whishes or desires.</rdfs:comment>
        <rdfs:comment xml:lang="ru">Наклонение, часто используемое для выражения неопределенности, желания или волеизъявления.</rdfs:comment>
        <owl:versionInfo>1:0</owl:versionInfo>
        <dcr:datcat rdf:resource="http://www.isocat.org/datcat/DC-1843"/>
        <dcr:datcat rdf:resource="http://www.isocat.org/datcat/DC-368"/>
        <rdfs:isDefinedBy rdf:resource="http://www.lexinfo.net/ontology/2.0/lexinfo"/>
    </owl:Thing>
    


    <!-- http://www.lexinfo.net/ontology/2.0/lexinfo#sublativeCase -->

    <owl:Thing rdf:about="&lexinfo;sublativeCase">
        <rdf:type rdf:resource="&lexinfo;Case"/>
        <rdf:type rdf:resource="&owl;NamedIndividual"/>
        <rdfs:label xml:lang="en">sublative case</rdfs:label>
        <rdfs:label xml:lang="ru">сублатив</rdfs:label>        
        <owl:versionInfo>1:0</owl:versionInfo>
        <rdfs:comment xml:lang="en">Case for a move of something to the surface of another object.</rdfs:comment>
        <rdfs:comment xml:lang="ru">Падеж для обозначения перемещения чего-либо на поверхность другого объекта.</rdfs:comment>
        <dc:creator>Francopoulo, Gil</dc:creator>
        <dcr:datcat rdf:resource="http://www.isocat.org/datcat/DC-1392"/>
        <rdfs:isDefinedBy rdf:resource="http://www.lexinfo.net/ontology/2.0/lexinfo"/>
    </owl:Thing>
    


    <!-- http://www.lexinfo.net/ontology/2.0/lexinfo#subordinatingConjunction -->

    <owl:Thing rdf:about="&lexinfo;subordinatingConjunction">
        <rdf:type rdf:resource="&lexinfo;ConjunctionPOS"/>
        <rdf:type rdf:resource="&lexinfo;PartOfSpeech"/>
        <rdf:type rdf:resource="&owl;NamedIndividual"/>
        <rdfs:label xml:lang="en">subordinating conjunction</rdfs:label>
        <rdfs:label xml:lang="ru">подчинительный союз</rdfs:label>        
        <owl:versionInfo>1:0</owl:versionInfo>
        <rdfs:comment xml:lang="en">Conjunction that links constructions by making one of them a constituent of another. The subordinating conjunction typically marks the incorporated constituent.</rdfs:comment>
        <rdfs:comment xml:lang="ru">Союз, который связывает конструкции, делая одну из них составным элементом другой. Подчинительный союз обычно указывает на элемент, входящий в структуру.</rdfs:comment>
        <dc:creator>Francopoulo, Gil</dc:creator>
        <dcr:datcat rdf:resource="http://www.isocat.org/datcat/DC-1393"/>
        <rdfs:isDefinedBy rdf:resource="http://www.lexinfo.net/ontology/2.0/lexinfo"/>
    </owl:Thing>
    


    <!-- http://www.lexinfo.net/ontology/2.0/lexinfo#suffix -->

    <owl:Thing rdf:about="&lexinfo;suffix">
        <rdf:type rdf:resource="&lexinfo;TermElement"/>
        <rdf:type rdf:resource="&owl;NamedIndividual"/>
        <rdfs:isDefinedBy rdf:resource="http://www.lexinfo.net/ontology/2.0/lexinfo"/>
    </owl:Thing>
    


    <!-- http://www.lexinfo.net/ontology/2.0/lexinfo#superessiveCase -->

    <owl:Thing rdf:about="&lexinfo;superessiveCase">
        <rdf:type rdf:resource="&lexinfo;Case"/>
        <rdf:type rdf:resource="&owl;NamedIndividual"/>
        <rdfs:label xml:lang="en">superessive case</rdfs:label>
        <rdfs:label xml:lang="ru">суперессив</rdfs:label>        
        <dc:creator>Francopoulo, Gil</dc:creator>
        <owl:versionInfo>1:0</owl:versionInfo>
        <rdfs:comment xml:lang="en">Case indicating location on top of something or on the surface of something.</rdfs:comment>
        <rdfs:comment xml:lang="ru">Падеж, указывающий на местоположение поверх чего-то или на поверхности чего-то.</rdfs:comment>        
        <dcr:datcat rdf:resource="http://www.isocat.org/datcat/DC-1396"/>
        <rdfs:isDefinedBy rdf:resource="http://www.lexinfo.net/ontology/2.0/lexinfo"/>
    </owl:Thing>
    


    <!-- http://www.lexinfo.net/ontology/2.0/lexinfo#superlative -->

    <owl:Thing rdf:about="&lexinfo;superlative">
        <rdf:type rdf:resource="&lexinfo;Degree"/>
        <rdf:type rdf:resource="&owl;NamedIndividual"/>
        <rdfs:label xml:lang="en">superlative</rdfs:label>
        <rdfs:label xml:lang="ru">превосходная</rdfs:label>        
        <dc:creator>Francopoulo, Gil</dc:creator>
        <rdfs:comment xml:lang="en">Value used in a comparison between more than two entities.</rdfs:comment>
        <rdfs:comment xml:lang="ru">Значение, используемое при сравнении более чем двух сущностей.</rdfs:comment>
        <owl:versionInfo>1:0</owl:versionInfo>
        <dcr:datcat rdf:resource="http://www.isocat.org/datcat/DC-1422"/>
        <rdfs:isDefinedBy rdf:resource="http://www.lexinfo.net/ontology/2.0/lexinfo"/>
    </owl:Thing>
    


    <!-- http://www.lexinfo.net/ontology/2.0/lexinfo#superlativeParticle -->

    <owl:Thing rdf:about="&lexinfo;superlativeParticle">
        <rdf:type rdf:resource="&lexinfo;PartOfSpeech"/>
        <rdf:type rdf:resource="&lexinfo;ParticlePOS"/>
        <rdf:type rdf:resource="&owl;NamedIndividual"/>
        <rdfs:label xml:lang="en">superlative particle</rdfs:label>
        <rdfs:label xml:lang="ru">превосходная частица</rdfs:label>        
        <rdfs:comment xml:lang="en">Particle expressing superlative degree. Superlative is the comparison between more than two entities and contrasts with comparative where only two entities are involved and positive where no comparison is implied.</rdfs:comment>
        <rdfs:comment xml:lang="ru">Частица, которая выражает превосходную степень. Превосходная степень  - это сравнение между более чем двумя сущностями, отличается от компаратива, в котором сравниваются только две сущности, и от положительной степени, в которой  не подразумевается сравнение.</rdfs:comment>        
        <dc:creator>Francopoulo, Gil</dc:creator>
        <owl:versionInfo>1:0</owl:versionInfo>
        <dcr:datcat rdf:resource="http://www.isocat.org/datcat/DC-1923"/>
        <rdfs:isDefinedBy rdf:resource="http://www.lexinfo.net/ontology/2.0/lexinfo"/>
    </owl:Thing>
    


    <!-- http://www.lexinfo.net/ontology/2.0/lexinfo#supersededTerm -->

    <owl:Thing rdf:about="&lexinfo;supersededTerm">
        <rdf:type rdf:resource="&lexinfo;NormativeAuthorization"/>
        <rdf:type rdf:resource="&owl;NamedIndividual"/>
        <rdfs:label xml:lang="en">superseded term</rdfs:label>
        <rdfs:label xml:lang="ru">вытесненный термин</rdfs:label>        
        <dc:creator>Wright, Sue Ellen</dc:creator>
        <rdfs:comment xml:lang="en">A term that is no longer preferred or admitted.</rdfs:comment>
        <rdfs:comment xml:lang="ru">Термин, который больше не является предпочтительным или допустимым</rdfs:comment>
        <owl:versionInfo>1:0</owl:versionInfo>
        <dcr:datcat rdf:resource="http://www.isocat.org/datcat/DC-379"/>
        <rdfs:isDefinedBy rdf:resource="http://www.lexinfo.net/ontology/2.0/lexinfo"/>
    </owl:Thing>
    


    <!-- http://www.lexinfo.net/ontology/2.0/lexinfo#suspensionPoints -->

    <owl:Thing rdf:about="&lexinfo;suspensionPoints">
        <rdf:type rdf:resource="&lexinfo;PartOfSpeech"/>
        <rdf:type rdf:resource="&lexinfo;SymbolPOS"/>
        <rdf:type rdf:resource="&owl;NamedIndividual"/>
        <rdfs:label xml:lang="en">suspension points</rdfs:label>
        <rdfs:label xml:lang="ru">многоточие</rdfs:label>        
        <owl:versionInfo>1:0</owl:versionInfo>
        <rdfs:comment xml:lang="en">Sequence of three dots having the same meaning as &amp;quot;et cetera&amp;quot; (full form) or &amp;quot;etc&amp;quot; (abbreviated form).</rdfs:comment>
        <rdfs:comment xml:lang="ru">Последовательность из трех точек, имеющих то же значение, что и &amp;quot;et cetera&amp;quot; - &amp;quot;и так далее&amp;quot; (полная форма) или &amp;quot;etc&amp;quot;  - &amp;quot;и т. д.&amp;quot; (сокращенная форма).</rdfs:comment>
        <dc:creator>Francopoulo, Gil</dc:creator>
        <dcr:datcat rdf:resource="http://www.isocat.org/datcat/DC-1447"/>
        <rdfs:isDefinedBy rdf:resource="http://www.lexinfo.net/ontology/2.0/lexinfo"/>
    </owl:Thing>
    


    <!-- http://www.lexinfo.net/ontology/2.0/lexinfo#syllable -->

    <owl:Thing rdf:about="&lexinfo;syllable">
        <rdf:type rdf:resource="&lexinfo;TermElement"/>
        <rdf:type rdf:resource="&owl;NamedIndividual"/>
        <rdfs:label xml:lang="en">syllable</rdfs:label>
        <rdfs:label xml:lang="ru">слог</rdfs:label>        
        <dc:creator>Wright, Sue Ellen</dc:creator>
        <owl:versionInfo>1:0</owl:versionInfo>
        <rdfs:comment xml:lang="en">A unit of spoken language that is next bigger than a speech sound and consists of one or more vowel sounds alone or of a syllabic consonant alone or of either with one or more consonant sounds preceding or following.</rdfs:comment>
        <rdfs:comment xml:lang="ru">Единица устной речи, следующая по величине за звуком речи. Слог состоит из одного или нескольких гласных звуков или одного слогового согласного или согласного в сочетании с еще одним или  несколькими предшествующими или последующими согласными звуками.</rdfs:comment>        
        <dcr:datcat rdf:resource="http://www.isocat.org/datcat/DC-297"/>
        <rdfs:isDefinedBy rdf:resource="http://www.lexinfo.net/ontology/2.0/lexinfo"/>
    </owl:Thing>
    


    <!-- http://www.lexinfo.net/ontology/2.0/lexinfo#symbol -->

    <owl:Thing rdf:about="&lexinfo;symbol">
        <rdf:type rdf:resource="&lexinfo;TermType"/>
        <rdf:type rdf:resource="&owl;NamedIndividual"/>
        <rdfs:isDefinedBy rdf:resource="http://www.lexinfo.net/ontology/2.0/lexinfo"/>
    </owl:Thing>
    


    <!-- http://www.lexinfo.net/ontology/2.0/lexinfo#tabooRegister -->

    <owl:Thing rdf:about="&lexinfo;tabooRegister">
        <rdf:type rdf:resource="&lexinfo;Register"/>
        <rdf:type rdf:resource="&owl;NamedIndividual"/>
        <rdfs:isDefinedBy rdf:resource="http://www.lexinfo.net/ontology/2.0/lexinfo"/>
    </owl:Thing>
    


    <!-- http://www.lexinfo.net/ontology/2.0/lexinfo#technicalRegister -->

    <owl:Thing rdf:about="&lexinfo;technicalRegister">
        <rdf:type rdf:resource="&lexinfo;Register"/>
        <rdf:type rdf:resource="&owl;NamedIndividual"/>
        <rdfs:label xml:lang="en">technical register</rdfs:label>
        <rdfs:label xml:lang="ru">технический реестр</rdfs:label>        
        <dc:creator>Wright, Sue Ellen</dc:creator>
        <dc:creator>Francopoulo, Gil</dc:creator>
        <owl:versionInfo>1:0</owl:versionInfo>
        <rdfs:comment xml:lang="en">The register appropriate to scientific texts or special languages.</rdfs:comment>
        <rdfs:comment xml:lang="ru">реестр, соответствующий научным текстам или специальным языкам.</rdfs:comment>
        <dcr:datcat rdf:resource="http://www.isocat.org/datcat/DC-1997"/>
        <dcr:datcat rdf:resource="http://www.isocat.org/datcat/DC-425"/>
        <rdfs:isDefinedBy rdf:resource="http://www.lexinfo.net/ontology/2.0/lexinfo"/>
    </owl:Thing>
    


    <!-- http://www.lexinfo.net/ontology/2.0/lexinfo#terminativeCase -->

    <owl:Thing rdf:about="&lexinfo;terminativeCase">
        <rdf:type rdf:resource="&lexinfo;Case"/>
        <rdf:type rdf:resource="&owl;NamedIndividual"/>
        <rdfs:label xml:lang="en">terminative case</rdfs:label>
        <rdfs:label xml:lang="ru">терминативный падеж</rdfs:label>        
        <owl:versionInfo>1:0</owl:versionInfo>
        <dc:creator>Francopoulo, Gil</dc:creator>
        <rdfs:comment xml:lang="en">Case that indicates to what or where something ends.</rdfs:comment>
        <rdfs:comment xml:lang="ru">Падеж, который указывает, как или где что-либо заканчивается.</rdfs:comment>
        <dcr:datcat rdf:resource="http://www.isocat.org/datcat/DC-1401"/>
        <rdfs:isDefinedBy rdf:resource="http://www.lexinfo.net/ontology/2.0/lexinfo"/>
    </owl:Thing>
    


    <!-- http://www.lexinfo.net/ontology/2.0/lexinfo#thirdPerson -->

    <owl:Thing rdf:about="&lexinfo;thirdPerson">
        <rdf:type rdf:resource="&lexinfo;Person"/>
        <rdf:type rdf:resource="&owl;NamedIndividual"/>
        <rdfs:label xml:lang="en">third person</rdfs:label>
        <rdfs:label xml:lang="ru">третье лицо</rdfs:label>        
        <rdfs:comment xml:lang="en">Third person deixis is deictic reference to a referent(s) not identified as the speaker or addressee.</rdfs:comment>
        <rdfs:comment xml:lang="ru">Указание на третье лицо - это указание на объект(ы), не идентифицируемый(е) как говорящий или адресат.</rdfs:comment>
        <dc:creator>Francopoulo, Gil</dc:creator>
        <owl:versionInfo>1:0</owl:versionInfo>
        <dcr:datcat rdf:resource="http://www.isocat.org/datcat/DC-1402"/>
        <rdfs:isDefinedBy rdf:resource="http://www.lexinfo.net/ontology/2.0/lexinfo"/>
    </owl:Thing>
    


    <!-- http://www.lexinfo.net/ontology/2.0/lexinfo#transcribedForm -->

    <owl:Thing rdf:about="&lexinfo;transcribedForm">
        <rdf:type rdf:resource="&lexinfo;TermType"/>
        <rdf:type rdf:resource="&owl;NamedIndividual"/>
        <rdfs:label xml:lang="en">transcribed form</rdfs:label>
        <rdfs:label xml:lang="ru">транскрибированная форма</rdfs:label>
        <owl:versionInfo>1:0</owl:versionInfo>
        <rdfs:comment xml:lang="en">A form of a term or lexeme resulting from an operation whereby the characters of one writing system are represented by characters from another writing system, taking into account the pronunciation of the characters converted.</rdfs:comment>
        <rdfs:comment xml:lang="ru">Форма слова или лексемы, появившаяся в результате действия, при котором символы одной системы записи представлены символами другой системы записи, принимая во внимание произношение преобразованных символов.</rdfs:comment>
        <dc:creator>Wright, Sue Ellen</dc:creator>
        <dcr:datcat rdf:resource="http://www.isocat.org/datcat/DC-322"/>
        <rdfs:isDefinedBy rdf:resource="http://www.lexinfo.net/ontology/2.0/lexinfo"/>
    </owl:Thing>
    


    <!-- http://www.lexinfo.net/ontology/2.0/lexinfo#translativeCase -->

    <owl:Thing rdf:about="&lexinfo;translativeCase">
        <rdf:type rdf:resource="&lexinfo;Case"/>
        <rdf:type rdf:resource="&owl;NamedIndividual"/>
        <rdfs:label xml:lang="en">translative case</rdfs:label>
        <rdfs:label xml:lang="ru">транслятивный падеж</rdfs:label>        
        <dc:creator>Francopoulo, Gil</dc:creator>
        <rdfs:comment xml:lang="en">Case indicating that the referent of the noun, or the quality of the adjective, that it marks is the result of a process of change.</rdfs:comment>
        <rdfs:comment xml:lang="ru">Падеж, указывающий, что референт существительного или качество прилагательного являются результатом процесса изменения.</rdfs:comment>
        <owl:versionInfo>1:0</owl:versionInfo>
        <dcr:datcat rdf:resource="http://www.isocat.org/datcat/DC-1406"/>
        <rdfs:isDefinedBy rdf:resource="http://www.lexinfo.net/ontology/2.0/lexinfo"/>
    </owl:Thing>
    


    <!-- http://www.lexinfo.net/ontology/2.0/lexinfo#trial -->

    <owl:Thing rdf:about="&lexinfo;trial">
        <rdf:type rdf:resource="&lexinfo;Number"/>
        <rdf:type rdf:resource="&owl;NamedIndividual"/>
        <rdfs:label xml:lang="en">trial</rdfs:label>
        <rdfs:label xml:lang="ru">тройственное число</rdfs:label>        
        <dc:creator>Francopoulo, Gil</dc:creator>
        <rdfs:comment xml:lang="en">Grammatical number referring to &apos;three things&apos;, as opposed to &apos;singular&apos; and &apos;plural&apos;.</rdfs:comment>
        <rdfs:comment xml:lang="ru">Грамматическое число, относящееся к &apos;трем вещам&apos;, в отличие от &apos;единственного&apos; и &apos;множественного&apos;.</rdfs:comment>
        <owl:versionInfo>1:0</owl:versionInfo>
        <dcr:datcat rdf:resource="http://www.isocat.org/datcat/DC-1407"/>
        <rdfs:isDefinedBy rdf:resource="http://www.lexinfo.net/ontology/2.0/lexinfo"/>
    </owl:Thing>
    


    <!-- http://www.lexinfo.net/ontology/2.0/lexinfo#unaccomplished -->

    <owl:Thing rdf:about="&lexinfo;unaccomplished">
        <rdf:type rdf:resource="&lexinfo;Aspect"/>
        <rdf:type rdf:resource="&owl;NamedIndividual"/>
        <rdfs:label xml:lang="en">unaccomplished</rdfs:label>
        <rdfs:label xml:lang="ru">незавершенный</rdfs:label>        
        <owl:versionInfo>1:0</owl:versionInfo>
        <dc:creator>Francopoulo, Gil</dc:creator>
        <rdfs:comment xml:lang="en">aspect that expresses an event or state that is not finished.</rdfs:comment>
        <rdfs:comment xml:lang="ru">Вид, который выражает незаконченное событие или состояние.</rdfs:comment>
        <dcr:datcat rdf:resource="http://www.isocat.org/datcat/DC-2217"/>
        <rdfs:isDefinedBy rdf:resource="http://www.lexinfo.net/ontology/2.0/lexinfo"/>
    </owl:Thing>
    


    <!-- http://www.lexinfo.net/ontology/2.0/lexinfo#unclassifiedParticle -->

    <owl:Thing rdf:about="&lexinfo;unclassifiedParticle">
        <rdf:type rdf:resource="&lexinfo;PartOfSpeech"/>
        <rdf:type rdf:resource="&lexinfo;ParticlePOS"/>
        <rdf:type rdf:resource="&owl;NamedIndividual"/>
        <rdfs:label xml:lang="en">unclassified particle</rdfs:label>
        <rdfs:label xml:lang="ru">Неклассифицированная частица</rdfs:label>        
        <owl:versionInfo>1:0</owl:versionInfo>
        <dc:creator>Francopoulo, Gil</dc:creator>
        <rdfs:comment xml:lang="en">Particle that is not covered by other sorts of particle definitions.</rdfs:comment>
        <rdfs:comment xml:lang="ru">Частица, которая не описывается другими определениями частиц.</rdfs:comment>
        <dcr:datcat rdf:resource="http://www.isocat.org/datcat/DC-1897"/>
        <rdfs:isDefinedBy rdf:resource="http://www.lexinfo.net/ontology/2.0/lexinfo"/>
    </owl:Thing>
    


    <!-- http://www.lexinfo.net/ontology/2.0/lexinfo#verb -->

    <owl:Thing rdf:about="&lexinfo;verb">
        <rdf:type rdf:resource="&lexinfo;PartOfSpeech"/>
        <rdf:type rdf:resource="&lexinfo;VerbPOS"/>
        <rdf:type rdf:resource="&owl;NamedIndividual"/>
        <rdfs:label xml:lang="en">verb</rdfs:label>
        <rdfs:label xml:lang="ru">глагол</rdfs:label>        
        <rdfs:comment xml:lang="en">Element which, singly or in combination with other verbs is used as the minimal predicate of a sentence, co-occurring with a subject. If the predicate contains other elements (e.g. object, complement), then it is the verb which more than any other is the unit which influences the choice and extent of these elements.</rdfs:comment>
        <rdfs:comment xml:lang="ru">Элемент, который самостоятельно или в сочетании с другими глаголами используется как минимальный предикат предложения вместе с субъектом. Если предикат содержит другие элементы (например, объект, дополнение), то глагол, больше чем любая другая единица, влияет на выбор и распространенность этих элементов.</rdfs:comment>
        <dc:creator>Francopoulo, Gil</dc:creator>
        <owl:versionInfo>1:0</owl:versionInfo>
        <dcr:datcat rdf:resource="http://www.isocat.org/datcat/DC-1424"/>
        <rdfs:isDefinedBy rdf:resource="http://www.lexinfo.net/ontology/2.0/lexinfo"/>
    </owl:Thing>
    


    <!-- http://www.lexinfo.net/ontology/2.0/lexinfo#vocativeCase -->

    <owl:Thing rdf:about="&lexinfo;vocativeCase">
        <rdf:type rdf:resource="&lexinfo;Case"/>
        <rdf:type rdf:resource="&owl;NamedIndividual"/>
        <rdfs:label xml:lang="en">vocative case</rdfs:label>
        <rdfs:label xml:lang="ru">звательный падеж</rdfs:label>        
        <dc:creator>Francopoulo, Gil</dc:creator>
        <rdfs:comment xml:lang="en">Case used to indicate direct address.</rdfs:comment>
        <rdfs:comment xml:lang="ru">Падеж, используемый для прямого обращения.</rdfs:comment>
        <owl:versionInfo>1:0</owl:versionInfo>
        <dcr:datcat rdf:resource="http://www.isocat.org/datcat/DC-1412"/>
        <rdfs:isDefinedBy rdf:resource="http://www.lexinfo.net/ontology/2.0/lexinfo"/>
    </owl:Thing>
    


    <!-- http://www.lexinfo.net/ontology/2.0/lexinfo#vulgarRegister -->

    <owl:Thing rdf:about="&lexinfo;vulgarRegister">
        <rdf:type rdf:resource="&lexinfo;Register"/>
        <rdf:type rdf:resource="&owl;NamedIndividual"/>
        <rdfs:label xml:lang="en">vulgar register</rdfs:label>
        <rdfs:label xml:lang="ru">грубый реестр</rdfs:label>        
        <rdfs:comment xml:lang="en">Register of a term or text type that can be characterized as profane or socially unacceptable.</rdfs:comment>
        <rdfs:comment xml:lang="ru">Реестр терминов или текстов, который можно охарактеризовать как непристойный или социально неприемлемый.</rdfs:comment>
        <rdfs:comment xml:lang="en">The register of a term or text type that can be characterized as profane or socially unacceptable.</rdfs:comment>
        <rdfs:comment xml:lang="ru">Реестр терминов или текстов, который можно охарактеризовать как непристойный или социально неприемлемый.</rdfs:comment>
        <dc:creator>Wright, Sue Ellen</dc:creator>
        <owl:versionInfo>1:0</owl:versionInfo>
        <dc:creator>Francopoulo, Gil</dc:creator>
        <dcr:datcat rdf:resource="http://www.isocat.org/datcat/DC-1998"/>
        <dcr:datcat rdf:resource="http://www.isocat.org/datcat/DC-429"/>
        <rdfs:isDefinedBy rdf:resource="http://www.lexinfo.net/ontology/2.0/lexinfo"/>
    </owl:Thing>
    


    <!-- http://www.lexinfo.net/ontology/2.0/lexinfo#weakPersonalPronoun -->

    <owl:Thing rdf:about="&lexinfo;weakPersonalPronoun">
        <rdf:type rdf:resource="&lexinfo;PartOfSpeech"/>
        <rdf:type rdf:resource="&lexinfo;PronounPOS"/>
        <rdf:type rdf:resource="&owl;NamedIndividual"/>
        <rdfs:label xml:lang="en">weak personal pronoun</rdfs:label>
        <rdfs:label xml:lang="ru">слабое личное местоимение</rdfs:label>        
        <rdfs:comment xml:lang="en">Personal pronoun that cannot occupy the position after a preposition and/or reinforce a strong personal pronoun.</rdfs:comment>
        <rdfs:comment xml:lang="ru">Личное местоимение, которое не может занимать позицию после предлога и/или усиливать сильное личное местоимение.</rdfs:comment>
        <dc:creator>Francopoulo, Gil</dc:creator>
        <owl:versionInfo>1:0</owl:versionInfo>
        <dcr:datcat rdf:resource="http://www.isocat.org/datcat/DC-1414"/>
        <rdfs:isDefinedBy rdf:resource="http://www.lexinfo.net/ontology/2.0/lexinfo"/>
    </owl:Thing>
    


    <!-- http://www.lexinfo.net/ontology/2.0/lexinfo#wordElement -->

    <owl:Thing rdf:about="&lexinfo;wordElement">
        <rdf:type rdf:resource="&lexinfo;TermElement"/>
        <rdf:type rdf:resource="&owl;NamedIndividual"/>
        <rdfs:label xml:lang="en">wordElement</rdfs:label>
        <rdfs:label xml:lang="ru">часть слова</rdfs:label>        
        <owl:versionInfo>1:0</owl:versionInfo>
        <dc:creator>Wright, Sue Ellen</dc:creator>
        <rdfs:comment xml:lang="en">Any lexeme element in a compound lexical unit that is itself a word.</rdfs:comment>
        <rdfs:comment xml:lang="ru">Любой элемент в составной лексической единице, который сам по себе является словом.</rdfs:comment>
        <dcr:datcat rdf:resource="http://www.isocat.org/datcat/DC-298"/>
        <rdfs:isDefinedBy rdf:resource="http://www.lexinfo.net/ontology/2.0/lexinfo"/>
    </owl:Thing>
    


    <!-- http://www.lexinfo.net/ontology/2.0/lexinfo#yes -->

    <owl:Thing rdf:about="&lexinfo;yes">
        <rdf:type rdf:resource="&lexinfo;Cliticness"/>
        <rdf:type rdf:resource="&lexinfo;Negative"/>
        <rdf:type rdf:resource="&owl;NamedIndividual"/>
        <rdfs:label xml:lang="en">yes</rdfs:label>
        <rdfs:label xml:lang="ru">да</rdfs:label>
        <rdfs:comment xml:lang="en">Positive value</rdfs:comment>
        <rdfs:comment xml:lang="ru">Положительное значение</rdfs:comment>
        <dc:creator>Francopoulo, Gil</dc:creator>
        <owl:versionInfo>1:0</owl:versionInfo>
        <dcr:datcat rdf:resource="http://www.isocat.org/datcat/DC-1904"/>
        <rdfs:isDefinedBy rdf:resource="http://www.lexinfo.net/ontology/2.0/lexinfo"/>
    </owl:Thing>
</rdf:RDF>



<!-- Generated by the OWL API (version 3.4.2) http://owlapi.sourceforge.net -->

